<?xml version="1.0"?>
<rdf:RDF xmlns="http://www.semanticweb.org/evahe/ontologies/2024/4/dco#"
     xml:base="http://www.semanticweb.org/evahe/ontologies/2024/4/dco"
     xmlns:ns="http://www.w3.org/2003/06/sw-vocab-status/ns#"
     xmlns:beo="https://pi.pauwel.be/voc/buildingelement#"
     xmlns:bot="https://w3id.org/bot#"
     xmlns:bpo="https://www.projekt-scope.de/ontologies/bpo/#"
     xmlns:dco="http://www.semanticweb.org/covon/ontologies/2022/11/deconstruction-ontology#"
     xmlns:dor="http://www.semanticweb.org/arnak/ontologies/2022/7/DOR#"
     xmlns:dot="https://w3id.org/dot#"
     xmlns:ns2="http://www.w3.org/2006/vcard/ns#"
     xmlns:owl="http://www.w3.org/2002/07/owl#"
     xmlns:rdf="http://www.w3.org/1999/02/22-rdf-syntax-ns#"
     xmlns:xml="http://www.w3.org/XML/1998/namespace"
     xmlns:xsd="http://www.w3.org/2001/XMLSchema#"
     xmlns:dcim="https://w3id.org/digitalconstruction/0.5/Materials#"
     xmlns:foaf="http://xmlns.com/foaf/0.1/"
     xmlns:rdfs="http://www.w3.org/2000/01/rdf-schema#"
     xmlns:dicbm="https://w3id.org/digitalconstruction/0.3/BuildingMaterials#"
     xmlns:terms="http://purl.org/dc/terms/"
     xmlns:schema="http://schema.org/#"
     xmlns:schema1="https://schema.org/">
    <owl:Ontology rdf:about="http://www.semanticweb.org/evahe/ontologies/2024/4/dco">
        <rdfs:comment xml:lang="de">Die Rückbau-Ontologie ist eine einfache Ontologie zur Darstellung der Kernkonzepte und -prozesse, die im Rahmen eines Rückbauprojektes Anwendung finden.</rdfs:comment>
        <rdfs:comment xml:lang="en">The deconstruction-ontology is a simple ontology for the representation of core concepts and processes that are applied in a deconstruction project.</rdfs:comment>
    </owl:Ontology>
    


    <!-- 
    ///////////////////////////////////////////////////////////////////////////////////////
    //
    // Annotation properties
    //
    ///////////////////////////////////////////////////////////////////////////////////////
     -->

    


    <!-- http://purl.org/dc/terms/description -->

    <owl:AnnotationProperty rdf:about="http://purl.org/dc/terms/description"/>
    


    <!-- http://schema.org/#domainIncludes -->

    <owl:AnnotationProperty rdf:about="http://schema.org/#domainIncludes"/>
    


    <!-- http://www.w3.org/2003/06/sw-vocab-status/ns#term_status -->

    <owl:AnnotationProperty rdf:about="http://www.w3.org/2003/06/sw-vocab-status/ns#term_status"/>
    


    <!-- http://www.w3.org/2006/vcard/ns#fn -->

    <owl:AnnotationProperty rdf:about="http://www.w3.org/2006/vcard/ns#fn"/>
    


    <!-- http://xmlns.com/foaf/0.1/name -->

    <owl:AnnotationProperty rdf:about="http://xmlns.com/foaf/0.1/name"/>
    


    <!-- https://schema.org/domainIncludes -->

    <owl:AnnotationProperty rdf:about="https://schema.org/domainIncludes"/>
    


    <!-- https://schema.org/name -->

    <owl:AnnotationProperty rdf:about="https://schema.org/name"/>
    


    <!-- https://schema.org/rangeIncludes -->

    <owl:AnnotationProperty rdf:about="https://schema.org/rangeIncludes"/>
    


    <!-- 
    ///////////////////////////////////////////////////////////////////////////////////////
    //
    // Object Properties
    //
    ///////////////////////////////////////////////////////////////////////////////////////
     -->

    


    <!-- http://www.semanticweb.org/arnak/ontologies/2022/7/DOR#auditsFor -->

    <owl:ObjectProperty rdf:about="http://www.semanticweb.org/arnak/ontologies/2022/7/DOR#auditsFor">
        <rdfs:domain rdf:resource="http://www.semanticweb.org/arnak/ontologies/2022/7/DOR#PreDeconstructionAuditor"/>
        <rdfs:range rdf:resource="http://www.semanticweb.org/arnak/ontologies/2022/7/DOR#CircularPotential"/>
        <rdfs:comment>The action that an Auditor carries out.</rdfs:comment>
        <rdfs:label>Audits For</rdfs:label>
    </owl:ObjectProperty>
    


    <!-- http://www.semanticweb.org/arnak/ontologies/2022/7/DOR#designsFor -->

    <owl:ObjectProperty rdf:about="http://www.semanticweb.org/arnak/ontologies/2022/7/DOR#designsFor">
        <rdfs:domain rdf:resource="http://www.semanticweb.org/arnak/ontologies/2022/7/DOR#Designer"/>
        <rdfs:range rdf:resource="http://www.semanticweb.org/arnak/ontologies/2022/7/DOR#CircularPotential"/>
        <rdfs:comment>The action that a Designer carries out. A designer can design a component for a ceratin circular potential.</rdfs:comment>
        <rdfs:label>Designs For</rdfs:label>
    </owl:ObjectProperty>
    


    <!-- http://www.semanticweb.org/arnak/ontologies/2022/7/DOR#hasCircularPotential -->

    <owl:ObjectProperty rdf:about="http://www.semanticweb.org/arnak/ontologies/2022/7/DOR#hasCircularPotential">
        <rdfs:range rdf:resource="http://www.semanticweb.org/arnak/ontologies/2022/7/DOR#CircularPotential"/>
        <rdfs:comment>Any Building or Functional Layer or Component has a circular potential. This object property links the circular potential to the designated item.</rdfs:comment>
        <rdfs:label xml:lang="en">has Circular Potential</rdfs:label>
    </owl:ObjectProperty>
    


    <!-- http://www.semanticweb.org/arnak/ontologies/2022/7/DOR#hasCircularRequirement -->

    <owl:ObjectProperty rdf:about="http://www.semanticweb.org/arnak/ontologies/2022/7/DOR#hasCircularRequirement">
        <rdfs:domain rdf:resource="http://www.semanticweb.org/arnak/ontologies/2022/7/DOR#CircularPotential"/>
        <rdfs:range rdf:resource="http://www.semanticweb.org/arnak/ontologies/2022/7/DOR#CircularRequirement"/>
        <rdfs:comment>This object property connects the requirements necessary for realising a circular potential and the designated circular potential.</rdfs:comment>
        <rdfs:label xml:lang="en">has Circular Requirement</rdfs:label>
    </owl:ObjectProperty>
    


    <!-- http://www.semanticweb.org/arnak/ontologies/2022/7/DOR#hasConnectionType -->

    <owl:ObjectProperty rdf:about="http://www.semanticweb.org/arnak/ontologies/2022/7/DOR#hasConnectionType">
        <rdf:type rdf:resource="http://www.w3.org/2002/07/owl#FunctionalProperty"/>
        <rdfs:range rdf:resource="http://www.semanticweb.org/arnak/ontologies/2022/7/DOR#ConnectionType"/>
        <rdfs:comment>This object property elaborates the type of connection a &quot;Component Connection&quot; or &quot;Installation Connection&quot; has.</rdfs:comment>
        <rdfs:label xml:lang="en">has Connection Type</rdfs:label>
    </owl:ObjectProperty>
    


    <!-- http://www.semanticweb.org/arnak/ontologies/2022/7/DOR#hasFinalCircularPotential -->

    <owl:ObjectProperty rdf:about="http://www.semanticweb.org/arnak/ontologies/2022/7/DOR#hasFinalCircularPotential">
        <rdf:type rdf:resource="http://www.w3.org/2002/07/owl#FunctionalProperty"/>
        <rdfs:range rdf:resource="http://www.semanticweb.org/arnak/ontologies/2022/7/DOR#CircularPotential"/>
        <rdfs:comment xml:lang="en">is an object property that can be used to indicate the final circular potential of a product when it has reached the end of its life cycle. It can be used to link a product to its final circular potential, which may be different from its current or previous circular potentials.

For example, a product may have a reuse potential, a recycling potential, and a repurposing potential, but when it can no longer be repurposed, it may have a final circular potential of disposal or waste. The hasFinalCircularPotential property can be used to link the product to this final potential.

The range of hasFinalCircularPotential could be the class CircularPotential, while its domain would be the class Component or any other class that represents a thing that has circular potential.</rdfs:comment>
        <rdfs:label xml:lang="en">has Final Circular Potential</rdfs:label>
    </owl:ObjectProperty>
    


    <!-- http://www.semanticweb.org/arnak/ontologies/2022/7/DOR#hasFunctionalLayer -->

    <owl:ObjectProperty rdf:about="http://www.semanticweb.org/arnak/ontologies/2022/7/DOR#hasFunctionalLayer">
        <rdfs:domain rdf:resource="https://w3id.org/bot#Building"/>
        <rdfs:range rdf:resource="http://www.semanticweb.org/arnak/ontologies/2022/7/DOR#FunctionalLayer"/>
        <rdfs:comment>Object Property between a Building and a Functional layer belongs to that building. 
A Building has different fucntional layers.</rdfs:comment>
        <rdfs:label xml:lang="en">has Functional Layer</rdfs:label>
    </owl:ObjectProperty>
    


    <!-- http://www.semanticweb.org/arnak/ontologies/2022/7/DOR#hasRecommendedInspection -->

    <owl:ObjectProperty rdf:about="http://www.semanticweb.org/arnak/ontologies/2022/7/DOR#hasRecommendedInspection">
        <rdfs:comment>Property between a Component and an Inspection for those inspections that are recommended and not mandatory to be conducted during the material bank assessment process or after the deconstruction process and before reuse.</rdfs:comment>
        <rdfs:label>has Recommended Inspection</rdfs:label>
    </owl:ObjectProperty>
    


    <!-- http://www.semanticweb.org/arnak/ontologies/2022/7/DOR#hasRecommendedInspectionMethod -->

    <owl:ObjectProperty rdf:about="http://www.semanticweb.org/arnak/ontologies/2022/7/DOR#hasRecommendedInspectionMethod">
        <rdfs:subPropertyOf rdf:resource="http://www.semanticweb.org/arnak/ontologies/2022/7/DOR#hasRecommendedInspection"/>
        <rdfs:range rdf:resource="http://www.semanticweb.org/arnak/ontologies/2022/7/DOR#Inspection_Method"/>
        <rdfs:comment>Property between a Component and an Inspection Method for those inspections that are recommended and not mandatory to be conducted during the material bank assessment process or after the deconstruction process and before reuse.</rdfs:comment>
        <rdfs:label>has Recommended Inspection Method</rdfs:label>
    </owl:ObjectProperty>
    


    <!-- http://www.semanticweb.org/arnak/ontologies/2022/7/DOR#hasRecommendedInspectionMode -->

    <owl:ObjectProperty rdf:about="http://www.semanticweb.org/arnak/ontologies/2022/7/DOR#hasRecommendedInspectionMode">
        <rdfs:subPropertyOf rdf:resource="http://www.semanticweb.org/arnak/ontologies/2022/7/DOR#hasRecommendedInspection"/>
        <rdfs:range rdf:resource="http://www.semanticweb.org/arnak/ontologies/2022/7/DOR#InspectionMode"/>
        <rdfs:comment>Property between a Component and an Inspection Mode for those inspections that are recommended and not mandatory to be conducted during the material bank assessment process or after the deconstruction process and before reuse.</rdfs:comment>
        <rdfs:label>has Recommended Inspection Mode</rdfs:label>
    </owl:ObjectProperty>
    


    <!-- http://www.semanticweb.org/arnak/ontologies/2022/7/DOR#hasRequiredInspection -->

    <owl:ObjectProperty rdf:about="http://www.semanticweb.org/arnak/ontologies/2022/7/DOR#hasRequiredInspection">
        <rdfs:domain rdf:resource="https://w3id.org/bot#Element"/>
        <rdfs:comment>Property between a Component and an Inspection for those inspections that are required or mandatory to be conducted during the material bank assessment process or after the deconstruction process and before reuse.</rdfs:comment>
        <rdfs:label>has Required Inspection</rdfs:label>
    </owl:ObjectProperty>
    


    <!-- http://www.semanticweb.org/arnak/ontologies/2022/7/DOR#hasRequiredInspectionMethod -->

    <owl:ObjectProperty rdf:about="http://www.semanticweb.org/arnak/ontologies/2022/7/DOR#hasRequiredInspectionMethod">
        <rdfs:subPropertyOf rdf:resource="http://www.semanticweb.org/arnak/ontologies/2022/7/DOR#hasRequiredInspection"/>
        <rdfs:range rdf:resource="http://www.semanticweb.org/arnak/ontologies/2022/7/DOR#Inspection_Method"/>
        <rdfs:comment>Property between a Component and an Inspection Method for those inspections that are required or mandatory to be conducted during the material bank assessment process or after the deconstruction process and before reuse.</rdfs:comment>
        <rdfs:label>has Required Inspection Method</rdfs:label>
    </owl:ObjectProperty>
    


    <!-- http://www.semanticweb.org/arnak/ontologies/2022/7/DOR#hasRequiredInspectionMode -->

    <owl:ObjectProperty rdf:about="http://www.semanticweb.org/arnak/ontologies/2022/7/DOR#hasRequiredInspectionMode">
        <rdfs:subPropertyOf rdf:resource="http://www.semanticweb.org/arnak/ontologies/2022/7/DOR#hasRequiredInspection"/>
        <rdfs:range rdf:resource="http://www.semanticweb.org/arnak/ontologies/2022/7/DOR#InspectionMode"/>
        <rdfs:comment>Property between a Component and an Inspection Mode for those inspections that are required or mandatory to be conducted during the material bank assessment process or after the deconstruction process and before reuse.</rdfs:comment>
        <rdfs:label>has Required Inspection Mode</rdfs:label>
    </owl:ObjectProperty>
    


    <!-- http://www.semanticweb.org/arnak/ontologies/2022/7/DOR#hasRequirement -->

    <owl:ObjectProperty rdf:about="http://www.semanticweb.org/arnak/ontologies/2022/7/DOR#hasRequirement">
        <rdfs:domain rdf:resource="http://www.semanticweb.org/arnak/ontologies/2022/7/DOR#CircularPotential"/>
        <rdfs:range rdf:resource="http://www.semanticweb.org/arnak/ontologies/2022/7/DOR#CircularRequirement"/>
    </owl:ObjectProperty>
    


    <!-- http://www.semanticweb.org/arnak/ontologies/2022/7/DOR#hasSourceType -->

    <owl:ObjectProperty rdf:about="http://www.semanticweb.org/arnak/ontologies/2022/7/DOR#hasSourceType">
        <rdf:type rdf:resource="http://www.w3.org/2002/07/owl#AsymmetricProperty"/>
        <rdfs:domain rdf:resource="https://w3id.org/digitalconstruction/0.3/BuildingMaterials#Material"/>
        <rdfs:range rdf:resource="http://www.semanticweb.org/arnak/ontologies/2022/7/DOR#MaterialSourceType"/>
        <rdfs:comment>The &quot;has Source Type&quot; object property is used to specify the source type of a material. DICM:Material is its domain and its range  is Material Source Type.
By using the &quot;has Source Type&quot; property, one can associate a material with a specific source type, such as &quot;hazardous material,&quot; &quot;non-hazardous material,&quot; &quot;non-renewable material,&quot; &quot;primary raw material,&quot; &quot;recyclable material,&quot; or &quot;renewable material&quot; in order to capture information about the origin or nature of a material, allowing for more detailed analysis and reasoning about materials in post-consumer phase.</rdfs:comment>
        <rdfs:label xml:lang="en">has Source Type</rdfs:label>
    </owl:ObjectProperty>
    


    <!-- http://www.semanticweb.org/arnak/ontologies/2022/7/DOR#producesFor -->

    <owl:ObjectProperty rdf:about="http://www.semanticweb.org/arnak/ontologies/2022/7/DOR#producesFor">
        <rdfs:domain rdf:resource="http://www.semanticweb.org/arnak/ontologies/2022/7/DOR#Manufacturer"/>
        <rdfs:range rdf:resource="http://www.semanticweb.org/arnak/ontologies/2022/7/DOR#CircularPotential"/>
        <rdfs:comment>The action that a Producer or Manufacturer carries out. A producer or manufacturer can produces a component for a ceratin circular potential.</rdfs:comment>
        <rdfs:label>Produces For</rdfs:label>
    </owl:ObjectProperty>
    


    <!-- http://www.semanticweb.org/arnak/ontologies/2022/7/DOR#recertifiesFor -->

    <owl:ObjectProperty rdf:about="http://www.semanticweb.org/arnak/ontologies/2022/7/DOR#recertifiesFor">
        <rdfs:domain rdf:resource="http://www.semanticweb.org/arnak/ontologies/2022/7/DOR#MaterialBankAgent"/>
        <rdfs:range rdf:resource="http://www.semanticweb.org/arnak/ontologies/2022/7/DOR#CircularPotential"/>
        <rdfs:comment>The action that a Material Bank carries out. A material bank agent or entity can recertify components after assessment to have a certain circular potential.</rdfs:comment>
        <rdfs:label>Recertifies For</rdfs:label>
    </owl:ObjectProperty>
    


    <!-- http://www.semanticweb.org/covon/ontologies/2022/11/deconstruction-ontology#adjacentBuilding -->

    <owl:ObjectProperty rdf:about="http://www.semanticweb.org/covon/ontologies/2022/11/deconstruction-ontology#adjacentBuilding">
        <rdfs:subPropertyOf rdf:resource="http://www.w3.org/2002/07/owl#topObjectProperty"/>
        <rdfs:domain rdf:resource="http://www.semanticweb.org/covon/ontologies/2022/11/deconstruction-ontology#DeconstructionObject"/>
        <rdfs:range rdf:resource="http://www.semanticweb.org/covon/ontologies/2022/11/deconstruction-ontology#NeighboringObject"/>
        <rdfs:comment xml:lang="de">Diese Eigenschaft verknüpft ein Rückbauobjekt mit seinen umliegenden Nachbargebäuden.</rdfs:comment>
        <rdfs:comment xml:lang="en">This property connects a deconstruction object with its surrounding neighboring buildings.</rdfs:comment>
        <rdfs:label xml:lang="de">anliegende Nachbargebäude</rdfs:label>
    </owl:ObjectProperty>
    


    <!-- http://www.semanticweb.org/covon/ontologies/2022/11/deconstruction-ontology#applicationRequirement -->

    <owl:ObjectProperty rdf:about="http://www.semanticweb.org/covon/ontologies/2022/11/deconstruction-ontology#applicationRequirement">
        <rdfs:subPropertyOf rdf:resource="http://www.w3.org/2002/07/owl#topObjectProperty"/>
        <rdf:type rdf:resource="http://www.w3.org/2002/07/owl#TransitiveProperty"/>
        <rdfs:domain rdf:resource="http://www.semanticweb.org/covon/ontologies/2022/11/deconstruction-ontology#DeconstructionMethod"/>
        <rdfs:range rdf:resource="http://www.semanticweb.org/covon/ontologies/2022/11/deconstruction-ontology#DeconstructionMethod"/>
        <rdfs:comment xml:lang="de">Diese Eigenschaft verknüpft ein Rückbauverfahren mit anderen Rückbauverfahren, sofern diese Voraussetzung zur Anwendung des erstgenannten Verfahrens sind.</rdfs:comment>
        <rdfs:comment xml:lang="en">This property links a deconstruction method with other deconstruction methods, provided that these are prerequisites for the application of the first-mentioned method.</rdfs:comment>
        <rdfs:label xml:lang="de">Anwendungsvoraussetzung</rdfs:label>
    </owl:ObjectProperty>
    


    <!-- http://www.semanticweb.org/covon/ontologies/2022/11/deconstruction-ontology#canBeQualifiedAs -->

    <owl:ObjectProperty rdf:about="http://www.semanticweb.org/covon/ontologies/2022/11/deconstruction-ontology#canBeQualifiedAs">
        <rdfs:subPropertyOf rdf:resource="http://www.w3.org/2002/07/owl#topObjectProperty"/>
        <rdfs:comment xml:lang="de">Diese Eigenschaft ordnet einem identifizierten Schaden die zugehörige Schadensart zu.</rdfs:comment>
        <rdfs:comment xml:lang="en">This property assigns the associated damage type to an identified damage.</rdfs:comment>
        <rdfs:label xml:lang="de">kann qualifiziert/klassifiziert werden als</rdfs:label>
    </owl:ObjectProperty>
    


    <!-- http://www.semanticweb.org/covon/ontologies/2022/11/deconstruction-ontology#consistsOfMaterial -->

    <owl:ObjectProperty rdf:about="http://www.semanticweb.org/covon/ontologies/2022/11/deconstruction-ontology#consistsOfMaterial">
        <rdfs:subPropertyOf rdf:resource="http://www.w3.org/2002/07/owl#topObjectProperty"/>
        <owl:propertyChainAxiom rdf:parseType="Collection">
            <rdf:Description rdf:about="http://www.semanticweb.org/covon/ontologies/2022/11/deconstruction-ontology#hasComponent"/>
            <rdf:Description rdf:about="http://www.semanticweb.org/covon/ontologies/2022/11/deconstruction-ontology#consistsOfMaterial"/>
        </owl:propertyChainAxiom>
        <rdfs:comment xml:lang="de">Diese Eigenschaft ordnet einer Komponente die zugehörigen Materialien zu, aus denen die Komponente besteht.</rdfs:comment>
        <rdfs:comment xml:lang="en">This property assigns the associated materials to a component that are used to create the component.</rdfs:comment>
        <rdfs:label xml:lang="de">besteht aus Material</rdfs:label>
    </owl:ObjectProperty>
    


    <!-- http://www.semanticweb.org/covon/ontologies/2022/11/deconstruction-ontology#directBuildingAdjacency -->

    <owl:ObjectProperty rdf:about="http://www.semanticweb.org/covon/ontologies/2022/11/deconstruction-ontology#directBuildingAdjacency">
        <rdfs:subPropertyOf rdf:resource="http://www.semanticweb.org/covon/ontologies/2022/11/deconstruction-ontology#adjacentBuilding"/>
        <owl:propertyDisjointWith rdf:resource="http://www.semanticweb.org/covon/ontologies/2022/11/deconstruction-ontology#indirectBuildingAdjacency"/>
        <rdfs:comment xml:lang="de">Diese Eigenschaft verknüpft ein Rückbauobjekt mit einem oder mehreren Nachbargebäuden, die unmittelbar, d.h. ohne Luftraum, an das Rückbauobjekt grenzen.</rdfs:comment>
        <rdfs:comment xml:lang="en">This property connects a deconstruction object to one or more neighboring buildings that are directly adjacent to the deconstruction object, i.e., without airspace.</rdfs:comment>
        <rdfs:label xml:lang="de">unmittelbare Gebäude Angrenzung</rdfs:label>
    </owl:ObjectProperty>
    


    <!-- http://www.semanticweb.org/covon/ontologies/2022/11/deconstruction-ontology#exteriorComponent -->

    <owl:ObjectProperty rdf:about="http://www.semanticweb.org/covon/ontologies/2022/11/deconstruction-ontology#exteriorComponent">
        <rdfs:subPropertyOf rdf:resource="http://www.semanticweb.org/covon/ontologies/2022/11/deconstruction-ontology#hasComponent"/>
        <rdfs:comment xml:lang="de">Diese Eigenschaft ordnet einem Bauteil eine außenliegende, d.h. an die Umgebung gerichtete, Komponente zu.</rdfs:comment>
        <rdfs:comment xml:lang="en">This property assigns an exterior component, i.e. directed to the environment, to an element.</rdfs:comment>
        <rdfs:label xml:lang="de">außenliegende Komponente</rdfs:label>
    </owl:ObjectProperty>
    


    <!-- http://www.semanticweb.org/covon/ontologies/2022/11/deconstruction-ontology#hasComponent -->

    <owl:ObjectProperty rdf:about="http://www.semanticweb.org/covon/ontologies/2022/11/deconstruction-ontology#hasComponent">
        <rdfs:subPropertyOf rdf:resource="http://www.w3.org/2002/07/owl#topObjectProperty"/>
        <rdfs:range rdf:resource="http://www.semanticweb.org/covon/ontologies/2022/11/deconstruction-ontology#Component"/>
        <rdfs:comment xml:lang="de">Diese Eigenschaft ordnet einem Bauteil eine Komponente zu.</rdfs:comment>
        <rdfs:comment xml:lang="en">This property assigns a component to an element.</rdfs:comment>
        <rdfs:label xml:lang="de">hat Komponente</rdfs:label>
    </owl:ObjectProperty>
    


    <!-- http://www.semanticweb.org/covon/ontologies/2022/11/deconstruction-ontology#indirectBuildingAdjacency -->

    <owl:ObjectProperty rdf:about="http://www.semanticweb.org/covon/ontologies/2022/11/deconstruction-ontology#indirectBuildingAdjacency">
        <rdfs:subPropertyOf rdf:resource="http://www.semanticweb.org/covon/ontologies/2022/11/deconstruction-ontology#adjacentBuilding"/>
        <rdfs:comment xml:lang="de">Diese Eigenschaft verknüpft ein Rückbauobjekt mit einem oder mehreren Nachbargebäuden, die mittelbar an das Rückbauobjekt grenzen bzw. im Einflussbereich des Rückbauobjektes liegen.</rdfs:comment>
        <rdfs:comment xml:lang="en">This property connects a deconstruction object to one or more neighboring buildings that are indirectly adjacent to or within the area of influence of the deconstruction object.</rdfs:comment>
        <rdfs:label xml:lang="de">mittelbare Gebäude Angrenzung</rdfs:label>
    </owl:ObjectProperty>
    


    <!-- http://www.semanticweb.org/covon/ontologies/2022/11/deconstruction-ontology#interiorComponent -->

    <owl:ObjectProperty rdf:about="http://www.semanticweb.org/covon/ontologies/2022/11/deconstruction-ontology#interiorComponent">
        <rdfs:subPropertyOf rdf:resource="http://www.semanticweb.org/covon/ontologies/2022/11/deconstruction-ontology#hasComponent"/>
        <rdfs:comment xml:lang="de">Diese Eigenschaft ordnet einem Bauteil eine innenliegende, d.h. in den Raum gerichtete, Komponente zu.</rdfs:comment>
        <rdfs:comment xml:lang="en">This property assigns an interior component, i.e. one that is directed into the room, to an element.</rdfs:comment>
        <rdfs:label xml:lang="de">innenliegende Komponente</rdfs:label>
    </owl:ObjectProperty>
    


    <!-- http://www.semanticweb.org/covon/ontologies/2022/11/deconstruction-ontology#intermediateComponent -->

    <owl:ObjectProperty rdf:about="http://www.semanticweb.org/covon/ontologies/2022/11/deconstruction-ontology#intermediateComponent">
        <rdfs:subPropertyOf rdf:resource="http://www.semanticweb.org/covon/ontologies/2022/11/deconstruction-ontology#hasComponent"/>
        <rdfs:comment xml:lang="de">Diese Eigenschaft ordnet einem Bauteil eine Komponente zu, die zwischen zwei Komponenten liegt.</rdfs:comment>
        <rdfs:comment xml:lang="en">This property assigns a component to an element that is located between two components.</rdfs:comment>
        <rdfs:label xml:lang="de">zwischenliegende Komponente</rdfs:label>
    </owl:ObjectProperty>
    


    <!-- http://www.semanticweb.org/covon/ontologies/2022/11/deconstruction-ontology#isSecondarilyContaminatedBy -->

    <owl:ObjectProperty rdf:about="http://www.semanticweb.org/covon/ontologies/2022/11/deconstruction-ontology#isSecondarilyContaminatedBy">
        <rdfs:subPropertyOf rdf:resource="http://www.w3.org/2002/07/owl#topObjectProperty"/>
        <rdfs:domain rdf:resource="http://www.semanticweb.org/covon/ontologies/2022/11/deconstruction-ontology#Component"/>
        <rdfs:comment xml:lang="de">Diese Eigenschaft verknüpft eine Komponente mit einem Schadstoff, wobei die Schadstoffbelastung auf die Einwirkung anderer, primärbelasteter Komponenten (baustoffimmanent) zurückzuführen ist.</rdfs:comment>
        <rdfs:comment xml:lang="en">This property links a component to a contaminanted material, where the contamination is due to the influence of other, primary contaminated components (immanent to the building material).</rdfs:comment>
        <rdfs:label xml:lang="de">ist sekundärbelastet durch</rdfs:label>
    </owl:ObjectProperty>
    


    <!-- http://www.semanticweb.org/covon/ontologies/2022/11/deconstruction-ontology#isTreatedAs -->

    <owl:ObjectProperty rdf:about="http://www.semanticweb.org/covon/ontologies/2022/11/deconstruction-ontology#isTreatedAs">
        <rdfs:subPropertyOf rdf:resource="http://www.w3.org/2002/07/owl#topObjectProperty"/>
        <rdfs:domain rdf:resource="http://www.semanticweb.org/covon/ontologies/2022/11/deconstruction-ontology#Component"/>
        <rdfs:comment xml:lang="de">Diese Eigenschaft ordnet einer Komponente einen Behandlungsweg zu.</rdfs:comment>
        <rdfs:comment xml:lang="en">This property assigns a treatment path to a component.</rdfs:comment>
        <rdfs:label xml:lang="de">wird behandelt als</rdfs:label>
    </owl:ObjectProperty>
    


    <!-- http://www.semanticweb.org/covon/ontologies/2022/11/deconstruction-ontology#needs -->

    <owl:ObjectProperty rdf:about="http://www.semanticweb.org/covon/ontologies/2022/11/deconstruction-ontology#needs">
        <rdfs:range rdf:resource="http://www.semanticweb.org/covon/ontologies/2022/11/deconstruction-ontology#PersonalProtectiveEquipment"/>
    </owl:ObjectProperty>
    


    <!-- http://www.semanticweb.org/covon/ontologies/2022/11/deconstruction-ontology#willBeDeconstructedBy -->

    <owl:ObjectProperty rdf:about="http://www.semanticweb.org/covon/ontologies/2022/11/deconstruction-ontology#willBeDeconstructedBy">
        <rdfs:subPropertyOf rdf:resource="http://www.w3.org/2002/07/owl#topObjectProperty"/>
        <rdfs:range rdf:resource="http://www.semanticweb.org/covon/ontologies/2022/11/deconstruction-ontology#DeconstructionMethod"/>
        <rdfs:comment xml:lang="de">Diese Eigenschaft ordnet einer Komponente ein Rückbauverfahren zu.</rdfs:comment>
        <rdfs:comment xml:lang="en">This property assigns a deconstruction method to a component.</rdfs:comment>
        <rdfs:label xml:lang="de">wird rückgebaut durch</rdfs:label>
    </owl:ObjectProperty>
    


    <!-- http://www.w3.org/2002/07/owl#topObjectProperty -->

    <owl:ObjectProperty rdf:about="http://www.w3.org/2002/07/owl#topObjectProperty">
        <owl:inverseOf rdf:resource="http://www.w3.org/2002/07/owl#topObjectProperty"/>
        <rdf:type rdf:resource="http://www.w3.org/2002/07/owl#SymmetricProperty"/>
        <rdf:type rdf:resource="http://www.w3.org/2002/07/owl#TransitiveProperty"/>
        <rdf:type rdf:resource="http://www.w3.org/2002/07/owl#ReflexiveProperty"/>
    </owl:ObjectProperty>
    


    <!-- http://xmlns.com/foaf/0.1/currentProject -->

    <owl:ObjectProperty rdf:about="http://xmlns.com/foaf/0.1/currentProject">
        <rdfs:range rdf:resource="http://www.w3.org/2002/07/owl#Thing"/>
        <rdfs:comment>A current project this person works on.</rdfs:comment>
        <rdfs:isDefinedBy rdf:resource="http://xmlns.com/foaf/0.1/"/>
        <rdfs:label>current project</rdfs:label>
        <ns:term_status>testing</ns:term_status>
    </owl:ObjectProperty>
    


    <!-- http://xmlns.com/foaf/0.1/depiction -->

    <owl:ObjectProperty rdf:about="http://xmlns.com/foaf/0.1/depiction">
        <owl:inverseOf rdf:resource="http://xmlns.com/foaf/0.1/depicts"/>
        <rdfs:domain rdf:resource="http://www.w3.org/2002/07/owl#Thing"/>
        <rdfs:comment>A depiction of some thing.</rdfs:comment>
        <rdfs:isDefinedBy rdf:resource="http://xmlns.com/foaf/0.1/"/>
        <rdfs:label>depiction</rdfs:label>
        <ns:term_status>testing</ns:term_status>
    </owl:ObjectProperty>
    


    <!-- http://xmlns.com/foaf/0.1/depicts -->

    <owl:ObjectProperty rdf:about="http://xmlns.com/foaf/0.1/depicts">
        <rdfs:range rdf:resource="http://www.w3.org/2002/07/owl#Thing"/>
        <rdfs:comment>A thing depicted in this representation.</rdfs:comment>
        <rdfs:isDefinedBy rdf:resource="http://xmlns.com/foaf/0.1/"/>
        <rdfs:label>depicts</rdfs:label>
        <ns:term_status>testing</ns:term_status>
    </owl:ObjectProperty>
    


    <!-- http://xmlns.com/foaf/0.1/focus -->

    <owl:ObjectProperty rdf:about="http://xmlns.com/foaf/0.1/focus">
        <rdfs:range rdf:resource="http://www.w3.org/2002/07/owl#Thing"/>
        <rdfs:comment>The underlying or &apos;focal&apos; entity associated with some SKOS-described concept.</rdfs:comment>
        <rdfs:isDefinedBy rdf:resource="http://xmlns.com/foaf/0.1/"/>
        <rdfs:label>focus</rdfs:label>
        <ns:term_status>testing</ns:term_status>
    </owl:ObjectProperty>
    


    <!-- http://xmlns.com/foaf/0.1/fundedBy -->

    <owl:ObjectProperty rdf:about="http://xmlns.com/foaf/0.1/fundedBy">
        <rdfs:domain rdf:resource="http://www.w3.org/2002/07/owl#Thing"/>
        <rdfs:range rdf:resource="http://www.w3.org/2002/07/owl#Thing"/>
        <rdfs:comment>An organization funding a project or person.</rdfs:comment>
        <rdfs:isDefinedBy rdf:resource="http://xmlns.com/foaf/0.1/"/>
        <rdfs:label>funded by</rdfs:label>
        <ns:term_status>archaic</ns:term_status>
    </owl:ObjectProperty>
    


    <!-- http://xmlns.com/foaf/0.1/homepage -->

    <owl:ObjectProperty rdf:about="http://xmlns.com/foaf/0.1/homepage">
        <rdfs:subPropertyOf rdf:resource="http://xmlns.com/foaf/0.1/isPrimaryTopicOf"/>
        <rdfs:subPropertyOf rdf:resource="http://xmlns.com/foaf/0.1/page"/>
        <rdfs:subPropertyOf>
            <rdf:Description>
                <owl:inverseOf rdf:resource="http://xmlns.com/foaf/0.1/primaryTopic"/>
            </rdf:Description>
        </rdfs:subPropertyOf>
        <rdf:type rdf:resource="http://www.w3.org/2002/07/owl#InverseFunctionalProperty"/>
        <rdfs:domain rdf:resource="http://www.w3.org/2002/07/owl#Thing"/>
        <rdfs:comment>A homepage for some thing.</rdfs:comment>
        <rdfs:isDefinedBy rdf:resource="http://xmlns.com/foaf/0.1/"/>
        <rdfs:label>homepage</rdfs:label>
        <ns:term_status>stable</ns:term_status>
    </owl:ObjectProperty>
    


    <!-- http://xmlns.com/foaf/0.1/img -->

    <owl:ObjectProperty rdf:about="http://xmlns.com/foaf/0.1/img">
        <rdfs:subPropertyOf rdf:resource="http://xmlns.com/foaf/0.1/depiction"/>
        <rdfs:subPropertyOf>
            <rdf:Description>
                <owl:inverseOf rdf:resource="http://xmlns.com/foaf/0.1/depicts"/>
            </rdf:Description>
        </rdfs:subPropertyOf>
        <rdfs:comment>An image that can be used to represent some thing (ie. those depictions which are particularly representative of something, eg. one&apos;s photo on a homepage).</rdfs:comment>
        <rdfs:isDefinedBy rdf:resource="http://xmlns.com/foaf/0.1/"/>
        <rdfs:label>image</rdfs:label>
        <ns:term_status>testing</ns:term_status>
    </owl:ObjectProperty>
    


    <!-- http://xmlns.com/foaf/0.1/isPrimaryTopicOf -->

    <owl:ObjectProperty rdf:about="http://xmlns.com/foaf/0.1/isPrimaryTopicOf">
        <rdfs:subPropertyOf rdf:resource="http://xmlns.com/foaf/0.1/page"/>
        <rdfs:subPropertyOf>
            <rdf:Description>
                <owl:inverseOf rdf:resource="http://xmlns.com/foaf/0.1/topic"/>
            </rdf:Description>
        </rdfs:subPropertyOf>
        <owl:inverseOf rdf:resource="http://xmlns.com/foaf/0.1/primaryTopic"/>
        <rdf:type rdf:resource="http://www.w3.org/2002/07/owl#InverseFunctionalProperty"/>
        <rdfs:domain rdf:resource="http://www.w3.org/2002/07/owl#Thing"/>
        <rdfs:comment>A document that this thing is the primary topic of.</rdfs:comment>
        <rdfs:isDefinedBy rdf:resource="http://xmlns.com/foaf/0.1/"/>
        <rdfs:label>is primary topic of</rdfs:label>
        <ns:term_status>stable</ns:term_status>
    </owl:ObjectProperty>
    


    <!-- http://xmlns.com/foaf/0.1/jabberID -->

    <owl:ObjectProperty rdf:about="http://xmlns.com/foaf/0.1/jabberID">
        <rdf:type rdf:resource="http://www.w3.org/2002/07/owl#InverseFunctionalProperty"/>
    </owl:ObjectProperty>
    


    <!-- http://xmlns.com/foaf/0.1/logo -->

    <owl:ObjectProperty rdf:about="http://xmlns.com/foaf/0.1/logo">
        <rdf:type rdf:resource="http://www.w3.org/2002/07/owl#InverseFunctionalProperty"/>
        <rdfs:domain rdf:resource="http://www.w3.org/2002/07/owl#Thing"/>
        <rdfs:range rdf:resource="http://www.w3.org/2002/07/owl#Thing"/>
        <rdfs:comment>A logo representing some thing.</rdfs:comment>
        <rdfs:isDefinedBy rdf:resource="http://xmlns.com/foaf/0.1/"/>
        <rdfs:label>logo</rdfs:label>
        <ns:term_status>testing</ns:term_status>
    </owl:ObjectProperty>
    


    <!-- http://xmlns.com/foaf/0.1/made -->

    <owl:ObjectProperty rdf:about="http://xmlns.com/foaf/0.1/made">
        <owl:inverseOf rdf:resource="http://xmlns.com/foaf/0.1/maker"/>
        <rdfs:range rdf:resource="http://www.w3.org/2002/07/owl#Thing"/>
        <rdfs:comment>Something that was made by this agent.</rdfs:comment>
        <rdfs:isDefinedBy rdf:resource="http://xmlns.com/foaf/0.1/"/>
        <rdfs:label>made</rdfs:label>
        <ns:term_status>stable</ns:term_status>
    </owl:ObjectProperty>
    


    <!-- http://xmlns.com/foaf/0.1/maker -->

    <owl:ObjectProperty rdf:about="http://xmlns.com/foaf/0.1/maker">
        <rdfs:domain rdf:resource="http://www.w3.org/2002/07/owl#Thing"/>
        <rdfs:comment>An agent that  made this thing.</rdfs:comment>
        <rdfs:isDefinedBy rdf:resource="http://xmlns.com/foaf/0.1/"/>
        <rdfs:label>maker</rdfs:label>
        <ns:term_status>stable</ns:term_status>
    </owl:ObjectProperty>
    


    <!-- http://xmlns.com/foaf/0.1/mbox -->

    <owl:ObjectProperty rdf:about="http://xmlns.com/foaf/0.1/mbox">
        <rdf:type rdf:resource="http://www.w3.org/2002/07/owl#InverseFunctionalProperty"/>
        <rdfs:range rdf:resource="http://www.w3.org/2002/07/owl#Thing"/>
        <rdfs:comment>A  personal mailbox, ie. an Internet mailbox associated with exactly one owner, the first owner of this mailbox. This is a &apos;static inverse functional property&apos;, in that  there is (across time and change) at most one individual that ever has any particular value for foaf:mbox.</rdfs:comment>
        <rdfs:isDefinedBy rdf:resource="http://xmlns.com/foaf/0.1/"/>
        <rdfs:label>personal mailbox</rdfs:label>
        <ns:term_status>stable</ns:term_status>
    </owl:ObjectProperty>
    


    <!-- http://xmlns.com/foaf/0.1/openid -->

    <owl:ObjectProperty rdf:about="http://xmlns.com/foaf/0.1/openid">
        <rdfs:subPropertyOf rdf:resource="http://xmlns.com/foaf/0.1/isPrimaryTopicOf"/>
        <rdfs:subPropertyOf>
            <rdf:Description>
                <owl:inverseOf rdf:resource="http://xmlns.com/foaf/0.1/primaryTopic"/>
            </rdf:Description>
        </rdfs:subPropertyOf>
        <rdf:type rdf:resource="http://www.w3.org/2002/07/owl#InverseFunctionalProperty"/>
        <rdfs:comment>An OpenID for an Agent.</rdfs:comment>
        <rdfs:isDefinedBy rdf:resource="http://xmlns.com/foaf/0.1/"/>
        <rdfs:label>openid</rdfs:label>
        <ns:term_status>testing</ns:term_status>
    </owl:ObjectProperty>
    


    <!-- http://xmlns.com/foaf/0.1/page -->

    <owl:ObjectProperty rdf:about="http://xmlns.com/foaf/0.1/page">
        <owl:inverseOf rdf:resource="http://xmlns.com/foaf/0.1/topic"/>
        <rdfs:domain rdf:resource="http://www.w3.org/2002/07/owl#Thing"/>
        <rdfs:comment>A page or document about this thing.</rdfs:comment>
        <rdfs:isDefinedBy rdf:resource="http://xmlns.com/foaf/0.1/"/>
        <rdfs:label>page</rdfs:label>
        <ns:term_status>stable</ns:term_status>
    </owl:ObjectProperty>
    


    <!-- http://xmlns.com/foaf/0.1/pastProject -->

    <owl:ObjectProperty rdf:about="http://xmlns.com/foaf/0.1/pastProject">
        <rdfs:range rdf:resource="http://www.w3.org/2002/07/owl#Thing"/>
        <rdfs:comment>A project this person has previously worked on.</rdfs:comment>
        <rdfs:isDefinedBy rdf:resource="http://xmlns.com/foaf/0.1/"/>
        <rdfs:label>past project</rdfs:label>
        <ns:term_status>testing</ns:term_status>
    </owl:ObjectProperty>
    


    <!-- http://xmlns.com/foaf/0.1/primaryTopic -->

    <owl:ObjectProperty rdf:about="http://xmlns.com/foaf/0.1/primaryTopic">
        <rdfs:subPropertyOf rdf:resource="http://xmlns.com/foaf/0.1/topic"/>
        <rdfs:subPropertyOf>
            <rdf:Description>
                <owl:inverseOf rdf:resource="http://xmlns.com/foaf/0.1/page"/>
            </rdf:Description>
        </rdfs:subPropertyOf>
        <rdf:type rdf:resource="http://www.w3.org/2002/07/owl#FunctionalProperty"/>
        <rdfs:range rdf:resource="http://www.w3.org/2002/07/owl#Thing"/>
        <rdfs:comment>The primary topic of some page or document.</rdfs:comment>
        <rdfs:isDefinedBy rdf:resource="http://xmlns.com/foaf/0.1/"/>
        <rdfs:label>primary topic</rdfs:label>
        <ns:term_status>stable</ns:term_status>
    </owl:ObjectProperty>
    


    <!-- http://xmlns.com/foaf/0.1/theme -->

    <owl:ObjectProperty rdf:about="http://xmlns.com/foaf/0.1/theme">
        <rdfs:domain rdf:resource="http://www.w3.org/2002/07/owl#Thing"/>
        <rdfs:range rdf:resource="http://www.w3.org/2002/07/owl#Thing"/>
        <rdfs:comment>A theme.</rdfs:comment>
        <rdfs:isDefinedBy rdf:resource="http://xmlns.com/foaf/0.1/"/>
        <rdfs:label>theme</rdfs:label>
        <ns:term_status>archaic</ns:term_status>
    </owl:ObjectProperty>
    


    <!-- http://xmlns.com/foaf/0.1/tipjar -->

    <owl:ObjectProperty rdf:about="http://xmlns.com/foaf/0.1/tipjar">
        <rdfs:subPropertyOf rdf:resource="http://xmlns.com/foaf/0.1/page"/>
        <rdfs:subPropertyOf>
            <rdf:Description>
                <owl:inverseOf rdf:resource="http://xmlns.com/foaf/0.1/topic"/>
            </rdf:Description>
        </rdfs:subPropertyOf>
        <rdfs:comment>A tipjar document for this agent, describing means for payment and reward.</rdfs:comment>
        <rdfs:isDefinedBy rdf:resource="http://xmlns.com/foaf/0.1/"/>
        <rdfs:label>tipjar</rdfs:label>
        <ns:term_status>testing</ns:term_status>
    </owl:ObjectProperty>
    


    <!-- http://xmlns.com/foaf/0.1/topic -->

    <owl:ObjectProperty rdf:about="http://xmlns.com/foaf/0.1/topic">
        <rdfs:range rdf:resource="http://www.w3.org/2002/07/owl#Thing"/>
        <rdfs:comment>A topic of some page or document.</rdfs:comment>
        <rdfs:isDefinedBy rdf:resource="http://xmlns.com/foaf/0.1/"/>
        <rdfs:label>topic</rdfs:label>
        <ns:term_status>testing</ns:term_status>
    </owl:ObjectProperty>
    


    <!-- http://xmlns.com/foaf/0.1/topic_interest -->

    <owl:ObjectProperty rdf:about="http://xmlns.com/foaf/0.1/topic_interest">
        <rdfs:range rdf:resource="http://www.w3.org/2002/07/owl#Thing"/>
        <rdfs:comment>A thing of interest to this person.</rdfs:comment>
        <rdfs:isDefinedBy rdf:resource="http://xmlns.com/foaf/0.1/"/>
        <rdfs:label>topic_interest</rdfs:label>
        <ns:term_status>testing</ns:term_status>
    </owl:ObjectProperty>
    


    <!-- http://xmlns.com/foaf/0.1/weblog -->

    <owl:ObjectProperty rdf:about="http://xmlns.com/foaf/0.1/weblog">
        <rdfs:subPropertyOf rdf:resource="http://xmlns.com/foaf/0.1/page"/>
        <rdfs:subPropertyOf>
            <rdf:Description>
                <owl:inverseOf rdf:resource="http://xmlns.com/foaf/0.1/topic"/>
            </rdf:Description>
        </rdfs:subPropertyOf>
        <rdf:type rdf:resource="http://www.w3.org/2002/07/owl#InverseFunctionalProperty"/>
        <rdfs:comment>A weblog of some thing (whether person, group, company etc.).</rdfs:comment>
        <rdfs:isDefinedBy rdf:resource="http://xmlns.com/foaf/0.1/"/>
        <rdfs:label>weblog</rdfs:label>
        <ns:term_status>stable</ns:term_status>
    </owl:ObjectProperty>
    


    <!-- https://w3id.org/bot#adjacentElement -->

    <owl:ObjectProperty rdf:about="https://w3id.org/bot#adjacentElement">
        <rdfs:subPropertyOf rdf:resource="https://w3id.org/bot#hasElement"/>
        <owl:propertyDisjointWith rdf:resource="https://w3id.org/bot#intersectingElement"/>
        <rdfs:comment xml:lang="de">Beziehung zwischen einer Zone und dessen angrenzenden Bauteilen. Die Bauteile begrenzen die Zone.</rdfs:comment>
        <rdfs:comment xml:lang="tr">Bir bölge ile bitişik bina parçaları arasındaki ilişki, fiziksel alanı sınırlar.</rdfs:comment>
        <rdfs:comment xml:lang="ca">Relació entre una zona i els seus elements arquitectònics adjacents, que limiten l&apos;espai físic.</rdfs:comment>
        <rdfs:comment xml:lang="es">Relación entre una zona y sus elementos arquitectónicos adyacentes, que limitan el espacio físico.</rdfs:comment>
        <rdfs:comment xml:lang="nl">Relatie tussen een zone en zijn aangrenzende gebouwelementen. Het gebouwelement begrenst de zone.</rdfs:comment>
        <rdfs:comment xml:lang="en">Relation between a zone and its adjacent building elements, bounding the zone.</rdfs:comment>
        <rdfs:comment xml:lang="fr">Relation entre une zone et ses éléments adjacents, délimitant l&apos;espace physique</rdfs:comment>
        <rdfs:comment xml:lang="sv">Relation mellan en zon och dess angränsande byggdelar, som avgränsar det fysiska utrymmet.</rdfs:comment>
        <rdfs:comment xml:lang="da">Relation mellem en zone og dens tilstødende bygningsdele, som afgrænser det fysiske rum.</rdfs:comment>
        <rdfs:comment xml:lang="it">Relazione tra una zona e i suoi elementi di costruzione adiacenti che delimitano la zona stessa.</rdfs:comment>
        <rdfs:comment xml:lang="pt">Relação entre uma zona e os elementos da construção que lhe são adjacentes, delimitando a zona.</rdfs:comment>
        <rdfs:comment xml:lang="fi">Suhde vyöhykkeen ja sen viereisten, sitä rajaavien rakennuselementtien välillä.</rdfs:comment>
        <rdfs:comment xml:lang="cs">Vztah mezi zónou a její přilehlými stavebními prvky, obklopujícími danou zónu.</rdfs:comment>
        <rdfs:comment xml:lang="sk">Vzťah medzi zónou a stavebnými prvkami obklopujúcimi túto zónu.</rdfs:comment>
        <rdfs:comment xml:lang="fa">رابطه بین یک منطقه و المانهای ساختمانی همجوارش که حدود منطقه را مشخص می کنند. </rdfs:comment>
        <rdfs:comment xml:lang="zh-cn">区域中相邻建筑构件之间的关系，以该区域为界。</rdfs:comment>
        <rdfs:isDefinedBy rdf:resource="https://w3id.org/bot#"/>
        <rdfs:label xml:lang="tr">Bitisik eleman</rdfs:label>
        <rdfs:label xml:lang="nl">aangrenzend element</rdfs:label>
        <rdfs:label xml:lang="en">adjacent element</rdfs:label>
        <rdfs:label xml:lang="sv">angränsande element</rdfs:label>
        <rdfs:label xml:lang="de">benachbartes Bauteil</rdfs:label>
        <rdfs:label xml:lang="ca">element adjacent</rdfs:label>
        <rdfs:label xml:lang="it">elemento adiacente</rdfs:label>
        <rdfs:label xml:lang="pt">elemento adjacente</rdfs:label>
        <rdfs:label xml:lang="es">elemento adyacente</rdfs:label>
        <rdfs:label xml:lang="sk">priľahlý element-prvok</rdfs:label>
        <rdfs:label xml:lang="cs">přilehlý element-prvek</rdfs:label>
        <rdfs:label xml:lang="da">tilstødende element</rdfs:label>
        <rdfs:label xml:lang="fi">viereinen elementti</rdfs:label>
        <rdfs:label xml:lang="fr">élément adjacent</rdfs:label>
        <rdfs:label xml:lang="fa">المان همجوار</rdfs:label>
        <rdfs:label xml:lang="zh-cn">相邻构件</rdfs:label>
        <ns:term_status>stable</ns:term_status>
    </owl:ObjectProperty>
    


    <!-- https://w3id.org/bot#adjacentZone -->

    <owl:ObjectProperty rdf:about="https://w3id.org/bot#adjacentZone">
        <owl:inverseOf rdf:resource="https://w3id.org/bot#adjacentZone"/>
        <rdf:type rdf:resource="http://www.w3.org/2002/07/owl#SymmetricProperty"/>
        <rdfs:domain rdf:resource="https://w3id.org/bot#Zone"/>
        <rdfs:range rdf:resource="https://w3id.org/bot#Zone"/>
        <owl:propertyDisjointWith rdf:resource="https://w3id.org/bot#intersectsZone"/>
        <rdfs:comment xml:lang="de">Beziehung zwischen zwei Zonen die eine gemeinsame Grenzfläche haben, aber sich nicht schneiden.</rdfs:comment>
        <rdfs:comment xml:lang="tr">Ortak bir arayüzü paylaşan iki bölge arasındaki bağlantı.</rdfs:comment>
        <rdfs:comment xml:lang="ca">Relació entre dues zones que comparteixen una interfície comuna, però que no interseccionen</rdfs:comment>
        <rdfs:comment xml:lang="es">Relación entre dos zonas que comparten una interfaz común, pero que no intersecan.</rdfs:comment>
        <rdfs:comment xml:lang="nl">Relatie tussen twee zones die een interface delen, maar niet doorsnijdend zijn</rdfs:comment>
        <rdfs:comment xml:lang="fr">Relation entre deux zones partageant une interface commune, sans intersection</rdfs:comment>
        <rdfs:comment xml:lang="sv">Relation mellan två zoner som delar ett gemensamt gränssnitt men som inte korsar varandra.</rdfs:comment>
        <rdfs:comment xml:lang="da">Relation mellem to zoner, der deler en fælles grænseflade.</rdfs:comment>
        <rdfs:comment xml:lang="en">Relationship between two zones that share a common interface, but do not intersect.</rdfs:comment>
        <rdfs:comment xml:lang="it">Relazione tra due zone che condividono un&apos;interfaccia senza però intersecarsi.</rdfs:comment>
        <rdfs:comment xml:lang="pt">Relação entre duas zonas que partilham um interface comum mas que não se intersectam.</rdfs:comment>
        <rdfs:comment xml:lang="fi">Suhde kahden vyöhykkeen välillä, jotka jakavat yhteisen rajapinnan mutta eivät leikkaa toisiaan.</rdfs:comment>
        <rdfs:comment xml:lang="cs">Vztah mezi dvěmi zónami, které se dotýkají, ale neprotínají se.</rdfs:comment>
        <rdfs:comment xml:lang="sk">Vzťah medzi dvomi zónami, ktoré sa dotýkajú, ale nepretínajú sa.</rdfs:comment>
        <rdfs:comment xml:lang="fa">رابطه بین دو منطقه که یک رابط مشترک دارند، ولی منقطع نیستند.</rdfs:comment>
        <rdfs:comment xml:lang="zh-cn">两个区域之间共享公共界面但不相交的关系</rdfs:comment>
        <rdfs:isDefinedBy rdf:resource="https://w3id.org/bot#"/>
        <rdfs:label xml:lang="tr">Bitisik bölge</rdfs:label>
        <rdfs:label xml:lang="nl">aangrenzende zone</rdfs:label>
        <rdfs:label xml:lang="en">adjacent zone</rdfs:label>
        <rdfs:label xml:lang="de">angrenzende Zone</rdfs:label>
        <rdfs:label xml:lang="sv">angränsande zon</rdfs:label>
        <rdfs:label xml:lang="sk">priľahlá zóna</rdfs:label>
        <rdfs:label xml:lang="cs">přilehlá zóna</rdfs:label>
        <rdfs:label xml:lang="da">tilstødende zone</rdfs:label>
        <rdfs:label xml:lang="fi">viereinen vyöhyke</rdfs:label>
        <rdfs:label xml:lang="it">zona adiacente</rdfs:label>
        <rdfs:label xml:lang="ca">zona adjacent</rdfs:label>
        <rdfs:label xml:lang="pt">zona adjacente</rdfs:label>
        <rdfs:label xml:lang="es">zona adyacente</rdfs:label>
        <rdfs:label xml:lang="fr">zone adjacente</rdfs:label>
        <rdfs:label xml:lang="fa">منطقه همجوار</rdfs:label>
        <rdfs:label xml:lang="zh-cn">相邻区域</rdfs:label>
        <ns:term_status>stable</ns:term_status>
        <schema1:domainIncludes rdf:resource="https://w3id.org/bot#Building"/>
        <schema1:domainIncludes rdf:resource="https://w3id.org/bot#Site"/>
        <schema1:domainIncludes rdf:resource="https://w3id.org/bot#Space"/>
        <schema1:domainIncludes rdf:resource="https://w3id.org/bot#Storey"/>
        <schema1:rangeIncludes rdf:resource="https://w3id.org/bot#Building"/>
        <schema1:rangeIncludes rdf:resource="https://w3id.org/bot#Site"/>
        <schema1:rangeIncludes rdf:resource="https://w3id.org/bot#Space"/>
        <schema1:rangeIncludes rdf:resource="https://w3id.org/bot#Storey"/>
    </owl:ObjectProperty>
    


    <!-- https://w3id.org/bot#containsElement -->

    <owl:ObjectProperty rdf:about="https://w3id.org/bot#containsElement">
        <rdfs:subPropertyOf rdf:resource="https://w3id.org/bot#hasElement"/>
        <owl:propertyChainAxiom rdf:parseType="Collection">
            <rdf:Description rdf:about="https://w3id.org/bot#containsZone"/>
            <rdf:Description rdf:about="https://w3id.org/bot#containsElement"/>
        </owl:propertyChainAxiom>
        <rdfs:comment xml:lang="de">Beziehung einer Zone zu einem Bauteil, dass es enthält.</rdfs:comment>
        <rdfs:comment xml:lang="tr">Bir bölgede bulunan bir bina parçasıyla ilişki.</rdfs:comment>
        <rdfs:comment xml:lang="ca">Relació a un element arquitectònic contingut en una zona.</rdfs:comment>
        <rdfs:comment xml:lang="es">Relación a un elemento arquitectónico contenido en una zona.</rdfs:comment>
        <rdfs:comment xml:lang="nl">Relatie tussen zone en een gebouwelement bevat in die zone.</rdfs:comment>
        <rdfs:comment xml:lang="da">Relation til en bygningsdel, som er indeholdt i en zone.</rdfs:comment>
        <rdfs:comment xml:lang="sv">Relation till en byggdel som inryms i en zon.</rdfs:comment>
        <rdfs:comment xml:lang="en">Relation to a building element contained in a zone.</rdfs:comment>
        <rdfs:comment xml:lang="fr">Relation à définir entre un élément de bâti et la zone le contenant</rdfs:comment>
        <rdfs:comment xml:lang="it">Relazione con elementi di costruzione contenuti in una zona.</rdfs:comment>
        <rdfs:comment xml:lang="pt">Relação com um elemento da construção contido numa zona.</rdfs:comment>
        <rdfs:comment xml:lang="fi">Suhde vyöhykkeen sisältämään rakennuselementtiin.</rdfs:comment>
        <rdfs:comment xml:lang="cs">Vztah k stavebnímu prvku obsaženém v zóně.</rdfs:comment>
        <rdfs:comment xml:lang="sk">Vzťah k stavebnému prvku, obsiahnutom v zóne.</rdfs:comment>
        <rdfs:comment xml:lang="fa">رابطه بین یک منطقه با المان ساختمانی که آنرا در بر گرفته است.</rdfs:comment>
        <rdfs:comment xml:lang="zh-cn">区域中包含的建筑构件的关系。</rdfs:comment>
        <rdfs:isDefinedBy rdf:resource="https://w3id.org/bot#"/>
        <rdfs:label xml:lang="tr">Eleman icerir</rdfs:label>
        <rdfs:label xml:lang="nl">bevat element</rdfs:label>
        <rdfs:label xml:lang="pt">comtém elemento</rdfs:label>
        <rdfs:label xml:lang="en">contains element</rdfs:label>
        <rdfs:label xml:lang="es">contiene elemento</rdfs:label>
        <rdfs:label xml:lang="it">contiene elemento</rdfs:label>
        <rdfs:label xml:lang="fr">contient élément</rdfs:label>
        <rdfs:label xml:lang="ca">conté un element</rdfs:label>
        <rdfs:label xml:lang="de">enthält Bauteil</rdfs:label>
        <rdfs:label xml:lang="da">indeholder bygningsdel</rdfs:label>
        <rdfs:label xml:lang="sv">innehåller byggdel</rdfs:label>
        <rdfs:label xml:lang="cs">obsahuje element-prvek</rdfs:label>
        <rdfs:label xml:lang="sk">obsahuje element-prvok</rdfs:label>
        <rdfs:label xml:lang="fi">sisältää elementin</rdfs:label>
        <rdfs:label xml:lang="fa">المان دربرگیرنده</rdfs:label>
        <rdfs:label xml:lang="zh-cn">包含构件</rdfs:label>
        <ns:term_status>stable</ns:term_status>
    </owl:ObjectProperty>
    


    <!-- https://w3id.org/bot#containsZone -->

    <owl:ObjectProperty rdf:about="https://w3id.org/bot#containsZone">
        <rdf:type rdf:resource="http://www.w3.org/2002/07/owl#TransitiveProperty"/>
        <rdfs:domain rdf:resource="https://w3id.org/bot#Zone"/>
        <rdfs:range rdf:resource="https://w3id.org/bot#Zone"/>
        <rdfs:comment xml:lang="de">Beziehung zwischen Zonen, wobei eine die andere enthält. Zum Beispiel kann eine Raumzone in einer Geschossszone enthalten sein, die wiederrum in einer Gebäudezone enthalten ist. bot:containsZone is eine transitive Beziehung, dass heisst zwischen der Raumzone im vorherigen Beispiel und der Gebäudezone besteht auch die Beziehung bot:containsZone.</rdfs:comment>
        <rdfs:comment xml:lang="tr">Daha büyük bir bölgedeki içerinde yeralan alt bölgelerin birbirleriyle bağlantısı. Örneğin, bir arsa bölgesi, bir bina bölgesini icerebilir ve bir bina bölgesi bir oda bölgesini icerebilir. bot:includeZone geçişli bir özelliktir, yani önceki örnekteki boşluk bölgesi de bina bölgesinde yer alır.</rdfs:comment>
        <rdfs:comment xml:lang="ca">Relació entre subzones amb una zona principal. Per exemple, una zona espacial podria estar continguda en una zona de pis que a la vegada està continguda en una zona d&apos;edifici. bot:containsZone és una propietat transitiva. Això implica que en l&apos;exemple anterior es manté una relació entre la zona espacial i la zona de edifici a través de bot:containsZone.</rdfs:comment>
        <rdfs:comment xml:lang="es">Relación entre subzonas con una una zona principal. Por ejemplo, una zona espacial podría estar contenida en una zona de piso que a su vez está contenida en una zona de edificio. bot:containsZone es una propiedad transitiva. Esto implica que en el ejemplo anterior se mantiene una relación entre la zona espacial y la zona de edificio a través de bot:containsZone.</rdfs:comment>
        <rdfs:comment xml:lang="nl">Relatie tussen subzones van een hoofd zone. Een ruimtezone kan bijvoorbeeld worden bevat door een verdiepingszone, die wederom bevat wordt door een gebouwzone. bot:containsZone is een transitieve eigenschap, wat betekent dat in het vorige voorbeeld de ruimtezone ook bevat wordt door de gebouwzone.</rdfs:comment>
        <rdfs:comment xml:lang="fr">Relation entre les sous-zones composant une zone plus grande. Cette propriété est transitive.</rdfs:comment>
        <rdfs:comment xml:lang="da">Relation til underzoner i en større zone. En rum-zone kan for eksempel være indeholdt i en etage-zone som ydermere er indeholdt i en bygnings-zone. bot:containsZone er en transitiv egenskab, hvilket betyder at rum-zonen i det forrige eksempel også er indeholdt i bygnings-zonen.</rdfs:comment>
        <rdfs:comment xml:lang="sv">Relation till delzoner i en huvudzon. En rumszon kan till exempel inrymmas i en våningszon som i sin tur inryms i en byggnadszon. bot:containsZone är en transitiv relation vilket i exemplet betyder att rumszonen också inryms i byggnadszonen.</rdfs:comment>
        <rdfs:comment xml:lang="en">Relationship to the subzones of a major zone. A space zone could for instance be contained in a storey zone which is further contained in a building zone. bot:containsZone is a transitive property. This implies that in the previous example a bot:containsZone relationship holds between the space zone and the building zone.</rdfs:comment>
        <rdfs:comment xml:lang="it">Relazione tra una zona e una sotto-zona. Per esempio, una zona spaziale può essere contenuta nella zona di un piano che a sua volta è contenuto nella zona di un edificio. bot:containsZone è una proprietà transitiva. Ciò implica che nel precedente esempio la relazione bot:containsZone si verifica anche tra la zona spaziale e la zona dell&apos;edificio.</rdfs:comment>
        <rdfs:comment xml:lang="pt">Relação entre subzonas de uma zona maior. Uma zona espacial pode, por exemplo, estar contida na zona de um piso que está, por sua vez, contida na zona de um edifício.
bot:containsZone é uma propriedade transitiva. Isto implica que, no exemplo anterior, exista uma relação bot:containsZone entre uma zona espacial e a zona do edifício.</rdfs:comment>
        <rdfs:comment xml:lang="fi">Suhde päävyöhykkeen osavyöhykkeisiin. Tila voi esimerkiksi sisältyä kerrokseen, joka puolestaan voi sisältyä rakennukseen. bot:containsZone on transitiivinen ominaisuus. Tästä seuraa, että edellisessä esimerkissä myös rakennuksen ja tilan välillä pätee bot:containsZone.</rdfs:comment>
        <rdfs:comment xml:lang="cs">Vztah hlavní zóny k pod-zónám. Prostorová zóna může být napříklat umístěna v zóně podlaží, která jako zóna je umístěna v zóně budova. bot:containsZone je přenositelná vlastnost, co znamená, že daná vlastnost vyšší zóny v dané hierarchii se promítá i do zón které jsou součástí vyšší zóny.</rdfs:comment>
        <rdfs:comment xml:lang="sk">Vzťah hlavnej zóny k pod-zónam. Priestorová zóna môže napríklad byť umiestnená v zóne podlažia, ktoré ako zóna môže byť ďalej umiestnené v zóne budovy. bot:containsZone je prenositeľná vlastnost, ktorá znamená, že pokiaľ väčšia zóna A je v zóne budova, aj menšie zóny, ktorú zóna A obsahuje, sú v budove.</rdfs:comment>
        <rdfs:comment xml:lang="fa">رابطه با زیر منطقه های یک منطقه اصلی. به عنوان مثال یک منطقه فضایی می تواند در یک منطقه طبقه قرار گرفته باشد که آن به خودی خود در یک منطقه ساختمان قرار گرفته. رابطه‌ی  bot:containsZone یک رابطه‌ی انتقالی است. به این معنا که در مثال قبلی رابطه‌ی bot:containsZone بین بخش فضا و بخش ساختمان نیز برقرار میشود.</rdfs:comment>
        <rdfs:comment xml:lang="zh-cn">主要区域和其子区域的从属关系。 空间区域实例可以包含在楼层区域中，该楼层区域进一步包含在建筑物区域中。 bot：containsZone是传递属性。 这意味着在前面的示例中，空间区域和建筑物区域之间也保持着bot：containsZone关系。</rdfs:comment>
        <rdfs:isDefinedBy rdf:resource="https://w3id.org/bot#"/>
        <rdfs:label xml:lang="tr">Bölge icerir</rdfs:label>
        <rdfs:label xml:lang="nl">bevat zone</rdfs:label>
        <rdfs:label xml:lang="en">contains zone</rdfs:label>
        <rdfs:label xml:lang="es">contiene zona</rdfs:label>
        <rdfs:label xml:lang="it">contiene zona</rdfs:label>
        <rdfs:label xml:lang="fr">contient zone</rdfs:label>
        <rdfs:label xml:lang="ca">conté zona</rdfs:label>
        <rdfs:label xml:lang="pt">contém zona</rdfs:label>
        <rdfs:label xml:lang="de">enthält Zone</rdfs:label>
        <rdfs:label xml:lang="da">indeholder zone</rdfs:label>
        <rdfs:label xml:lang="sv">innehåller zon</rdfs:label>
        <rdfs:label xml:lang="cs">obsahuje zónu</rdfs:label>
        <rdfs:label xml:lang="sk">obsahuje zónu</rdfs:label>
        <rdfs:label xml:lang="fi">sisältää vyöhykkeen</rdfs:label>
        <rdfs:label xml:lang="fa">منطقه دربرگیرنده</rdfs:label>
        <rdfs:label xml:lang="zh-cn">包含区域</rdfs:label>
        <ns:term_status>stable</ns:term_status>
        <schema1:domainIncludes rdf:resource="https://w3id.org/bot#Building"/>
        <schema1:domainIncludes rdf:resource="https://w3id.org/bot#Site"/>
        <schema1:domainIncludes rdf:resource="https://w3id.org/bot#Space"/>
        <schema1:domainIncludes rdf:resource="https://w3id.org/bot#Storey"/>
        <schema1:rangeIncludes rdf:resource="https://w3id.org/bot#Building"/>
        <schema1:rangeIncludes rdf:resource="https://w3id.org/bot#Site"/>
        <schema1:rangeIncludes rdf:resource="https://w3id.org/bot#Space"/>
        <schema1:rangeIncludes rdf:resource="https://w3id.org/bot#Storey"/>
    </owl:ObjectProperty>
    


    <!-- https://w3id.org/bot#hasBuilding -->

    <owl:ObjectProperty rdf:about="https://w3id.org/bot#hasBuilding">
        <rdfs:subPropertyOf rdf:resource="https://w3id.org/bot#containsZone"/>
        <rdfs:domain rdf:resource="https://w3id.org/bot#Zone"/>
        <rdfs:range rdf:resource="https://w3id.org/bot#Building"/>
        <rdfs:comment xml:lang="de">Beziehung zwischen Gebäuden, die in einer Zone enthalten sind. Oft ist hier die rdfs:domain eine Instanz von bot:Site.</rdfs:comment>
        <rdfs:comment xml:lang="tr">Bir bölgeye dahil binalara ile ilişkisi. Bot:hasBuilding için tipik etki alanları bot:Site örnekleridir.</rdfs:comment>
        <rdfs:comment xml:lang="ca">Relació amb els edificis continguts en una zona. Els dominis típics de bot:hasBuilding són instàncies de bot:Site</rdfs:comment>
        <rdfs:comment xml:lang="es">Relación con los edificios contenidos en una zona. Los dominios típicos de bot:hasBuilding son instancias de bot:Site.</rdfs:comment>
        <rdfs:comment xml:lang="nl">Relatie tot gebouwen die zich in een zone bevinden. De typische domeinen van bot:hasBuilding zijn instanties van bot:Site</rdfs:comment>
        <rdfs:comment xml:lang="da">Relation til bygninger indeholdt i en zone. De typiske domæner for bot:hasBuilding er forekomster af bot:Site.</rdfs:comment>
        <rdfs:comment xml:lang="sv">Relation till byggnader som inryms i en zon. Typiska domäner för bot:hasBuilding är förekomster av bot:Site.</rdfs:comment>
        <rdfs:comment xml:lang="en">Relation to buildings contained in a zone. The typical domains of bot:hasBuilding are instances of bot:Site.</rdfs:comment>
        <rdfs:comment xml:lang="fr">Relation à définir entre les bâtiments d&apos;une même zone. Cette propriété s&apos;applique typiquement sur des instances de bot:Site.</rdfs:comment>
        <rdfs:comment xml:lang="it">Relazione con gli edifici contenuti in una zona. Il tipico dominio di bot:hasBuilding è bot:Site.</rdfs:comment>
        <rdfs:comment xml:lang="pt">Relação com edifícios contidos numa zona. Os domínios típicos de bot:hasBuilding são instâncias de bot:Site.</rdfs:comment>
        <rdfs:comment xml:lang="fi">Suhde vyöhykkeeseen kuuluviin rakennuksiin. Tyypillinen lähtöjoukko on luokan bot:Site instanssit.</rdfs:comment>
        <rdfs:comment xml:lang="cs">Vztah budov které jsou přilehlé k zóně. Typickým příkladem je bot:hasBuilding která je instancí bot:Site tzn. staveniště (stav. pozemeek) má budovu, budova stojí na pozemku.</rdfs:comment>
        <rdfs:comment xml:lang="sk">Vzťah budovy a pozemku, na ktorom stojí. Typická doména bot:hasBuilding je inštanciou bot:Site. Tzn. stavenisko(stavebný pozemok) má budovu.</rdfs:comment>
        <rdfs:comment xml:lang="fa">ارتباط  با ساختمانهابی که دربرگرفته شده‌اند. دامنه اصلی bot:hasBuilding عنصرهایی از جنس bot:Site هستند.</rdfs:comment>
        <rdfs:comment xml:lang="zh-cn">区域中含有建筑的关系。 bot：hasBuilding的典型使用范围是bot：Site中的实例。</rdfs:comment>
        <rdfs:isDefinedBy rdf:resource="https://w3id.org/bot#"/>
        <rdfs:label xml:lang="tr">Binası var</rdfs:label>
        <rdfs:label xml:lang="fr">contient bâtiment</rdfs:label>
        <rdfs:label xml:lang="it">ha edificio</rdfs:label>
        <rdfs:label xml:lang="sv">har byggnad</rdfs:label>
        <rdfs:label xml:lang="da">har bygning</rdfs:label>
        <rdfs:label xml:lang="en">has building</rdfs:label>
        <rdfs:label xml:lang="de">hat Gebäude</rdfs:label>
        <rdfs:label xml:lang="nl">heeft gebouw</rdfs:label>
        <rdfs:label xml:lang="cs">má budovu</rdfs:label>
        <rdfs:label xml:lang="sk">má budovu</rdfs:label>
        <rdfs:label xml:lang="fi">omaa rakennuksen</rdfs:label>
        <rdfs:label xml:lang="pt">tem edifício</rdfs:label>
        <rdfs:label xml:lang="es">tiene edificio</rdfs:label>
        <rdfs:label xml:lang="ca">té edifici</rdfs:label>
        <rdfs:label xml:lang="fa">ساختمان دارد</rdfs:label>
        <rdfs:label xml:lang="zh-cn">包含建筑</rdfs:label>
        <ns:term_status>stable</ns:term_status>
        <schema1:domainIncludes rdf:resource="https://w3id.org/bot#Site"/>
    </owl:ObjectProperty>
    


    <!-- https://w3id.org/bot#hasElement -->

    <owl:ObjectProperty rdf:about="https://w3id.org/bot#hasElement">
        <rdfs:domain rdf:resource="https://w3id.org/bot#Building"/>
        <rdfs:domain rdf:resource="https://w3id.org/bot#Zone"/>
        <rdfs:range rdf:resource="https://w3id.org/bot#Element"/>
        <owl:propertyChainAxiom rdf:parseType="Collection">
            <rdf:Description rdf:about="https://w3id.org/bot#containsZone"/>
            <rdf:Description rdf:about="https://w3id.org/bot#hasElement"/>
        </owl:propertyChainAxiom>
        <rdfs:comment xml:lang="de">Beziehung zwischen einer Zone und einem Bauteil, dass entweder in der Zone enthalten ist, angrenzend ist, oder sich mit ihr schneidet. Diese Beziehung sollte nicht explizit benutzt werden, sondern ergibt sich implizit aus den Unterbeziehungen. Es ermöglicht, zum Beispiel, dass mit einer Abfrage alle Türen eines Gebäudes, die sich mit einer Zone schneiden ermittelt werden können.</rdfs:comment>
        <rdfs:comment xml:lang="tr">Bir Bölgeyi, Bölgenin içinde veya yanında bulunan bir bina parçasına bağlar. Bu ilişkinin açık bir şekilde ifade edilmesi değil, alt özellikleri türetilmesi amaçlanmaktadır. Örneğin, bunların binadaki odalara bitişik ya da bitişik olduğu göz önüne alındığında, bir binadaki tüm kapılar için bir sorgu&apos;ya izin verecektir.</rdfs:comment>
        <rdfs:comment xml:lang="it">Collega una zona ad un elemento che è contenuto, adiacente o intersecante la zona stessa. Non si prevede l&apos;uso esplicito di questa relazione che deve essere inferita dalle sue sotto-proprietà. Per esempio, permette di cercare tutte le porte di un edificio dato che sono adiacenti agli spazi di un edificio.</rdfs:comment>
        <rdfs:comment xml:lang="da">Forbinder en Zone til en bygningsdel der enten er indeholdt i eller tilstødende til zonen. Det er ikke hensigten at denne relation angives eksplicit, men at den udledes af dennes underegneskaber. Det vil for eksempel tillade en forespørgsel på alle døre i en bygning givet at disse er enten tilstødende eller indeholdt i rum i bygningen.</rdfs:comment>
        <rdfs:comment xml:lang="fi">Liittää vyöhykkeen (bot:Zone) elementtiin (bot:Element) joka on joko vyöhykkeen sisällä tai vierellä, tai leikkaa sen. Tätä suhdetta ei ole tarkoitus käyttää eksplisiittisesti, vaan se on pääteltävissä sen alaominaisuuksista. Mahdollistaa esimerkiksi kaikkien rakennuksen ovien hakemisen, kunhan ovet on merkitty rakennuksen tilojen viereisiksi elementeiksi (bot:adjacentElement).</rdfs:comment>
        <rdfs:comment xml:lang="en">Links a Zone to an Element that is either contained in, adjacent to or intersecting with the Zone. The intended use of this relationship is not to be stated explicitly, but to be inferred from its sub-properties. It will, for example, allow one to query for all the doors of a building given that they have an adjacency to spaces of the building.</rdfs:comment>
        <rdfs:comment xml:lang="sv">Länkar en Zon till en Byggnadsdel som antingen inryms i eller ligger jämte zonen. Den här relationen är inte avseddd att uttryckas explicit, utan den kommer att härledas från under-relationer. Detta möjliggör till exempel att man kan fråga efter samtliga dörrar i en byggnad givet att de ligger i anslutning till utrymmen i byggnaden.</rdfs:comment>
        <rdfs:comment xml:lang="cs">Napojuje zónu na stavební prvek, který se buďto nachází v dané zóně, nebo je na její rozhraní. Využitelnost tohoto vztahu není daná explicitně, ale je vyvozená z vlastností zúčastněných prvků. Například to umožní vyhledat všechny dveře, které se dotýkají konkrétních zón.</rdfs:comment>
        <rdfs:comment xml:lang="sk">Napojuje zónu na stavebný prvok, ktorý sa buď nachádza v danej zóne alebo je na jej rozhraní. Využitie tohto vzťahu nie je definované explicitne, ale je vyvodené z vlastností zúčastnených prvkov. Napríklad to umožní vyhľadať všetky dvere v budove, ktoré sa dotýkajú nejakých zón.</rdfs:comment>
        <rdfs:comment xml:lang="pt">Relaciona uma zona com um elemento que está contido em, é adjacente ou intersecta a zona. Não se pretende que esta relação seja declarada explicitamente mas que seja inferida através das suas sub-propriedades. Esta propriedade permitirá, por exemplo, que se faça um query a todas as portas de um edifício que sejam adjacentes a espaços do edifício.</rdfs:comment>
        <rdfs:comment xml:lang="fr">Relie une zone à un élément qui est soit contenu dans la zone, adjacent à celle-ci, ou intersectant. L&apos;utilisation prévue de cette relation ne doit pas être indiquée explicitement, mais doit être déduite de ses sous-propriétés. Elle permettra, par exemple, d&apos;interroger toutes les portes d&apos;un bâtiment si elles sont adjacentes à certains des espaces du bâtiment.</rdfs:comment>
        <rdfs:comment xml:lang="nl">Verbindt een bot:Zone instantie met een bot:Element instantie die er ofwel door bevat wordt, aangrenzend aan is of snijdend mee is. Het is aangeraden om deze relatie niet expliciet te maken, maar af te leiden uit het gebruik van zijn sub relaties. Deze relatie maakt het bijvoorbeeld mogelijk om alle deuren van een gebouw op te vragen als die aangrenzend gedefinieerd zijn aan de ruimtes van het gebouw.</rdfs:comment>
        <rdfs:comment xml:lang="ca">Vincula una zona a un element que està contingut en, o és adjacent a, o interseca amb la zona. L&apos;ús previst d&apos;aquesta relació no s&apos;ha d&apos;establir explícitament, sinó inferir-se de les seves subpropietats. Permetrà, per exemple, consultar totes les portes d&apos;un edifici donat que tenen una adjacència als espais de l&apos;edifici.</rdfs:comment>
        <rdfs:comment xml:lang="es">Vincula una zona a un elemento que está contenido en, o es adyacente a, o interseca con la zona. El uso previsto de esta relación no es su definición explícita, sino inferirse de sus subpropiedades. Permitirá, por ejemplo, consultar todas las puertas de un edificio dado que tienen una adyacencia a los espacios del edificio.</rdfs:comment>
        <rdfs:comment xml:lang="fa">رابطه یک منطقه با المانی که یا توسط منطقه در برگرفته شده و یا همجوار است. کاربرد این رابطه نه لزوماً به صورت مستقیم که بلکه برای نتیجه‌گیری حاصل از زیر-روابط ابراز شده است.این رابطه، به عنوان مثال، امکان استعلام (query) از همه درهای یک ساختمان که در مجاورت فضای خاصی هستند را فراهم می کند.</rdfs:comment>
        <rdfs:comment xml:lang="zh-cn">将区域链接到包含在区域中或附近的构件。 该关系的预期用途不是明确说明的，而是要从其子属性中推断出来。例如，如果构件与建筑物的空间相邻，可以借此查询建筑物的所有门。</rdfs:comment>
        <rdfs:isDefinedBy rdf:resource="https://w3id.org/bot#"/>
        <rdfs:label xml:lang="tr">Elemanı var</rdfs:label>
        <rdfs:label xml:lang="fr">a élément</rdfs:label>
        <rdfs:label xml:lang="es">alberga elemento</rdfs:label>
        <rdfs:label xml:lang="it">ha elemento</rdfs:label>
        <rdfs:label xml:lang="da">har element</rdfs:label>
        <rdfs:label xml:lang="en">has element</rdfs:label>
        <rdfs:label xml:lang="de">hat Bauteil</rdfs:label>
        <rdfs:label xml:lang="nl">heeft element</rdfs:label>
        <rdfs:label xml:lang="cs">má element</rdfs:label>
        <rdfs:label xml:lang="sk">má element</rdfs:label>
        <rdfs:label xml:lang="fi">omaa elementin</rdfs:label>
        <rdfs:label xml:lang="pt">tem elemento</rdfs:label>
        <rdfs:label xml:lang="ca">té element</rdfs:label>
        <rdfs:label xml:lang="sv">värd för element</rdfs:label>
        <rdfs:label xml:lang="fa">المان دارد</rdfs:label>
        <rdfs:label xml:lang="zh-cn">含构件</rdfs:label>
        <ns:term_status>stable</ns:term_status>
    </owl:ObjectProperty>
    


    <!-- https://w3id.org/bot#hasSpace -->

    <owl:ObjectProperty rdf:about="https://w3id.org/bot#hasSpace">
        <rdfs:subPropertyOf rdf:resource="https://w3id.org/bot#containsZone"/>
        <rdfs:domain rdf:resource="https://w3id.org/bot#Zone"/>
        <rdfs:range rdf:resource="https://w3id.org/bot#Space"/>
        <rdfs:comment xml:lang="de">Beziehung von Räumen, die sich in einer Zone befinden. Oft ist die rdfs:domain eine Instanz von bot:Storey oder bot:Building.</rdfs:comment>
        <rdfs:comment xml:lang="tr">Bir bölgede bulunan odalarla ilişkisi. Bot:hasSpace için tipik etki alanları bot:Building ve bot:Storey örnekleridir.</rdfs:comment>
        <rdfs:comment xml:lang="ca">Relació a espais continguts en una zona. Els dominis típics de bot:hasSpace són instàncies de bot:Storey o bot:Building.</rdfs:comment>
        <rdfs:comment xml:lang="es">Relación a espacios contenidos en una zona. Los dominios típicos de bot:hasSpace son instancias de bot:Storey o bot:Building.</rdfs:comment>
        <rdfs:comment xml:lang="nl">Relatie tot ruimtes die zich in een zone bevinden. De typische domeinen van bot:hasSpace zijn instanties van bot:Storey of bot:Building.</rdfs:comment>
        <rdfs:comment xml:lang="da">Relation til rum indeholdt i en zone. De typiske domæner for bot:hasSpace er forekomster af bot:Storey og bot:Building.</rdfs:comment>
        <rdfs:comment xml:lang="sv">Relation till rum som inryms i en zon. Typiska domäner för bot:hasSpace är förekomster av bot:Storey och bot:Building.</rdfs:comment>
        <rdfs:comment xml:lang="en">Relation to spaces contained in a zone. The typical domains of bot:hasSpace are instances of bot:Storey or bot:Building.</rdfs:comment>
        <rdfs:comment xml:lang="fr">Relation à définir entre les pièces d&apos;une même zone. Cette propriété s&apos;applique typiquement sur des instances de bot:Storey et bot:Building.</rdfs:comment>
        <rdfs:comment xml:lang="it">Relazione con gli spazi contenuti in una zona. Il tipico dominio di bot:hasSpace è l&apos;unione di bot:Storey e bot:Building.</rdfs:comment>
        <rdfs:comment xml:lang="pt">Relação com espaços contidos numa zona. Os domínios típicos de bot:hasSpace são instâncias de bot:Storey ou de bot:Building.</rdfs:comment>
        <rdfs:comment xml:lang="fi">Suhde vyöhykkeeseen kuuluviin tiloihin. Tyypillinen lähtöjoukko ovat luokkien bot:Storey tai bot:Building instanssit.</rdfs:comment>
        <rdfs:comment xml:lang="cs">Vztah prostorů nacházejících se v zóně a dané zóny. Typická doména bot:hasSpace jsou instance bot:Storey a bot:Building.</rdfs:comment>
        <rdfs:comment xml:lang="sk">Vzťah priestorov nachádzajúcich sa v zóne a danej zóny. Typická doména bot:hasSpace sú inštancie bot:Storey a bot:Buuilding.</rdfs:comment>
        <rdfs:comment xml:lang="fa">ارتباط با فضاهایی که دربرگرفته شده‌اند. دامنه‌ی اصلی  bot:hasSpace عنصرهایی از جنس bot:Building  وbot:Storey هستند.</rdfs:comment>
        <rdfs:comment xml:lang="zh-cn">区域含有空间的关系。 bot：hasSpace的典型使用范围是bot：Storey和bot：Building中的实例。</rdfs:comment>
        <rdfs:isDefinedBy rdf:resource="https://w3id.org/bot#"/>
        <rdfs:label xml:lang="tr">Odası var</rdfs:label>
        <rdfs:label xml:lang="fr">contient pièce</rdfs:label>
        <rdfs:label xml:lang="it">ha spazio</rdfs:label>
        <rdfs:label xml:lang="da">har rum</rdfs:label>
        <rdfs:label xml:lang="sv">har rum</rdfs:label>
        <rdfs:label xml:lang="en">has space</rdfs:label>
        <rdfs:label xml:lang="de">hat Raum</rdfs:label>
        <rdfs:label xml:lang="nl">heeft ruimte</rdfs:label>
        <rdfs:label xml:lang="sk">má priestor</rdfs:label>
        <rdfs:label xml:lang="cs">má prostor</rdfs:label>
        <rdfs:label xml:lang="fi">omaa tilan</rdfs:label>
        <rdfs:label xml:lang="pt">tem espaço</rdfs:label>
        <rdfs:label xml:lang="es">tiene espacio</rdfs:label>
        <rdfs:label xml:lang="ca">té espai</rdfs:label>
        <rdfs:label xml:lang="fa">فضا دارد</rdfs:label>
        <rdfs:label xml:lang="zh-cn">包含空间</rdfs:label>
        <ns:term_status>stable</ns:term_status>
        <schema1:domainIncludes rdf:resource="https://w3id.org/bot#Storey"/>
    </owl:ObjectProperty>
    


    <!-- https://w3id.org/bot#hasStorey -->

    <owl:ObjectProperty rdf:about="https://w3id.org/bot#hasStorey">
        <rdfs:subPropertyOf rdf:resource="https://w3id.org/bot#containsZone"/>
        <rdfs:domain rdf:resource="https://w3id.org/bot#Zone"/>
        <rdfs:range rdf:resource="https://w3id.org/bot#Storey"/>
        <rdfs:comment xml:lang="de">Beziehung zwischen Geschossen, die in einer Zone enthalten sind. Oft ist die rdfs:domain eine Instanz von bot:Building.</rdfs:comment>
        <rdfs:comment xml:lang="tr">Bir bölgede bulunan katlarla ilişkisi. Bot:hasStorey için tipik etki alanları bot:Building örnekleridir.</rdfs:comment>
        <rdfs:comment xml:lang="ca">Relació amb els pisos continguts en una zona. Els dominis típics de bot: hasStorey son instàncies de bot:Building.</rdfs:comment>
        <rdfs:comment xml:lang="es">Relación con los pisos contenidos en una zona. Los dominios típicos de bot:hasStorey son instancias de bot:Building.</rdfs:comment>
        <rdfs:comment xml:lang="nl">Relatie tot de verdiepingen die zich in een zone bevinden. De typische domeinen van bot:hasStorey zijn instanties van bot:Building.</rdfs:comment>
        <rdfs:comment xml:lang="sv">Relation som uttrycker vilka våningar som finns i en Zon. Används typiskt med instanser av bot:Building.</rdfs:comment>
        <rdfs:comment xml:lang="da">Relation til etager indeholdt i en zone. De typiske domæner for bot:hasStorey er forekomster af bot:Building.</rdfs:comment>
        <rdfs:comment xml:lang="en">Relation to storeys contained in a zone. The typical domains of bot:hasStorey are instances of bot:Building.</rdfs:comment>
        <rdfs:comment xml:lang="fr">Relation à définir entre les étages d&apos;une même zone. Cette propriété s&apos;applique typiquement sur des instances de bot:Building.</rdfs:comment>
        <rdfs:comment xml:lang="it">Relazione con i piani contenuti in una zona. Il tipico dominio di bot:hasStorey è bot:Building.</rdfs:comment>
        <rdfs:comment xml:lang="pt">Relação com os pisos contidos numa zona. Os domínios típicos de bot:hasStorey são instâncias de bot:Building.</rdfs:comment>
        <rdfs:comment xml:lang="fi">Suhde vyöhykkeeseen kuuluviin kerroksiin. Tyypillinen lähtöjoukko on luokan bot:Building instanssit.</rdfs:comment>
        <rdfs:comment xml:lang="cs">Vztah zóny-podlaží a zóny, ve které se nachází. Typická doména bot:hasStorey jsou instance bot:Building.</rdfs:comment>
        <rdfs:comment xml:lang="sk">Vzťah zóny-podlažia a zóny, v ktorej sa nachádza. Typická doména bot:hasStorey sú inštancie bot:Building.</rdfs:comment>
        <rdfs:comment xml:lang="fa">ارتباط با طبقه‌هایی که دربرگرفته شده‌اند. دامنه‌ی اصلی bot:hasStorey عنصرهایی از جنس bot:Building هستند.</rdfs:comment>
        <rdfs:comment xml:lang="zh-cn">区域中含有楼层的关系。 bot：hasStorey的典型使用范围是bot：Building中的实例。</rdfs:comment>
        <rdfs:isDefinedBy rdf:resource="https://w3id.org/bot#"/>
        <rdfs:label xml:lang="tr">Katı var</rdfs:label>
        <rdfs:label xml:lang="fr">a étage</rdfs:label>
        <rdfs:label xml:lang="it">ha piano</rdfs:label>
        <rdfs:label xml:lang="da">har etage</rdfs:label>
        <rdfs:label xml:lang="sv">har våning</rdfs:label>
        <rdfs:label xml:lang="en">has storey</rdfs:label>
        <rdfs:label xml:lang="de">hat Geschoss</rdfs:label>
        <rdfs:label xml:lang="nl">heeft verdieping</rdfs:label>
        <rdfs:label xml:lang="sk">má podlažie</rdfs:label>
        <rdfs:label xml:lang="cs">má podlaží</rdfs:label>
        <rdfs:label xml:lang="fi">omaa kerroksen</rdfs:label>
        <rdfs:label xml:lang="pt">tem piso</rdfs:label>
        <rdfs:label xml:lang="es">tiene piso</rdfs:label>
        <rdfs:label xml:lang="ca">té pis</rdfs:label>
        <rdfs:label xml:lang="fa">طبقه دارد</rdfs:label>
        <rdfs:label xml:lang="zh-cn">包含楼层</rdfs:label>
        <ns:term_status>stable</ns:term_status>
        <schema1:domainIncludes rdf:resource="https://w3id.org/bot#Building"/>
    </owl:ObjectProperty>
    


    <!-- https://w3id.org/bot#hasSubElement -->

    <owl:ObjectProperty rdf:about="https://w3id.org/bot#hasSubElement">
        <rdfs:domain rdf:resource="https://w3id.org/bot#Element"/>
        <rdfs:range rdf:resource="https://w3id.org/bot#Element"/>
        <rdfs:comment xml:lang="de">Beziehung zwischen zwei Bauteilen, wobei entweder eines das andere enthält (z.B. eine Wand enthält ein Fenster) oder ein ganzes, das aus anderen Teilen zusammen gesetzt ist (z.B. eine Lüftungsanlage hat eine Komponente Lüfter).</rdfs:comment>
        <rdfs:comment xml:lang="tr">Bir a) bina parçası ve b) bina parçası arasındaki bağlantının a) tarafından barındırmasıdır. Örneğin: inst:wall bot:hasSubElement inst:window.</rdfs:comment>
        <rdfs:comment xml:lang="ca">Relació entre dos elements de construcció, ja sigui un element que allotja un altre (per exemple, una mur que conté una finestra) o una subcomposició d&apos;un element de construcció en parts més petites (per exemple, una unitat de ventilació té una part que és un ventilador).</rdfs:comment>
        <rdfs:comment xml:lang="es">Relación entre dos elementos de construcción, ya sea un elemento que aloja a otro (por ejemplo, una ventana alojada en una pared) o una subcomposición de un elemento de construcción en partes más pequeñas (por ejemplo, una unidad de ventilación tiene una parte que es un ventilador).</rdfs:comment>
        <rdfs:comment xml:lang="nl">Relatie tussen twee gebouwelementen, ofwel één element dat een andere element bevat (bv. een muur die een raam bevat) of een subcompositie van een gebouwelement in kleinere delen (bv. een luchtbehandelingskast die een ventilator bevat).</rdfs:comment>
        <rdfs:comment xml:lang="en">Relation between two building elements, either one element hosting another (e.g. a wall hosts a window) or a subcomposition of a building element into smaller parts (e.g. an air handling unit has as a part a fan).</rdfs:comment>
        <rdfs:comment xml:lang="fr">Relation entre deux éléments du bâti, soit un élément hébergeant un autre (ex., un mur héberge une fenêtre), ou une décomposition d&apos;un élément en sous-parties (ex., un système de gestion de l&apos;air et un ventilateur qu&apos;il contient)</rdfs:comment>
        <rdfs:comment xml:lang="sv">Relation mellan två byggdelar där antingen endera är monterad i den andra (t.ex. ett fönster som är monterat i en vägg) eller endera är del av den andra (t.ex. en fläkt som är del av ett ventilationsaggregat).</rdfs:comment>
        <rdfs:comment xml:lang="da">Relation mellem to bygningsdele, enten en bygningsdel, der er &quot;hostet&quot; af en anden (fx et vindue, der &quot;hostet&quot; af en væg) eller en underkomposition af en bygningsdel i mindre dele (fx en ventilator som en del af et ventilationsaggregat).</rdfs:comment>
        <rdfs:comment xml:lang="it">Relazione tra due elementi di costruzione che può realizzarsi perché un elemento ne ospita un altro (es. un muro ospita una finestra) o la scomposizione di un elemento in parti più piccole (es. un&apos;unità di trattamento aria ha un ventilatore come sua parte).</rdfs:comment>
        <rdfs:comment xml:lang="pt">Relação entre dois elementos arquitectónicos, quer seja um elemento contendo outro (p.e. uma parede aloja uma janela) ou a subcomposição de um elemento arquitectónico por partes menores (p.e. uma unidade de ventilação contém uma parte que é um ventilador).</rdfs:comment>
        <rdfs:comment xml:lang="fi">Suhde kahden elementin välillä, joko yhdestä elementistä siihen asennettuun toiseen elementtiin (esimerkiksi seinään asennettu ikkuna) tai elementin osittelu pienempiin osiin (esimerkiksi ilmankäsittelykonella on osana puhallin).</rdfs:comment>
        <rdfs:comment xml:lang="cs">Vztah mezi prvkem a) a dalším prvkem b), který je součástí prvku a)</rdfs:comment>
        <rdfs:comment xml:lang="sk">Vzťah medzi prvkom a) a ďalším prvkom b), ktorý je súčasťou prvku a)</rdfs:comment>
        <rdfs:comment xml:lang="fa">ارتباط بین دو المان ساختمان؛ یا رابطه یک المان میزبان با المان دیگر (برای مثال یک پنجره میزبانی میشود توسط یک دیوار)؛ یا رابطه یک المان با زیرمجموعه‌ای از المانهای کوچکتر ساختمان (برای مثال یک فن به عنوان بخشی از واحد کنترل هوا).</rdfs:comment>
        <rdfs:comment xml:lang="zh-cn">两个建筑构件之间的关系，要么是一个元素承载另一个元素（例如，一扇窗户由墙壁承载），要么是将建筑构件细分为较小的部分（例如，作为空气处理单元一部分的风扇）。</rdfs:comment>
        <rdfs:isDefinedBy rdf:resource="https://w3id.org/bot#"/>
        <rdfs:label xml:lang="fr">a sous-élément</rdfs:label>
        <rdfs:label xml:lang="es">alberga sub elemento</rdfs:label>
        <rdfs:label xml:lang="tr">alt öğesi var</rdfs:label>
        <rdfs:label xml:lang="it">ha sotto-elemento</rdfs:label>
        <rdfs:label xml:lang="da">har underbygningsdel</rdfs:label>
        <rdfs:label xml:lang="en">has sub-element</rdfs:label>
        <rdfs:label xml:lang="de">hat Unterbauteil</rdfs:label>
        <rdfs:label xml:lang="nl">heeft subelement</rdfs:label>
        <rdfs:label xml:lang="cs">má součást</rdfs:label>
        <rdfs:label xml:lang="sk">má súčasť</rdfs:label>
        <rdfs:label xml:lang="fi">omaa osaelementin</rdfs:label>
        <rdfs:label xml:lang="pt">tem sub elemento</rdfs:label>
        <rdfs:label xml:lang="ca">té un subelement</rdfs:label>
        <rdfs:label xml:lang="sv">värd för sub element</rdfs:label>
        <rdfs:label xml:lang="fa">زیرالمان دارد</rdfs:label>
        <rdfs:label xml:lang="zh-cn">包含子构件</rdfs:label>
        <ns:term_status>stable</ns:term_status>
    </owl:ObjectProperty>
    


    <!-- https://w3id.org/bot#hasZeroPoint -->

    <owl:ObjectProperty rdf:about="https://w3id.org/bot#hasZeroPoint">
        <rdfs:domain rdf:resource="https://w3id.org/bot#Site"/>
        <rdfs:comment xml:lang="it">Collega un bot:Site ad un&apos;istanza che codifica la latitudine e longitudine del punto zero di un sito. Questa può essere l&apos;istanza di wgs84:Point. La definizioen di GIS e geometrie non rientra nell&apos;ambito di BOT ed è pertanto necessario che l&apos;utente selezioni una ontologia adeguata. L&apos;uso di questa proprietà è potenzialmente ambiguo e potrebbe essere rimossa o revisionata in successive edizioni dell&apos;ontologia.</rdfs:comment>
        <rdfs:comment xml:lang="da">Forbinder et bot:Site med en forekomst, der beskriver en længde- og breddegrad for byggegrundens nulpunkt. Dette kunne være en forekomst af et wgs84:Point. Definitionen af GIS og geometri er ikke omfattet af BOT og en passende ontologi må her vælges af brugeren. Brugen af denne egenskab er potentielt tvetydig, og den kan fjernes eller revideres i fremtidige udgaver af ontologien.</rdfs:comment>
        <rdfs:comment xml:lang="fr">Lie un bot:Site à un individu qui encode la latitude et la longitude du point zéro du site du bâtiment. Ceci peut être une instance de wgs84:Point. La définition du système de coordonnée géographique et de la géométrie n&apos;est pas défini par BOT et l&apos;utilisateur doit choisir l&apos;ontologie appropriée. L&apos;utilisation de cette propriété est potentiellement ambigue et elle pourrait être supprimée ou modifiée dans les prochaines versions de l&apos;ontologie.</rdfs:comment>
        <rdfs:comment xml:lang="fi">Liittää bot:Site:n instanssiin, jolla merkitään rakennustyömaan nollakohdan leveys- ja pituuspiirit. Tämä voi olla esimerkki wgs84:Point-luokan instanssi. BOT ei kata GIS:ä tai geometriaa, joten käyttäjän tulee valita sopiva ontologia.Tämän propertyn käyttö on mahdollisesti moniselitteistä, ja se voidaan poistaa tai tarkistaa ontologian tulevissa versioissa.</rdfs:comment>
        <rdfs:comment xml:lang="en">Links a bot:Site to an instance that encodes the latitude and longitude of the Zero Point of the building site. This could be an instance of a wgs84:Point. The definition of GIS and geometry is not within the scope of BOT and an appropriate ontology needs to be selected here by the user. The use of this property is potentially ambiguous and it might be removed or revised in future editions of the ontology.</rdfs:comment>
        <rdfs:comment xml:lang="sv">Länkar en byggnadsplats (en instans av bot:Site) till en instans som uttrycker latitud och longitud för den berörda byggnadsplatsens origo. Detta kan exempelvis vara en instans av wgs84:Point. Definitioner för GIS och geometrier är utanför BOTs scope och användaren ansvarar själv för att välja en lämplig ontologi för detta syfte. Användningen av denna relation är potentiellt tvetydig och den kan komma att revideras eller tas bort i framtida versioner av ontologin.</rdfs:comment>
        <rdfs:comment xml:lang="cs">Napojuje bot:Site na instanci, který definuje zeměpisnou šířku a délku nulového bodu budovy. To může být instancí wgs84:Point. Definice GIS a geometrie není v rozsahu BOT a je potřebné použít jinou adekvátní ontologii. Využití této vlastnosti je potenciálně nepřesné a nejasné a může být odstraněno nebo revidováno v budoucích úpravách této ontologie.</rdfs:comment>
        <rdfs:comment xml:lang="sk">Napojuje bot:Site na inštanciu ktorá definuje zemepisnú šírku a dĺžku nulového bodu budovy. To môže byť inštanciou wgs84:Pint. Definícia GIS a geometrie nie je v rozsahu BOT a je potrebné použiť inú adekvátnu ontológiu. Využitie tejto vlastnosti je potenciálne nepresné a nejasné a môže byť odstránené alebo revidované v budúcich úpravách tejto ontológie.</rdfs:comment>
        <rdfs:comment xml:lang="pt">Relaciona um bot:Site com uma instância que codifica a latitude e longitude do ponto zero de um sítio de construção. Este poderá ser uma instância de um wgs84:Point. As definições de SIG e de geometria não estão no escopo de BOT, sendo necessário que o/a utilizador/a seleccione uma ontologia adequada para o efeito. A utilização desta propriedade é potencialmente ambígua, podendo esta ser removida ou revista em versões futuras desta ontologia.</rdfs:comment>
        <rdfs:comment xml:lang="de">Verbindet eine Instanz von bot:Site mit einer Instanz, die den Längen- und Breitengrad des Nullpunkts des Grundstücks definiert. Dies kann eine Instanz eines wgs84:Point sein. Die Definition von GIS und Geometrie ist nicht Bestandteil von BOT. Die Nutzung dieses Properties ist potenziell zweideutig und es besteht die Möglichkeit das es in Zukunft überarbeitet oder entfernt wird.</rdfs:comment>
        <rdfs:comment xml:lang="nl">Verbindt een bot:Zone instantie met een instantie die de lengtegraad en breedtegraad definieert van het nulpunt van een bot:Site instantie. Dit kan een instantie zijn van wgs84:Point. De definitie van GIS en geometrie valt niet in de scope van BOT en de gebruiker moet een gepaste ontology hiervoor selecteren. Het gebruik van deze eigenschap is potentieel ambigu en kan verwijderd of herzien worden in toekomstige versies van deze ontologie.</rdfs:comment>
        <rdfs:comment xml:lang="es">Vincula un bot:Site a una instancia que codifica la latitud y longitud del punto cero del sitio del edificio. Esta puede ser una instancia de un wgs84:Point. La definición de SIG y de la geometría no está dentro del alcance de BOT por lo que el usuario deberá utilizar para ello una ontología apropiada en combinación con BOT. El uso de esta propiedad es potencialmente ambigua y podría ser eliminada o revisada en ediciones futuras de la ontología.</rdfs:comment>
        <rdfs:comment xml:lang="ca">Vincula un bot:Site a una instància que codifica la latitud i longitud de el punt zero del lloc de l&apos;edifici. Aquesta pot ser una instància d&apos;un wgs84:Point. La definició de SIG i de la geometria no està dins de l&apos;abast de la BOT, per tant, l&apos;usuari haurà de seleccionar una ontologia apropiada. L&apos;ús d&apos;aquesta propietat és potencialment ambigua i podria ser eliminada o revisada en edicions futures de l&apos;ontologia.</rdfs:comment>
        <rdfs:comment xml:lang="tr">bir bot:Site ile bir olusumla bağlantı kurar: Bina alanının sıfır noktasında enlem ve boylamını tanımlayan bir örnekle bağlar. Bu bir wgs84:Point örneği olabilir. GPS ve geometrinin tanımı BOT kapsamında değildir ve kullanıcı tarafından uygun bir ontoloji seçilmelidir. Bu özelliğin kullanımı potansiyel olarak belirsizdir ve gelecekteki ontolojinin sürümlerinde kaldırılabilir veya revize edilebilir.</rdfs:comment>
        <rdfs:comment xml:lang="fa">رابطه یک عنصر bot:Site با عنصری که طول وعرض جغرافیایی نقطه صفر سایت ساختمان را مشخص می کند. این میتواند یک عنصراز wgs84:Point باشد. تعریف GIS و هندسه در دایره‌ وضایف آنتالوژی جاینگاری ساختمان (BOT) نیست و لازم است یک آنتالوژی مناسب توسط کاربر برای این موضوع انتخاب شود. استفاده از این ویژگی به طور بالقوه ای مبهم است و ممکن است در نسخه های بعدی این آنتالوژی حذف یا اصلاح شود.</rdfs:comment>
        <rdfs:comment xml:lang="zh-cn">将bot：Site链接到一个实例，对该实例建筑位置原点的纬度和经度进行编码。 这可以是wgs84：Point的一个实例。 GIS和几何的定义不在BOT的范围内，用户需要在此处选择适当的本体。该属性的使用可能是模棱两可的，并且在以后的本体版本中可能会删除或修改它。</rdfs:comment>
        <rdfs:isDefinedBy rdf:resource="https://w3id.org/bot#"/>
        <rdfs:label xml:lang="tr">Sıfır noktasi var</rdfs:label>
        <rdfs:label xml:lang="fr">a point origine</rdfs:label>
        <rdfs:label xml:lang="it">ha punto zero</rdfs:label>
        <rdfs:label xml:lang="da">har nulpunkt</rdfs:label>
        <rdfs:label xml:lang="sv">har origo</rdfs:label>
        <rdfs:label xml:lang="en">has zero point</rdfs:label>
        <rdfs:label xml:lang="de">hat Nullpunkt</rdfs:label>
        <rdfs:label xml:lang="nl">heeft nulpunt</rdfs:label>
        <rdfs:label xml:lang="cs">má nulový bod</rdfs:label>
        <rdfs:label xml:lang="sk">má nulový bod</rdfs:label>
        <rdfs:label xml:lang="fi">omaa nollapisteen</rdfs:label>
        <rdfs:label xml:lang="pt">tem ponto zero</rdfs:label>
        <rdfs:label xml:lang="es">tiene punto cero</rdfs:label>
        <rdfs:label xml:lang="ca">té un punt zero</rdfs:label>
        <rdfs:label xml:lang="fa">نقطه صفر دارد</rdfs:label>
        <rdfs:label xml:lang="zh-cn">含有原点</rdfs:label>
        <rdfs:seeAlso rdf:resource="https://github.com/w3c-lbd-cg/bot/issues/41"/>
        <ns:term_status>unstable</ns:term_status>
    </owl:ObjectProperty>
    


    <!-- https://w3id.org/bot#hostsElement -->

    <owl:ObjectProperty rdf:about="https://w3id.org/bot#hostsElement">
        <rdfs:domain rdf:resource="https://w3id.org/bot#Element"/>
        <rdfs:range rdf:resource="https://w3id.org/bot#Element"/>
        <rdfs:comment xml:lang="nl">This property is DEPRECATED, use bot:hasSubElement instead // ORIGINAL definition: Relatie tussen een gebouwelement a) en een ander element b) dat een ander element in zich heeft a). Voorbeeld: inst:wall bot:hostsElement inst:window</rdfs:comment>
        <rdfs:comment xml:lang="en">This property is DEPRECATED, use bot:hasSubElement instead // ORIGINAL definition: Relation between an element a) and another element b) hosted by element a). Example: inst:wall bot:hostsElement inst:window</rdfs:comment>
        <rdfs:comment xml:lang="da">This property is DEPRECATED, use bot:hasSubElement instead // ORIGINAL definition: Relation mellem en bygningsdel a) og en anden bygningsdel b) hostet af element a). Eksempel: inst:wall bot:hostsElement inst:window</rdfs:comment>
        <rdfs:label xml:lang="nl">heeft element</rdfs:label>
        <rdfs:label xml:lang="da">hoster element</rdfs:label>
        <rdfs:label xml:lang="nl">hoster element</rdfs:label>
        <rdfs:label xml:lang="en">hosts element</rdfs:label>
        <rdfs:seeAlso rdf:resource="https://w3id.org/bot#hasSubElement"/>
        <owl:deprecated rdf:datatype="http://www.w3.org/2001/XMLSchema#boolean">true</owl:deprecated>
    </owl:ObjectProperty>
    


    <!-- https://w3id.org/bot#interfaceOf -->

    <owl:ObjectProperty rdf:about="https://w3id.org/bot#interfaceOf">
        <rdfs:domain rdf:resource="https://w3id.org/bot#Interface"/>
        <rdfs:comment xml:lang="de">Beziehung zwischen einer Schnittstelle und einem anderen Ding (Gebäude zone, Bauteil oder owl:Thing).</rdfs:comment>
        <rdfs:comment xml:lang="tr">Bir arabirim ile bitişik bir bölge veya bina parçası arasındaki ilişki.</rdfs:comment>
        <rdfs:comment xml:lang="ca">Relació entre una interfície i una altra cosa (zona de construcció, element o owl:Thing)</rdfs:comment>
        <rdfs:comment xml:lang="es">Relación entre una interfaz y otra cosa (zona de construcción, elemento o owl:Thing)</rdfs:comment>
        <rdfs:comment xml:lang="nl">Relatie tussen een interface en een ander ding (gebouwzone, gebouwelement of owl:Thing).</rdfs:comment>
        <rdfs:comment xml:lang="sv">Relation mellan ett gränssnitt och något angränsande (en zon, en byggdel, eller owl:Thing).</rdfs:comment>
        <rdfs:comment xml:lang="da">Relation mellem en grænseflade og en anden ting (bygningszone, bygningsdel eller owl:Thing).</rdfs:comment>
        <rdfs:comment xml:lang="fr">Relation à définir entre une interface et une zone ou un élément adjacents.</rdfs:comment>
        <rdfs:comment xml:lang="en">Relationship between an interface and another thing (building zone, element or owl:Thing)</rdfs:comment>
        <rdfs:comment xml:lang="it">Relazione tra un&apos;interfaccia e un&apos;altra cosa (zona di edificio, elemento di costruzione o owl:Thing)</rdfs:comment>
        <rdfs:comment xml:lang="pt">Relação entre um interface e outra coisa (zona do edifício, elemento ou owl:Thing)</rdfs:comment>
        <rdfs:comment xml:lang="fi">Suhde rajapinnan ja toisen asian välillä (rakennuksen vyöhyke, elementti, tai owl:Thing).</rdfs:comment>
        <rdfs:comment xml:lang="cs">Vztah mezi rozhraním a přilehlou zónou nebo prvkem.</rdfs:comment>
        <rdfs:comment xml:lang="sk">Vzťah medzi rozhraním a priľahlou zónou alebo prvkom.</rdfs:comment>
        <rdfs:comment xml:lang="fa">رابطه بین یک رابط و یک عنصر دیگر (منطقه ساختمان، المان، و یا owl:Thing)</rdfs:comment>
        <rdfs:comment xml:lang="zh-cn">界面与其他对象（建筑热区，构件或owl:Thing）之间的关系。</rdfs:comment>
        <rdfs:isDefinedBy rdf:resource="https://w3id.org/bot#"/>
        <rdfs:label xml:lang="tr">Arayüzü</rdfs:label>
        <rdfs:label xml:lang="de">Schnittstelle von</rdfs:label>
        <rdfs:label xml:lang="sv">gränssnitt för</rdfs:label>
        <rdfs:label xml:lang="da">grænseflade for</rdfs:label>
        <rdfs:label xml:lang="it">interfaccia di</rdfs:label>
        <rdfs:label xml:lang="fr">interface de</rdfs:label>
        <rdfs:label xml:lang="pt">interface de</rdfs:label>
        <rdfs:label xml:lang="en">interface of</rdfs:label>
        <rdfs:label xml:lang="nl">interface van</rdfs:label>
        <rdfs:label xml:lang="es">interfaz de</rdfs:label>
        <rdfs:label xml:lang="ca">interfície de</rdfs:label>
        <rdfs:label xml:lang="sk">je rozhranie/rozhraním</rdfs:label>
        <rdfs:label xml:lang="cs">je rozhraní/je rozhraním</rdfs:label>
        <rdfs:label xml:lang="fi">rajapintana</rdfs:label>
        <rdfs:label xml:lang="fa">رابط است</rdfs:label>
        <rdfs:label xml:lang="zh-cn">交界面于</rdfs:label>
        <ns:term_status>stable</ns:term_status>
    </owl:ObjectProperty>
    


    <!-- https://w3id.org/bot#intersectingElement -->

    <owl:ObjectProperty rdf:about="https://w3id.org/bot#intersectingElement">
        <rdfs:subPropertyOf rdf:resource="https://w3id.org/bot#hasElement"/>
        <rdfs:comment xml:lang="de">Beziehung zwischen einer Zone und einem Bauteil, das die Zone schneidet.</rdfs:comment>
        <rdfs:comment xml:lang="tr">Bir Bölge ve onunla kesişen bir yapı Elemanı arasındaki ilişki.</rdfs:comment>
        <rdfs:comment xml:lang="da">Forholdet mellem en zone og et bygningselement, der krydser det.</rdfs:comment>
        <rdfs:comment xml:lang="ca">Relació entre una zona i un element constructiu que la intersecta.</rdfs:comment>
        <rdfs:comment xml:lang="es">Relación entre una zona y un elemento constructivo que la interseca.</rdfs:comment>
        <rdfs:comment xml:lang="nl">Relatie tussen een zone en een gebouwelement die de zone doorsnijdt.</rdfs:comment>
        <rdfs:comment xml:lang="en">Relation between a Zone and a building Element that intersects it.</rdfs:comment>
        <rdfs:comment xml:lang="fr">Relation entre une zone et un élément du bâtiment qui la traverse.</rdfs:comment>
        <rdfs:comment xml:lang="sv">Relationen mellan en zon och en byggdel som korsar zonen.</rdfs:comment>
        <rdfs:comment xml:lang="it">Relazione tra una zona e un elemento di costruzione che la interseca.</rdfs:comment>
        <rdfs:comment xml:lang="pt">Relação entre uma Zona e um Elemento construtivo que a intersecta.</rdfs:comment>
        <rdfs:comment xml:lang="fi">Suhde vyöhykkeen ja sitä leikkaavan rakennuselementin välillä.</rdfs:comment>
        <rdfs:comment xml:lang="cs">Vztah mezi zónou a stavebním prvkem, který ji protíná.</rdfs:comment>
        <rdfs:comment xml:lang="sk">Vzťah medzi zónou a stavebným prvkom, ktorý ju pretína.</rdfs:comment>
        <rdfs:comment xml:lang="fa">رابطه بین یک منطقه با المان ساختمانی که با آن در تلاقی است.</rdfs:comment>
        <rdfs:comment xml:lang="zh-cn">区域中相交建筑构件之间的关系。</rdfs:comment>
        <rdfs:isDefinedBy rdf:resource="https://w3id.org/bot#"/>
        <rdfs:label xml:lang="tr">Eleman ile temas</rdfs:label>
        <rdfs:label xml:lang="nl">doorsnijdend element</rdfs:label>
        <rdfs:label xml:lang="ca">element d&apos;intersecció</rdfs:label>
        <rdfs:label xml:lang="es">elemento de intersección</rdfs:label>
        <rdfs:label xml:lang="it">elemento intersecante</rdfs:label>
        <rdfs:label xml:lang="pt">elemento intersectante</rdfs:label>
        <rdfs:label xml:lang="en">intersecting element</rdfs:label>
        <rdfs:label xml:lang="sv">korsande byggdel</rdfs:label>
        <rdfs:label xml:lang="da">krydsende Bygningsdel</rdfs:label>
        <rdfs:label xml:lang="fi">leikkaava elementti</rdfs:label>
        <rdfs:label xml:lang="sk">pretína element-prvok</rdfs:label>
        <rdfs:label xml:lang="cs">protíná element-prvek</rdfs:label>
        <rdfs:label xml:lang="de">schneidendes Bauteil</rdfs:label>
        <rdfs:label xml:lang="fr">élément intersectant</rdfs:label>
        <rdfs:label xml:lang="fa">المان متلاقی</rdfs:label>
        <rdfs:label xml:lang="zh-cn">相交构件</rdfs:label>
        <ns:term_status>stable</ns:term_status>
    </owl:ObjectProperty>
    


    <!-- https://w3id.org/bot#intersectsZone -->

    <owl:ObjectProperty rdf:about="https://w3id.org/bot#intersectsZone">
        <owl:inverseOf rdf:resource="https://w3id.org/bot#intersectsZone"/>
        <rdf:type rdf:resource="http://www.w3.org/2002/07/owl#SymmetricProperty"/>
        <rdfs:domain rdf:resource="https://w3id.org/bot#Zone"/>
        <rdfs:range rdf:resource="https://w3id.org/bot#Zone"/>
        <rdfs:comment xml:lang="tr">3D kapsamı kesişen iki bölge arasındaki ilişki. Örneğin, bir merdiven boşluğu farklı katlarla kesişir.</rdfs:comment>
        <rdfs:comment xml:lang="de">Beziehung zwischen zwei Zonen, die sich schneiden. Zum Beispiel schneidet eine Treppe verschiedene Geschosse.</rdfs:comment>
        <rdfs:comment xml:lang="nl">Een relatie tussen twee zones waarvan de driedimensionale omvang doorsnijdend is. Bijvoorbeeld een traphal die verschillende verdiepingen doorsnijdt.</rdfs:comment>
        <rdfs:comment xml:lang="da">Forholdet mellem to zoner, hvis 3D-omfang skærer hinanden. For eksempel skærer et trappehus forskellige etager.</rdfs:comment>
        <rdfs:comment xml:lang="ca">Relació entre dues zones l&apos;extensió fa que una interseccioni amb l&apos;altra. Per exemple, una escala creua diferents pisos.</rdfs:comment>
        <rdfs:comment xml:lang="es">Relación entre dos zonas cuya extensión hace que una interseccione con la otra. Por ejemplo, una escalera cruza diferentes pisos.</rdfs:comment>
        <rdfs:comment xml:lang="fr">Relation entre deux zones dont l&apos;étendue 3D se croise. Par exemple, une cage d&apos;escalier croise différents étages.</rdfs:comment>
        <rdfs:comment xml:lang="sv">Relationen mellan två zoner vars tredimensionella utsträckning korsar varandra. Till exempel, ett trapphus som skär igenom flera våningar.</rdfs:comment>
        <rdfs:comment xml:lang="en">Relationship between two zones whose 3D extent intersect. For example, a stairwell intersects different storeys.</rdfs:comment>
        <rdfs:comment xml:lang="it">Relazione tra due zone le cui estensioni 3D si intersecano. Per esempio, una tromba delle scale interseca vari piani.</rdfs:comment>
        <rdfs:comment xml:lang="pt">Relação entre duas zonas cuja extensão tridimensional se intersecta. Por exemplo, uma caixa de escadas intersecta vários pisos.</rdfs:comment>
        <rdfs:comment xml:lang="fi">Suhde kahden vyöhykkeen välillä, jotka leikkaavat toisiaan. Esimerkiksi rappuset leikkaavat useita kerroksia.</rdfs:comment>
        <rdfs:comment xml:lang="cs">Vztah dvou zón, které se protínají svým prostorovým ohraničením. Na příklad, eskalátor protíná vícero podlažních zón.</rdfs:comment>
        <rdfs:comment xml:lang="sk">Vzťach dvoch zón, ktoré sa pretínajú svojim priestorovým rozhraním. Príkladom môže byť eskalátor prestupujúci cez vac zón-podlaží.</rdfs:comment>
        <rdfs:comment xml:lang="fa">رابطه بین دو منطقه که حدود سه بعدی آنها با هم تلاقی دارد. برای مثال، یک راه پله از منطقه های مختلف عبور می کند و با آنها تلاقی دارد.</rdfs:comment>
        <rdfs:comment xml:lang="zh-cn">两个区域之间三维空间相交的关系。 例如，楼梯间与不同楼层的相交</rdfs:comment>
        <rdfs:isDefinedBy rdf:resource="https://w3id.org/bot#"/>
        <rdfs:label xml:lang="tr">Bölge ile temas</rdfs:label>
        <rdfs:label xml:lang="ca">interseca amb zona</rdfs:label>
        <rdfs:label xml:lang="es">interseca con zona</rdfs:label>
        <rdfs:label xml:lang="it">interseca zona</rdfs:label>
        <rdfs:label xml:lang="pt">intersecta zona</rdfs:label>
        <rdfs:label xml:lang="fr">intersecte zone</rdfs:label>
        <rdfs:label xml:lang="en">intersects zone</rdfs:label>
        <rdfs:label xml:lang="fi">leikkaa vyöhykettä</rdfs:label>
        <rdfs:label xml:lang="sk">pretína zónu</rdfs:label>
        <rdfs:label xml:lang="cs">protíná zónu</rdfs:label>
        <rdfs:label xml:lang="de">sich schneidende Zone</rdfs:label>
        <rdfs:label xml:lang="sv">skär zon</rdfs:label>
        <rdfs:label xml:lang="da">skærer zone</rdfs:label>
        <rdfs:label xml:lang="nl">snijdt door zone</rdfs:label>
        <rdfs:label xml:lang="fa">منطقه متلاقی</rdfs:label>
        <rdfs:label xml:lang="zh-cn">相交区域</rdfs:label>
        <ns:term_status>stable</ns:term_status>
        <schema1:domainIncludes rdf:resource="https://w3id.org/bot#Building"/>
        <schema1:domainIncludes rdf:resource="https://w3id.org/bot#Site"/>
        <schema1:domainIncludes rdf:resource="https://w3id.org/bot#Space"/>
        <schema1:domainIncludes rdf:resource="https://w3id.org/bot#Storey"/>
        <schema1:rangeIncludes rdf:resource="https://w3id.org/bot#Building"/>
        <schema1:rangeIncludes rdf:resource="https://w3id.org/bot#Site"/>
        <schema1:rangeIncludes rdf:resource="https://w3id.org/bot#Space"/>
        <schema1:rangeIncludes rdf:resource="https://w3id.org/bot#Storey"/>
    </owl:ObjectProperty>
    


    <!-- https://w3id.org/digitalconstruction/0.3/BuildingMaterials#IsInnerLayerOf -->

    <owl:ObjectProperty rdf:about="https://w3id.org/digitalconstruction/0.3/BuildingMaterials#IsInnerLayerOf">
        <rdfs:domain rdf:resource="https://w3id.org/digitalconstruction/0.3/BuildingMaterials#Layer"/>
    </owl:ObjectProperty>
    


    <!-- https://w3id.org/digitalconstruction/0.3/BuildingMaterials#IsOuterLayerOf -->

    <owl:ObjectProperty rdf:about="https://w3id.org/digitalconstruction/0.3/BuildingMaterials#IsOuterLayerOf">
        <rdfs:domain rdf:resource="https://w3id.org/digitalconstruction/0.3/BuildingMaterials#Layer"/>
    </owl:ObjectProperty>
    


    <!-- https://w3id.org/digitalconstruction/0.3/BuildingMaterials#adjacentLayer -->

    <owl:ObjectProperty rdf:about="https://w3id.org/digitalconstruction/0.3/BuildingMaterials#adjacentLayer">
        <owl:inverseOf rdf:resource="https://w3id.org/digitalconstruction/0.3/BuildingMaterials#adjacentLayer"/>
        <rdf:type rdf:resource="http://www.w3.org/2002/07/owl#SymmetricProperty"/>
        <rdfs:domain rdf:resource="https://w3id.org/digitalconstruction/0.3/BuildingMaterials#Layer"/>
        <rdfs:range rdf:resource="https://w3id.org/digitalconstruction/0.3/BuildingMaterials#Layer"/>
    </owl:ObjectProperty>
    


    <!-- https://w3id.org/digitalconstruction/0.3/BuildingMaterials#hasLayers -->

    <owl:ObjectProperty rdf:about="https://w3id.org/digitalconstruction/0.3/BuildingMaterials#hasLayers">
        <rdfs:domain rdf:resource="https://w3id.org/digitalconstruction/0.3/BuildingMaterials#LayerSet"/>
        <rdfs:range rdf:resource="https://w3id.org/digitalconstruction/0.3/BuildingMaterials#Layer"/>
    </owl:ObjectProperty>
    


    <!-- https://w3id.org/digitalconstruction/0.3/BuildingMaterials#hasMaterial -->

    <owl:ObjectProperty rdf:about="https://w3id.org/digitalconstruction/0.3/BuildingMaterials#hasMaterial">
        <rdfs:domain rdf:resource="https://w3id.org/digitalconstruction/0.3/BuildingMaterials#MaterialDefinition"/>
        <rdfs:range rdf:resource="https://w3id.org/digitalconstruction/0.3/BuildingMaterials#Material"/>
    </owl:ObjectProperty>
    


    <!-- https://w3id.org/digitalconstruction/0.3/BuildingMaterials#hasMaterialName -->

    <owl:ObjectProperty rdf:about="https://w3id.org/digitalconstruction/0.3/BuildingMaterials#hasMaterialName">
        <rdfs:domain rdf:resource="https://w3id.org/digitalconstruction/0.3/BuildingMaterials#Material"/>
        <rdfs:range rdf:resource="https://w3id.org/digitalconstruction/0.3/BuildingMaterials#MaterialType"/>
        <rdfs:comment>It will assign the material name(material type) to the material</rdfs:comment>
    </owl:ObjectProperty>
    


    <!-- https://w3id.org/digitalconstruction/0.3/BuildingMaterials#hasProfiles -->

    <owl:ObjectProperty rdf:about="https://w3id.org/digitalconstruction/0.3/BuildingMaterials#hasProfiles">
        <rdfs:domain rdf:resource="https://w3id.org/digitalconstruction/0.3/BuildingMaterials#ProfileSet"/>
        <rdfs:range rdf:resource="https://w3id.org/digitalconstruction/0.3/BuildingMaterials#Profile"/>
    </owl:ObjectProperty>
    


    <!-- https://w3id.org/digitalconstruction/0.5/Materials#hasMaterial -->

    <owl:ObjectProperty rdf:about="https://w3id.org/digitalconstruction/0.5/Materials#hasMaterial">
        <rdf:type rdf:resource="http://www.w3.org/2002/07/owl#AsymmetricProperty"/>
        <rdfs:range rdf:resource="https://w3id.org/digitalconstruction/0.3/BuildingMaterials#Material"/>
        <rdfs:label xml:lang="en">has Material</rdfs:label>
    </owl:ObjectProperty>
    


    <!-- https://w3id.org/dot#adjacentDamageElement -->

    <owl:ObjectProperty rdf:about="https://w3id.org/dot#adjacentDamageElement">
        <owl:inverseOf rdf:resource="https://w3id.org/dot#adjacentDamageElement"/>
        <rdf:type rdf:resource="http://www.w3.org/2002/07/owl#SymmetricProperty"/>
        <rdfs:domain rdf:resource="https://w3id.org/dot#DamageElement"/>
        <rdfs:range rdf:resource="https://w3id.org/dot#DamageElement"/>
        <rdfs:comment xml:lang="en">Defines the relationship between two instances of Damage Element that are physically connected with each other.</rdfs:comment>
        <rdfs:label xml:lang="en">adjacent Damage Element</rdfs:label>
    </owl:ObjectProperty>
    


    <!-- https://w3id.org/dot#aggregatesDamageElement -->

    <owl:ObjectProperty rdf:about="https://w3id.org/dot#aggregatesDamageElement">
        <rdfs:domain rdf:resource="https://w3id.org/dot#DamageArea"/>
        <rdfs:range rdf:resource="https://w3id.org/dot#DamageElement"/>
        <owl:propertyChainAxiom rdf:parseType="Collection">
            <rdf:Description rdf:about="https://w3id.org/dot#aggregatesDamageElement"/>
            <rdf:Description rdf:about="https://w3id.org/dot#adjacentDamageElement"/>
        </owl:propertyChainAxiom>
        <owl:propertyChainAxiom rdf:parseType="Collection">
            <rdf:Description rdf:about="https://w3id.org/dot#aggregatesDamagePattern"/>
            <rdf:Description rdf:about="https://w3id.org/dot#groupsDamageElement"/>
        </owl:propertyChainAxiom>
        <rdfs:comment xml:lang="en">A relationship between an instance of Damage Area and its consisting Damage Element instance.</rdfs:comment>
        <rdfs:label xml:lang="en">aggregates Damage Element</rdfs:label>
    </owl:ObjectProperty>
    


    <!-- https://w3id.org/dot#aggregatesDamagePattern -->

    <owl:ObjectProperty rdf:about="https://w3id.org/dot#aggregatesDamagePattern">
        <rdfs:domain rdf:resource="https://w3id.org/dot#DamageArea"/>
        <rdfs:range rdf:resource="https://w3id.org/dot#DamagePattern"/>
        <rdfs:comment xml:lang="en">A relationship between an instance of Damage Area and its consisting Damage Pattern instance.</rdfs:comment>
        <rdfs:label xml:lang="en">aggregates Damage Pattern</rdfs:label>
    </owl:ObjectProperty>
    


    <!-- https://w3id.org/dot#coveredByInspection -->

    <owl:ObjectProperty rdf:about="https://w3id.org/dot#coveredByInspection">
        <rdfs:range rdf:resource="https://w3id.org/dot#Inspection"/>
        <owl:propertyChainAxiom rdf:parseType="Collection">
            <rdf:Description rdf:about="https://w3id.org/dot#coveredInDocumentation"/>
            <rdf:Description rdf:about="https://w3id.org/dot#documentationFromInspection"/>
        </owl:propertyChainAxiom>
        <schema:domainIncludes rdf:resource="https://w3id.org/bot#Element"/>
        <schema:domainIncludes rdf:resource="https://w3id.org/bot#Zone"/>
        <schema:domainIncludes rdf:resource="https://w3id.org/dot#Damage"/>
        <schema:domainIncludes rdf:resource="https://wisib.de/ontologie/brot#BridgeElement"/>
        <schema:domainIncludes rdf:resource="https://wisib.de/ontologie/brot#BridgeSpatialZone"/>
        <rdfs:comment xml:lang="en">Relationship between a documented object (damage or component / zone) and the Inspection in which the object has been covered.</rdfs:comment>
        <rdfs:label xml:lang="en">covered by inspection</rdfs:label>
    </owl:ObjectProperty>
    


    <!-- https://w3id.org/dot#coveredInDocumentation -->

    <owl:ObjectProperty rdf:about="https://w3id.org/dot#coveredInDocumentation">
        <rdfs:range rdf:resource="https://w3id.org/dot#Documentation"/>
        <schema:domainIncludes rdf:resource="https://w3id.org/bot#Element"/>
        <schema:domainIncludes rdf:resource="https://w3id.org/bot#Zone"/>
        <schema:domainIncludes rdf:resource="https://w3id.org/dot#Damage"/>
        <schema:domainIncludes rdf:resource="https://wisib.de/ontologie/brot#BridgeElement"/>
        <schema:domainIncludes rdf:resource="https://wisib.de/ontologie/brot#BridgeSpatialZone"/>
        <rdfs:comment xml:lang="en">Relationship between a Documentation and the relevant documented or inspected object (e.g. Damage Area or bot:Element). Should only be used for damage-relevant documentations.</rdfs:comment>
        <rdfs:label xml:lang="en">covered by documentation</rdfs:label>
    </owl:ObjectProperty>
    


    <!-- https://w3id.org/dot#documentationFromInspection -->

    <owl:ObjectProperty rdf:about="https://w3id.org/dot#documentationFromInspection">
        <owl:inverseOf rdf:resource="https://w3id.org/dot#hasDocumentation"/>
        <rdfs:comment xml:lang="en">Relationship between a Documentation and the Inspection to which the Documentation refers. Inverse object property of dot:hasDocumentation .</rdfs:comment>
        <rdfs:label xml:lang="en">documentation from inspection</rdfs:label>
    </owl:ObjectProperty>
    


    <!-- https://w3id.org/dot#groupsDamageElement -->

    <owl:ObjectProperty rdf:about="https://w3id.org/dot#groupsDamageElement">
        <rdfs:domain rdf:resource="https://w3id.org/dot#DamagePattern"/>
        <rdfs:range rdf:resource="https://w3id.org/dot#DamageElement"/>
        <owl:propertyChainAxiom rdf:parseType="Collection">
            <rdf:Description rdf:about="https://w3id.org/dot#groupsDamageElement"/>
            <rdf:Description rdf:about="https://w3id.org/dot#adjacentDamageElement"/>
        </owl:propertyChainAxiom>
        <rdfs:comment xml:lang="en">Groups instances of Damage Element that are physically connected in a Damage Pattern.</rdfs:comment>
        <rdfs:label xml:lang="en">groups Damage Element</rdfs:label>
    </owl:ObjectProperty>
    


    <!-- https://w3id.org/dot#hasCausation -->

    <owl:ObjectProperty rdf:about="https://w3id.org/dot#hasCausation">
        <rdfs:domain rdf:resource="https://w3id.org/dot#Damage"/>
        <rdfs:range rdf:resource="https://w3id.org/dot#Causation"/>
        <rdfs:comment xml:lang="en">Relationship between a Damage and its Causation.</rdfs:comment>
        <rdfs:label xml:lang="en">has Causation</rdfs:label>
    </owl:ObjectProperty>
    


    <!-- https://w3id.org/dot#hasDamage -->

    <owl:ObjectProperty rdf:about="https://w3id.org/dot#hasDamage">
        <rdfs:range rdf:resource="https://w3id.org/dot#Damage"/>
        <schema:domainIncludes rdf:resource="https://w3id.org/bot#Element"/>
        <schema:domainIncludes rdf:resource="https://w3id.org/bot#Zone"/>
        <schema:domainIncludes rdf:resource="https://wisib.de/ontologie/brot#BridgeElement"/>
        <schema:domainIncludes rdf:resource="https://wisib.de/ontologie/brot#BridgeSpatialZone"/>
        <rdfs:comment xml:lang="en">Defines the relationship between an affected component or structure (e.g. bot:Element) and a Damage.</rdfs:comment>
        <rdfs:label xml:lang="en">has Damage</rdfs:label>
    </owl:ObjectProperty>
    


    <!-- https://w3id.org/dot#hasDamageArea -->

    <owl:ObjectProperty rdf:about="https://w3id.org/dot#hasDamageArea">
        <rdfs:subPropertyOf rdf:resource="https://w3id.org/dot#hasDamage"/>
        <rdfs:range rdf:resource="https://w3id.org/dot#DamageArea"/>
        <rdfs:comment xml:lang="en">Defines the relationship between an affected component or structure (e.g. bot:Element) and a Damage Area.</rdfs:comment>
        <rdfs:label xml:lang="en">has Damage Area</rdfs:label>
    </owl:ObjectProperty>
    


    <!-- https://w3id.org/dot#hasDamageElement -->

    <owl:ObjectProperty rdf:about="https://w3id.org/dot#hasDamageElement">
        <rdfs:subPropertyOf rdf:resource="https://w3id.org/dot#hasDamage"/>
        <rdfs:range rdf:resource="https://w3id.org/dot#DamageElement"/>
        <owl:propertyChainAxiom rdf:parseType="Collection">
            <rdf:Description rdf:about="https://w3id.org/dot#hasDamageArea"/>
            <rdf:Description rdf:about="https://w3id.org/dot#aggregatesDamageElement"/>
        </owl:propertyChainAxiom>
        <rdfs:comment xml:lang="en">Defines the relationship between an affected component or structure (e.g. bot:Element) and a Damage Element.</rdfs:comment>
        <rdfs:label xml:lang="en">has Damage Element</rdfs:label>
    </owl:ObjectProperty>
    


    <!-- https://w3id.org/dot#hasDocumentation -->

    <owl:ObjectProperty rdf:about="https://w3id.org/dot#hasDocumentation">
        <rdfs:domain rdf:resource="https://w3id.org/dot#Inspection"/>
        <rdfs:range rdf:resource="https://w3id.org/dot#Documentation"/>
        <rdfs:comment xml:lang="en">Relationship between an Inspection and the corresponding Documentation</rdfs:comment>
        <rdfs:label xml:lang="en">has documentation</rdfs:label>
    </owl:ObjectProperty>
    


    <!-- https://w3id.org/dot#hasInspector -->

    <owl:ObjectProperty rdf:about="https://w3id.org/dot#hasInspector">
        <rdfs:domain rdf:resource="https://w3id.org/dot#Inspection"/>
        <rdfs:comment xml:lang="en">Relationship between an Inspector and the Inspection that has been performed by him.</rdfs:comment>
        <rdfs:label xml:lang="en">has Inspector</rdfs:label>
    </owl:ObjectProperty>
    


    <!-- 
    ///////////////////////////////////////////////////////////////////////////////////////
    //
    // Data properties
    //
    ///////////////////////////////////////////////////////////////////////////////////////
     -->

    


    <!-- http://www.semanticweb.org/arnak/ontologies/2022/7/DOR#hasCircularPotentialIndicator -->

    <owl:DatatypeProperty rdf:about="http://www.semanticweb.org/arnak/ontologies/2022/7/DOR#hasCircularPotentialIndicator">
        <rdf:type rdf:resource="http://www.w3.org/2002/07/owl#FunctionalProperty"/>
        <rdfs:range rdf:resource="http://www.w3.org/2001/XMLSchema#string"/>
        <rdfs:comment xml:lang="en">allows for the quantification of circular potential for different components, buildings or functional layers. Depeneding on the indicator definition of the ontology user, e.g., percentage or ranking, a value could be attributed to demonstrate the circualr potential based on the desired indicator defintion.</rdfs:comment>
        <rdfs:label>has Circular Potential Indicator</rdfs:label>
    </owl:DatatypeProperty>
    


    <!-- http://www.semanticweb.org/arnak/ontologies/2022/7/DOR#hasConstructionDate -->

    <owl:DatatypeProperty rdf:about="http://www.semanticweb.org/arnak/ontologies/2022/7/DOR#hasConstructionDate">
        <rdfs:domain rdf:resource="https://w3id.org/bot#Building"/>
        <rdfs:range rdf:resource="http://www.w3.org/2001/XMLSchema#dateTime"/>
        <rdfs:comment>The date when the building was constructed.</rdfs:comment>
        <rdfs:label xml:lang="en">has Construction Date</rdfs:label>
    </owl:DatatypeProperty>
    


    <!-- http://www.semanticweb.org/arnak/ontologies/2022/7/DOR#hasCurrentUseCount -->

    <owl:DatatypeProperty rdf:about="http://www.semanticweb.org/arnak/ontologies/2022/7/DOR#hasCurrentUseCount">
        <rdf:type rdf:resource="http://www.w3.org/2002/07/owl#FunctionalProperty"/>
        <rdfs:range rdf:resource="http://www.w3.org/2001/XMLSchema#nonNegativeInteger"/>
        <rdfs:comment xml:lang="en">represent the number of use counts that product is currently being used,  from the total reuse count that the product is designed for.</rdfs:comment>
        <rdfs:label xml:lang="en">has Current Use Count</rdfs:label>
    </owl:DatatypeProperty>
    


    <!-- http://www.semanticweb.org/arnak/ontologies/2022/7/DOR#hasDecommissioningDate -->

    <owl:DatatypeProperty rdf:about="http://www.semanticweb.org/arnak/ontologies/2022/7/DOR#hasDecommissioningDate">
        <rdfs:domain rdf:resource="https://w3id.org/bot#Building"/>
        <rdfs:range rdf:resource="http://www.w3.org/2001/XMLSchema#dateTime"/>
        <rdfs:comment>The date when the building is scheduled or planned to be decommissioned.</rdfs:comment>
        <rdfs:label xml:lang="en">has Decommissioing Date</rdfs:label>
    </owl:DatatypeProperty>
    


    <!-- http://www.semanticweb.org/arnak/ontologies/2022/7/DOR#hasDesignLife -->

    <owl:DatatypeProperty rdf:about="http://www.semanticweb.org/arnak/ontologies/2022/7/DOR#hasDesignLife">
        <rdfs:range rdf:resource="http://www.w3.org/2001/XMLSchema#nonNegativeInteger"/>
        <rdfs:comment>Design Life  is considered as a useful period of life time where major modifications are not needed. 
A reusable element can have one design life and multiple service lives, whereas a conventional element usually has the same design life as service life.</rdfs:comment>
        <rdfs:label xml:lang="en">has Design Life</rdfs:label>
    </owl:DatatypeProperty>
    


    <!-- http://www.semanticweb.org/arnak/ontologies/2022/7/DOR#hasEconomicLife -->

    <owl:DatatypeProperty rdf:about="http://www.semanticweb.org/arnak/ontologies/2022/7/DOR#hasEconomicLife">
        <rdfs:range rdf:resource="http://www.w3.org/2001/XMLSchema#nonNegativeInteger"/>
        <rdfs:comment>Economic Life refers ro the amount of time an element is in service before it is more economically advantageous to decommission or replace it. This dataproperty,
has Economic life, can be used in cases where the exact service life or design life is not known, or if it does not match the expected service life of an existing building.</rdfs:comment>
        <rdfs:label xml:lang="en">has Economic Life</rdfs:label>
    </owl:DatatypeProperty>
    


    <!-- http://www.semanticweb.org/arnak/ontologies/2022/7/DOR#hasRemainingReuseCount -->

    <owl:DatatypeProperty rdf:about="http://www.semanticweb.org/arnak/ontologies/2022/7/DOR#hasRemainingReuseCount">
        <rdf:type rdf:resource="http://www.w3.org/2002/07/owl#FunctionalProperty"/>
        <rdfs:range rdf:resource="http://www.w3.org/2001/XMLSchema#nonNegativeInteger"/>
        <rdfs:comment xml:lang="en">represent the number of reuses that are remaining from the total reuse count that the product is designed for.</rdfs:comment>
        <rdfs:label xml:lang="en">has Remaining Reuse Count</rdfs:label>
    </owl:DatatypeProperty>
    


    <!-- http://www.semanticweb.org/arnak/ontologies/2022/7/DOR#hasServiceLife -->

    <owl:DatatypeProperty rdf:about="http://www.semanticweb.org/arnak/ontologies/2022/7/DOR#hasServiceLife">
        <rdfs:range rdf:resource="http://www.w3.org/2001/XMLSchema#nonNegativeInteger"/>
        <rdfs:comment>According to ISO 20887, service life is the “period of time after installation during which a facility or its component parts meet or exceed the performance requirements.&quot;
A reusable element can have one design life and multiple service lives, whereas a conventional element usually has the same design life as service life.</rdfs:comment>
        <rdfs:label xml:lang="en">has Service Life</rdfs:label>
    </owl:DatatypeProperty>
    


    <!-- http://www.semanticweb.org/arnak/ontologies/2022/7/DOR#hasTotalReuseCount -->

    <owl:DatatypeProperty rdf:about="http://www.semanticweb.org/arnak/ontologies/2022/7/DOR#hasTotalReuseCount">
        <rdf:type rdf:resource="http://www.w3.org/2002/07/owl#FunctionalProperty"/>
        <rdfs:range rdf:resource="http://www.w3.org/2001/XMLSchema#nonNegativeInteger"/>
        <rdfs:comment xml:lang="en">indicates the total number of reuses, i.e., reuse counts, that the product is designed for.</rdfs:comment>
        <rdfs:label xml:lang="en">has Total Reuse Count</rdfs:label>
    </owl:DatatypeProperty>
    


    <!-- http://www.semanticweb.org/arnak/ontologies/2022/7/DOR#hasWasteCode -->

    <owl:DatatypeProperty rdf:about="http://www.semanticweb.org/arnak/ontologies/2022/7/DOR#hasWasteCode">
        <rdf:type rdf:resource="http://www.w3.org/2002/07/owl#FunctionalProperty"/>
        <rdfs:domain rdf:resource="https://w3id.org/digitalconstruction/0.3/BuildingMaterials#Material"/>
        <rdfs:range rdf:resource="http://www.w3.org/2001/XMLSchema#string"/>
        <rdfs:comment xml:lang="en">Represents the waste code associated with the material, as per waste management classification systems, for instance, the European Waste Code (EWC)</rdfs:comment>
        <rdfs:label>has Waste Code</rdfs:label>
    </owl:DatatypeProperty>
    


    <!-- http://www.semanticweb.org/covon/ontologies/2022/11/deconstruction-ontology#MaterialChemicalProperty -->

    <owl:DatatypeProperty rdf:about="http://www.semanticweb.org/covon/ontologies/2022/11/deconstruction-ontology#MaterialChemicalProperty">
        <rdfs:subPropertyOf rdf:resource="http://www.w3.org/2002/07/owl#topDataProperty"/>
    </owl:DatatypeProperty>
    


    <!-- http://www.semanticweb.org/covon/ontologies/2022/11/deconstruction-ontology#MaterialCombustibilityProperty -->

    <owl:DatatypeProperty rdf:about="http://www.semanticweb.org/covon/ontologies/2022/11/deconstruction-ontology#MaterialCombustibilityProperty">
        <rdfs:subPropertyOf rdf:resource="http://www.w3.org/2002/07/owl#topDataProperty"/>
    </owl:DatatypeProperty>
    


    <!-- http://www.semanticweb.org/covon/ontologies/2022/11/deconstruction-ontology#MaterialCombustionProperty -->

    <owl:DatatypeProperty rdf:about="http://www.semanticweb.org/covon/ontologies/2022/11/deconstruction-ontology#MaterialCombustionProperty">
        <rdfs:subPropertyOf rdf:resource="http://www.w3.org/2002/07/owl#topDataProperty"/>
    </owl:DatatypeProperty>
    


    <!-- http://www.semanticweb.org/covon/ontologies/2022/11/deconstruction-ontology#MaterialContaminationProperty -->

    <owl:DatatypeProperty rdf:about="http://www.semanticweb.org/covon/ontologies/2022/11/deconstruction-ontology#MaterialContaminationProperty">
        <rdfs:subPropertyOf rdf:resource="http://www.w3.org/2002/07/owl#topDataProperty"/>
        <rdfs:range rdf:resource="http://www.w3.org/2001/XMLSchema#boolean"/>
    </owl:DatatypeProperty>
    


    <!-- http://www.semanticweb.org/covon/ontologies/2022/11/deconstruction-ontology#MaterialEnergyProperty -->

    <owl:DatatypeProperty rdf:about="http://www.semanticweb.org/covon/ontologies/2022/11/deconstruction-ontology#MaterialEnergyProperty">
        <rdfs:subPropertyOf rdf:resource="http://www.w3.org/2002/07/owl#topDataProperty"/>
    </owl:DatatypeProperty>
    


    <!-- http://www.semanticweb.org/covon/ontologies/2022/11/deconstruction-ontology#MaterialFuelProperty -->

    <owl:DatatypeProperty rdf:about="http://www.semanticweb.org/covon/ontologies/2022/11/deconstruction-ontology#MaterialFuelProperty">
        <rdfs:subPropertyOf rdf:resource="http://www.w3.org/2002/07/owl#topDataProperty"/>
    </owl:DatatypeProperty>
    


    <!-- http://www.semanticweb.org/covon/ontologies/2022/11/deconstruction-ontology#MaterialHygroscopicProperty -->

    <owl:DatatypeProperty rdf:about="http://www.semanticweb.org/covon/ontologies/2022/11/deconstruction-ontology#MaterialHygroscopicProperty">
        <rdfs:subPropertyOf rdf:resource="http://www.w3.org/2002/07/owl#topDataProperty"/>
    </owl:DatatypeProperty>
    


    <!-- http://www.semanticweb.org/covon/ontologies/2022/11/deconstruction-ontology#MaterialMechanicalProperty -->

    <owl:DatatypeProperty rdf:about="http://www.semanticweb.org/covon/ontologies/2022/11/deconstruction-ontology#MaterialMechanicalProperty">
        <rdfs:subPropertyOf rdf:resource="http://www.w3.org/2002/07/owl#topDataProperty"/>
    </owl:DatatypeProperty>
    


    <!-- http://www.semanticweb.org/covon/ontologies/2022/11/deconstruction-ontology#MaterialOpticalProperty -->

    <owl:DatatypeProperty rdf:about="http://www.semanticweb.org/covon/ontologies/2022/11/deconstruction-ontology#MaterialOpticalProperty">
        <rdfs:subPropertyOf rdf:resource="http://www.w3.org/2002/07/owl#topDataProperty"/>
    </owl:DatatypeProperty>
    


    <!-- http://www.semanticweb.org/covon/ontologies/2022/11/deconstruction-ontology#MaterialPhysicalProperty -->

    <owl:DatatypeProperty rdf:about="http://www.semanticweb.org/covon/ontologies/2022/11/deconstruction-ontology#MaterialPhysicalProperty">
        <rdfs:subPropertyOf rdf:resource="http://www.w3.org/2002/07/owl#topDataProperty"/>
    </owl:DatatypeProperty>
    


    <!-- http://www.semanticweb.org/covon/ontologies/2022/11/deconstruction-ontology#MaterialThermalProperty -->

    <owl:DatatypeProperty rdf:about="http://www.semanticweb.org/covon/ontologies/2022/11/deconstruction-ontology#MaterialThermalProperty">
        <rdfs:subPropertyOf rdf:resource="http://www.w3.org/2002/07/owl#topDataProperty"/>
    </owl:DatatypeProperty>
    


    <!-- http://www.semanticweb.org/covon/ontologies/2022/11/deconstruction-ontology#Safeguard -->

    <owl:DatatypeProperty rdf:about="http://www.semanticweb.org/covon/ontologies/2022/11/deconstruction-ontology#Safeguard">
        <rdfs:subPropertyOf rdf:resource="http://www.w3.org/2002/07/owl#topDataProperty"/>
        <rdfs:range rdf:resource="http://www.w3.org/2001/XMLSchema#string"/>
        <rdfs:comment xml:lang="de">Diese Eigenschaft dient der Zuordnung von Sicherungsmaßnahmen.</rdfs:comment>
        <rdfs:comment xml:lang="en">This property is used for assigning safeguards.</rdfs:comment>
        <rdfs:label xml:lang="de">Sicherheitsmaßnahmen</rdfs:label>
    </owl:DatatypeProperty>
    


    <!-- http://www.semanticweb.org/covon/ontologies/2022/11/deconstruction-ontology#Suitability -->

    <owl:DatatypeProperty rdf:about="http://www.semanticweb.org/covon/ontologies/2022/11/deconstruction-ontology#Suitability">
        <rdfs:subPropertyOf rdf:resource="http://www.w3.org/2002/07/owl#topDataProperty"/>
        <rdfs:domain rdf:resource="http://www.semanticweb.org/covon/ontologies/2022/11/deconstruction-ontology#DeconstructionMethod"/>
        <rdfs:range rdf:resource="http://www.w3.org/2001/XMLSchema#string"/>
        <rdfs:comment xml:lang="de">Diese Eigenschaft ordnet einem Rückbauverfahren ein bestimmtes / bevorzugtes Einsatzgebiet zu.</rdfs:comment>
        <rdfs:comment xml:lang="en">This property assigns a specific / preferred application area to a deconstruction method.</rdfs:comment>
        <rdfs:label xml:lang="de">Eignungsfähigkeit</rdfs:label>
    </owl:DatatypeProperty>
    


    <!-- http://www.semanticweb.org/covon/ontologies/2022/11/deconstruction-ontology#constructionMethod -->

    <owl:DatatypeProperty rdf:about="http://www.semanticweb.org/covon/ontologies/2022/11/deconstruction-ontology#constructionMethod">
        <rdfs:subPropertyOf rdf:resource="http://www.w3.org/2002/07/owl#topDataProperty"/>
        <rdfs:domain rdf:resource="http://www.semanticweb.org/covon/ontologies/2022/11/deconstruction-ontology#DeconstructionObject"/>
        <rdfs:range>
            <rdfs:Datatype>
                <owl:oneOf>
                    <rdf:Description>
                        <rdf:type rdf:resource="http://www.w3.org/1999/02/22-rdf-syntax-ns#List"/>
                        <rdf:first>inSituConcreteConstruction</rdf:first>
                        <rdf:rest>
                            <rdf:Description>
                                <rdf:type rdf:resource="http://www.w3.org/1999/02/22-rdf-syntax-ns#List"/>
                                <rdf:first>masonryConstruction</rdf:first>
                                <rdf:rest>
                                    <rdf:Description>
                                        <rdf:type rdf:resource="http://www.w3.org/1999/02/22-rdf-syntax-ns#List"/>
                                        <rdf:first>precastConstruction</rdf:first>
                                        <rdf:rest>
                                            <rdf:Description>
                                                <rdf:type rdf:resource="http://www.w3.org/1999/02/22-rdf-syntax-ns#List"/>
                                                <rdf:first>steelConstruction</rdf:first>
                                                <rdf:rest>
                                                    <rdf:Description>
                                                        <rdf:type rdf:resource="http://www.w3.org/1999/02/22-rdf-syntax-ns#List"/>
                                                        <rdf:first>woodConstruction</rdf:first>
                                                        <rdf:rest rdf:resource="http://www.w3.org/1999/02/22-rdf-syntax-ns#nil"/>
                                                    </rdf:Description>
                                                </rdf:rest>
                                            </rdf:Description>
                                        </rdf:rest>
                                    </rdf:Description>
                                </rdf:rest>
                            </rdf:Description>
                        </rdf:rest>
                    </rdf:Description>
                </owl:oneOf>
            </rdfs:Datatype>
        </rdfs:range>
        <rdfs:comment xml:lang="de">Diese Eigenschaft ordnet einem Rückbauobjekt eine Bauweise zu.</rdfs:comment>
        <rdfs:comment xml:lang="en">This property assigns a construction method to a deconstruction object.</rdfs:comment>
        <rdfs:label xml:lang="de">Bauweise</rdfs:label>
    </owl:DatatypeProperty>
    


    <!-- http://www.semanticweb.org/covon/ontologies/2022/11/deconstruction-ontology#constructionPeriod -->

    <owl:DatatypeProperty rdf:about="http://www.semanticweb.org/covon/ontologies/2022/11/deconstruction-ontology#constructionPeriod">
        <rdfs:subPropertyOf rdf:resource="http://www.w3.org/2002/07/owl#topDataProperty"/>
        <rdfs:domain rdf:resource="http://www.semanticweb.org/covon/ontologies/2022/11/deconstruction-ontology#DeconstructionObject"/>
        <rdfs:range>
            <rdfs:Datatype>
                <owl:unionOf rdf:parseType="Collection">
                    <rdf:Description rdf:about="http://www.w3.org/2001/XMLSchema#integer"/>
                    <rdf:Description rdf:about="http://www.w3.org/2001/XMLSchema#string"/>
                </owl:unionOf>
            </rdfs:Datatype>
        </rdfs:range>
        <rdfs:comment xml:lang="de">Diese Eigenschaft ordnet einem Rückbauobjekt ein Baujahr oder -zeitraum zu.</rdfs:comment>
        <rdfs:comment xml:lang="en">This property assigns a construction year or period to a deconstruction object.</rdfs:comment>
        <rdfs:label xml:lang="de">Bauperiode</rdfs:label>
    </owl:DatatypeProperty>
    


    <!-- http://www.semanticweb.org/covon/ontologies/2022/11/deconstruction-ontology#constructionType -->

    <owl:DatatypeProperty rdf:about="http://www.semanticweb.org/covon/ontologies/2022/11/deconstruction-ontology#constructionType">
        <rdfs:subPropertyOf rdf:resource="http://www.w3.org/2002/07/owl#topDataProperty"/>
        <rdfs:domain rdf:resource="http://www.semanticweb.org/covon/ontologies/2022/11/deconstruction-ontology#DeconstructionObject"/>
        <rdfs:range>
            <rdfs:Datatype>
                <owl:oneOf>
                    <rdf:Description>
                        <rdf:type rdf:resource="http://www.w3.org/1999/02/22-rdf-syntax-ns#List"/>
                        <rdf:first>closeConstructionType</rdf:first>
                        <rdf:rest>
                            <rdf:Description>
                                <rdf:type rdf:resource="http://www.w3.org/1999/02/22-rdf-syntax-ns#List"/>
                                <rdf:first>openConstructionType</rdf:first>
                                <rdf:rest rdf:resource="http://www.w3.org/1999/02/22-rdf-syntax-ns#nil"/>
                            </rdf:Description>
                        </rdf:rest>
                    </rdf:Description>
                </owl:oneOf>
            </rdfs:Datatype>
        </rdfs:range>
        <rdfs:comment xml:lang="de">Diese Eigenschaft ordnet einem Rückbauobjekt eine Bebauungsweise zu.</rdfs:comment>
        <rdfs:comment xml:lang="en">This property assigns a construction type to a deconstruction object.</rdfs:comment>
        <rdfs:label xml:lang="de">Bebauungsweise</rdfs:label>
    </owl:DatatypeProperty>
    


    <!-- http://www.semanticweb.org/covon/ontologies/2022/11/deconstruction-ontology#dischargeOfContaminatedSubstance -->

    <owl:DatatypeProperty rdf:about="http://www.semanticweb.org/covon/ontologies/2022/11/deconstruction-ontology#dischargeOfContaminatedSubstance">
        <rdfs:subPropertyOf rdf:resource="http://www.w3.org/2002/07/owl#topDataProperty"/>
        <rdfs:range rdf:resource="http://www.w3.org/2001/XMLSchema#string"/>
        <rdfs:comment xml:lang="de">Diese Eigenschaft ordnet einem kontaminiertem Material die Art der Schadstofffreisetzung zu.</rdfs:comment>
        <rdfs:comment xml:lang="en">This property assigns the type of contaminant release to a contaminated material.</rdfs:comment>
        <rdfs:label xml:lang="de">Art der Schadstofffreisetzung</rdfs:label>
    </owl:DatatypeProperty>
    


    <!-- http://www.semanticweb.org/covon/ontologies/2022/11/deconstruction-ontology#functionalApplicationArea -->

    <owl:DatatypeProperty rdf:about="http://www.semanticweb.org/covon/ontologies/2022/11/deconstruction-ontology#functionalApplicationArea">
        <rdfs:subPropertyOf rdf:resource="http://www.semanticweb.org/covon/ontologies/2022/11/deconstruction-ontology#Suitability"/>
        <rdfs:comment xml:lang="de">Diese Eigenschaft ordnet einem Rückbauverfahren ein funktionelles Anwendungsgebiet zu.</rdfs:comment>
        <rdfs:comment xml:lang="en">This property assigns a functional application area to a deconstruction method.</rdfs:comment>
        <rdfs:label xml:lang="de">funktioneller Anwendungsbereich</rdfs:label>
    </owl:DatatypeProperty>
    


    <!-- http://www.semanticweb.org/covon/ontologies/2022/11/deconstruction-ontology#hasAcidityConcentration -->

    <owl:DatatypeProperty rdf:about="http://www.semanticweb.org/covon/ontologies/2022/11/deconstruction-ontology#hasAcidityConcentration">
        <rdfs:subPropertyOf rdf:resource="http://www.semanticweb.org/covon/ontologies/2022/11/deconstruction-ontology#MaterialChemicalProperty"/>
        <rdfs:comment>Maximum CaCO3 equivalent that would neutralize the acid.</rdfs:comment>
    </owl:DatatypeProperty>
    


    <!-- http://www.semanticweb.org/covon/ontologies/2022/11/deconstruction-ontology#hasAlkalinityConcentration -->

    <owl:DatatypeProperty rdf:about="http://www.semanticweb.org/covon/ontologies/2022/11/deconstruction-ontology#hasAlkalinityConcentration">
        <rdfs:subPropertyOf rdf:resource="http://www.semanticweb.org/covon/ontologies/2022/11/deconstruction-ontology#MaterialChemicalProperty"/>
        <rdfs:comment>Maximum alkalinity concentration (maximum sum of concentrations of each of the negative ions substances measured as CaCO3).</rdfs:comment>
    </owl:DatatypeProperty>
    


    <!-- http://www.semanticweb.org/covon/ontologies/2022/11/deconstruction-ontology#hasArtificialMineralFiber -->

    <owl:DatatypeProperty rdf:about="http://www.semanticweb.org/covon/ontologies/2022/11/deconstruction-ontology#hasArtificialMineralFiber">
        <rdfs:subPropertyOf rdf:resource="http://www.semanticweb.org/covon/ontologies/2022/11/deconstruction-ontology#MaterialContaminationProperty"/>
        <rdfs:range rdf:resource="http://www.w3.org/2001/XMLSchema#boolean"/>
    </owl:DatatypeProperty>
    


    <!-- http://www.semanticweb.org/covon/ontologies/2022/11/deconstruction-ontology#hasAsbestos -->

    <owl:DatatypeProperty rdf:about="http://www.semanticweb.org/covon/ontologies/2022/11/deconstruction-ontology#hasAsbestos">
        <rdfs:subPropertyOf rdf:resource="http://www.semanticweb.org/covon/ontologies/2022/11/deconstruction-ontology#MaterialContaminationProperty"/>
        <rdfs:range rdf:resource="http://www.w3.org/2001/XMLSchema#boolean"/>
    </owl:DatatypeProperty>
    


    <!-- http://www.semanticweb.org/covon/ontologies/2022/11/deconstruction-ontology#hasCO2Content -->

    <owl:DatatypeProperty rdf:about="http://www.semanticweb.org/covon/ontologies/2022/11/deconstruction-ontology#hasCO2Content">
        <rdfs:subPropertyOf rdf:resource="http://www.semanticweb.org/covon/ontologies/2022/11/deconstruction-ontology#MaterialCombustionProperty"/>
    </owl:DatatypeProperty>
    


    <!-- http://www.semanticweb.org/covon/ontologies/2022/11/deconstruction-ontology#hasCOContent -->

    <owl:DatatypeProperty rdf:about="http://www.semanticweb.org/covon/ontologies/2022/11/deconstruction-ontology#hasCOContent">
        <rdfs:subPropertyOf rdf:resource="http://www.semanticweb.org/covon/ontologies/2022/11/deconstruction-ontology#MaterialCombustionProperty"/>
    </owl:DatatypeProperty>
    


    <!-- http://www.semanticweb.org/covon/ontologies/2022/11/deconstruction-ontology#hasCarbonContent -->

    <owl:DatatypeProperty rdf:about="http://www.semanticweb.org/covon/ontologies/2022/11/deconstruction-ontology#hasCarbonContent">
        <rdfs:subPropertyOf rdf:resource="http://www.semanticweb.org/covon/ontologies/2022/11/deconstruction-ontology#MaterialFuelProperty"/>
        <rdfs:comment>The carbon content in the fuel. This is measured in weight of carbon per unit weight of fuel and is therefore unitless. [ISO 16739-1:2018]</rdfs:comment>
    </owl:DatatypeProperty>
    


    <!-- http://www.semanticweb.org/covon/ontologies/2022/11/deconstruction-ontology#hasCombustionTemperature -->

    <owl:DatatypeProperty rdf:about="http://www.semanticweb.org/covon/ontologies/2022/11/deconstruction-ontology#hasCombustionTemperature">
        <rdfs:subPropertyOf rdf:resource="http://www.semanticweb.org/covon/ontologies/2022/11/deconstruction-ontology#MaterialFuelProperty"/>
        <rdfs:comment>Combustion temperature of the material when air is at 298 K and 100 kPa. [ISO 16739-1:2018]</rdfs:comment>
    </owl:DatatypeProperty>
    


    <!-- http://www.semanticweb.org/covon/ontologies/2022/11/deconstruction-ontology#hasGasPressure -->

    <owl:DatatypeProperty rdf:about="http://www.semanticweb.org/covon/ontologies/2022/11/deconstruction-ontology#hasGasPressure">
        <rdfs:subPropertyOf rdf:resource="http://www.semanticweb.org/covon/ontologies/2022/11/deconstruction-ontology#MaterialEnergyProperty"/>
        <rdfs:comment>Fill pressure (e.g. for between-pane gas fills): the pressure exerted by a mass of gas confined in a constant volume. [ISO 16739-1:2018]</rdfs:comment>
    </owl:DatatypeProperty>
    


    <!-- http://www.semanticweb.org/covon/ontologies/2022/11/deconstruction-ontology#hasHalogenatedHydrocarbon -->

    <owl:DatatypeProperty rdf:about="http://www.semanticweb.org/covon/ontologies/2022/11/deconstruction-ontology#hasHalogenatedHydrocarbon">
        <rdfs:subPropertyOf rdf:resource="http://www.semanticweb.org/covon/ontologies/2022/11/deconstruction-ontology#MaterialContaminationProperty"/>
        <rdfs:range rdf:resource="http://www.w3.org/2001/XMLSchema#boolean"/>
    </owl:DatatypeProperty>
    


    <!-- http://www.semanticweb.org/covon/ontologies/2022/11/deconstruction-ontology#hasHardness -->

    <owl:DatatypeProperty rdf:about="http://www.semanticweb.org/covon/ontologies/2022/11/deconstruction-ontology#hasHardness">
        <rdfs:subPropertyOf rdf:resource="http://www.semanticweb.org/covon/ontologies/2022/11/deconstruction-ontology#MaterialChemicalProperty"/>
        <rdfs:comment>Water hardness as positive, multivalent ion concentration in the water (usually concentrations of calcium and magnesium ions in terms of calcium carbonate).</rdfs:comment>
    </owl:DatatypeProperty>
    


    <!-- http://www.semanticweb.org/covon/ontologies/2022/11/deconstruction-ontology#hasHeavyMetal -->

    <owl:DatatypeProperty rdf:about="http://www.semanticweb.org/covon/ontologies/2022/11/deconstruction-ontology#hasHeavyMetal">
        <rdfs:subPropertyOf rdf:resource="http://www.semanticweb.org/covon/ontologies/2022/11/deconstruction-ontology#MaterialContaminationProperty"/>
        <rdfs:range rdf:resource="http://www.w3.org/2001/XMLSchema#boolean"/>
    </owl:DatatypeProperty>
    


    <!-- http://www.semanticweb.org/covon/ontologies/2022/11/deconstruction-ontology#hasHigherHeatingValue -->

    <owl:DatatypeProperty rdf:about="http://www.semanticweb.org/covon/ontologies/2022/11/deconstruction-ontology#hasHigherHeatingValue">
        <rdfs:subPropertyOf rdf:resource="http://www.semanticweb.org/covon/ontologies/2022/11/deconstruction-ontology#MaterialFuelProperty"/>
        <rdfs:comment>Higher Heating Value is defined as the amount of energy released (MJ/kg) when a fuel is burned completely, and H2O is in liquid form in the combustion products. [ISO 16739-1:2018]</rdfs:comment>
    </owl:DatatypeProperty>
    


    <!-- http://www.semanticweb.org/covon/ontologies/2022/11/deconstruction-ontology#hasImpactOn -->

    <owl:DatatypeProperty rdf:about="http://www.semanticweb.org/covon/ontologies/2022/11/deconstruction-ontology#hasImpactOn">
        <rdfs:subPropertyOf rdf:resource="http://www.w3.org/2002/07/owl#topDataProperty"/>
        <rdfs:range>
            <rdfs:Datatype>
                <owl:oneOf>
                    <rdf:Description>
                        <rdf:type rdf:resource="http://www.w3.org/1999/02/22-rdf-syntax-ns#List"/>
                        <rdf:first>None</rdf:first>
                        <rdf:rest>
                            <rdf:Description>
                                <rdf:type rdf:resource="http://www.w3.org/1999/02/22-rdf-syntax-ns#List"/>
                                <rdf:first>Stability</rdf:first>
                                <rdf:rest>
                                    <rdf:Description>
                                        <rdf:type rdf:resource="http://www.w3.org/1999/02/22-rdf-syntax-ns#List"/>
                                        <rdf:first>environmentalIngressOfContaminatedSubstance</rdf:first>
                                        <rdf:rest>
                                            <rdf:Description>
                                                <rdf:type rdf:resource="http://www.w3.org/1999/02/22-rdf-syntax-ns#List"/>
                                                <rdf:first>leakageOfContaminatedMaterial</rdf:first>
                                                <rdf:rest rdf:resource="http://www.w3.org/1999/02/22-rdf-syntax-ns#nil"/>
                                            </rdf:Description>
                                        </rdf:rest>
                                    </rdf:Description>
                                </rdf:rest>
                            </rdf:Description>
                        </rdf:rest>
                    </rdf:Description>
                </owl:oneOf>
            </rdfs:Datatype>
        </rdfs:range>
        <rdfs:comment xml:lang="de">Diese Eigenschaft ordnet einem identifizierten Schaden die möglichen Auswirkungen zu.</rdfs:comment>
        <rdfs:comment xml:lang="en">This property assigns the potential impacts to an identified damage.</rdfs:comment>
        <rdfs:label xml:lang="de">hat Auswirkungen auf</rdfs:label>
    </owl:DatatypeProperty>
    


    <!-- http://www.semanticweb.org/covon/ontologies/2022/11/deconstruction-ontology#hasIsothermalMoistureCapacity -->

    <owl:DatatypeProperty rdf:about="http://www.semanticweb.org/covon/ontologies/2022/11/deconstruction-ontology#hasIsothermalMoistureCapacity">
        <rdfs:subPropertyOf rdf:resource="http://www.semanticweb.org/covon/ontologies/2022/11/deconstruction-ontology#MaterialHygroscopicProperty"/>
        <rdfs:comment>Based on water vapor density. [ISO 16739-1:2018]</rdfs:comment>
    </owl:DatatypeProperty>
    


    <!-- http://www.semanticweb.org/covon/ontologies/2022/11/deconstruction-ontology#hasLowerHeatingValue -->

    <owl:DatatypeProperty rdf:about="http://www.semanticweb.org/covon/ontologies/2022/11/deconstruction-ontology#hasLowerHeatingValue">
        <rdfs:subPropertyOf rdf:resource="http://www.semanticweb.org/covon/ontologies/2022/11/deconstruction-ontology#MaterialFuelProperty"/>
        <rdfs:comment>Lower Heating Value is defined as the amount of energy released (MJ/kg) when a fuel is burned completely, and H2O is in vapor form in the combustion products. [ISO 16739-1:2018]</rdfs:comment>
    </owl:DatatypeProperty>
    


    <!-- http://www.semanticweb.org/covon/ontologies/2022/11/deconstruction-ontology#hasLowerVaporResistanceFactor -->

    <owl:DatatypeProperty rdf:about="http://www.semanticweb.org/covon/ontologies/2022/11/deconstruction-ontology#hasLowerVaporResistanceFactor">
        <rdfs:subPropertyOf rdf:resource="http://www.semanticweb.org/covon/ontologies/2022/11/deconstruction-ontology#MaterialHygroscopicProperty"/>
        <rdfs:comment>The vapor permeability relationship of air/material (typically value &gt; 1), measured in low relative humidity (typically in 0/50 % RH). [ISO 16739-1:2018]</rdfs:comment>
    </owl:DatatypeProperty>
    


    <!-- http://www.semanticweb.org/covon/ontologies/2022/11/deconstruction-ontology#hasMoistureCapacityThermalGradient -->

    <owl:DatatypeProperty rdf:about="http://www.semanticweb.org/covon/ontologies/2022/11/deconstruction-ontology#hasMoistureCapacityThermalGradient">
        <rdfs:subPropertyOf rdf:resource="http://www.semanticweb.org/covon/ontologies/2022/11/deconstruction-ontology#MaterialEnergyProperty"/>
        <rdfs:comment>Thermal gradient coefficient for moisture capacity. Based on water vapor density.[ISO 16739-1:2018]</rdfs:comment>
    </owl:DatatypeProperty>
    


    <!-- http://www.semanticweb.org/covon/ontologies/2022/11/deconstruction-ontology#hasMoistureDiffusivity -->

    <owl:DatatypeProperty rdf:about="http://www.semanticweb.org/covon/ontologies/2022/11/deconstruction-ontology#hasMoistureDiffusivity">
        <rdfs:subPropertyOf rdf:resource="http://www.semanticweb.org/covon/ontologies/2022/11/deconstruction-ontology#MaterialHygroscopicProperty"/>
        <rdfs:comment>Moisture diffusivity is a transport property that is frequently used in the hygrothermal analysis of building envelope components. [ISO 16739-1:2018]</rdfs:comment>
    </owl:DatatypeProperty>
    


    <!-- http://www.semanticweb.org/covon/ontologies/2022/11/deconstruction-ontology#hasN20Content -->

    <owl:DatatypeProperty rdf:about="http://www.semanticweb.org/covon/ontologies/2022/11/deconstruction-ontology#hasN20Content">
        <rdfs:subPropertyOf rdf:resource="http://www.semanticweb.org/covon/ontologies/2022/11/deconstruction-ontology#MaterialCombustionProperty"/>
    </owl:DatatypeProperty>
    


    <!-- http://www.semanticweb.org/covon/ontologies/2022/11/deconstruction-ontology#hasNonHalogenatedHydrocarbon -->

    <owl:DatatypeProperty rdf:about="http://www.semanticweb.org/covon/ontologies/2022/11/deconstruction-ontology#hasNonHalogenatedHydrocarbon">
        <rdfs:subPropertyOf rdf:resource="http://www.semanticweb.org/covon/ontologies/2022/11/deconstruction-ontology#MaterialContaminationProperty"/>
        <rdfs:range rdf:resource="http://www.w3.org/2001/XMLSchema#boolean"/>
    </owl:DatatypeProperty>
    


    <!-- http://www.semanticweb.org/covon/ontologies/2022/11/deconstruction-ontology#hasPHLevel -->

    <owl:DatatypeProperty rdf:about="http://www.semanticweb.org/covon/ontologies/2022/11/deconstruction-ontology#hasPHLevel">
        <rdfs:subPropertyOf rdf:resource="http://www.semanticweb.org/covon/ontologies/2022/11/deconstruction-ontology#MaterialChemicalProperty"/>
        <rdfs:comment>Maximum water PH in a range from 0-14.</rdfs:comment>
    </owl:DatatypeProperty>
    


    <!-- http://www.semanticweb.org/covon/ontologies/2022/11/deconstruction-ontology#hasSpecificHeatTemperatureDerivative -->

    <owl:DatatypeProperty rdf:about="http://www.semanticweb.org/covon/ontologies/2022/11/deconstruction-ontology#hasSpecificHeatTemperatureDerivative">
        <rdfs:subPropertyOf rdf:resource="http://www.semanticweb.org/covon/ontologies/2022/11/deconstruction-ontology#MaterialEnergyProperty"/>
        <rdfs:comment>Specific heat temperature derivative. [ISO 16739-1:2018]</rdfs:comment>
    </owl:DatatypeProperty>
    


    <!-- http://www.semanticweb.org/covon/ontologies/2022/11/deconstruction-ontology#hasThermalConductivityTemperatureDerivative -->

    <owl:DatatypeProperty rdf:about="http://www.semanticweb.org/covon/ontologies/2022/11/deconstruction-ontology#hasThermalConductivityTemperatureDerivative">
        <rdfs:subPropertyOf rdf:resource="http://www.semanticweb.org/covon/ontologies/2022/11/deconstruction-ontology#MaterialEnergyProperty"/>
        <rdfs:comment>Thermal conductivity temperature derivative. [ISO 16739-1:2018]</rdfs:comment>
    </owl:DatatypeProperty>
    


    <!-- http://www.semanticweb.org/covon/ontologies/2022/11/deconstruction-ontology#hasUpperVaporResistanceFactor -->

    <owl:DatatypeProperty rdf:about="http://www.semanticweb.org/covon/ontologies/2022/11/deconstruction-ontology#hasUpperVaporResistanceFactor">
        <rdfs:subPropertyOf rdf:resource="http://www.semanticweb.org/covon/ontologies/2022/11/deconstruction-ontology#MaterialHygroscopicProperty"/>
        <rdfs:comment>The vapor permeability relationship of air/material (typically value &gt; 1), measured in high relative humidity (typically in 95/50 % RH). [ISO 16739-1:2018]</rdfs:comment>
    </owl:DatatypeProperty>
    


    <!-- http://www.semanticweb.org/covon/ontologies/2022/11/deconstruction-ontology#hasVaporPermeability -->

    <owl:DatatypeProperty rdf:about="http://www.semanticweb.org/covon/ontologies/2022/11/deconstruction-ontology#hasVaporPermeability">
        <rdfs:subPropertyOf rdf:resource="http://www.semanticweb.org/covon/ontologies/2022/11/deconstruction-ontology#MaterialHygroscopicProperty"/>
        <rdfs:comment>The rate of water vapor transmission per unit area per unit of vapor pressure differential under test conditions. [ISO 16739-1:2018]</rdfs:comment>
    </owl:DatatypeProperty>
    


    <!-- http://www.semanticweb.org/covon/ontologies/2022/11/deconstruction-ontology#hasViscosityTemperatureDerivative -->

    <owl:DatatypeProperty rdf:about="http://www.semanticweb.org/covon/ontologies/2022/11/deconstruction-ontology#hasViscosityTemperatureDerivative">
        <rdfs:subPropertyOf rdf:resource="http://www.semanticweb.org/covon/ontologies/2022/11/deconstruction-ontology#MaterialEnergyProperty"/>
        <rdfs:comment>Viscosity temperature derivative. [ISO 16739-1:2018]</rdfs:comment>
    </owl:DatatypeProperty>
    


    <!-- http://www.semanticweb.org/covon/ontologies/2022/11/deconstruction-ontology#hasVisibleRefractionIndex -->

    <owl:DatatypeProperty rdf:about="http://www.semanticweb.org/covon/ontologies/2022/11/deconstruction-ontology#hasVisibleRefractionIndex">
        <rdfs:subPropertyOf rdf:resource="http://www.semanticweb.org/covon/ontologies/2022/11/deconstruction-ontology#MaterialEnergyProperty"/>
        <rdfs:comment>Index of refraction (visible) defines the &quot;bending&quot; of the sola! r ray in the visible spectrum when it passes from one medium into another. [ISO 16739-1:2018]</rdfs:comment>
    </owl:DatatypeProperty>
    


    <!-- http://www.semanticweb.org/covon/ontologies/2022/11/deconstruction-ontology#isEnvironmentallyContaminatedBy -->

    <owl:DatatypeProperty rdf:about="http://www.semanticweb.org/covon/ontologies/2022/11/deconstruction-ontology#isEnvironmentallyContaminatedBy">
        <rdfs:subPropertyOf rdf:resource="http://www.w3.org/2002/07/owl#topDataProperty"/>
        <rdfs:domain rdf:resource="http://www.semanticweb.org/covon/ontologies/2022/11/deconstruction-ontology#Component"/>
        <rdfs:range rdf:resource="http://www.w3.org/2001/XMLSchema#string"/>
        <rdfs:comment xml:lang="de">Diese Eigenschaft ordnet einer Komponente einen Schadstoff zu, der von außen (umweltbedingt) in die Komponente eintritt.</rdfs:comment>
        <rdfs:comment xml:lang="en">This property assigns a pollutant to a component that penetrates the component from the outside (environmentally).</rdfs:comment>
        <rdfs:label xml:lang="de">ist umweltbedingt belastet durch</rdfs:label>
    </owl:DatatypeProperty>
    


    <!-- http://www.semanticweb.org/covon/ontologies/2022/11/deconstruction-ontology#isPartOf -->

    <owl:DatatypeProperty rdf:about="http://www.semanticweb.org/covon/ontologies/2022/11/deconstruction-ontology#isPartOf">
        <rdfs:subPropertyOf rdf:resource="http://www.w3.org/2002/07/owl#topDataProperty"/>
        <rdfs:domain rdf:resource="http://www.semanticweb.org/covon/ontologies/2022/11/deconstruction-ontology#Component"/>
        <rdfs:range>
            <rdfs:Datatype>
                <owl:oneOf>
                    <rdf:Description>
                        <rdf:type rdf:resource="http://www.w3.org/1999/02/22-rdf-syntax-ns#List"/>
                        <rdf:first>Demolition</rdf:first>
                        <rdf:rest>
                            <rdf:Description>
                                <rdf:type rdf:resource="http://www.w3.org/1999/02/22-rdf-syntax-ns#List"/>
                                <rdf:first>Dismantling</rdf:first>
                                <rdf:rest>
                                    <rdf:Description>
                                        <rdf:type rdf:resource="http://www.w3.org/1999/02/22-rdf-syntax-ns#List"/>
                                        <rdf:first>coreRemoval</rdf:first>
                                        <rdf:rest rdf:resource="http://www.w3.org/1999/02/22-rdf-syntax-ns#nil"/>
                                    </rdf:Description>
                                </rdf:rest>
                            </rdf:Description>
                        </rdf:rest>
                    </rdf:Description>
                </owl:oneOf>
            </rdfs:Datatype>
        </rdfs:range>
        <rdfs:comment xml:lang="de">Diese Eigenschaft ordnet einer Komponente einen bestimmten Rückbauabschnitt bzw. eine bestimmte Teilleistung zu.</rdfs:comment>
        <rdfs:comment xml:lang="en">This property assigns a specific deconstruction section or partial service to a component.</rdfs:comment>
        <rdfs:label xml:lang="de">ist Teil von</rdfs:label>
    </owl:DatatypeProperty>
    


    <!-- http://www.semanticweb.org/covon/ontologies/2022/11/deconstruction-ontology#levelOfDustExposure -->

    <owl:DatatypeProperty rdf:about="http://www.semanticweb.org/covon/ontologies/2022/11/deconstruction-ontology#levelOfDustExposure">
        <rdfs:subPropertyOf rdf:resource="http://www.semanticweb.org/covon/ontologies/2022/11/deconstruction-ontology#levelOfExposure"/>
        <rdfs:comment xml:lang="de">Diese Eigenschaft ordnet einem Rückbauverfahren den Grad der Staubeinwirkungen zu.</rdfs:comment>
        <rdfs:comment xml:lang="en">This property assigns the level of dust exposure to a deconstruction method.</rdfs:comment>
        <rdfs:label xml:lang="de">Grad der Staubeinwirkung</rdfs:label>
    </owl:DatatypeProperty>
    


    <!-- http://www.semanticweb.org/covon/ontologies/2022/11/deconstruction-ontology#levelOfExposure -->

    <owl:DatatypeProperty rdf:about="http://www.semanticweb.org/covon/ontologies/2022/11/deconstruction-ontology#levelOfExposure">
        <rdfs:subPropertyOf rdf:resource="http://www.w3.org/2002/07/owl#topDataProperty"/>
        <rdfs:domain rdf:resource="http://www.semanticweb.org/covon/ontologies/2022/11/deconstruction-ontology#DeconstructionMethod"/>
        <rdfs:range rdf:resource="http://www.w3.org/2001/XMLSchema#string"/>
        <rdfs:comment xml:lang="de">Diese Eigenschaft ordnet einem Rückbauverfahren den Grad der Emissionen zu.</rdfs:comment>
        <rdfs:comment xml:lang="en">This property assigns the level of exposure to a deconstruction method.</rdfs:comment>
        <rdfs:label xml:lang="de">Emissionsgrad</rdfs:label>
    </owl:DatatypeProperty>
    


    <!-- http://www.semanticweb.org/covon/ontologies/2022/11/deconstruction-ontology#levelOfMaterialExposure -->

    <owl:DatatypeProperty rdf:about="http://www.semanticweb.org/covon/ontologies/2022/11/deconstruction-ontology#levelOfMaterialExposure">
        <rdfs:subPropertyOf rdf:resource="http://www.semanticweb.org/covon/ontologies/2022/11/deconstruction-ontology#levelOfExposure"/>
        <rdfs:comment xml:lang="de">Diese Eigenschaft ordnet einem Rückbauverfahren den Grad der Streuflugeinwirkungen zu.</rdfs:comment>
        <rdfs:comment xml:lang="en">This property assigns the level of material exposure to a deconstruction method.</rdfs:comment>
        <rdfs:label xml:lang="de">Grad der Streuflugeinwirkung</rdfs:label>
    </owl:DatatypeProperty>
    


    <!-- http://www.semanticweb.org/covon/ontologies/2022/11/deconstruction-ontology#levelOfNoiseExposure -->

    <owl:DatatypeProperty rdf:about="http://www.semanticweb.org/covon/ontologies/2022/11/deconstruction-ontology#levelOfNoiseExposure">
        <rdfs:subPropertyOf rdf:resource="http://www.semanticweb.org/covon/ontologies/2022/11/deconstruction-ontology#levelOfExposure"/>
        <rdfs:comment xml:lang="de">Diese Eigenschaft ordnet einem Rückbauverfahren den Grad der Lärmeinwirkungen zu.</rdfs:comment>
        <rdfs:comment xml:lang="en">This property assigns the level of noise exposure to a deconstruction method.</rdfs:comment>
        <rdfs:label xml:lang="de">Grad der Lärmeinwirkung</rdfs:label>
    </owl:DatatypeProperty>
    


    <!-- http://www.semanticweb.org/covon/ontologies/2022/11/deconstruction-ontology#levelOfVibrationExposure -->

    <owl:DatatypeProperty rdf:about="http://www.semanticweb.org/covon/ontologies/2022/11/deconstruction-ontology#levelOfVibrationExposure">
        <rdfs:subPropertyOf rdf:resource="http://www.semanticweb.org/covon/ontologies/2022/11/deconstruction-ontology#levelOfExposure"/>
        <rdfs:comment xml:lang="de">Diese Eigenschaft ordnet einem Rückbauverfahren den Grad der Erschütterungseinwirkungen zu.</rdfs:comment>
        <rdfs:comment xml:lang="en">This property assigns the level of vibration exposure to a deconstruction method.</rdfs:comment>
        <rdfs:label xml:lang="de">Grad der Erschütterungseinwirkung</rdfs:label>
    </owl:DatatypeProperty>
    


    <!-- http://www.semanticweb.org/covon/ontologies/2022/11/deconstruction-ontology#levelOfWaterExposure -->

    <owl:DatatypeProperty rdf:about="http://www.semanticweb.org/covon/ontologies/2022/11/deconstruction-ontology#levelOfWaterExposure">
        <rdfs:subPropertyOf rdf:resource="http://www.semanticweb.org/covon/ontologies/2022/11/deconstruction-ontology#levelOfExposure"/>
        <rdfs:comment xml:lang="de">Diese Eigenschaft ordnet einem Rückbauverfahren den Grad der Wassereinwirkungen zu.</rdfs:comment>
        <rdfs:comment xml:lang="en">This property assigns the level of water exposure to a deconstruction method.</rdfs:comment>
        <rdfs:label xml:lang="de">Grad der Wassereinwirkung</rdfs:label>
    </owl:DatatypeProperty>
    


    <!-- http://www.semanticweb.org/covon/ontologies/2022/11/deconstruction-ontology#materialApplicationArea -->

    <owl:DatatypeProperty rdf:about="http://www.semanticweb.org/covon/ontologies/2022/11/deconstruction-ontology#materialApplicationArea">
        <rdfs:subPropertyOf rdf:resource="http://www.semanticweb.org/covon/ontologies/2022/11/deconstruction-ontology#Suitability"/>
        <rdfs:comment xml:lang="de">Diese Eigenschaft ordnet einem Rückbauverfahren ein materielles Anwendungsgebiet zu.</rdfs:comment>
        <rdfs:comment xml:lang="en">This property assigns a material application area to a deconstruction method.</rdfs:comment>
        <rdfs:label xml:lang="de">materieller Anwendungsbereich</rdfs:label>
    </owl:DatatypeProperty>
    


    <!-- http://www.semanticweb.org/covon/ontologies/2022/11/deconstruction-ontology#riskOfCollapse -->

    <owl:DatatypeProperty rdf:about="http://www.semanticweb.org/covon/ontologies/2022/11/deconstruction-ontology#riskOfCollapse">
        <rdfs:subPropertyOf rdf:resource="http://www.w3.org/2002/07/owl#topDataProperty"/>
        <rdfs:domain rdf:resource="http://www.semanticweb.org/covon/ontologies/2022/11/deconstruction-ontology#DeconstructionObject"/>
        <rdfs:range rdf:resource="http://www.w3.org/2001/XMLSchema#boolean"/>
        <rdfs:comment xml:lang="de">Diese Eigenschaft ordnet einem Rückbauobjekt das Merkmal der Einsturzgefährdung zu.</rdfs:comment>
        <rdfs:comment xml:lang="en">This property assigns the characteristic of collapse risk to a deconstruction object.</rdfs:comment>
        <rdfs:label xml:lang="de">Einsturzgefährdung</rdfs:label>
    </owl:DatatypeProperty>
    


    <!-- http://www.semanticweb.org/covon/ontologies/2022/11/deconstruction-ontology#specificApplicationArea -->

    <owl:DatatypeProperty rdf:about="http://www.semanticweb.org/covon/ontologies/2022/11/deconstruction-ontology#specificApplicationArea">
        <rdfs:subPropertyOf rdf:resource="http://www.semanticweb.org/covon/ontologies/2022/11/deconstruction-ontology#Suitability"/>
        <rdfs:comment xml:lang="de">Diese Eigenschaft ordnet einem Rückbauverfahren ein spezifisches Anwendungsgebiet zu, wie z.B. die Eignung für den Rückbau von Schadstoffen.</rdfs:comment>
        <rdfs:comment xml:lang="en">This property assigns a specific application area to a deconstruction method, e.g. suitability for deconstruction of pollutants.</rdfs:comment>
        <rdfs:label xml:lang="de">spezifischer Anwendungsbereich</rdfs:label>
    </owl:DatatypeProperty>
    


    <!-- http://www.semanticweb.org/covon/ontologies/2022/11/deconstruction-ontology#typeOfUse -->

    <owl:DatatypeProperty rdf:about="http://www.semanticweb.org/covon/ontologies/2022/11/deconstruction-ontology#typeOfUse">
        <rdfs:subPropertyOf rdf:resource="http://www.w3.org/2002/07/owl#topDataProperty"/>
        <rdfs:range rdf:resource="http://www.w3.org/2001/XMLSchema#string"/>
        <rdfs:comment xml:lang="de">Diese Eigenschaft ordnet einem Gebäude die Nutzungsart zu.</rdfs:comment>
        <rdfs:comment xml:lang="en">This property assigns the type of use to a building.</rdfs:comment>
        <rdfs:label xml:lang="de">Nutzungsart</rdfs:label>
    </owl:DatatypeProperty>
    


    <!-- http://www.semanticweb.org/covon/ontologies/2022/11/deconstruction-ontology#wasTypicallyUsedIn -->

    <owl:DatatypeProperty rdf:about="http://www.semanticweb.org/covon/ontologies/2022/11/deconstruction-ontology#wasTypicallyUsedIn">
        <rdfs:subPropertyOf rdf:resource="http://www.w3.org/2002/07/owl#topDataProperty"/>
        <rdfs:range rdf:resource="http://www.w3.org/2001/XMLSchema#string"/>
        <rdfs:comment xml:lang="de">Diese Eigenschaft ordnet einem Schadstoff einen typischen Verwendungszweck zu.</rdfs:comment>
        <rdfs:comment xml:lang="en">This property assigns a typical use to a pollutant.</rdfs:comment>
        <rdfs:label xml:lang="de">wurde üblicherweise verwendet in</rdfs:label>
    </owl:DatatypeProperty>
    


    <!-- http://www.semanticweb.org/covon/ontologies/2022/11/deconstruction-ontology#wasUsedUntil -->

    <owl:DatatypeProperty rdf:about="http://www.semanticweb.org/covon/ontologies/2022/11/deconstruction-ontology#wasUsedUntil">
        <rdfs:subPropertyOf rdf:resource="http://www.w3.org/2002/07/owl#topDataProperty"/>
        <rdfs:range rdf:resource="http://www.w3.org/2001/XMLSchema#integer"/>
        <rdfs:comment xml:lang="de">Diese Eigenschaft ordnet einem Schadstoff das Jahr zu, in dem der Schadstoff verboten worden ist.</rdfs:comment>
        <rdfs:comment xml:lang="en">This property assigns the year, in which the pollutant was prohibited, to a pollutant.</rdfs:comment>
        <rdfs:label xml:lang="de">wurde üblicherweise verwendet bis</rdfs:label>
    </owl:DatatypeProperty>
    


    <!-- http://www.semanticweb.org/evahe/ontologies/2024/1/dco#hasBoilingPoint -->

    <owl:DatatypeProperty rdf:about="http://www.semanticweb.org/evahe/ontologies/2024/1/dco#hasBoilingPoint">
        <rdfs:subPropertyOf rdf:resource="http://www.semanticweb.org/covon/ontologies/2022/11/deconstruction-ontology#MaterialThermalProperty"/>
    </owl:DatatypeProperty>
    


    <!-- http://www.semanticweb.org/evahe/ontologies/2024/1/dco#hasDynamicViscosity -->

    <owl:DatatypeProperty rdf:about="http://www.semanticweb.org/evahe/ontologies/2024/1/dco#hasDynamicViscosity">
        <rdfs:subPropertyOf rdf:resource="http://www.semanticweb.org/covon/ontologies/2022/11/deconstruction-ontology#MaterialMechanicalProperty"/>
        <rdfs:comment>A measure of the viscous resistance of the material. [ISO 16739-1:2018]</rdfs:comment>
    </owl:DatatypeProperty>
    


    <!-- http://www.semanticweb.org/evahe/ontologies/2024/1/dco#hasFreezingPoint -->

    <owl:DatatypeProperty rdf:about="http://www.semanticweb.org/evahe/ontologies/2024/1/dco#hasFreezingPoint">
        <rdfs:subPropertyOf rdf:resource="http://www.semanticweb.org/covon/ontologies/2022/11/deconstruction-ontology#MaterialThermalProperty"/>
    </owl:DatatypeProperty>
    


    <!-- http://www.semanticweb.org/evahe/ontologies/2024/1/dco#hasMassDensity -->

    <owl:DatatypeProperty rdf:about="http://www.semanticweb.org/evahe/ontologies/2024/1/dco#hasMassDensity">
        <rdfs:subPropertyOf rdf:resource="http://www.semanticweb.org/covon/ontologies/2022/11/deconstruction-ontology#MaterialPhysicalProperty"/>
        <rdfs:comment>Material mass density. [ISO 16739-1:2018]</rdfs:comment>
    </owl:DatatypeProperty>
    


    <!-- http://www.semanticweb.org/evahe/ontologies/2024/1/dco#hasMolecularWeight -->

    <owl:DatatypeProperty rdf:about="http://www.semanticweb.org/evahe/ontologies/2024/1/dco#hasMolecularWeight">
        <rdfs:subPropertyOf rdf:resource="http://www.semanticweb.org/covon/ontologies/2022/11/deconstruction-ontology#MaterialPhysicalProperty"/>
    </owl:DatatypeProperty>
    


    <!-- http://www.semanticweb.org/evahe/ontologies/2024/1/dco#hasPoissonRatio -->

    <owl:DatatypeProperty rdf:about="http://www.semanticweb.org/evahe/ontologies/2024/1/dco#hasPoissonRatio">
        <rdfs:subPropertyOf rdf:resource="http://www.semanticweb.org/covon/ontologies/2022/11/deconstruction-ontology#MaterialMechanicalProperty"/>
        <rdfs:comment>A measure of the lateral deformations in the elastic range. [ISO 16739-1:2018]</rdfs:comment>
    </owl:DatatypeProperty>
    


    <!-- http://www.semanticweb.org/evahe/ontologies/2024/1/dco#hasPorosity -->

    <owl:DatatypeProperty rdf:about="http://www.semanticweb.org/evahe/ontologies/2024/1/dco#hasPorosity">
        <rdfs:subPropertyOf rdf:resource="http://www.semanticweb.org/covon/ontologies/2022/11/deconstruction-ontology#MaterialPhysicalProperty"/>
    </owl:DatatypeProperty>
    


    <!-- http://www.semanticweb.org/evahe/ontologies/2024/1/dco#hasShearModulus -->

    <owl:DatatypeProperty rdf:about="http://www.semanticweb.org/evahe/ontologies/2024/1/dco#hasShearModulus">
        <rdfs:subPropertyOf rdf:resource="http://www.semanticweb.org/covon/ontologies/2022/11/deconstruction-ontology#MaterialMechanicalProperty"/>
        <rdfs:comment>A measure of the shear modulus of elasticity of the material. [ISO 16739-1:2018]</rdfs:comment>
    </owl:DatatypeProperty>
    


    <!-- http://www.semanticweb.org/evahe/ontologies/2024/1/dco#hasSolarReflectanceBack -->

    <owl:DatatypeProperty rdf:about="http://www.semanticweb.org/evahe/ontologies/2024/1/dco#hasSolarReflectanceBack">
        <rdfs:subPropertyOf rdf:resource="http://www.semanticweb.org/covon/ontologies/2022/11/deconstruction-ontology#MaterialOpticalProperty"/>
        <rdfs:comment>Reflectance at normal incidence (solar): back side. Defines the fraction of the solar ray that is reflected and not transmitted when the ray passes from one medium into another, at the &quot;back&quot; side of the other material, perpendicular to the surface. Dependent on material and surface characteristics. [ISO 16739-1:2018]</rdfs:comment>
    </owl:DatatypeProperty>
    


    <!-- http://www.semanticweb.org/evahe/ontologies/2024/1/dco#hasSolarReflectanceFront -->

    <owl:DatatypeProperty rdf:about="http://www.semanticweb.org/evahe/ontologies/2024/1/dco#hasSolarReflectanceFront">
        <rdfs:subPropertyOf rdf:resource="http://www.semanticweb.org/covon/ontologies/2022/11/deconstruction-ontology#MaterialOpticalProperty"/>
        <rdfs:comment>Reflectance at normal incidence (solar): front side. Defines the fraction of the solar ray that is reflected and not transmitted when the ray passes from one medium into another, at the &quot;front&quot; side of the other material, perpendicular to the surface. Dependent on material and surface characteristics.[ISO 16739-1:2018]</rdfs:comment>
    </owl:DatatypeProperty>
    


    <!-- http://www.semanticweb.org/evahe/ontologies/2024/1/dco#hasSolarRefractionIndex -->

    <owl:DatatypeProperty rdf:about="http://www.semanticweb.org/evahe/ontologies/2024/1/dco#hasSolarRefractionIndex">
        <rdfs:subPropertyOf rdf:resource="http://www.semanticweb.org/covon/ontologies/2022/11/deconstruction-ontology#MaterialOpticalProperty"/>
        <rdfs:comment>Index of refraction (solar) defines the &quot;bending&quot; of the solar ray when it passes from one medium into another. [ISO 16739-1:2018]</rdfs:comment>
    </owl:DatatypeProperty>
    


    <!-- http://www.semanticweb.org/evahe/ontologies/2024/1/dco#hasSolarTransmittance -->

    <owl:DatatypeProperty rdf:about="http://www.semanticweb.org/evahe/ontologies/2024/1/dco#hasSolarTransmittance">
        <rdfs:subPropertyOf rdf:resource="http://www.semanticweb.org/covon/ontologies/2022/11/deconstruction-ontology#MaterialOpticalProperty"/>
        <rdfs:comment>Transmittance at normal incidence (solar). Defines the fraction of solar radiation that passes through per unit area, perpendicular to the surface. [ISO 16739-1:2018]</rdfs:comment>
    </owl:DatatypeProperty>
    


    <!-- http://www.semanticweb.org/evahe/ontologies/2024/1/dco#hasSpecificHeatCapacity -->

    <owl:DatatypeProperty rdf:about="http://www.semanticweb.org/evahe/ontologies/2024/1/dco#hasSpecificHeatCapacity">
        <rdfs:subPropertyOf rdf:resource="http://www.semanticweb.org/covon/ontologies/2022/11/deconstruction-ontology#MaterialThermalProperty"/>
    </owl:DatatypeProperty>
    


    <!-- http://www.semanticweb.org/evahe/ontologies/2024/1/dco#hasThermalCapacity -->

    <owl:DatatypeProperty rdf:about="http://www.semanticweb.org/evahe/ontologies/2024/1/dco#hasThermalCapacity">
        <rdfs:subPropertyOf rdf:resource="http://www.semanticweb.org/covon/ontologies/2022/11/deconstruction-ontology#MaterialThermalProperty"/>
    </owl:DatatypeProperty>
    


    <!-- http://www.semanticweb.org/evahe/ontologies/2024/1/dco#hasThermalConductivity -->

    <owl:DatatypeProperty rdf:about="http://www.semanticweb.org/evahe/ontologies/2024/1/dco#hasThermalConductivity">
        <rdfs:subPropertyOf rdf:resource="http://www.semanticweb.org/covon/ontologies/2022/11/deconstruction-ontology#MaterialThermalProperty"/>
    </owl:DatatypeProperty>
    


    <!-- http://www.semanticweb.org/evahe/ontologies/2024/1/dco#hasThermalExpansionCoefficient -->

    <owl:DatatypeProperty rdf:about="http://www.semanticweb.org/evahe/ontologies/2024/1/dco#hasThermalExpansionCoefficient">
        <rdfs:subPropertyOf rdf:resource="http://www.semanticweb.org/covon/ontologies/2022/11/deconstruction-ontology#MaterialMechanicalProperty"/>
        <rdfs:comment>A measure of the expansion coefficient for warming up the material about one Kelvin. [ISO 16739-1:2018]</rdfs:comment>
    </owl:DatatypeProperty>
    


    <!-- http://www.semanticweb.org/evahe/ontologies/2024/1/dco#hasThermalIrEmissivityBack -->

    <owl:DatatypeProperty rdf:about="http://www.semanticweb.org/evahe/ontologies/2024/1/dco#hasThermalIrEmissivityBack">
        <rdfs:subPropertyOf rdf:resource="http://www.semanticweb.org/covon/ontologies/2022/11/deconstruction-ontology#MaterialOpticalProperty"/>
        <rdfs:comment>Thermal IR emissivity: back side. Defines the fraction of thermal energy emitted per unit area to &quot;blackbody&quot; at the same temperature, through the &quot;back&quot; side of the material. [ISO 16739-1:2018]</rdfs:comment>
    </owl:DatatypeProperty>
    


    <!-- http://www.semanticweb.org/evahe/ontologies/2024/1/dco#hasThermalIrEmissivityFront -->

    <owl:DatatypeProperty rdf:about="http://www.semanticweb.org/evahe/ontologies/2024/1/dco#hasThermalIrEmissivityFront">
        <rdfs:subPropertyOf rdf:resource="http://www.semanticweb.org/covon/ontologies/2022/11/deconstruction-ontology#MaterialOpticalProperty"/>
        <rdfs:comment>Thermal IR emissivity: front side. Defines the fraction of thermal energy emitted per unit area to &quot;blackbody&quot; at the same temperature, through the &quot;front&quot; side of the material.[ISO 16739-1:2018]</rdfs:comment>
    </owl:DatatypeProperty>
    


    <!-- http://www.semanticweb.org/evahe/ontologies/2024/1/dco#hasThermalIrTransmittance -->

    <owl:DatatypeProperty rdf:about="http://www.semanticweb.org/evahe/ontologies/2024/1/dco#hasThermalIrTransmittance">
        <rdfs:subPropertyOf rdf:resource="http://www.semanticweb.org/covon/ontologies/2022/11/deconstruction-ontology#MaterialOpticalProperty"/>
        <rdfs:comment>Thermal IR transmittance at normal incidence. Defines the fraction of thermal energy that passes through per unit area, perpendicular to the surface. [ISO 16739-1:2018]</rdfs:comment>
    </owl:DatatypeProperty>
    


    <!-- http://www.semanticweb.org/evahe/ontologies/2024/1/dco#hasThermalResistivity -->

    <owl:DatatypeProperty rdf:about="http://www.semanticweb.org/evahe/ontologies/2024/1/dco#hasThermalResistivity">
        <rdfs:subPropertyOf rdf:resource="http://www.semanticweb.org/covon/ontologies/2022/11/deconstruction-ontology#MaterialThermalProperty"/>
    </owl:DatatypeProperty>
    


    <!-- http://www.semanticweb.org/evahe/ontologies/2024/1/dco#hasVisibleReflectanceBack -->

    <owl:DatatypeProperty rdf:about="http://www.semanticweb.org/evahe/ontologies/2024/1/dco#hasVisibleReflectanceBack">
        <rdfs:subPropertyOf rdf:resource="http://www.semanticweb.org/covon/ontologies/2022/11/deconstruction-ontology#MaterialOpticalProperty"/>
        <rdfs:comment>Reflectance at normal incidence (visible): back side. Defines the fraction of the solar ray in the visible spectrum that is reflected and not transmitted when the ray passes from one medium into another, at the &quot;back&quot; side of the other material, perpendicular to the surface. Dependent on material and surface characteristics.[ISO 16739-1:2018]</rdfs:comment>
    </owl:DatatypeProperty>
    


    <!-- http://www.semanticweb.org/evahe/ontologies/2024/1/dco#hasVisibleReflectanceFront -->

    <owl:DatatypeProperty rdf:about="http://www.semanticweb.org/evahe/ontologies/2024/1/dco#hasVisibleReflectanceFront">
        <rdfs:subPropertyOf rdf:resource="http://www.semanticweb.org/covon/ontologies/2022/11/deconstruction-ontology#MaterialOpticalProperty"/>
        <rdfs:comment>Reflectance at normal incidence (visible): front side. Defines the fraction of the solar ray in the visible spectrum that is reflected and not transmitted when the ray passes from one medium into another, at the &quot;front&quot; side of the other material, perpendicular to the surface. Dependent on material and surface characteristics.[ISO 16739-1:2018]</rdfs:comment>
    </owl:DatatypeProperty>
    


    <!-- http://www.semanticweb.org/evahe/ontologies/2024/1/dco#hasVisibleTransmittance -->

    <owl:DatatypeProperty rdf:about="http://www.semanticweb.org/evahe/ontologies/2024/1/dco#hasVisibleTransmittance">
        <rdfs:subPropertyOf rdf:resource="http://www.semanticweb.org/covon/ontologies/2022/11/deconstruction-ontology#MaterialOpticalProperty"/>
        <rdfs:comment>Transmittance at normal incidence (visible). Defines the fraction of the visible spectrum of solar radiation that passes through per unit area, perpendicular to the surface. [ISO 16739-1:2018]</rdfs:comment>
    </owl:DatatypeProperty>
    


    <!-- http://www.semanticweb.org/evahe/ontologies/2024/1/dco#hasYoungModulus -->

    <owl:DatatypeProperty rdf:about="http://www.semanticweb.org/evahe/ontologies/2024/1/dco#hasYoungModulus">
        <rdfs:subPropertyOf rdf:resource="http://www.semanticweb.org/covon/ontologies/2022/11/deconstruction-ontology#MaterialMechanicalProperty"/>
        <rdfs:comment>A measure of the Young&apos;s modulus of elasticity of the material. [ISO 16739-1:2018]</rdfs:comment>
    </owl:DatatypeProperty>
    


    <!-- http://xmlns.com/foaf/0.1/accountName -->

    <owl:DatatypeProperty rdf:about="http://xmlns.com/foaf/0.1/accountName">
        <rdfs:range rdf:resource="http://www.w3.org/2000/01/rdf-schema#Literal"/>
        <rdfs:comment>Indicates the name (identifier) associated with this online account.</rdfs:comment>
        <rdfs:isDefinedBy rdf:resource="http://xmlns.com/foaf/0.1/"/>
        <rdfs:label>account name</rdfs:label>
        <ns:term_status>testing</ns:term_status>
    </owl:DatatypeProperty>
    


    <!-- http://xmlns.com/foaf/0.1/age -->

    <owl:DatatypeProperty rdf:about="http://xmlns.com/foaf/0.1/age">
        <rdf:type rdf:resource="http://www.w3.org/2002/07/owl#FunctionalProperty"/>
        <rdfs:range rdf:resource="http://www.w3.org/2000/01/rdf-schema#Literal"/>
        <rdfs:comment>The age in years of some agent.</rdfs:comment>
        <rdfs:isDefinedBy rdf:resource="http://xmlns.com/foaf/0.1/"/>
        <rdfs:label>age</rdfs:label>
        <ns:term_status>unstable</ns:term_status>
    </owl:DatatypeProperty>
    


    <!-- http://xmlns.com/foaf/0.1/aimChatID -->

    <owl:DatatypeProperty rdf:about="http://xmlns.com/foaf/0.1/aimChatID">
        <rdfs:range rdf:resource="http://www.w3.org/2000/01/rdf-schema#Literal"/>
    </owl:DatatypeProperty>
    


    <!-- http://xmlns.com/foaf/0.1/birthday -->

    <owl:DatatypeProperty rdf:about="http://xmlns.com/foaf/0.1/birthday">
        <rdf:type rdf:resource="http://www.w3.org/2002/07/owl#FunctionalProperty"/>
        <rdfs:range rdf:resource="http://www.w3.org/2000/01/rdf-schema#Literal"/>
        <rdfs:comment>The birthday of this Agent, represented in mm-dd string form, eg. &apos;12-31&apos;.</rdfs:comment>
        <rdfs:isDefinedBy rdf:resource="http://xmlns.com/foaf/0.1/"/>
        <rdfs:label>birthday</rdfs:label>
        <ns:term_status>unstable</ns:term_status>
    </owl:DatatypeProperty>
    


    <!-- http://xmlns.com/foaf/0.1/dnaChecksum -->

    <owl:DatatypeProperty rdf:about="http://xmlns.com/foaf/0.1/dnaChecksum">
        <rdfs:range rdf:resource="http://www.w3.org/2000/01/rdf-schema#Literal"/>
        <rdfs:comment>A checksum for the DNA of some thing. Joke.</rdfs:comment>
        <rdfs:isDefinedBy rdf:resource="http://xmlns.com/foaf/0.1/"/>
        <rdfs:label>DNA checksum</rdfs:label>
        <ns:term_status>archaic</ns:term_status>
    </owl:DatatypeProperty>
    


    <!-- http://xmlns.com/foaf/0.1/familyName -->

    <owl:DatatypeProperty rdf:about="http://xmlns.com/foaf/0.1/familyName">
        <rdfs:range rdf:resource="http://www.w3.org/2000/01/rdf-schema#Literal"/>
        <rdfs:comment>The family name of some person.</rdfs:comment>
        <rdfs:isDefinedBy rdf:resource="http://xmlns.com/foaf/0.1/"/>
        <rdfs:label>familyName</rdfs:label>
        <ns:term_status>testing</ns:term_status>
    </owl:DatatypeProperty>
    


    <!-- http://xmlns.com/foaf/0.1/family_name -->

    <owl:DatatypeProperty rdf:about="http://xmlns.com/foaf/0.1/family_name">
        <rdfs:range rdf:resource="http://www.w3.org/2000/01/rdf-schema#Literal"/>
        <rdfs:comment>The family name of some person.</rdfs:comment>
        <rdfs:isDefinedBy rdf:resource="http://xmlns.com/foaf/0.1/"/>
        <rdfs:label>family_name</rdfs:label>
        <ns:term_status>archaic</ns:term_status>
    </owl:DatatypeProperty>
    


    <!-- http://xmlns.com/foaf/0.1/firstName -->

    <owl:DatatypeProperty rdf:about="http://xmlns.com/foaf/0.1/firstName">
        <rdfs:range rdf:resource="http://www.w3.org/2000/01/rdf-schema#Literal"/>
        <rdfs:comment>The first name of a person.</rdfs:comment>
        <rdfs:isDefinedBy rdf:resource="http://xmlns.com/foaf/0.1/"/>
        <rdfs:label>firstName</rdfs:label>
        <ns:term_status>testing</ns:term_status>
    </owl:DatatypeProperty>
    


    <!-- http://xmlns.com/foaf/0.1/geekcode -->

    <owl:DatatypeProperty rdf:about="http://xmlns.com/foaf/0.1/geekcode">
        <rdfs:range rdf:resource="http://www.w3.org/2000/01/rdf-schema#Literal"/>
        <rdfs:comment>A textual geekcode for this person, see http://www.geekcode.com/geek.html</rdfs:comment>
        <rdfs:isDefinedBy rdf:resource="http://xmlns.com/foaf/0.1/"/>
        <rdfs:label>geekcode</rdfs:label>
        <ns:term_status>archaic</ns:term_status>
    </owl:DatatypeProperty>
    


    <!-- http://xmlns.com/foaf/0.1/gender -->

    <owl:DatatypeProperty rdf:about="http://xmlns.com/foaf/0.1/gender">
        <rdf:type rdf:resource="http://www.w3.org/2002/07/owl#FunctionalProperty"/>
        <rdfs:range rdf:resource="http://www.w3.org/2000/01/rdf-schema#Literal"/>
        <rdfs:comment>The gender of this Agent (typically but not necessarily &apos;male&apos; or &apos;female&apos;).</rdfs:comment>
        <rdfs:isDefinedBy rdf:resource="http://xmlns.com/foaf/0.1/"/>
        <rdfs:label>gender</rdfs:label>
        <ns:term_status>testing</ns:term_status>
    </owl:DatatypeProperty>
    


    <!-- http://xmlns.com/foaf/0.1/icqChatID -->

    <owl:DatatypeProperty rdf:about="http://xmlns.com/foaf/0.1/icqChatID">
        <rdfs:range rdf:resource="http://www.w3.org/2000/01/rdf-schema#Literal"/>
    </owl:DatatypeProperty>
    


    <!-- http://xmlns.com/foaf/0.1/lastName -->

    <owl:DatatypeProperty rdf:about="http://xmlns.com/foaf/0.1/lastName">
        <rdfs:range rdf:resource="http://www.w3.org/2000/01/rdf-schema#Literal"/>
        <rdfs:comment>The last name of a person.</rdfs:comment>
        <rdfs:isDefinedBy rdf:resource="http://xmlns.com/foaf/0.1/"/>
        <rdfs:label>lastName</rdfs:label>
        <ns:term_status>testing</ns:term_status>
    </owl:DatatypeProperty>
    


    <!-- http://xmlns.com/foaf/0.1/mbox_sha1sum -->

    <owl:DatatypeProperty rdf:about="http://xmlns.com/foaf/0.1/mbox_sha1sum">
        <rdfs:range rdf:resource="http://www.w3.org/2000/01/rdf-schema#Literal"/>
    </owl:DatatypeProperty>
    


    <!-- http://xmlns.com/foaf/0.1/msnChatID -->

    <owl:DatatypeProperty rdf:about="http://xmlns.com/foaf/0.1/msnChatID">
        <rdfs:range rdf:resource="http://www.w3.org/2000/01/rdf-schema#Literal"/>
    </owl:DatatypeProperty>
    


    <!-- http://xmlns.com/foaf/0.1/myersBriggs -->

    <owl:DatatypeProperty rdf:about="http://xmlns.com/foaf/0.1/myersBriggs">
        <rdfs:range rdf:resource="http://www.w3.org/2000/01/rdf-schema#Literal"/>
        <rdfs:comment>A Myers Briggs (MBTI) personality classification.</rdfs:comment>
        <rdfs:isDefinedBy rdf:resource="http://xmlns.com/foaf/0.1/"/>
        <rdfs:label>myersBriggs</rdfs:label>
        <ns:term_status>testing</ns:term_status>
    </owl:DatatypeProperty>
    


    <!-- http://xmlns.com/foaf/0.1/plan -->

    <owl:DatatypeProperty rdf:about="http://xmlns.com/foaf/0.1/plan">
        <rdfs:range rdf:resource="http://www.w3.org/2000/01/rdf-schema#Literal"/>
        <rdfs:comment>A .plan comment, in the tradition of finger and &apos;.plan&apos; files.</rdfs:comment>
        <rdfs:isDefinedBy rdf:resource="http://xmlns.com/foaf/0.1/"/>
        <rdfs:label>plan</rdfs:label>
        <ns:term_status>testing</ns:term_status>
    </owl:DatatypeProperty>
    


    <!-- http://xmlns.com/foaf/0.1/skypeID -->

    <owl:DatatypeProperty rdf:about="http://xmlns.com/foaf/0.1/skypeID">
        <rdfs:range rdf:resource="http://www.w3.org/2000/01/rdf-schema#Literal"/>
    </owl:DatatypeProperty>
    


    <!-- http://xmlns.com/foaf/0.1/status -->

    <owl:DatatypeProperty rdf:about="http://xmlns.com/foaf/0.1/status">
        <rdfs:range rdf:resource="http://www.w3.org/2000/01/rdf-schema#Literal"/>
        <rdfs:comment>A string expressing what the user is happy for the general public (normally) to know about their current activity.</rdfs:comment>
        <rdfs:isDefinedBy rdf:resource="http://xmlns.com/foaf/0.1/"/>
        <rdfs:label>status</rdfs:label>
        <ns:term_status>unstable</ns:term_status>
    </owl:DatatypeProperty>
    


    <!-- http://xmlns.com/foaf/0.1/surname -->

    <owl:DatatypeProperty rdf:about="http://xmlns.com/foaf/0.1/surname">
        <rdfs:range rdf:resource="http://www.w3.org/2000/01/rdf-schema#Literal"/>
        <rdfs:comment>The surname of some person.</rdfs:comment>
        <rdfs:isDefinedBy rdf:resource="http://xmlns.com/foaf/0.1/"/>
        <rdfs:label>Surname</rdfs:label>
        <ns:term_status>archaic</ns:term_status>
    </owl:DatatypeProperty>
    


    <!-- http://xmlns.com/foaf/0.1/yahooChatID -->

    <owl:DatatypeProperty rdf:about="http://xmlns.com/foaf/0.1/yahooChatID">
        <rdfs:range rdf:resource="http://www.w3.org/2000/01/rdf-schema#Literal"/>
    </owl:DatatypeProperty>
    


    <!-- https://w3id.org/digitalconstruction/0.3/BuildingMaterials#hasDefinedValue -->

    <owl:DatatypeProperty rdf:about="https://w3id.org/digitalconstruction/0.3/BuildingMaterials#hasDefinedValue">
        <rdfs:subPropertyOf rdf:resource="https://w3id.org/digitalconstruction/0.3/BuildingMaterials#hasValue"/>
        <rdfs:range rdf:resource="http://www.w3.org/2001/XMLSchema#double"/>
        <rdfs:comment>Defined value is the standard value taken from the authenticated sources. For example, it is a value taken from the standards.</rdfs:comment>
    </owl:DatatypeProperty>
    


    <!-- https://w3id.org/digitalconstruction/0.3/BuildingMaterials#hasEstimatedValue -->

    <owl:DatatypeProperty rdf:about="https://w3id.org/digitalconstruction/0.3/BuildingMaterials#hasEstimatedValue">
        <rdfs:subPropertyOf rdf:resource="https://w3id.org/digitalconstruction/0.3/BuildingMaterials#hasValue"/>
        <rdfs:range rdf:resource="http://www.w3.org/2001/XMLSchema#double"/>
        <rdfs:comment>Estimated value is the derived value or calculated value by using other property values</rdfs:comment>
    </owl:DatatypeProperty>
    


    <!-- https://w3id.org/digitalconstruction/0.3/BuildingMaterials#hasMeasuredValue -->

    <owl:DatatypeProperty rdf:about="https://w3id.org/digitalconstruction/0.3/BuildingMaterials#hasMeasuredValue">
        <rdfs:subPropertyOf rdf:resource="https://w3id.org/digitalconstruction/0.3/BuildingMaterials#hasValue"/>
        <rdfs:range rdf:resource="http://www.w3.org/2001/XMLSchema#double"/>
        <rdfs:comment>Measured Value is the resulted value from the measurement process</rdfs:comment>
    </owl:DatatypeProperty>
    


    <!-- https://w3id.org/digitalconstruction/0.3/BuildingMaterials#hasReference -->

    <owl:DatatypeProperty rdf:about="https://w3id.org/digitalconstruction/0.3/BuildingMaterials#hasReference">
        <rdfs:subPropertyOf rdf:resource="http://www.w3.org/2002/07/owl#topDataProperty"/>
        <rdfs:range rdf:resource="http://www.w3.org/2001/XMLSchema#string"/>
        <owl:propertyDisjointWith rdf:resource="https://w3id.org/digitalconstruction/0.3/BuildingMaterials#hasValue"/>
        <rdfs:comment>hasRefrence: is used to represent the relation between property and the source from where it is taken.</rdfs:comment>
    </owl:DatatypeProperty>
    


    <!-- https://w3id.org/digitalconstruction/0.3/BuildingMaterials#hasThickness -->

    <owl:DatatypeProperty rdf:about="https://w3id.org/digitalconstruction/0.3/BuildingMaterials#hasThickness">
        <rdfs:domain rdf:resource="https://w3id.org/digitalconstruction/0.3/BuildingMaterials#Layer"/>
    </owl:DatatypeProperty>
    


    <!-- https://w3id.org/digitalconstruction/0.3/BuildingMaterials#hasValue -->

    <owl:DatatypeProperty rdf:about="https://w3id.org/digitalconstruction/0.3/BuildingMaterials#hasValue">
        <rdfs:subPropertyOf rdf:resource="http://www.w3.org/2002/07/owl#topDataProperty"/>
        <rdfs:range rdf:resource="http://www.w3.org/2001/XMLSchema#double"/>
    </owl:DatatypeProperty>
    


    <!-- https://w3id.org/dot#filePath -->

    <owl:DatatypeProperty rdf:about="https://w3id.org/dot#filePath">
        <rdfs:domain rdf:resource="https://w3id.org/dot#ExternalResource"/>
        <rdfs:range rdf:resource="http://www.w3.org/2001/XMLSchema#anyURI"/>
        <rdfs:comment xml:lang="en">Defines the unique location in a file system of an External Resource</rdfs:comment>
        <rdfs:label xml:lang="en">file path</rdfs:label>
    </owl:DatatypeProperty>
    


    <!-- 
    ///////////////////////////////////////////////////////////////////////////////////////
    //
    // Classes
    //
    ///////////////////////////////////////////////////////////////////////////////////////
     -->

    


    <!-- http://purl.org/goodrelations/v1#SomeItems -->

    <owl:Class rdf:about="http://purl.org/goodrelations/v1#SomeItems"/>
    


    <!-- http://www.semanticweb.org/arnak/ontologies/2022/7/DOR#Certification -->

    <owl:Class rdf:about="http://www.semanticweb.org/arnak/ontologies/2022/7/DOR#Certification">
        <rdfs:subClassOf rdf:resource="http://www.semanticweb.org/arnak/ontologies/2022/7/DOR#CircularRequirement"/>
        <rdfs:comment>Certification requirements refer to the specific criteria or standards that need to be met in order to obtain certification for certain products, processes, or components within the context of circular economy practices. Not all circular potentials may require certification, but certification can be necessary for certain reusable structural parts or components. A certificate serves as a validation or endorsement that the product or component meets specific standards, regulations, or specifications related to safety, quality, environmental impact, or other relevant criteria.</rdfs:comment>
        <rdfs:label xml:lang="en">Certification</rdfs:label>
    </owl:Class>
    


    <!-- http://www.semanticweb.org/arnak/ontologies/2022/7/DOR#ChemicalConnection -->

    <owl:Class rdf:about="http://www.semanticweb.org/arnak/ontologies/2022/7/DOR#ChemicalConnection">
        <rdfs:subClassOf rdf:resource="http://www.semanticweb.org/arnak/ontologies/2022/7/DOR#ConnectionType"/>
        <owl:disjointWith rdf:resource="http://www.semanticweb.org/arnak/ontologies/2022/7/DOR#GravitationalConnection"/>
        <owl:disjointWith rdf:resource="http://www.semanticweb.org/arnak/ontologies/2022/7/DOR#MechanicalConnection"/>
        <owl:disjointWith>
            <owl:Class>
                <owl:unionOf rdf:parseType="Collection">
                    <rdf:Description rdf:about="http://www.semanticweb.org/arnak/ontologies/2022/7/DOR#GravitationalConnection"/>
                    <rdf:Description rdf:about="http://www.semanticweb.org/arnak/ontologies/2022/7/DOR#MechanicalConnection"/>
                </owl:unionOf>
            </owl:Class>
        </owl:disjointWith>
        <rdfs:comment xml:lang="en">This type of connection is formed through chemical reactions between two components, resulting in an irreversible bond. For example, the use of adhesives such as epoxy. A chemical connection could be Irreversible Connection.

Note: The irreversibility of this bond can pose challenges in the future, such as difficulty in disassembling or repairing the structure, thus leading to the preference for alternative methods of connection that possess greater versatility and ease of manipulation. The ChemicalConnection, while a common method utilized in conventional construction practices, is not necessarily deemed an optimal choice due to its permanent nature.</rdfs:comment>
        <rdfs:label xml:lang="en">Chemical Connection</rdfs:label>
    </owl:Class>
    


    <!-- http://www.semanticweb.org/arnak/ontologies/2022/7/DOR#CircularPotential -->

    <owl:Class rdf:about="http://www.semanticweb.org/arnak/ontologies/2022/7/DOR#CircularPotential">
        <rdfs:comment>To define what happens in the End-of-Life cycle of a building or functional layer or component, a circular potential can be attributed to it.</rdfs:comment>
        <rdfs:label xml:lang="en">Circular Potential</rdfs:label>
    </owl:Class>
    


    <!-- http://www.semanticweb.org/arnak/ontologies/2022/7/DOR#CircularRequirement -->

    <owl:Class rdf:about="http://www.semanticweb.org/arnak/ontologies/2022/7/DOR#CircularRequirement">
        <terms:description>For a Circular Potential to be realised after the deconstruction, often one or some requirements muct be met. This class is the range of hasCircularRequirement object property.</terms:description>
        <rdfs:comment>For a Circular Potential to be realised after the deconstruction, often one or some requirements muct be met. This class is the range of hasCircularRequirement object property.</rdfs:comment>
        <rdfs:label>Circular Requirement</rdfs:label>
    </owl:Class>
    


    <!-- http://www.semanticweb.org/arnak/ontologies/2022/7/DOR#ConnectionType -->

    <owl:Class rdf:about="http://www.semanticweb.org/arnak/ontologies/2022/7/DOR#ConnectionType">
        <rdfs:comment>A superclass that allows to describe the type of the connection.</rdfs:comment>
        <rdfs:label xml:lang="en">Connection Type</rdfs:label>
    </owl:Class>
    


    <!-- http://www.semanticweb.org/arnak/ontologies/2022/7/DOR#Designer -->

    <owl:Class rdf:about="http://www.semanticweb.org/arnak/ontologies/2022/7/DOR#Designer">
        <rdfs:subClassOf rdf:resource="http://xmlns.com/foaf/0.1/ProjectParticipant"/>
        <terms:description></terms:description>
        <rdfs:comment>A Designer is an actor who &quot;Designs For&quot; a certain circurlar potential</rdfs:comment>
        <rdfs:label xml:lang="en">Designer</rdfs:label>
    </owl:Class>
    


    <!-- http://www.semanticweb.org/arnak/ontologies/2022/7/DOR#DirectConnection -->

    <owl:Class rdf:about="http://www.semanticweb.org/arnak/ontologies/2022/7/DOR#DirectConnection">
        <rdfs:subClassOf rdf:resource="http://www.semanticweb.org/arnak/ontologies/2022/7/DOR#ConnectionType"/>
        <owl:disjointWith rdf:resource="http://www.semanticweb.org/arnak/ontologies/2022/7/DOR#IndirectConnection"/>
        <rdfs:comment xml:lang="en">The Direct Connection refers to a type of connection where two components are in direct physical contact with each other, with their surfaces touching. An example of a Direct Connection in the context of construction products would be the use of interlocking joints.

Note:The simplicity and directness of the Direct Connection make it a useful design choice in circualr construction projects, particularly in situations where a strong, stable connection is desired with minimal intervention.</rdfs:comment>
        <rdfs:label xml:lang="en">Direct Connection</rdfs:label>
    </owl:Class>
    


    <!-- http://www.semanticweb.org/arnak/ontologies/2022/7/DOR#DiscardPotential -->

    <owl:Class rdf:about="http://www.semanticweb.org/arnak/ontologies/2022/7/DOR#DiscardPotential">
        <owl:equivalentClass>
            <owl:Restriction>
                <owl:onProperty rdf:resource="http://www.semanticweb.org/arnak/ontologies/2022/7/DOR#hasCircularPotential"/>
                <owl:allValuesFrom>
                    <owl:Class>
                        <owl:intersectionOf rdf:parseType="Collection">
                            <owl:Class>
                                <owl:complementOf rdf:resource="http://www.semanticweb.org/arnak/ontologies/2022/7/DOR#RecyclingPotential"/>
                            </owl:Class>
                            <owl:Class>
                                <owl:complementOf rdf:resource="http://www.semanticweb.org/arnak/ontologies/2022/7/DOR#RemanufacturingPotential"/>
                            </owl:Class>
                            <owl:Class>
                                <owl:complementOf rdf:resource="http://www.semanticweb.org/arnak/ontologies/2022/7/DOR#RepurposingPotential"/>
                            </owl:Class>
                            <owl:Class>
                                <owl:complementOf rdf:resource="http://www.semanticweb.org/arnak/ontologies/2022/7/DOR#ReusePotential"/>
                            </owl:Class>
                        </owl:intersectionOf>
                    </owl:Class>
                </owl:allValuesFrom>
            </owl:Restriction>
        </owl:equivalentClass>
        <rdfs:subClassOf rdf:resource="http://www.semanticweb.org/arnak/ontologies/2022/7/DOR#CircularPotential"/>
        <owl:disjointWith rdf:resource="http://www.semanticweb.org/covon/ontologies/2022/11/deconstruction-ontology#WastePreventation"/>
        <owl:disjointWith rdf:resource="http://www.semanticweb.org/covon/ontologies/2022/11/deconstruction-ontology#WasteRemoval"/>
        <rdfs:comment>When an item can no longer be reused, remanufactured, or recycled, it will have Discard Potential.</rdfs:comment>
        <rdfs:label xml:lang="en">Discard Potential</rdfs:label>
    </owl:Class>
    


    <!-- http://www.semanticweb.org/arnak/ontologies/2022/7/DOR#Exposure -->

    <owl:Class rdf:about="http://www.semanticweb.org/arnak/ontologies/2022/7/DOR#Exposure">
        <rdfs:subClassOf rdf:resource="http://www.semanticweb.org/arnak/ontologies/2022/7/DOR#CircularRequirement"/>
        <rdfs:comment>Exposure is the class that helps with describing how a reusable item was (or should be) exposed to certain environmental conditions. If certain criteria must be met to keep the deconstructed elements in environmental conditions that stop their elements from deteriorating, these could be described in this class. Moreover, their storage conditions could also be described in this class.</rdfs:comment>
        <rdfs:label xml:lang="en">Exposure</rdfs:label>
    </owl:Class>
    


    <!-- http://www.semanticweb.org/arnak/ontologies/2022/7/DOR#Facade -->

    <owl:Class rdf:about="http://www.semanticweb.org/arnak/ontologies/2022/7/DOR#Facade">
        <rdfs:subClassOf rdf:resource="http://www.semanticweb.org/arnak/ontologies/2022/7/DOR#FunctionalLayer"/>
        <owl:disjointWith rdf:resource="http://www.semanticweb.org/covon/ontologies/2022/11/deconstruction-ontology#DeconstructionObject"/>
        <owl:disjointWith rdf:resource="http://www.semanticweb.org/covon/ontologies/2022/11/deconstruction-ontology#NeighboringObject"/>
        <owl:disjointWith rdf:resource="https://w3id.org/bot#Building"/>
        <owl:disjointWith rdf:resource="https://w3id.org/bot#Element"/>
        <rdfs:comment>According to Brent (1994), buildings are comprised of multiple layers of change, with each layer evolving on a timescale of its own. The Facade, or Skin, represents the exterior layer of a building, which undergoes more frequent changes compared to the structure.This class may be used for when the circular actors audit/recertify the facade layer of an existing building to be reused.</rdfs:comment>
        <rdfs:label xml:lang="en">Facade</rdfs:label>
    </owl:Class>
    


    <!-- http://www.semanticweb.org/arnak/ontologies/2022/7/DOR#FunctionalLayer -->

    <owl:Class rdf:about="http://www.semanticweb.org/arnak/ontologies/2022/7/DOR#FunctionalLayer">
        <owl:disjointWith rdf:resource="http://www.semanticweb.org/covon/ontologies/2022/11/deconstruction-ontology#DeconstructionObject"/>
        <owl:disjointWith rdf:resource="http://www.semanticweb.org/covon/ontologies/2022/11/deconstruction-ontology#NeighboringObject"/>
        <owl:disjointWith rdf:resource="https://w3id.org/bot#Building"/>
        <owl:disjointWith rdf:resource="https://w3id.org/bot#Element"/>
        <rdfs:comment>Fucntional Layer is disjoint with building and coponents.</rdfs:comment>
        <rdfs:label xml:lang="en">Functional Layer</rdfs:label>
    </owl:Class>
    


    <!-- http://www.semanticweb.org/arnak/ontologies/2022/7/DOR#GravitationalConnection -->

    <owl:Class rdf:about="http://www.semanticweb.org/arnak/ontologies/2022/7/DOR#GravitationalConnection">
        <rdfs:subClassOf rdf:resource="http://www.semanticweb.org/arnak/ontologies/2022/7/DOR#ConnectionType"/>
        <owl:disjointWith rdf:resource="http://www.semanticweb.org/arnak/ontologies/2022/7/DOR#MechanicalConnection"/>
        <owl:disjointWith>
            <owl:Class>
                <owl:unionOf rdf:parseType="Collection">
                    <rdf:Description rdf:about="http://www.semanticweb.org/arnak/ontologies/2022/7/DOR#ChemicalConnection"/>
                    <rdf:Description rdf:about="http://www.semanticweb.org/arnak/ontologies/2022/7/DOR#MechanicalConnection"/>
                </owl:unionOf>
            </owl:Class>
        </owl:disjointWith>
        <rdfs:comment xml:lang="en">Gravitational Connection is elaborated here based on the work of (Durmisevic, 2006).Gravitational Connection is introduced, but not thoroughly examined in DOR. Despite gravity&apos;s power to attract two objects, it is not widely utilized in construction projects. There is room for further elaboration and extension of this class. 

Reference: Durmisevic, E., 2006. Transformable building structures : design for dissassembly as a way to introduce sustainable engineering to building design &amp; construction (doctoral thesis). TUDelft.</rdfs:comment>
        <rdfs:label xml:lang="en">Gravitational Connection</rdfs:label>
    </owl:Class>
    


    <!-- http://www.semanticweb.org/arnak/ontologies/2022/7/DOR#HazardousMaterial -->

    <owl:Class rdf:about="http://www.semanticweb.org/arnak/ontologies/2022/7/DOR#HazardousMaterial">
        <rdfs:subClassOf rdf:resource="http://www.semanticweb.org/arnak/ontologies/2022/7/DOR#MaterialSourceType"/>
        <rdfs:subClassOf>
            <owl:Class>
                <owl:complementOf rdf:resource="http://www.semanticweb.org/arnak/ontologies/2022/7/DOR#NonHazardousMaterial"/>
            </owl:Class>
        </rdfs:subClassOf>
        <owl:disjointWith rdf:resource="http://www.semanticweb.org/arnak/ontologies/2022/7/DOR#NonHazardousMaterial"/>
        <rdfs:comment>According to the Waste Directive 2008/98/EC, hazardous materials are sourced from the type of resources that will cause health damage to humans, animals, plants, living organisms, and the environment.</rdfs:comment>
        <rdfs:label xml:lang="en">Hazardous Material</rdfs:label>
    </owl:Class>
    


    <!-- http://www.semanticweb.org/arnak/ontologies/2022/7/DOR#IndirectConnection -->

    <owl:Class rdf:about="http://www.semanticweb.org/arnak/ontologies/2022/7/DOR#IndirectConnection">
        <rdfs:subClassOf rdf:resource="http://www.semanticweb.org/arnak/ontologies/2022/7/DOR#ConnectionType"/>
        <rdfs:comment xml:lang="en">Indirect Connection</rdfs:comment>
    </owl:Class>
    


    <!-- http://www.semanticweb.org/arnak/ontologies/2022/7/DOR#Inspection -->

    <owl:Class rdf:about="http://www.semanticweb.org/arnak/ontologies/2022/7/DOR#Inspection">
        <rdfs:subClassOf rdf:resource="http://www.semanticweb.org/arnak/ontologies/2022/7/DOR#CircularRequirement"/>
        <rdfs:comment>An inspection might be a necessary requirment during or at the end of the life cycle for a component to reach its designated circualr potential.</rdfs:comment>
        <rdfs:label xml:lang="en">Inspection</rdfs:label>
    </owl:Class>
    


    <!-- http://www.semanticweb.org/arnak/ontologies/2022/7/DOR#InspectionMode -->

    <owl:Class rdf:about="http://www.semanticweb.org/arnak/ontologies/2022/7/DOR#InspectionMode">
        <rdfs:subClassOf rdf:resource="http://www.semanticweb.org/arnak/ontologies/2022/7/DOR#Inspection"/>
        <owl:disjointWith rdf:resource="http://www.semanticweb.org/arnak/ontologies/2022/7/DOR#Inspection_Method"/>
        <rdfs:comment>Inspection Mode refers to the different modes of conducting inspections, such as visual inspection, digital inspection, automated inspection, and so on.</rdfs:comment>
        <rdfs:label xml:lang="en">Inspection Mode</rdfs:label>
    </owl:Class>
    


    <!-- http://www.semanticweb.org/arnak/ontologies/2022/7/DOR#Inspection_Method -->

    <owl:Class rdf:about="http://www.semanticweb.org/arnak/ontologies/2022/7/DOR#Inspection_Method">
        <rdfs:subClassOf rdf:resource="http://www.semanticweb.org/arnak/ontologies/2022/7/DOR#Inspection"/>
        <rdfs:comment>Inspection Method refers to the different methods or types of inspections based on the necessary documentation or national and international standards.</rdfs:comment>
        <rdfs:label xml:lang="en">Inspection Method</rdfs:label>
    </owl:Class>
    


    <!-- http://www.semanticweb.org/arnak/ontologies/2022/7/DOR#Intervention -->

    <owl:Class rdf:about="http://www.semanticweb.org/arnak/ontologies/2022/7/DOR#Intervention">
        <rdfs:subClassOf rdf:resource="http://www.semanticweb.org/arnak/ontologies/2022/7/DOR#CircularRequirement"/>
        <rdfs:comment>This class  is suggested for cases where circular potentials need to be realised with certain interventions. An intervention could be a minor or major modification after deconstruction, or an intervention during the life cycle. Similarly, this class can contain additional information when an intervention is of type of repaire or replacement and so on.</rdfs:comment>
        <rdfs:label xml:lang="en">Intervention</rdfs:label>
    </owl:Class>
    


    <!-- http://www.semanticweb.org/arnak/ontologies/2022/7/DOR#IrreversibleConnection -->

    <owl:Class rdf:about="http://www.semanticweb.org/arnak/ontologies/2022/7/DOR#IrreversibleConnection">
        <rdfs:subClassOf rdf:resource="http://www.semanticweb.org/arnak/ontologies/2022/7/DOR#ConnectionType"/>
        <rdfs:subClassOf>
            <owl:Class>
                <owl:complementOf rdf:resource="http://www.semanticweb.org/arnak/ontologies/2022/7/DOR#ReversibleConnection"/>
            </owl:Class>
        </rdfs:subClassOf>
        <owl:disjointWith rdf:resource="http://www.semanticweb.org/arnak/ontologies/2022/7/DOR#ReversibleConnection"/>
        <rdfs:comment xml:lang="en">Irreversible connections cannot be easily disconnected or disassembled without causing permanent damage to the components or connections themselves. Examples of irreversible connections include welded joints or adhesive bonds, where the connections are designed to be permanent and cannot be easily undone.</rdfs:comment>
        <rdfs:label>Reversible Connection</rdfs:label>
    </owl:Class>
    


    <!-- http://www.semanticweb.org/arnak/ontologies/2022/7/DOR#LegalRequirement -->

    <owl:Class rdf:about="http://www.semanticweb.org/arnak/ontologies/2022/7/DOR#LegalRequirement">
        <rdfs:subClassOf rdf:resource="http://www.semanticweb.org/arnak/ontologies/2022/7/DOR#CircularRequirement"/>
        <rdfs:comment>Legal requirements in the context of this ontology refer to the regulations, rules, and/or design and implementation standards that govern the treatment, handling, and reuse of components. By including legal requirements as part of the information models, stakeholders can ensure that the necessary legal considerations are observed.</rdfs:comment>
        <rdfs:label>Legal Requirement</rdfs:label>
    </owl:Class>
    


    <!-- http://www.semanticweb.org/arnak/ontologies/2022/7/DOR#Logistics -->

    <owl:Class rdf:about="http://www.semanticweb.org/arnak/ontologies/2022/7/DOR#Logistics">
        <rdfs:subClassOf rdf:resource="http://www.semanticweb.org/arnak/ontologies/2022/7/DOR#CircularRequirement"/>
        <rdfs:comment>Logistics requirements refer to the specific needs -such as packaging requirements, truck sizes, and other logistical considerations -  related to the movement, transportation, and delivery of reusable components.</rdfs:comment>
        <rdfs:label xml:lang="en">Logistics</rdfs:label>
    </owl:Class>
    


    <!-- http://www.semanticweb.org/arnak/ontologies/2022/7/DOR#Manufacturer -->

    <owl:Class rdf:about="http://www.semanticweb.org/arnak/ontologies/2022/7/DOR#Manufacturer">
        <rdfs:subClassOf rdf:resource="http://xmlns.com/foaf/0.1/ProjectParticipant"/>
        <rdfs:comment>A Manufacturer is an actor who &quot;Produces For&quot; a certain circurlar potential</rdfs:comment>
        <rdfs:label xml:lang="en">Manufacturer</rdfs:label>
    </owl:Class>
    


    <!-- http://www.semanticweb.org/arnak/ontologies/2022/7/DOR#MaterialBankAgent -->

    <owl:Class rdf:about="http://www.semanticweb.org/arnak/ontologies/2022/7/DOR#MaterialBankAgent">
        <rdfs:subClassOf rdf:resource="http://xmlns.com/foaf/0.1/ProjectParticipant"/>
        <rdfs:comment>An agent of Material Bank who has the agency to &quot;Recertify For&quot; a certain circurlar potential after the assessments are done to check whether or not a component is reusable</rdfs:comment>
        <rdfs:label xml:lang="en">Material Bank Agent</rdfs:label>
    </owl:Class>
    


    <!-- http://www.semanticweb.org/arnak/ontologies/2022/7/DOR#MaterialSourceType -->

    <owl:Class rdf:about="http://www.semanticweb.org/arnak/ontologies/2022/7/DOR#MaterialSourceType">
        <rdfs:comment>This class extends the DICM:Material from the DICM ontology through DOR:hasSourceType property. Material Source Type points out the source type of materials, e.g., renewable or hazardous, emphasising the crucial role of the source of the material in decision-making for reuse, EoL treatment and handling.</rdfs:comment>
        <rdfs:label xml:lang="en">Material Source Type</rdfs:label>
    </owl:Class>
    


    <!-- http://www.semanticweb.org/arnak/ontologies/2022/7/DOR#MechanicalConnection -->

    <owl:Class rdf:about="http://www.semanticweb.org/arnak/ontologies/2022/7/DOR#MechanicalConnection">
        <rdfs:subClassOf rdf:resource="http://www.semanticweb.org/arnak/ontologies/2022/7/DOR#ConnectionType"/>
        <owl:disjointWith>
            <owl:Class>
                <owl:unionOf rdf:parseType="Collection">
                    <rdf:Description rdf:about="http://www.semanticweb.org/arnak/ontologies/2022/7/DOR#ChemicalConnection"/>
                    <rdf:Description rdf:about="http://www.semanticweb.org/arnak/ontologies/2022/7/DOR#GravitationalConnection"/>
                </owl:unionOf>
            </owl:Class>
        </owl:disjointWith>
        <rdfs:comment xml:lang="en">Mechanical Connection refers to type of connections that are established through the application of mechanical forces such as shear or tension. In the context of construction products, an example of a Mechanical Connection would be the use of threaded fasteners, such as bolts and nuts, to secure two or more components together. A mechanical connection could be Reversible Connection. 

Note: These connections, such as those created through the use of bolts, embody the ideal characteristics for circular design as they are capable of being easily reversed. The versatility offered by the reversibility of the MechanicalConnection makes it a highly desirable option in construction projects.</rdfs:comment>
        <rdfs:label xml:lang="en">Mechanical Connection</rdfs:label>
    </owl:Class>
    


    <!-- http://www.semanticweb.org/arnak/ontologies/2022/7/DOR#NonHazardousMaterial -->

    <owl:Class rdf:about="http://www.semanticweb.org/arnak/ontologies/2022/7/DOR#NonHazardousMaterial">
        <rdfs:subClassOf rdf:resource="http://www.semanticweb.org/arnak/ontologies/2022/7/DOR#MaterialSourceType"/>
        <rdfs:subClassOf>
            <owl:Class>
                <owl:complementOf rdf:resource="http://www.semanticweb.org/arnak/ontologies/2022/7/DOR#HazardousMaterial"/>
            </owl:Class>
        </rdfs:subClassOf>
        <rdfs:comment>A  type of resource that is not classified as hazardous is non-hazardous material source type.</rdfs:comment>
        <rdfs:label xml:lang="en">Non-hazardous Material</rdfs:label>
    </owl:Class>
    


    <!-- http://www.semanticweb.org/arnak/ontologies/2022/7/DOR#NonRenewableMaterial -->

    <owl:Class rdf:about="http://www.semanticweb.org/arnak/ontologies/2022/7/DOR#NonRenewableMaterial">
        <rdfs:subClassOf rdf:resource="http://www.semanticweb.org/arnak/ontologies/2022/7/DOR#MaterialSourceType"/>
        <rdfs:subClassOf>
            <owl:Class>
                <owl:complementOf rdf:resource="http://www.semanticweb.org/arnak/ontologies/2022/7/DOR#RenewableMaterial"/>
            </owl:Class>
        </rdfs:subClassOf>
        <owl:disjointWith rdf:resource="http://www.semanticweb.org/arnak/ontologies/2022/7/DOR#RenewableMaterial"/>
        <rdfs:comment xml:lang="en">A type of resource that exists in a fixed amount and cannot be naturally replenished or cleansed on a human time scale</rdfs:comment>
        <rdfs:label xml:lang="en">Non-renewable Material</rdfs:label>
    </owl:Class>
    


    <!-- http://www.semanticweb.org/arnak/ontologies/2022/7/DOR#OffSite -->

    <owl:Class rdf:about="http://www.semanticweb.org/arnak/ontologies/2022/7/DOR#OffSite">
        <rdfs:subClassOf rdf:resource="http://www.semanticweb.org/arnak/ontologies/2022/7/DOR#SiteDependency"/>
        <owl:disjointWith rdf:resource="http://www.semanticweb.org/arnak/ontologies/2022/7/DOR#OnSite"/>
        <rdfs:comment>Off-site site dependency refers to the situation where components from a particular site are transported or moved to another location.</rdfs:comment>
        <rdfs:label xml:lang="en">Off-site</rdfs:label>
    </owl:Class>
    


    <!-- http://www.semanticweb.org/arnak/ontologies/2022/7/DOR#OnSite -->

    <owl:Class rdf:about="http://www.semanticweb.org/arnak/ontologies/2022/7/DOR#OnSite">
        <rdfs:subClassOf rdf:resource="http://www.semanticweb.org/arnak/ontologies/2022/7/DOR#SiteDependency"/>
        <rdfs:comment>On-site site dependency emphasises the preference and recommendation to use components on the same construction site where they are currently located.</rdfs:comment>
        <rdfs:label xml:lang="en">On-site</rdfs:label>
    </owl:Class>
    


    <!-- http://www.semanticweb.org/arnak/ontologies/2022/7/DOR#Personnel -->

    <owl:Class rdf:about="http://www.semanticweb.org/arnak/ontologies/2022/7/DOR#Personnel">
        <rdfs:subClassOf rdf:resource="http://www.semanticweb.org/arnak/ontologies/2022/7/DOR#CircularRequirement"/>
        <rdfs:comment>In the context of circular requirements, Personnel refers to the human resources (with or without particular qualifications or skills) needed to carry out specific tasks related to deconstruction, reassembly, or other circular practices within a project.</rdfs:comment>
        <rdfs:label xml:lang="en">Personnel</rdfs:label>
    </owl:Class>
    


    <!-- http://www.semanticweb.org/arnak/ontologies/2022/7/DOR#PreDeconstructionAuditor -->

    <owl:Class rdf:about="http://www.semanticweb.org/arnak/ontologies/2022/7/DOR#PreDeconstructionAuditor">
        <rdfs:subClassOf rdf:resource="http://xmlns.com/foaf/0.1/ProjectParticipant"/>
        <rdfs:comment>An actor who does an audit before decommissioining phase starts and can audit for a ceratin circular potential</rdfs:comment>
        <rdfs:label xml:lang="en">Pre-Deconstruction Auditor</rdfs:label>
    </owl:Class>
    


    <!-- http://www.semanticweb.org/arnak/ontologies/2022/7/DOR#PrimaryRawMaterial -->

    <owl:Class rdf:about="http://www.semanticweb.org/arnak/ontologies/2022/7/DOR#PrimaryRawMaterial">
        <rdfs:subClassOf rdf:resource="http://www.semanticweb.org/arnak/ontologies/2022/7/DOR#MaterialSourceType"/>
        <owl:disjointWith rdf:resource="http://www.semanticweb.org/arnak/ontologies/2022/7/DOR#SecondaryRawMaterial"/>
        <rdfs:comment xml:lang="en">A type of resource that is extracted from the planet and used as inputs for industrial production. They are not processed or altered and are used in the first life cycle stage in the creation of a finished product.</rdfs:comment>
        <rdfs:label xml:lang="en">Primary Raw Material</rdfs:label>
    </owl:Class>
    


    <!-- http://www.semanticweb.org/arnak/ontologies/2022/7/DOR#RecyclableMaterial -->

    <owl:Class rdf:about="http://www.semanticweb.org/arnak/ontologies/2022/7/DOR#RecyclableMaterial">
        <rdfs:subClassOf rdf:resource="http://www.semanticweb.org/arnak/ontologies/2022/7/DOR#MaterialSourceType"/>
        <rdfs:comment xml:lang="en">A type of resource that has the characteristic to be diverted from the waste stream thanks to available processes and programmes and can be collected, processed and returned to (re)use in the form of raw materials</rdfs:comment>
        <rdfs:label xml:lang="en">Recyclable Material</rdfs:label>
    </owl:Class>
    


    <!-- http://www.semanticweb.org/arnak/ontologies/2022/7/DOR#RecyclingPotential -->

    <owl:Class rdf:about="http://www.semanticweb.org/arnak/ontologies/2022/7/DOR#RecyclingPotential">
        <rdfs:subClassOf rdf:resource="http://www.semanticweb.org/arnak/ontologies/2022/7/DOR#CircularPotential"/>
        <owl:disjointWith rdf:resource="http://www.semanticweb.org/covon/ontologies/2022/11/deconstruction-ontology#WastePreventation"/>
        <owl:disjointWith rdf:resource="http://www.semanticweb.org/covon/ontologies/2022/11/deconstruction-ontology#WasteRemoval"/>
        <rdfs:comment xml:lang="en">When an item can no longer be reused, remanufactured, or repaired, it can be recycled if the material is inherently recyclable. This results in the item having &quot;RecyclingPotential.&quot; For an assembly made with multiple materials to have RecyclingPotential, each material must be recyclable.</rdfs:comment>
        <rdfs:label xml:lang="en">Recycling Potential</rdfs:label>
    </owl:Class>
    


    <!-- http://www.semanticweb.org/arnak/ontologies/2022/7/DOR#RemanufacturingPotential -->

    <owl:Class rdf:about="http://www.semanticweb.org/arnak/ontologies/2022/7/DOR#RemanufacturingPotential">
        <rdfs:subClassOf rdf:resource="http://www.semanticweb.org/arnak/ontologies/2022/7/DOR#CircularPotential"/>
        <owl:disjointWith rdf:resource="http://www.semanticweb.org/covon/ontologies/2022/11/deconstruction-ontology#WastePreventation"/>
        <owl:disjointWith rdf:resource="http://www.semanticweb.org/covon/ontologies/2022/11/deconstruction-ontology#WasteRemoval"/>
        <rdfs:comment>Remanufacturing Potential is second to Reuse Potential. If an assembly, some sub-parts of the assembly might need to be replaced or repaired before being reused in the next life cycle.
If an element, the element needs major interventions such as repaire before it is can be reused.</rdfs:comment>
        <rdfs:label xml:lang="en">Remanufacturing Potential</rdfs:label>
    </owl:Class>
    


    <!-- http://www.semanticweb.org/arnak/ontologies/2022/7/DOR#RenewableMaterial -->

    <owl:Class rdf:about="http://www.semanticweb.org/arnak/ontologies/2022/7/DOR#RenewableMaterial">
        <rdfs:subClassOf rdf:resource="http://www.semanticweb.org/arnak/ontologies/2022/7/DOR#MaterialSourceType"/>
        <rdfs:subClassOf>
            <owl:Class>
                <owl:complementOf rdf:resource="http://www.semanticweb.org/arnak/ontologies/2022/7/DOR#NonRenewableMaterial"/>
            </owl:Class>
        </rdfs:subClassOf>
        <rdfs:comment xml:lang="en">A type of resource that could be grown and can be naturally replenished or cleansed on a human time scale.</rdfs:comment>
        <rdfs:label xml:lang="en">Renewable Material</rdfs:label>
    </owl:Class>
    


    <!-- http://www.semanticweb.org/arnak/ontologies/2022/7/DOR#RepurposingPotential -->

    <owl:Class rdf:about="http://www.semanticweb.org/arnak/ontologies/2022/7/DOR#RepurposingPotential">
        <rdfs:subClassOf rdf:resource="http://www.semanticweb.org/arnak/ontologies/2022/7/DOR#CircularPotential"/>
        <owl:disjointWith rdf:resource="http://www.semanticweb.org/covon/ontologies/2022/11/deconstruction-ontology#WastePreventation"/>
        <owl:disjointWith rdf:resource="http://www.semanticweb.org/covon/ontologies/2022/11/deconstruction-ontology#WasteRemoval"/>
        <rdfs:comment>For concrete, which is technically not recyclable, Repurposing Potential can be anticipated.</rdfs:comment>
        <rdfs:label xml:lang="en">Repurposing Potential</rdfs:label>
    </owl:Class>
    


    <!-- http://www.semanticweb.org/arnak/ontologies/2022/7/DOR#ReusePotential -->

    <owl:Class rdf:about="http://www.semanticweb.org/arnak/ontologies/2022/7/DOR#ReusePotential">
        <rdfs:subClassOf rdf:resource="http://www.semanticweb.org/arnak/ontologies/2022/7/DOR#CircularPotential"/>
        <owl:disjointWith rdf:resource="http://www.semanticweb.org/covon/ontologies/2022/11/deconstruction-ontology#WastePreventation"/>
        <owl:disjointWith rdf:resource="http://www.semanticweb.org/covon/ontologies/2022/11/deconstruction-ontology#WasteRemoval"/>
        <rdfs:comment>Reuse Potential is for components that need no major intervention (Aesthetic fixes might be necessary). If an assembly, all sub-parts of the assembly can be reused as they are deconstructued. If an element, the element as it is can be reused.</rdfs:comment>
        <rdfs:label xml:lang="en">Reuse Potential</rdfs:label>
    </owl:Class>
    


    <!-- http://www.semanticweb.org/arnak/ontologies/2022/7/DOR#ReversibleConnection -->

    <owl:Class rdf:about="http://www.semanticweb.org/arnak/ontologies/2022/7/DOR#ReversibleConnection">
        <rdfs:subClassOf rdf:resource="http://www.semanticweb.org/arnak/ontologies/2022/7/DOR#ConnectionType"/>
        <rdfs:subClassOf>
            <owl:Class>
                <owl:complementOf rdf:resource="http://www.semanticweb.org/arnak/ontologies/2022/7/DOR#IrreversibleConnection"/>
            </owl:Class>
        </rdfs:subClassOf>
        <rdfs:comment xml:lang="en">Reversible connections refer to connections that can be disconnected or disassembled - without causing significant damage - allowing for easy alteration and addition to structures. A bolt can be considered a reversible connection.</rdfs:comment>
        <rdfs:label xml:lang="en">Reversible Connection</rdfs:label>
    </owl:Class>
    


    <!-- http://www.semanticweb.org/arnak/ontologies/2022/7/DOR#SecondaryRawMaterial -->

    <owl:Class rdf:about="http://www.semanticweb.org/arnak/ontologies/2022/7/DOR#SecondaryRawMaterial">
        <rdfs:subClassOf rdf:resource="http://www.semanticweb.org/arnak/ontologies/2022/7/DOR#MaterialSourceType"/>
        <rdfs:comment>A type of resource that is recovered from previous use or is recovered waste originating from another product system and utilised as an input in another product system. Often, secondary raw material sources are recycled ones.</rdfs:comment>
        <rdfs:label>Secondary Raw Material</rdfs:label>
    </owl:Class>
    


    <!-- http://www.semanticweb.org/arnak/ontologies/2022/7/DOR#SiteDependency -->

    <owl:Class rdf:about="http://www.semanticweb.org/arnak/ontologies/2022/7/DOR#SiteDependency">
        <rdfs:subClassOf rdf:resource="http://www.semanticweb.org/arnak/ontologies/2022/7/DOR#CircularRequirement"/>
        <rdfs:comment>Site dependency refers to the extent to which a construction project relies on the physical location of the current project. This circular requirement is important for decision makings in multiple layers and impacts the carbon and waste outputs of whether or not a component is reused on site or not.</rdfs:comment>
        <rdfs:label xml:lang="en">Site Dependency</rdfs:label>
    </owl:Class>
    


    <!-- http://www.semanticweb.org/arnak/ontologies/2022/7/DOR#SpacePlan -->

    <owl:Class rdf:about="http://www.semanticweb.org/arnak/ontologies/2022/7/DOR#SpacePlan">
        <rdfs:subClassOf rdf:resource="http://www.semanticweb.org/arnak/ontologies/2022/7/DOR#FunctionalLayer"/>
        <owl:disjointWith rdf:resource="http://www.semanticweb.org/covon/ontologies/2022/11/deconstruction-ontology#DeconstructionObject"/>
        <owl:disjointWith rdf:resource="http://www.semanticweb.org/covon/ontologies/2022/11/deconstruction-ontology#NeighboringObject"/>
        <owl:disjointWith rdf:resource="https://w3id.org/bot#Building"/>
        <owl:disjointWith rdf:resource="https://w3id.org/bot#Element"/>
        <rdfs:comment>According to Brent (1994), buildings are comprised of multiple layers of change, with each layer evolving on a timescale of its own.</rdfs:comment>
        <rdfs:label xml:lang="en">Space Plan</rdfs:label>
    </owl:Class>
    


    <!-- http://www.semanticweb.org/arnak/ontologies/2022/7/DOR#Structure -->

    <owl:Class rdf:about="http://www.semanticweb.org/arnak/ontologies/2022/7/DOR#Structure">
        <rdfs:subClassOf rdf:resource="http://www.semanticweb.org/arnak/ontologies/2022/7/DOR#FunctionalLayer"/>
        <owl:disjointWith rdf:resource="http://www.semanticweb.org/covon/ontologies/2022/11/deconstruction-ontology#DeconstructionObject"/>
        <owl:disjointWith rdf:resource="http://www.semanticweb.org/covon/ontologies/2022/11/deconstruction-ontology#NeighboringObject"/>
        <owl:disjointWith rdf:resource="https://w3id.org/bot#Building"/>
        <owl:disjointWith rdf:resource="https://w3id.org/bot#Element"/>
        <rdfs:comment>According to Brent (1994), buildings are comprised of multiple layers of change, with each layer evolving on a timescale of its own. The structure layer signified the foundation and other load-bearing components of a building, which are (1) challenging and costly to modify, (2) have longer life spans in comparision with other building components and layers, all of which leading to infrequent alterations. This class my be used for when the structure of a new construction building is designed to be completely reused in the future, or when the circualr actors audit/recertify the structure layer to be reused in an exisitng building.</rdfs:comment>
        <rdfs:label xml:lang="en">Structure</rdfs:label>
    </owl:Class>
    


    <!-- http://www.semanticweb.org/arnak/ontologies/2022/7/DOR#TrainedPersonnel -->

    <owl:Class rdf:about="http://www.semanticweb.org/arnak/ontologies/2022/7/DOR#TrainedPersonnel">
        <rdfs:subClassOf rdf:resource="http://www.semanticweb.org/arnak/ontologies/2022/7/DOR#Personnel"/>
        <rdfs:comment>Trained personnel possess the specialised knowledge, skills, and training necessary to perform specific tasks related to circular practices.</rdfs:comment>
        <rdfs:label xml:lang="en">Trainned Personnel</rdfs:label>
    </owl:Class>
    


    <!-- http://www.semanticweb.org/arnak/ontologies/2022/7/DOR#UntrainedPersonnel -->

    <owl:Class rdf:about="http://www.semanticweb.org/arnak/ontologies/2022/7/DOR#UntrainedPersonnel">
        <rdfs:subClassOf rdf:resource="http://www.semanticweb.org/arnak/ontologies/2022/7/DOR#Personnel"/>
        <rdfs:comment>Untrained personnel refers to individuals who do not possess specialised training or expertise but can still contribute to circular practices. They may not have the same level of knowledge or qualification as trained personnel to participate in certain disassembly or assembly activities.</rdfs:comment>
        <rdfs:label xml:lang="en">Untrainned Personnel</rdfs:label>
    </owl:Class>
    


    <!-- http://www.semanticweb.org/covon/ontologies/2022/11/deconstruction-ontology#AblatingMethod -->

    <owl:Class rdf:about="http://www.semanticweb.org/covon/ontologies/2022/11/deconstruction-ontology#AblatingMethod">
        <rdfs:subClassOf rdf:resource="http://www.semanticweb.org/covon/ontologies/2022/11/deconstruction-ontology#DeconstructionMethod"/>
        <rdfs:label xml:lang="de">Abtragende Verfahren</rdfs:label>
    </owl:Class>
    


    <!-- http://www.semanticweb.org/covon/ontologies/2022/11/deconstruction-ontology#BearingElement -->

    <owl:Class rdf:about="http://www.semanticweb.org/covon/ontologies/2022/11/deconstruction-ontology#BearingElement">
        <rdfs:subClassOf rdf:resource="https://w3id.org/bot#Element"/>
    </owl:Class>
    


    <!-- http://www.semanticweb.org/covon/ontologies/2022/11/deconstruction-ontology#BlastingDown -->

    <owl:Class rdf:about="http://www.semanticweb.org/covon/ontologies/2022/11/deconstruction-ontology#BlastingDown">
        <rdfs:subClassOf rdf:resource="http://www.semanticweb.org/covon/ontologies/2022/11/deconstruction-ontology#BlastingMethod"/>
        <rdfs:label xml:lang="de">Niederbringen durch Sprengen</rdfs:label>
    </owl:Class>
    


    <!-- http://www.semanticweb.org/covon/ontologies/2022/11/deconstruction-ontology#BlastingMethod -->

    <owl:Class rdf:about="http://www.semanticweb.org/covon/ontologies/2022/11/deconstruction-ontology#BlastingMethod">
        <rdfs:subClassOf rdf:resource="http://www.semanticweb.org/covon/ontologies/2022/11/deconstruction-ontology#DeconstructionMethod"/>
        <rdfs:label xml:lang="de">Sprengende Verfahren</rdfs:label>
    </owl:Class>
    


    <!-- http://www.semanticweb.org/covon/ontologies/2022/11/deconstruction-ontology#ChainSaw -->

    <owl:Class rdf:about="http://www.semanticweb.org/covon/ontologies/2022/11/deconstruction-ontology#ChainSaw">
        <rdfs:subClassOf rdf:resource="http://www.semanticweb.org/covon/ontologies/2022/11/deconstruction-ontology#SawingMethod"/>
        <rdfs:label xml:lang="de">Kettensägen</rdfs:label>
    </owl:Class>
    


    <!-- http://www.semanticweb.org/covon/ontologies/2022/11/deconstruction-ontology#Chiseling -->

    <owl:Class rdf:about="http://www.semanticweb.org/covon/ontologies/2022/11/deconstruction-ontology#Chiseling">
        <rdfs:subClassOf rdf:resource="http://www.semanticweb.org/covon/ontologies/2022/11/deconstruction-ontology#MechanicalMethod"/>
        <rdfs:label xml:lang="de">Stemmen</rdfs:label>
    </owl:Class>
    


    <!-- http://www.semanticweb.org/covon/ontologies/2022/11/deconstruction-ontology#CollapseBlasting -->

    <owl:Class rdf:about="http://www.semanticweb.org/covon/ontologies/2022/11/deconstruction-ontology#CollapseBlasting">
        <rdfs:subClassOf rdf:resource="http://www.semanticweb.org/covon/ontologies/2022/11/deconstruction-ontology#BlastingMethod"/>
        <rdfs:label xml:lang="de">Zusammenstürzen durch Sprengen</rdfs:label>
    </owl:Class>
    


    <!-- http://www.semanticweb.org/covon/ontologies/2022/11/deconstruction-ontology#Component -->

    <owl:Class rdf:about="http://www.semanticweb.org/covon/ontologies/2022/11/deconstruction-ontology#Component">
        <rdfs:comment xml:lang="en">Components are parts of an element.</rdfs:comment>
        <rdfs:comment xml:lang="de">Komponenten sind Teile eines Bauteils.</rdfs:comment>
        <rdfs:label xml:lang="de">Komponenten</rdfs:label>
    </owl:Class>
    


    <!-- http://www.semanticweb.org/covon/ontologies/2022/11/deconstruction-ontology#CoreDrilling -->

    <owl:Class rdf:about="http://www.semanticweb.org/covon/ontologies/2022/11/deconstruction-ontology#CoreDrilling">
        <rdfs:subClassOf rdf:resource="http://www.semanticweb.org/covon/ontologies/2022/11/deconstruction-ontology#DrillingMethod"/>
        <rdfs:label xml:lang="de">Kernbohren</rdfs:label>
    </owl:Class>
    


    <!-- http://www.semanticweb.org/covon/ontologies/2022/11/deconstruction-ontology#Crack -->

    <owl:Class rdf:about="http://www.semanticweb.org/covon/ontologies/2022/11/deconstruction-ontology#Crack">
        <rdfs:subClassOf rdf:resource="https://w3id.org/dot#ClassifiedDamage"/>
        <owl:disjointWith rdf:resource="https://w3id.org/dot#UnclassifiedDamage"/>
        <rdfs:comment xml:lang="en">Class for the representation of damages in the form of cracks.</rdfs:comment>
        <rdfs:comment xml:lang="de">Klasse zur Darstellung von Schäden in Form von Rissen.</rdfs:comment>
        <rdfs:label xml:lang="de">Riss</rdfs:label>
    </owl:Class>
    


    <!-- http://www.semanticweb.org/covon/ontologies/2022/11/deconstruction-ontology#Crushing -->

    <owl:Class rdf:about="http://www.semanticweb.org/covon/ontologies/2022/11/deconstruction-ontology#Crushing">
        <rdfs:subClassOf rdf:resource="http://www.semanticweb.org/covon/ontologies/2022/11/deconstruction-ontology#MechanicalMethod"/>
        <rdfs:label xml:lang="de">Zerkleinern</rdfs:label>
    </owl:Class>
    


    <!-- http://www.semanticweb.org/covon/ontologies/2022/11/deconstruction-ontology#DeconstructionMethod -->

    <owl:Class rdf:about="http://www.semanticweb.org/covon/ontologies/2022/11/deconstruction-ontology#DeconstructionMethod">
        <rdfs:comment xml:lang="de">Darstellung von Abbruchverfahren nach DIN 18007.</rdfs:comment>
        <rdfs:comment xml:lang="en">Representation of demolition methods according to DIN 18007.</rdfs:comment>
        <rdfs:label xml:lang="de">Abbruchverfahren</rdfs:label>
    </owl:Class>
    


    <!-- http://www.semanticweb.org/covon/ontologies/2022/11/deconstruction-ontology#DeconstructionObject -->

    <owl:Class rdf:about="http://www.semanticweb.org/covon/ontologies/2022/11/deconstruction-ontology#DeconstructionObject">
        <rdfs:subClassOf rdf:resource="https://w3id.org/bot#Building"/>
        <owl:disjointWith rdf:resource="http://www.semanticweb.org/covon/ontologies/2022/11/deconstruction-ontology#NeighboringObject"/>
        <owl:disjointWith rdf:resource="https://w3id.org/bot#Element"/>
        <owl:disjointWith rdf:resource="https://w3id.org/bot#Interface"/>
        <owl:disjointWith rdf:resource="https://w3id.org/bot#Site"/>
        <owl:disjointWith rdf:resource="https://w3id.org/bot#Space"/>
        <owl:disjointWith rdf:resource="https://w3id.org/bot#Storey"/>
        <rdfs:comment xml:lang="en">A building which is to be deconstructed.</rdfs:comment>
        <rdfs:comment xml:lang="de">Ein Gebäude, welches zurückgebaut werden soll.</rdfs:comment>
        <rdfs:label xml:lang="de">Rückbauobjekt</rdfs:label>
    </owl:Class>
    


    <!-- http://www.semanticweb.org/covon/ontologies/2022/11/deconstruction-ontology#Deformation -->

    <owl:Class rdf:about="http://www.semanticweb.org/covon/ontologies/2022/11/deconstruction-ontology#Deformation">
        <rdfs:subClassOf rdf:resource="https://w3id.org/dot#ClassifiedDamage"/>
        <owl:disjointWith rdf:resource="https://w3id.org/dot#UnclassifiedDamage"/>
        <rdfs:comment xml:lang="en">Class for the representation of damages in the form of deformations.</rdfs:comment>
        <rdfs:comment xml:lang="de">Klasse zur Darstellung von Schäden in Form von Verformungen.</rdfs:comment>
        <rdfs:label xml:lang="de">Verformung</rdfs:label>
    </owl:Class>
    


    <!-- http://www.semanticweb.org/covon/ontologies/2022/11/deconstruction-ontology#Denting -->

    <owl:Class rdf:about="http://www.semanticweb.org/covon/ontologies/2022/11/deconstruction-ontology#Denting">
        <rdfs:subClassOf rdf:resource="http://www.semanticweb.org/covon/ontologies/2022/11/deconstruction-ontology#MechanicalMethod"/>
        <rdfs:label xml:lang="de">Eindrücken</rdfs:label>
    </owl:Class>
    


    <!-- http://www.semanticweb.org/covon/ontologies/2022/11/deconstruction-ontology#DiamondChainSaw -->

    <owl:Class rdf:about="http://www.semanticweb.org/covon/ontologies/2022/11/deconstruction-ontology#DiamondChainSaw">
        <rdfs:subClassOf rdf:resource="http://www.semanticweb.org/covon/ontologies/2022/11/deconstruction-ontology#SawingMethod"/>
        <rdfs:label xml:lang="de">Diamantkettensägen</rdfs:label>
    </owl:Class>
    


    <!-- http://www.semanticweb.org/covon/ontologies/2022/11/deconstruction-ontology#Dismantling -->

    <owl:Class rdf:about="http://www.semanticweb.org/covon/ontologies/2022/11/deconstruction-ontology#Dismantling">
        <rdfs:subClassOf rdf:resource="http://www.semanticweb.org/covon/ontologies/2022/11/deconstruction-ontology#MechanicalMethod"/>
        <rdfs:label xml:lang="de">Demontieren</rdfs:label>
    </owl:Class>
    


    <!-- http://www.semanticweb.org/covon/ontologies/2022/11/deconstruction-ontology#DrillingMethod -->

    <owl:Class rdf:about="http://www.semanticweb.org/covon/ontologies/2022/11/deconstruction-ontology#DrillingMethod">
        <rdfs:subClassOf rdf:resource="http://www.semanticweb.org/covon/ontologies/2022/11/deconstruction-ontology#DeconstructionMethod"/>
        <rdfs:label xml:lang="de">Bohrende Verfahren</rdfs:label>
    </owl:Class>
    


    <!-- http://www.semanticweb.org/covon/ontologies/2022/11/deconstruction-ontology#FlameCutting -->

    <owl:Class rdf:about="http://www.semanticweb.org/covon/ontologies/2022/11/deconstruction-ontology#FlameCutting">
        <rdfs:subClassOf rdf:resource="http://www.semanticweb.org/covon/ontologies/2022/11/deconstruction-ontology#ThermalMethod"/>
        <rdfs:label xml:lang="de">Brennschneiden mit Pulverschneidbrennen</rdfs:label>
    </owl:Class>
    


    <!-- http://www.semanticweb.org/covon/ontologies/2022/11/deconstruction-ontology#FullDrilling -->

    <owl:Class rdf:about="http://www.semanticweb.org/covon/ontologies/2022/11/deconstruction-ontology#FullDrilling">
        <rdfs:subClassOf rdf:resource="http://www.semanticweb.org/covon/ontologies/2022/11/deconstruction-ontology#DrillingMethod"/>
        <rdfs:label xml:lang="de">Vollbohren</rdfs:label>
    </owl:Class>
    


    <!-- http://www.semanticweb.org/covon/ontologies/2022/11/deconstruction-ontology#GasPressurePuls -->

    <owl:Class rdf:about="http://www.semanticweb.org/covon/ontologies/2022/11/deconstruction-ontology#GasPressurePuls">
        <rdfs:subClassOf rdf:resource="http://www.semanticweb.org/covon/ontologies/2022/11/deconstruction-ontology#SplittingMethod"/>
        <rdfs:label xml:lang="de">Spalten durch Gasdruckimpuls (Treibladungen)</rdfs:label>
    </owl:Class>
    


    <!-- http://www.semanticweb.org/covon/ontologies/2022/11/deconstruction-ontology#Grinding -->

    <owl:Class rdf:about="http://www.semanticweb.org/covon/ontologies/2022/11/deconstruction-ontology#Grinding">
        <rdfs:subClassOf rdf:resource="http://www.semanticweb.org/covon/ontologies/2022/11/deconstruction-ontology#AblatingMethod"/>
        <rdfs:label xml:lang="de">Schleifen</rdfs:label>
    </owl:Class>
    


    <!-- http://www.semanticweb.org/covon/ontologies/2022/11/deconstruction-ontology#Hammering -->

    <owl:Class rdf:about="http://www.semanticweb.org/covon/ontologies/2022/11/deconstruction-ontology#Hammering">
        <rdfs:subClassOf rdf:resource="http://www.semanticweb.org/covon/ontologies/2022/11/deconstruction-ontology#MechanicalMethod"/>
        <rdfs:label xml:lang="de">Einschlagen</rdfs:label>
    </owl:Class>
    


    <!-- http://www.semanticweb.org/covon/ontologies/2022/11/deconstruction-ontology#Helmet -->

    <owl:Class rdf:about="http://www.semanticweb.org/covon/ontologies/2022/11/deconstruction-ontology#Helmet">
        <rdfs:subClassOf rdf:resource="http://www.semanticweb.org/covon/ontologies/2022/11/deconstruction-ontology#PersonalProtectiveEquipment"/>
    </owl:Class>
    


    <!-- http://www.semanticweb.org/covon/ontologies/2022/11/deconstruction-ontology#HighPressureWaterCutting -->

    <owl:Class rdf:about="http://www.semanticweb.org/covon/ontologies/2022/11/deconstruction-ontology#HighPressureWaterCutting">
        <rdfs:subClassOf rdf:resource="http://www.semanticweb.org/covon/ontologies/2022/11/deconstruction-ontology#HydrodynamicMethod"/>
        <rdfs:label xml:lang="de">Hochdruckwasserschneiden</rdfs:label>
    </owl:Class>
    


    <!-- http://www.semanticweb.org/covon/ontologies/2022/11/deconstruction-ontology#HighPressureWaterJetting -->

    <owl:Class rdf:about="http://www.semanticweb.org/covon/ontologies/2022/11/deconstruction-ontology#HighPressureWaterJetting">
        <rdfs:subClassOf rdf:resource="http://www.semanticweb.org/covon/ontologies/2022/11/deconstruction-ontology#HydrodynamicMethod"/>
        <rdfs:label xml:lang="de">Hochdruckwasserstrahlen</rdfs:label>
    </owl:Class>
    


    <!-- http://www.semanticweb.org/covon/ontologies/2022/11/deconstruction-ontology#HydrodynamicMethod -->

    <owl:Class rdf:about="http://www.semanticweb.org/covon/ontologies/2022/11/deconstruction-ontology#HydrodynamicMethod">
        <rdfs:subClassOf rdf:resource="http://www.semanticweb.org/covon/ontologies/2022/11/deconstruction-ontology#DeconstructionMethod"/>
        <rdfs:label xml:lang="de">Hydrodynamische Verfahren</rdfs:label>
    </owl:Class>
    


    <!-- http://www.semanticweb.org/covon/ontologies/2022/11/deconstruction-ontology#InterrelatedComponent -->

    <owl:Class rdf:about="http://www.semanticweb.org/covon/ontologies/2022/11/deconstruction-ontology#InterrelatedComponent">
        <rdfs:subClassOf rdf:resource="http://www.semanticweb.org/covon/ontologies/2022/11/deconstruction-ontology#Component"/>
        <rdfs:comment xml:lang="en">Interrelated components are components that consist of different parts and are usually evaluated as a whole (e.g. doors or windows).</rdfs:comment>
        <rdfs:comment xml:lang="de">Zusammenhängende Komponenten sind Komponenten, die aus verschiedenen Teilen bestehen und in der Regel als Ganzes bewertet werden (wie z.B. Türen oder Fenster).</rdfs:comment>
        <rdfs:label xml:lang="de">zusammenhängende Komponenten</rdfs:label>
    </owl:Class>
    


    <!-- http://www.semanticweb.org/covon/ontologies/2022/11/deconstruction-ontology#JointCutting -->

    <owl:Class rdf:about="http://www.semanticweb.org/covon/ontologies/2022/11/deconstruction-ontology#JointCutting">
        <rdfs:subClassOf rdf:resource="http://www.semanticweb.org/covon/ontologies/2022/11/deconstruction-ontology#SawingMethod"/>
        <rdfs:label xml:lang="de">Bodensägen (Fugenschneiden)</rdfs:label>
    </owl:Class>
    


    <!-- http://www.semanticweb.org/covon/ontologies/2022/11/deconstruction-ontology#LooseningBlasting -->

    <owl:Class rdf:about="http://www.semanticweb.org/covon/ontologies/2022/11/deconstruction-ontology#LooseningBlasting">
        <rdfs:subClassOf rdf:resource="http://www.semanticweb.org/covon/ontologies/2022/11/deconstruction-ontology#BlastingMethod"/>
        <rdfs:label xml:lang="de">Lockerungssprengung</rdfs:label>
    </owl:Class>
    


    <!-- http://www.semanticweb.org/covon/ontologies/2022/11/deconstruction-ontology#MaterialComponent -->

    <owl:Class rdf:about="http://www.semanticweb.org/covon/ontologies/2022/11/deconstruction-ontology#MaterialComponent">
        <rdfs:subClassOf rdf:resource="http://www.semanticweb.org/covon/ontologies/2022/11/deconstruction-ontology#Component"/>
        <rdfs:comment xml:lang="de">Materielle Komponenten sind Komponenten, die aus einem oder mehreren Materialien bestehen. Diese beschreiben den schichtenweisen und baustoffspezifischen Aufbau eines Bauteils.</rdfs:comment>
        <rdfs:label xml:lang="en">Material components are components that consist of one or more materials. These describe the layered and material-specific structure of an element.</rdfs:label>
        <rdfs:label xml:lang="de">materielle Komponenten</rdfs:label>
    </owl:Class>
    


    <!-- http://www.semanticweb.org/covon/ontologies/2022/11/deconstruction-ontology#MechanicalMethod -->

    <owl:Class rdf:about="http://www.semanticweb.org/covon/ontologies/2022/11/deconstruction-ontology#MechanicalMethod">
        <rdfs:subClassOf rdf:resource="http://www.semanticweb.org/covon/ontologies/2022/11/deconstruction-ontology#DeconstructionMethod"/>
        <rdfs:label xml:lang="de">Mechanische Verfahren</rdfs:label>
    </owl:Class>
    


    <!-- http://www.semanticweb.org/covon/ontologies/2022/11/deconstruction-ontology#Milling -->

    <owl:Class rdf:about="http://www.semanticweb.org/covon/ontologies/2022/11/deconstruction-ontology#Milling">
        <rdfs:subClassOf rdf:resource="http://www.semanticweb.org/covon/ontologies/2022/11/deconstruction-ontology#AblatingMethod"/>
        <rdfs:label xml:lang="de">Fräsen</rdfs:label>
    </owl:Class>
    


    <!-- http://www.semanticweb.org/covon/ontologies/2022/11/deconstruction-ontology#NeighboringObject -->

    <owl:Class rdf:about="http://www.semanticweb.org/covon/ontologies/2022/11/deconstruction-ontology#NeighboringObject">
        <rdfs:subClassOf rdf:resource="https://w3id.org/bot#Building"/>
        <owl:disjointWith rdf:resource="https://w3id.org/bot#Element"/>
        <owl:disjointWith rdf:resource="https://w3id.org/bot#Interface"/>
        <owl:disjointWith rdf:resource="https://w3id.org/bot#Site"/>
        <owl:disjointWith rdf:resource="https://w3id.org/bot#Space"/>
        <owl:disjointWith rdf:resource="https://w3id.org/bot#Storey"/>
        <rdfs:comment xml:lang="en">A building located directly or indirectly within the area of influence of the deconstruction object.</rdfs:comment>
        <rdfs:comment xml:lang="de">Ein Gebäude, welches mittelbar oder unmittelbar im Einflussgebiet des Rückbauobjektes steht.</rdfs:comment>
        <rdfs:label xml:lang="de">Nachbarobjekt</rdfs:label>
    </owl:Class>
    


    <!-- http://www.semanticweb.org/covon/ontologies/2022/11/deconstruction-ontology#NonBearingElement -->

    <owl:Class rdf:about="http://www.semanticweb.org/covon/ontologies/2022/11/deconstruction-ontology#NonBearingElement">
        <rdfs:subClassOf rdf:resource="https://w3id.org/bot#Element"/>
    </owl:Class>
    


    <!-- http://www.semanticweb.org/covon/ontologies/2022/11/deconstruction-ontology#OverturningBlasting -->

    <owl:Class rdf:about="http://www.semanticweb.org/covon/ontologies/2022/11/deconstruction-ontology#OverturningBlasting">
        <rdfs:subClassOf rdf:resource="http://www.semanticweb.org/covon/ontologies/2022/11/deconstruction-ontology#BlastingMethod"/>
        <rdfs:label xml:lang="de">Umlegen durch Sprengen</rdfs:label>
    </owl:Class>
    


    <!-- http://www.semanticweb.org/covon/ontologies/2022/11/deconstruction-ontology#OxyfuelBurning -->

    <owl:Class rdf:about="http://www.semanticweb.org/covon/ontologies/2022/11/deconstruction-ontology#OxyfuelBurning">
        <rdfs:subClassOf rdf:resource="http://www.semanticweb.org/covon/ontologies/2022/11/deconstruction-ontology#ThermalMethod"/>
        <rdfs:label xml:lang="de">Autogenbrennen</rdfs:label>
    </owl:Class>
    


    <!-- http://www.semanticweb.org/covon/ontologies/2022/11/deconstruction-ontology#OxygenCoreLances -->

    <owl:Class rdf:about="http://www.semanticweb.org/covon/ontologies/2022/11/deconstruction-ontology#OxygenCoreLances">
        <rdfs:subClassOf rdf:resource="http://www.semanticweb.org/covon/ontologies/2022/11/deconstruction-ontology#ThermalMethod"/>
        <rdfs:label xml:lang="de">Sauerstoffkernlanzen</rdfs:label>
    </owl:Class>
    


    <!-- http://www.semanticweb.org/covon/ontologies/2022/11/deconstruction-ontology#Peeling -->

    <owl:Class rdf:about="http://www.semanticweb.org/covon/ontologies/2022/11/deconstruction-ontology#Peeling">
        <rdfs:subClassOf rdf:resource="http://www.semanticweb.org/covon/ontologies/2022/11/deconstruction-ontology#AblatingMethod"/>
        <rdfs:label xml:lang="de">Abschälen</rdfs:label>
    </owl:Class>
    


    <!-- http://www.semanticweb.org/covon/ontologies/2022/11/deconstruction-ontology#PersonalProtectiveEquipment -->

    <owl:Class rdf:about="http://www.semanticweb.org/covon/ontologies/2022/11/deconstruction-ontology#PersonalProtectiveEquipment"/>
    


    <!-- http://www.semanticweb.org/covon/ontologies/2022/11/deconstruction-ontology#PlasmaCutting -->

    <owl:Class rdf:about="http://www.semanticweb.org/covon/ontologies/2022/11/deconstruction-ontology#PlasmaCutting">
        <rdfs:subClassOf rdf:resource="http://www.semanticweb.org/covon/ontologies/2022/11/deconstruction-ontology#ThermalMethod"/>
        <rdfs:label xml:lang="de">Plasmaschneidbrennen</rdfs:label>
    </owl:Class>
    


    <!-- http://www.semanticweb.org/covon/ontologies/2022/11/deconstruction-ontology#PressCutting -->

    <owl:Class rdf:about="http://www.semanticweb.org/covon/ontologies/2022/11/deconstruction-ontology#PressCutting">
        <rdfs:subClassOf rdf:resource="http://www.semanticweb.org/covon/ontologies/2022/11/deconstruction-ontology#MechanicalMethod"/>
        <rdfs:label xml:lang="de">Pressschneiden</rdfs:label>
    </owl:Class>
    


    <!-- http://www.semanticweb.org/covon/ontologies/2022/11/deconstruction-ontology#Pressing -->

    <owl:Class rdf:about="http://www.semanticweb.org/covon/ontologies/2022/11/deconstruction-ontology#Pressing">
        <rdfs:subClassOf rdf:resource="http://www.semanticweb.org/covon/ontologies/2022/11/deconstruction-ontology#SplittingMethod"/>
        <rdfs:label xml:lang="de">Spalten durch Pressen</rdfs:label>
    </owl:Class>
    


    <!-- http://www.semanticweb.org/covon/ontologies/2022/11/deconstruction-ontology#ProtectiveGoggles -->

    <owl:Class rdf:about="http://www.semanticweb.org/covon/ontologies/2022/11/deconstruction-ontology#ProtectiveGoggles">
        <rdfs:subClassOf rdf:resource="http://www.semanticweb.org/covon/ontologies/2022/11/deconstruction-ontology#PersonalProtectiveEquipment"/>
    </owl:Class>
    


    <!-- http://www.semanticweb.org/covon/ontologies/2022/11/deconstruction-ontology#Retraction -->

    <owl:Class rdf:about="http://www.semanticweb.org/covon/ontologies/2022/11/deconstruction-ontology#Retraction">
        <rdfs:subClassOf rdf:resource="http://www.semanticweb.org/covon/ontologies/2022/11/deconstruction-ontology#MechanicalMethod"/>
        <rdfs:label xml:lang="de">Einziehen</rdfs:label>
    </owl:Class>
    


    <!-- http://www.semanticweb.org/covon/ontologies/2022/11/deconstruction-ontology#SawingMethod -->

    <owl:Class rdf:about="http://www.semanticweb.org/covon/ontologies/2022/11/deconstruction-ontology#SawingMethod">
        <rdfs:subClassOf rdf:resource="http://www.semanticweb.org/covon/ontologies/2022/11/deconstruction-ontology#DeconstructionMethod"/>
        <rdfs:label xml:lang="de">Sägende Verfahren</rdfs:label>
    </owl:Class>
    


    <!-- http://www.semanticweb.org/covon/ontologies/2022/11/deconstruction-ontology#Shearing -->

    <owl:Class rdf:about="http://www.semanticweb.org/covon/ontologies/2022/11/deconstruction-ontology#Shearing">
        <rdfs:subClassOf rdf:resource="http://www.semanticweb.org/covon/ontologies/2022/11/deconstruction-ontology#MechanicalMethod"/>
        <rdfs:label xml:lang="de">Scherschneiden</rdfs:label>
    </owl:Class>
    


    <!-- http://www.semanticweb.org/covon/ontologies/2022/11/deconstruction-ontology#SplittingBlasting -->

    <owl:Class rdf:about="http://www.semanticweb.org/covon/ontologies/2022/11/deconstruction-ontology#SplittingBlasting">
        <rdfs:subClassOf rdf:resource="http://www.semanticweb.org/covon/ontologies/2022/11/deconstruction-ontology#BlastingMethod"/>
        <rdfs:label xml:lang="de">Spalten durch Sprengen</rdfs:label>
    </owl:Class>
    


    <!-- http://www.semanticweb.org/covon/ontologies/2022/11/deconstruction-ontology#SplittingMethod -->

    <owl:Class rdf:about="http://www.semanticweb.org/covon/ontologies/2022/11/deconstruction-ontology#SplittingMethod">
        <rdfs:subClassOf rdf:resource="http://www.semanticweb.org/covon/ontologies/2022/11/deconstruction-ontology#DeconstructionMethod"/>
        <rdfs:label xml:lang="de">Spaltende Verfahren</rdfs:label>
    </owl:Class>
    


    <!-- http://www.semanticweb.org/covon/ontologies/2022/11/deconstruction-ontology#SwellingPressure -->

    <owl:Class rdf:about="http://www.semanticweb.org/covon/ontologies/2022/11/deconstruction-ontology#SwellingPressure">
        <rdfs:subClassOf rdf:resource="http://www.semanticweb.org/covon/ontologies/2022/11/deconstruction-ontology#SplittingMethod"/>
        <rdfs:label xml:lang="de">Spalten durch Quelldrücken</rdfs:label>
    </owl:Class>
    


    <!-- http://www.semanticweb.org/covon/ontologies/2022/11/deconstruction-ontology#Tapping -->

    <owl:Class rdf:about="http://www.semanticweb.org/covon/ontologies/2022/11/deconstruction-ontology#Tapping">
        <rdfs:subClassOf rdf:resource="http://www.semanticweb.org/covon/ontologies/2022/11/deconstruction-ontology#MechanicalMethod"/>
        <rdfs:label xml:lang="de">Abgreifen</rdfs:label>
    </owl:Class>
    


    <!-- http://www.semanticweb.org/covon/ontologies/2022/11/deconstruction-ontology#Tearing -->

    <owl:Class rdf:about="http://www.semanticweb.org/covon/ontologies/2022/11/deconstruction-ontology#Tearing">
        <rdfs:subClassOf rdf:resource="http://www.semanticweb.org/covon/ontologies/2022/11/deconstruction-ontology#MechanicalMethod"/>
        <rdfs:label xml:lang="de">Reißen</rdfs:label>
    </owl:Class>
    


    <!-- http://www.semanticweb.org/covon/ontologies/2022/11/deconstruction-ontology#TechnicalComponent -->

    <owl:Class rdf:about="http://www.semanticweb.org/covon/ontologies/2022/11/deconstruction-ontology#TechnicalComponent">
        <rdfs:subClassOf rdf:resource="http://www.semanticweb.org/covon/ontologies/2022/11/deconstruction-ontology#Component"/>
        <rdfs:comment xml:lang="en">Technical components are components that are part of the technical building equipment.</rdfs:comment>
        <rdfs:comment xml:lang="de">Technische Komponenten sind Komponenten, die Bestandteil der technischen Gebäudeausrüstung sind.</rdfs:comment>
        <rdfs:label xml:lang="de">technische Komponenten</rdfs:label>
    </owl:Class>
    


    <!-- http://www.semanticweb.org/covon/ontologies/2022/11/deconstruction-ontology#ThermalMethod -->

    <owl:Class rdf:about="http://www.semanticweb.org/covon/ontologies/2022/11/deconstruction-ontology#ThermalMethod">
        <rdfs:subClassOf rdf:resource="http://www.semanticweb.org/covon/ontologies/2022/11/deconstruction-ontology#DeconstructionMethod"/>
        <rdfs:label xml:lang="de">Thermische Verfahren</rdfs:label>
    </owl:Class>
    


    <!-- http://www.semanticweb.org/covon/ontologies/2022/11/deconstruction-ontology#WallSaw -->

    <owl:Class rdf:about="http://www.semanticweb.org/covon/ontologies/2022/11/deconstruction-ontology#WallSaw">
        <rdfs:subClassOf rdf:resource="http://www.semanticweb.org/covon/ontologies/2022/11/deconstruction-ontology#SawingMethod"/>
        <rdfs:label xml:lang="de">Wandsägen</rdfs:label>
    </owl:Class>
    


    <!-- http://www.semanticweb.org/covon/ontologies/2022/11/deconstruction-ontology#WastePreventation -->

    <owl:Class rdf:about="http://www.semanticweb.org/covon/ontologies/2022/11/deconstruction-ontology#WastePreventation">
        <rdfs:subClassOf rdf:resource="http://www.semanticweb.org/arnak/ontologies/2022/7/DOR#CircularPotential"/>
        <owl:disjointWith rdf:resource="http://www.semanticweb.org/covon/ontologies/2022/11/deconstruction-ontology#WasteRemoval"/>
        <rdfs:comment xml:lang="de">Darstellung von Verfahren, die ergriffen werden, bevor ein Stoff, Material oder Erzeugnis zu Abfall wird. (§ 3 Abs. 20 S. 1 KrWG)</rdfs:comment>
        <rdfs:comment xml:lang="en">Representation of methods that are taken before a substance, material or product becomes waste. (§ 3 Sec. 20 S. 1 KrWG)</rdfs:comment>
        <rdfs:isDefinedBy rdf:resource="https://www.gesetze-im-internet.de/krwg/__3.html"/>
        <rdfs:label xml:lang="de">Abfallvermeidung</rdfs:label>
    </owl:Class>
    


    <!-- http://www.semanticweb.org/covon/ontologies/2022/11/deconstruction-ontology#WasteRemoval -->

    <owl:Class rdf:about="http://www.semanticweb.org/covon/ontologies/2022/11/deconstruction-ontology#WasteRemoval">
        <rdfs:subClassOf rdf:resource="http://www.semanticweb.org/arnak/ontologies/2022/7/DOR#CircularPotential"/>
        <rdfs:comment xml:lang="de">Darstellung von Verfahren, die nicht als Verwertungsverfahren eingestuft werden. (§ 3 Abs. 26 S. 1 KrWG)</rdfs:comment>
        <rdfs:comment xml:lang="en">Representation of methods that are not classified as recovery methods. (§ 3 Sec. 26 S. 1 KrWG)</rdfs:comment>
        <rdfs:isDefinedBy rdf:resource="https://www.gesetze-im-internet.de/krwg/__3.html"/>
        <rdfs:label xml:lang="de">Abfallbeseitigung</rdfs:label>
    </owl:Class>
    


    <!-- http://www.semanticweb.org/covon/ontologies/2022/11/deconstruction-ontology#Weakening -->

    <owl:Class rdf:about="http://www.semanticweb.org/covon/ontologies/2022/11/deconstruction-ontology#Weakening">
        <rdfs:subClassOf rdf:resource="https://w3id.org/dot#ClassifiedDamage"/>
        <owl:disjointWith rdf:resource="https://w3id.org/dot#UnclassifiedDamage"/>
        <rdfs:comment xml:lang="en">Class for the representation of damages in the form of weakening.</rdfs:comment>
        <rdfs:comment xml:lang="de">Klasse zur Darstellung von Schäden in Form von Schwächungen.</rdfs:comment>
        <rdfs:label xml:lang="de">Schwächung</rdfs:label>
    </owl:Class>
    


    <!-- http://www.semanticweb.org/covon/ontologies/2022/11/deconstruction-ontology#WireSaw -->

    <owl:Class rdf:about="http://www.semanticweb.org/covon/ontologies/2022/11/deconstruction-ontology#WireSaw">
        <rdfs:subClassOf rdf:resource="http://www.semanticweb.org/covon/ontologies/2022/11/deconstruction-ontology#SawingMethod"/>
        <rdfs:label xml:lang="de">Seilsägen</rdfs:label>
    </owl:Class>
    


    <!-- http://www.semanticweb.org/covon/ontologies/2022/11/deconstruction-ontology#surfaceChange -->

    <owl:Class rdf:about="http://www.semanticweb.org/covon/ontologies/2022/11/deconstruction-ontology#surfaceChange">
        <rdfs:subClassOf rdf:resource="https://w3id.org/dot#ClassifiedDamage"/>
        <owl:disjointWith rdf:resource="https://w3id.org/dot#UnclassifiedDamage"/>
        <rdfs:comment xml:lang="en">Class for the representation of damages in the form of surface changes.</rdfs:comment>
        <rdfs:comment xml:lang="de">Klasse zur Darstellung von Schäden in Form von Oberflächenveränderungen.</rdfs:comment>
        <rdfs:label xml:lang="de">Oberflächenveränderung</rdfs:label>
    </owl:Class>
    


    <!-- http://www.w3.org/2002/07/owl#Thing -->

    <rdf:Description rdf:about="http://www.w3.org/2002/07/owl#Thing">
        <rdfs:label>Thing</rdfs:label>
    </rdf:Description>
    


    <!-- http://xmlns.com/foaf/0.1/EngineeringOffice -->

    <owl:Class rdf:about="http://xmlns.com/foaf/0.1/EngineeringOffice">
        <rdfs:subClassOf rdf:resource="http://xmlns.com/foaf/0.1/ProjectParticipant"/>
        <owl:disjointWith rdf:resource="http://xmlns.com/foaf/0.1/PlantOperator"/>
        <owl:disjointWith rdf:resource="http://xmlns.com/foaf/0.1/PublicAdministration"/>
    </owl:Class>
    


    <!-- http://xmlns.com/foaf/0.1/PlantOperator -->

    <owl:Class rdf:about="http://xmlns.com/foaf/0.1/PlantOperator">
        <rdfs:subClassOf rdf:resource="http://xmlns.com/foaf/0.1/ProjectParticipant"/>
        <owl:disjointWith rdf:resource="http://xmlns.com/foaf/0.1/PublicAdministration"/>
    </owl:Class>
    


    <!-- http://xmlns.com/foaf/0.1/ProjectParticipant -->

    <owl:Class rdf:about="http://xmlns.com/foaf/0.1/ProjectParticipant"/>
    


    <!-- http://xmlns.com/foaf/0.1/PublicAdministration -->

    <owl:Class rdf:about="http://xmlns.com/foaf/0.1/PublicAdministration">
        <rdfs:subClassOf rdf:resource="http://xmlns.com/foaf/0.1/ProjectParticipant"/>
    </owl:Class>
    


    <!-- https://pi.pauwel.be/voc/buildingelement#Beam -->

    <owl:Class rdf:about="https://pi.pauwel.be/voc/buildingelement#Beam">
        <rdfs:subClassOf rdf:resource="https://pi.pauwel.be/voc/buildingelement#BuildingElement"/>
        <rdfs:comment xml:lang="en">A horizontal, or nearly horizontal, structural member that is capable of withstanding load primarily by resisting bending. It represents such a member from an architectural point of view. It is not required to be load bearing.</rdfs:comment>
        <rdfs:comment xml:lang="nb-no">A standard beam usually used horizontally.</rdfs:comment>
        <rdfs:comment xml:lang="en">http://bsdd.buildingsmart.org/#concept/details/3zXEi0qSCHuO00025QrE$V</rdfs:comment>
        <rdfs:label xml:lang="nl">Balk</rdfs:label>
        <rdfs:label xml:lang="en">Beam</rdfs:label>
        <rdfs:label xml:lang="da">Bjælke</rdfs:label>
        <rdfs:label xml:lang="de-de">balken</rdfs:label>
        <rdfs:label xml:lang="de-de">biegeträger</rdfs:label>
        <rdfs:label xml:lang="nb-no">bjelke</rdfs:label>
        <rdfs:label xml:lang="fr-fr">poutre</rdfs:label>
        <rdfs:seeAlso rdf:resource="http://www.buildingsmart-tech.org/ifcOWL/IFC4_ADD2#IfcBeam"/>
    </owl:Class>
    


    <!-- https://pi.pauwel.be/voc/buildingelement#Beam-BEAM -->

    <owl:Class rdf:about="https://pi.pauwel.be/voc/buildingelement#Beam-BEAM">
        <rdfs:subClassOf rdf:resource="https://pi.pauwel.be/voc/buildingelement#Beam"/>
        <rdfs:comment xml:lang="en">A horizontal, or nearly horizontal, structural member that is capable of withstanding load primarily by resisting bending. It represents such a member from an architectural point of view. It is not required to be load bearing.</rdfs:comment>
        <rdfs:comment xml:lang="nb-no">A standard beam usually used horizontally.</rdfs:comment>
        <rdfs:comment xml:lang="en">http://bsdd.buildingsmart.org/#concept/details/0KKIHMGYH7H8MAfgxbrxuV</rdfs:comment>
        <rdfs:label xml:lang="en">Beam</rdfs:label>
        <rdfs:label xml:lang="nl-nl">balk</rdfs:label>
        <rdfs:label xml:lang="de-de">balken</rdfs:label>
        <rdfs:label xml:lang="de-de">biegeträger</rdfs:label>
        <rdfs:label xml:lang="nb-no">bjelke</rdfs:label>
        <rdfs:label xml:lang="nl-nl">ligger</rdfs:label>
        <rdfs:label xml:lang="fr-fr">poutre</rdfs:label>
        <rdfs:seeAlso rdf:resource="http://www.buildingsmart-tech.org/ifcOWL/IFC4_ADD2#IfcBeamEnumType"/>
    </owl:Class>
    


    <!-- https://pi.pauwel.be/voc/buildingelement#Beam-HOLLOWCORE -->

    <owl:Class rdf:about="https://pi.pauwel.be/voc/buildingelement#Beam-HOLLOWCORE">
        <rdfs:subClassOf rdf:resource="https://pi.pauwel.be/voc/buildingelement#Beam"/>
        <rdfs:comment xml:lang="de-de">Platte mit rechteckigem Querschnitt, in der auf voller Länge in Längsrichtung kreisrunde oder ovale Hohlräume (Aussparungen) verlaufen</rdfs:comment>
        <rdfs:comment xml:lang="fr-fr">dalle de section rectangulaire comportant des vides longitudinaux sur toute leur longueur ou des vides de forme ovale</rdfs:comment>
        <rdfs:comment xml:lang="en">http://bsdd.buildingsmart.org/#concept/details/2gzZKHqELB$gPVKajRAFXc</rdfs:comment>
        <rdfs:comment xml:lang="es-es">losa de sección rectangular con huecos circulares o óvales para toda su longitud</rdfs:comment>
        <rdfs:comment xml:lang="en">monolithic prestressed or reinforced elements with a constant overall depth divided into an upper and lower flange, linked by vertical webs, so constituting cores as longitudinal voids the cross section of which is constant and presents one vertical axis.</rdfs:comment>
        <rdfs:comment xml:lang="pl-pl">prostokątna płyta z okrągłymi lub owalnymi przestrzeniami na całej długości</rdfs:comment>
        <rdfs:comment xml:lang="en-gb">rectangular section slab with full-length longitudinal circular or oval shaped voids</rdfs:comment>
        <rdfs:comment xml:lang="en">rectangular section slab with full-length longitudinal circular or oval shaped voids.</rdfs:comment>
        <rdfs:comment xml:lang="sv-se">rektangulärt bjälklag med längsgående cirkelformade eller ovalformade tomrum längs med hela bjälklaget</rdfs:comment>
        <rdfs:comment xml:lang="dk-dk">rektangulært element med hulrum i fuld længde i langsgående, cirkulær eller oval form</rdfs:comment>
        <rdfs:comment xml:lang="nb-no">rektangulært element med langsgående sirkulære eller ovale hulrom i full lengde</rdfs:comment>
        <rdfs:comment xml:lang="fi-fi">suorakaiteenmuotoinen laattaelementti, jossa on koko pituudeltaan pyöreitä tai ovaalinmuotoisia onteloita/tyhjätiloja</rdfs:comment>
        <rdfs:comment xml:lang="bg-bg">плоча с правоъгълно сечение и кухини по цялата дължина с надлъжна кръгла или овална форма </rdfs:comment>
        <rdfs:label xml:lang="en">Pre-cast Hollow Core Slab</rdfs:label>
        <rdfs:label xml:lang="fr-fr">dalle alvéolée préfabriquée en béton</rdfs:label>
        <rdfs:label xml:lang="sv-se">förtillverkade betongprodukter - håldäcksplattor</rdfs:label>
        <rdfs:label xml:lang="nb-no">hulldekke</rdfs:label>
        <rdfs:label xml:lang="nb-no">hulldekkeelement</rdfs:label>
        <rdfs:label xml:lang="it-it">lastre alveolari precompresse</rdfs:label>
        <rdfs:label xml:lang="es-es">losa alveolar prefabricada</rdfs:label>
        <rdfs:label xml:lang="fi-fi">ontelolaatta</rdfs:label>
        <rdfs:label xml:lang="en-gb">pre-cast hollow core slab</rdfs:label>
        <rdfs:label xml:lang="nb-no">prefabrikkert hulldekke</rdfs:label>
        <rdfs:label xml:lang="pl-pl">prefabrykowana płyta kanałowa stropowa</rdfs:label>
        <rdfs:label xml:lang="dk-dk">præfabrikeret huldækelement</rdfs:label>
        <rdfs:label xml:lang="de-de">werkseitig hergestellte Hohlplatte</rdfs:label>
        <rdfs:label xml:lang="bg-bg">готови плочи с кухини</rdfs:label>
        <rdfs:seeAlso rdf:resource="http://www.buildingsmart-tech.org/ifcOWL/IFC4_ADD2#IfcBeamEnumType"/>
    </owl:Class>
    


    <!-- https://pi.pauwel.be/voc/buildingelement#Beam-JOIST -->

    <owl:Class rdf:about="https://pi.pauwel.be/voc/buildingelement#Beam-JOIST">
        <rdfs:subClassOf rdf:resource="https://pi.pauwel.be/voc/buildingelement#Beam"/>
        <rdfs:comment xml:lang="en">http://bsdd.buildingsmart.org/#concept/details/1_zkjNhS95oA5oDSSTnEvO</rdfs:comment>
        <rdfs:label xml:lang="en">Joiste</rdfs:label>
        <rdfs:label xml:lang="nb-no">tilpasset bjelke</rdfs:label>
        <rdfs:seeAlso rdf:resource="http://www.buildingsmart-tech.org/ifcOWL/IFC4_ADD2#IfcBeamEnumType"/>
    </owl:Class>
    


    <!-- https://pi.pauwel.be/voc/buildingelement#Beam-LINTEL -->

    <owl:Class rdf:about="https://pi.pauwel.be/voc/buildingelement#Beam-LINTEL">
        <rdfs:subClassOf rdf:resource="https://pi.pauwel.be/voc/buildingelement#Beam"/>
        <rdfs:comment xml:lang="en">http://bsdd.buildingsmart.org/#concept/details/1PivEYC0575QGoaAFjN8c9</rdfs:comment>
        <rdfs:label xml:lang="en">Lintel</rdfs:label>
        <rdfs:label xml:lang="nb-no">overdekking</rdfs:label>
        <rdfs:seeAlso rdf:resource="http://www.buildingsmart-tech.org/ifcOWL/IFC4_ADD2#IfcBeamEnumType"/>
    </owl:Class>
    


    <!-- https://pi.pauwel.be/voc/buildingelement#Beam-SPANDREL -->

    <owl:Class rdf:about="https://pi.pauwel.be/voc/buildingelement#Beam-SPANDREL">
        <rdfs:subClassOf rdf:resource="https://pi.pauwel.be/voc/buildingelement#Beam"/>
        <rdfs:comment xml:lang="en">http://bsdd.buildingsmart.org/#concept/details/2$vr6UW$f3SwHilnemEZoH</rdfs:comment>
        <rdfs:label xml:lang="en">Spandrel</rdfs:label>
        <rdfs:label xml:lang="nb-no">brystning</rdfs:label>
        <rdfs:seeAlso rdf:resource="http://www.buildingsmart-tech.org/ifcOWL/IFC4_ADD2#IfcBeamEnumType"/>
    </owl:Class>
    


    <!-- https://pi.pauwel.be/voc/buildingelement#Beam-T_BEAM -->

    <owl:Class rdf:about="https://pi.pauwel.be/voc/buildingelement#Beam-T_BEAM">
        <rdfs:subClassOf rdf:resource="https://pi.pauwel.be/voc/buildingelement#Beam"/>
        <rdfs:comment xml:lang="en">http://bsdd.buildingsmart.org/#concept/details/1o9Up6wBr339DlpjWIWE$l</rdfs:comment>
        <rdfs:label xml:lang="en">T_Beam</rdfs:label>
        <rdfs:label xml:lang="nb-no">t_bjelke</rdfs:label>
        <rdfs:seeAlso rdf:resource="http://www.buildingsmart-tech.org/ifcOWL/IFC4_ADD2#IfcBeamEnumType"/>
    </owl:Class>
    


    <!-- https://pi.pauwel.be/voc/buildingelement#BuildingElement -->

    <owl:Class rdf:about="https://pi.pauwel.be/voc/buildingelement#BuildingElement">
        <rdfs:subClassOf rdf:resource="http://purl.org/goodrelations/v1#SomeItems"/>
        <rdfs:subClassOf rdf:resource="https://schema.org/Product"/>
        <rdfs:comment xml:lang="de-de">Bauelement</rdfs:comment>
        <rdfs:comment xml:lang="en">Comprises all elements that are primarily part of the construction of a building, i.e., its structural and space separating system. Building elements are all physically existent and tangible things.</rdfs:comment>
        <rdfs:comment xml:lang="en">http://bsdd.buildingsmart.org/#concept/details/2AFYKXkEn7RxYuvbduGfUV</rdfs:comment>
        <rdfs:label xml:lang="de-de">Bauteil</rdfs:label>
        <rdfs:label xml:lang="en">Building Element</rdfs:label>
        <rdfs:label xml:lang="fr-fr">Elément de construction</rdfs:label>
        <rdfs:seeAlso rdf:resource="http://www.buildingsmart-tech.org/ifcOWL/IFC4_ADD2#IfcBuildingElement"/>
    </owl:Class>
    


    <!-- https://pi.pauwel.be/voc/buildingelement#BuildingElementPart -->

    <owl:Class rdf:about="https://pi.pauwel.be/voc/buildingelement#BuildingElementPart">
        <rdfs:subClassOf rdf:resource="https://pi.pauwel.be/voc/buildingelement#ElementComponent"/>
        <rdfs:comment xml:lang="en">http://bsdd.buildingsmart.org/#concept/details/3v2S1DH0r50BHIhWE6QHMZ</rdfs:comment>
        <rdfs:comment xml:lang="en">ifcbuildingelementpart represents major components as subordinate parts of a building element. typical usage examples include precast concrete sandwich walls, where the layers may have different geometry representations. in this case the layered material representation does not sufficiently describe the element. each layer is represented by an own instance of the ifcbuildingelementpart with its own geometry description. the kind of building element part is further specified by a corresponding instance of ifcbuildingelementparttype, referred to by ifcreldefinesbytype.</rdfs:comment>
        <rdfs:label xml:lang="en">Building Element Part</rdfs:label>
        <rdfs:label xml:lang="de-de">Teil eines Bauelements</rdfs:label>
        <rdfs:label xml:lang="fr-fr">partie d&apos;élément de construction</rdfs:label>
        <rdfs:seeAlso rdf:resource="http://www.buildingsmart-tech.org/ifcOWL/IFC4_ADD2#IfcBuildingElementPart"/>
    </owl:Class>
    


    <!-- https://pi.pauwel.be/voc/buildingelement#BuildingElementPart-INSULATION -->

    <owl:Class rdf:about="https://pi.pauwel.be/voc/buildingelement#BuildingElementPart-INSULATION">
        <rdfs:subClassOf rdf:resource="https://pi.pauwel.be/voc/buildingelement#BuildingElementPart"/>
        <rdfs:comment xml:lang="en">http://bsdd.buildingsmart.org/#concept/details/2CF$o8Mgv2_xbw_kioa_YW</rdfs:comment>
        <rdfs:label xml:lang="en">Insulation</rdfs:label>
        <rdfs:label xml:lang="nb-no">isolasjon</rdfs:label>
        <rdfs:seeAlso rdf:resource="http://www.buildingsmart-tech.org/ifcOWL/IFC4_ADD2#IfcBuildingElementPartEnumType"/>
    </owl:Class>
    


    <!-- https://pi.pauwel.be/voc/buildingelement#BuildingElementPart-PRECASTPANEL -->

    <owl:Class rdf:about="https://pi.pauwel.be/voc/buildingelement#BuildingElementPart-PRECASTPANEL">
        <rdfs:subClassOf rdf:resource="https://pi.pauwel.be/voc/buildingelement#BuildingElementPart"/>
        <rdfs:comment xml:lang="en">http://bsdd.buildingsmart.org/#concept/details/0pt2K5QIXB89suCXlsQZw$</rdfs:comment>
        <rdfs:label xml:lang="en">Precast Panel</rdfs:label>
        <rdfs:seeAlso rdf:resource="http://www.buildingsmart-tech.org/ifcOWL/IFC4_ADD2#IfcBuildingElementPartEnumType"/>
    </owl:Class>
    


    <!-- https://pi.pauwel.be/voc/buildingelement#Chimney -->

    <owl:Class rdf:about="https://pi.pauwel.be/voc/buildingelement#Chimney">
        <rdfs:subClassOf rdf:resource="https://pi.pauwel.be/voc/buildingelement#BuildingElement"/>
        <rdfs:comment xml:lang="en">A vertical structure of brick, masonry, or steel that carries exhaust gases or steam away from a fire, engine, etc.</rdfs:comment>
        <rdfs:comment xml:lang="en">Typically vertical, or as near as vertical, parts of the construction of a building and part of the building fabric. Often constructed by pre-cast or insitu concrete, today seldom by bricks.</rdfs:comment>
        <rdfs:comment xml:lang="en">http://bsdd.buildingsmart.org/#concept/details/0xE4A0qSaHuO00025QrE$V</rdfs:comment>
        <rdfs:comment xml:lang="nb-no">konstruksjon bestående av én eller flere vegger som omslutter én eller flere røykkanaler</rdfs:comment>
        <rdfs:comment xml:lang="en">structure consisting of a wall or walls enclosing  a flue or flues</rdfs:comment>
        <rdfs:label xml:lang="de-de">Abgasanlage</rdfs:label>
        <rdfs:label xml:lang="de-de">Abgassanlage</rdfs:label>
        <rdfs:label xml:lang="en">Chimney</rdfs:label>
        <rdfs:label xml:lang="nl">Schoorsteen</rdfs:label>
        <rdfs:label xml:lang="nl-nl">Schoorsteen</rdfs:label>
        <rdfs:label xml:lang="de-de">Schornstein</rdfs:label>
        <rdfs:label xml:lang="da">Skorsten</rdfs:label>
        <rdfs:label xml:lang="fr-fr">cheminée</rdfs:label>
        <rdfs:label xml:lang="fr-fr">conduit de fumée</rdfs:label>
        <rdfs:label xml:lang="nb-no">pipe</rdfs:label>
        <rdfs:label xml:lang="nb-no">skorstein</rdfs:label>
        <rdfs:seeAlso rdf:resource="http://www.buildingsmart-tech.org/ifcOWL/IFC4_ADD2#IfcChimney"/>
    </owl:Class>
    


    <!-- https://pi.pauwel.be/voc/buildingelement#Column -->

    <owl:Class rdf:about="https://pi.pauwel.be/voc/buildingelement#Column">
        <rdfs:subClassOf rdf:resource="https://pi.pauwel.be/voc/buildingelement#BuildingElement"/>
        <rdfs:comment xml:lang="en">A vertical structural member which often is aligned with a structural grid intersection. It represents a vertical, or nearly vertical, structural member that transmits, through compression, the weight of the structure above to other structural elements below. It represents such a member from an architectural point of view. It is not required to be load bearing.</rdfs:comment>
        <rdfs:comment xml:lang="en">http://bsdd.buildingsmart.org/#concept/details/1CDOE0qSeHuO00025QrE$V</rdfs:comment>
        <rdfs:label xml:lang="en">Column</rdfs:label>
        <rdfs:label xml:lang="nl">Kolom</rdfs:label>
        <rdfs:label xml:lang="de-de">Stütze / Pfeiler</rdfs:label>
        <rdfs:label xml:lang="da">Søjle</rdfs:label>
        <rdfs:label xml:lang="fr-fr">poteau</rdfs:label>
        <rdfs:seeAlso rdf:resource="http://www.buildingsmart-tech.org/ifcOWL/IFC4_ADD2#IfcColumn"/>
    </owl:Class>
    


    <!-- https://pi.pauwel.be/voc/buildingelement#Column-COLUMN -->

    <owl:Class rdf:about="https://pi.pauwel.be/voc/buildingelement#Column-COLUMN">
        <rdfs:subClassOf rdf:resource="https://pi.pauwel.be/voc/buildingelement#Column"/>
        <rdfs:comment xml:lang="en">A vertical structural member which often is aligned with a structural grid intersection. It represents a vertical, or nearly vertical, structural member that transmits, through compression, the weight of the structure above to other structural elements below. It represents such a member from an architectural point of view. It is not required to be load bearing.</rdfs:comment>
        <rdfs:comment xml:lang="nb-no">Søyle</rdfs:comment>
        <rdfs:comment xml:lang="en">http://bsdd.buildingsmart.org/#concept/details/1k5QL8XejA8v7H3XePklst</rdfs:comment>
        <rdfs:label xml:lang="en">Column</rdfs:label>
        <rdfs:label xml:lang="de-de">Druckstab</rdfs:label>
        <rdfs:label xml:lang="de-de">Stütze</rdfs:label>
        <rdfs:label xml:lang="fr-fr">poteau</rdfs:label>
        <rdfs:seeAlso rdf:resource="http://www.buildingsmart-tech.org/ifcOWL/IFC4_ADD2#IfcColumnEnumType"/>
    </owl:Class>
    


    <!-- https://pi.pauwel.be/voc/buildingelement#Column-PILASTER -->

    <owl:Class rdf:about="https://pi.pauwel.be/voc/buildingelement#Column-PILASTER">
        <rdfs:subClassOf rdf:resource="https://pi.pauwel.be/voc/buildingelement#Column"/>
        <rdfs:comment xml:lang="nb-no">Pilaster</rdfs:comment>
        <rdfs:comment xml:lang="en">http://bsdd.buildingsmart.org/#concept/details/08F4W56in3zeQ$ucplQrmF</rdfs:comment>
        <rdfs:comment xml:lang="en">http://bsdd.buildingsmart.org/#concept/details/312dw0BS8Htm00025QrE$V</rdfs:comment>
        <rdfs:comment xml:lang="nb-no">vertikalt fremspring på vegg</rdfs:comment>
        <rdfs:label xml:lang="en">Pilaster</rdfs:label>
        <rdfs:label xml:lang="nl-nl">Pilaster</rdfs:label>
        <rdfs:seeAlso rdf:resource="http://www.buildingsmart-tech.org/ifcOWL/IFC4_ADD2#IfcColumnEnumType"/>
    </owl:Class>
    


    <!-- https://pi.pauwel.be/voc/buildingelement#Covering -->

    <owl:Class rdf:about="https://pi.pauwel.be/voc/buildingelement#Covering">
        <rdfs:subClassOf rdf:resource="https://pi.pauwel.be/voc/buildingelement#BuildingElement"/>
        <rdfs:comment xml:lang="en">An element which covers some part of another element and is fully dependent on that other element.</rdfs:comment>
        <rdfs:comment xml:lang="en">http://bsdd.buildingsmart.org/#concept/details/3uBPs0qSyHuO00025QrE$V</rdfs:comment>
        <rdfs:label xml:lang="de-de">Bekleidung / Belag</rdfs:label>
        <rdfs:label xml:lang="en">Covering</rdfs:label>
        <rdfs:label xml:lang="nb-no">kledning / belegg</rdfs:label>
        <rdfs:label xml:lang="fr-fr">revêtement</rdfs:label>
        <rdfs:seeAlso rdf:resource="http://www.buildingsmart-tech.org/ifcOWL/IFC4_ADD2#IfcCovering"/>
    </owl:Class>
    


    <!-- https://pi.pauwel.be/voc/buildingelement#Covering-CEILING -->

    <owl:Class rdf:about="https://pi.pauwel.be/voc/buildingelement#Covering-CEILING">
        <rdfs:subClassOf rdf:resource="https://pi.pauwel.be/voc/buildingelement#Covering"/>
        <rdfs:comment xml:lang="en">http://bsdd.buildingsmart.org/#concept/details/05pSAVKa99GQlGChUhmlv1</rdfs:comment>
        <rdfs:label xml:lang="en">Ceiling</rdfs:label>
        <rdfs:label xml:lang="nb-no">tak</rdfs:label>
        <rdfs:seeAlso rdf:resource="http://www.buildingsmart-tech.org/ifcOWL/IFC4_ADD2#IfcCoveringEnumType"/>
    </owl:Class>
    


    <!-- https://pi.pauwel.be/voc/buildingelement#Covering-CLADDING -->

    <owl:Class rdf:about="https://pi.pauwel.be/voc/buildingelement#Covering-CLADDING">
        <rdfs:subClassOf rdf:resource="https://pi.pauwel.be/voc/buildingelement#Covering"/>
        <rdfs:comment xml:lang="en">http://bsdd.buildingsmart.org/#concept/details/0MKWgDXdn9OfqhAzFzvTUH</rdfs:comment>
        <rdfs:label xml:lang="en">Cladding</rdfs:label>
        <rdfs:label xml:lang="nb-no">kledning</rdfs:label>
        <rdfs:seeAlso rdf:resource="http://www.buildingsmart-tech.org/ifcOWL/IFC4_ADD2#IfcCoveringEnumType"/>
    </owl:Class>
    


    <!-- https://pi.pauwel.be/voc/buildingelement#Covering-FLOORING -->

    <owl:Class rdf:about="https://pi.pauwel.be/voc/buildingelement#Covering-FLOORING">
        <rdfs:subClassOf rdf:resource="https://pi.pauwel.be/voc/buildingelement#Covering"/>
        <rdfs:comment xml:lang="en">http://bsdd.buildingsmart.org/#concept/details/1MZNPRnDz1jOV_XCmntitl</rdfs:comment>
        <rdfs:label xml:lang="en">Flooring</rdfs:label>
        <rdfs:label xml:lang="nb-no">gulv</rdfs:label>
        <rdfs:seeAlso rdf:resource="http://www.buildingsmart-tech.org/ifcOWL/IFC4_ADD2#IfcCoveringEnumType"/>
    </owl:Class>
    


    <!-- https://pi.pauwel.be/voc/buildingelement#Covering-INSULATION -->

    <owl:Class rdf:about="https://pi.pauwel.be/voc/buildingelement#Covering-INSULATION">
        <rdfs:subClassOf rdf:resource="https://pi.pauwel.be/voc/buildingelement#Covering"/>
        <rdfs:comment xml:lang="en">http://bsdd.buildingsmart.org/#concept/details/0m_WyU8An7RAFjJPRPQn1j</rdfs:comment>
        <rdfs:label xml:lang="en">Insulation</rdfs:label>
        <rdfs:label xml:lang="nb-no">isolasjon</rdfs:label>
        <rdfs:seeAlso rdf:resource="http://www.buildingsmart-tech.org/ifcOWL/IFC4_ADD2#IfcCoveringEnumType"/>
    </owl:Class>
    


    <!-- https://pi.pauwel.be/voc/buildingelement#Covering-MEMBRANE -->

    <owl:Class rdf:about="https://pi.pauwel.be/voc/buildingelement#Covering-MEMBRANE">
        <rdfs:subClassOf rdf:resource="https://pi.pauwel.be/voc/buildingelement#Covering"/>
        <rdfs:comment xml:lang="en">http://bsdd.buildingsmart.org/#concept/details/3vHSkCoT0Hsm00051Mm008</rdfs:comment>
        <rdfs:comment xml:lang="nb-no">vanntett og/eller damptett lag som er festet til sluket i gulvet, på gulvet eller på taket</rdfs:comment>
        <rdfs:comment xml:lang="en">watertight and/or damp proof layer attached to the gully either in the floor or on the floor or
roof</rdfs:comment>
        <rdfs:label xml:lang="de-de">Dichtungsbahn</rdfs:label>
        <rdfs:label xml:lang="en">Membrane</rdfs:label>
        <rdfs:label xml:lang="fr-fr">film d&apos;étanchéité</rdfs:label>
        <rdfs:label xml:lang="nb-no">membran</rdfs:label>
        <rdfs:seeAlso rdf:resource="http://www.buildingsmart-tech.org/ifcOWL/IFC4_ADD2#IfcCoveringEnumType"/>
    </owl:Class>
    


    <!-- https://pi.pauwel.be/voc/buildingelement#Covering-MOLDING -->

    <owl:Class rdf:about="https://pi.pauwel.be/voc/buildingelement#Covering-MOLDING">
        <rdfs:subClassOf rdf:resource="https://pi.pauwel.be/voc/buildingelement#Covering"/>
        <rdfs:comment xml:lang="en">http://bsdd.buildingsmart.org/#concept/details/0rO5hENaL0Sx5ncSZm5QWi</rdfs:comment>
        <rdfs:comment xml:lang="en">http://bsdd.buildingsmart.org/#concept/details/39P8INeF1DvPcZnWFCA0jO</rdfs:comment>
        <rdfs:label xml:lang="de-de">Gesims</rdfs:label>
        <rdfs:label xml:lang="fr-fr">Matériau de la moulure</rdfs:label>
        <rdfs:label xml:lang="en">Molding</rdfs:label>
        <rdfs:label xml:lang="nb-no">gerikt</rdfs:label>
        <rdfs:label xml:lang="nb-no">taklist</rdfs:label>
        <rdfs:seeAlso rdf:resource="http://www.buildingsmart-tech.org/ifcOWL/IFC4_ADD2#IfcCoveringEnumType"/>
    </owl:Class>
    


    <!-- https://pi.pauwel.be/voc/buildingelement#Covering-ROOFING -->

    <owl:Class rdf:about="https://pi.pauwel.be/voc/buildingelement#Covering-ROOFING">
        <rdfs:subClassOf rdf:resource="https://pi.pauwel.be/voc/buildingelement#Covering"/>
        <rdfs:comment xml:lang="en">http://bsdd.buildingsmart.org/#concept/details/1roIuYcU5AxfQM_Wf18q7t</rdfs:comment>
        <rdfs:label xml:lang="en">Roofing</rdfs:label>
        <rdfs:label xml:lang="nb-no">takdekke</rdfs:label>
        <rdfs:label xml:lang="nb-no">taktekking</rdfs:label>
        <rdfs:seeAlso rdf:resource="http://www.buildingsmart-tech.org/ifcOWL/IFC4_ADD2#IfcCoveringEnumType"/>
    </owl:Class>
    


    <!-- https://pi.pauwel.be/voc/buildingelement#Covering-SKIRTINGBOARD -->

    <owl:Class rdf:about="https://pi.pauwel.be/voc/buildingelement#Covering-SKIRTINGBOARD">
        <rdfs:subClassOf rdf:resource="https://pi.pauwel.be/voc/buildingelement#Covering"/>
        <rdfs:comment xml:lang="en">http://bsdd.buildingsmart.org/#concept/details/0rhD2N_cvFRRnqQ6pRM9aE</rdfs:comment>
        <rdfs:label xml:lang="fr-fr">Matériau de la plinthe</rdfs:label>
        <rdfs:label xml:lang="en">Skirting Board</rdfs:label>
        <rdfs:label xml:lang="de-de">Sockelleiste</rdfs:label>
        <rdfs:label xml:lang="en">skirtingboard</rdfs:label>
        <rdfs:label xml:lang="ja-jp">幅木材</rdfs:label>
        <rdfs:seeAlso rdf:resource="http://www.buildingsmart-tech.org/ifcOWL/IFC4_ADD2#IfcCoveringEnumType"/>
    </owl:Class>
    


    <!-- https://pi.pauwel.be/voc/buildingelement#Covering-SLEEVING -->

    <owl:Class rdf:about="https://pi.pauwel.be/voc/buildingelement#Covering-SLEEVING">
        <rdfs:subClassOf rdf:resource="https://pi.pauwel.be/voc/buildingelement#Covering"/>
        <rdfs:comment xml:lang="en">http://bsdd.buildingsmart.org/#concept/details/2mox_rbmb43xWuIkQmJqW1</rdfs:comment>
        <rdfs:label xml:lang="en">Sleeving</rdfs:label>
        <rdfs:label xml:lang="nb-no">strømpe</rdfs:label>
        <rdfs:seeAlso rdf:resource="http://www.buildingsmart-tech.org/ifcOWL/IFC4_ADD2#IfcCoveringEnumType"/>
    </owl:Class>
    


    <!-- https://pi.pauwel.be/voc/buildingelement#Covering-WRAPPING -->

    <owl:Class rdf:about="https://pi.pauwel.be/voc/buildingelement#Covering-WRAPPING">
        <rdfs:subClassOf rdf:resource="https://pi.pauwel.be/voc/buildingelement#Covering"/>
        <rdfs:comment xml:lang="en">http://bsdd.buildingsmart.org/#concept/details/16XES3__TAdwQ57Ox4T_V8</rdfs:comment>
        <rdfs:label xml:lang="en">Wrapping</rdfs:label>
        <rdfs:label xml:lang="nb-no">innkledning</rdfs:label>
        <rdfs:seeAlso rdf:resource="http://www.buildingsmart-tech.org/ifcOWL/IFC4_ADD2#IfcCoveringEnumType"/>
    </owl:Class>
    


    <!-- https://pi.pauwel.be/voc/buildingelement#CurtainWall -->

    <owl:Class rdf:about="https://pi.pauwel.be/voc/buildingelement#CurtainWall">
        <rdfs:subClassOf rdf:resource="https://pi.pauwel.be/voc/buildingelement#BuildingElement"/>
        <rdfs:comment xml:lang="en">An exterior wall of a building which is an assembly of components, hung from the edge of the floor/roof structure rather than bearing on a floor. </rdfs:comment>
        <rdfs:comment xml:lang="de-de">Vertikale und horizontale Bauteile, die untereinander verbunden und mit dem Tragwerk des Gebäudes verankert sind sowie gefüllt sind, um eine raumabschließende, durchgehende Außenschicht zu bilden, die alleine oder gemeinsam mit der übrigen Baukonstruktion, alle normalen Funktionen einer Außenwand bietet, jedoch keine lastabtragenden Funktionen erfüllt</rdfs:comment>
        <rdfs:comment xml:lang="it-it">elementi strutturali verticali e orizzontali, collegati assieme e ancorati alla struttura di supporto dell&apos;edificio e tamponati, a formare una pelle di chiusura continua che fornisce, da sola o in congiunzione con la costruzione, tutte le normali funzioni di un muro esterno, ma non assume nessuna delle caratteristiche portanti della struttura dell&apos;edificio</rdfs:comment>
        <rdfs:comment xml:lang="es-es">elementos estructurales verticales y horizontales, conectados entre sí y anclados a la estructura portante del edificio y rellenados, para formar un conjunto de piel continua que proporciona, por sí mismo o conjuntamente con la construcción del edificio, todas las funciones normales de una pared externa, pero no se hace cargo de ninguna de las características portantes de la estructura del edificio</rdfs:comment>
        <rdfs:comment xml:lang="en">http://bsdd.buildingsmart.org/#concept/details/1nBFK0qT0HuO00025QrE$V</rdfs:comment>
        <rdfs:comment xml:lang="fr-fr">les éléments de structure verticaux et horizontaux reliés ensemble et ancrés sur la structure portante du bâtiment et remplis pour former un espace renfermant une peau continue qui fournit, par elle-même ou en combinaison avec la construction du bâtiment, toutes les fonctions normales d&apos;un mur extérieur, mais n&apos;emprunte aucune des caractéristiques de résistance à la charge de la structure du bâtiment</rdfs:comment>
        <rdfs:comment xml:lang="dk-dk">lodrette og vandrette bygningselementer, der er bundet sammen og forankret til bygningens bærende konstruktion og fyldt, så de danner en fortløbende inddækning, der i sig selv eller sammen med bygningskonstruktionen leverer alle en ydermurs normale funktioner, men som ikke påtager sig nogen af bygningskonstruktionens bærende egenskaber</rdfs:comment>
        <rdfs:comment xml:lang="pl-pl">pionowe i poziome elementy konstrukcyjne, połączone ze sobą i zakotwiczone w konstrukcji nośnej budynku i w zabudowie typu plomba, tworzące przestrzeń obejmującą ciągłą warstwę, która zapewnia, samodzielnie lub w połączeniu z konstrukcją budynku, wszystkie normalne funkcje ściany zewnętrznej, ale nie spełnia żadnej funkcji nośnej dla konstrukcji budynku</rdfs:comment>
        <rdfs:comment xml:lang="fi-fi">pysty- ja vaakasuuntaisia rakenneosia, toisiinsa liitettyinä ja rakennuksen kantavaan rakenteeseen kiinnitettynä, täydennettynä muodostamaan suojaavan yhtenäisen pintatilan, jolla on sellaisenaan tai yhdessä rakennuksen kanssa kaikki ulkoisen seinän normaalit toimintaominaisuudet, mutta jota ei käytetä kantavana rakenteena</rdfs:comment>
        <rdfs:comment xml:lang="nb-no">utvendig, ikkebærende veggkonstruksjon forankret til bygningens hovedbærekonstruksjon. påhengsvegger bygges vanligvis av et rammeverk av metall, tre eller PVC med vertikale og horisontale komponenter som overfører påhengsveggens egenvekt og eventuelle vindkrefter til bygningens bærekonstruksjon</rdfs:comment>
        <rdfs:comment xml:lang="en">vertical and horizontal structural members, connected together and anchored to the supporting structure of the building and infilled, to form a space enclosing continuous skin, which provides, by itself or in conjunction with the building construction, all the normal functions of an external wall, but does not take on any of the load bearing characteristics of the building structure</rdfs:comment>
        <rdfs:comment xml:lang="sv-se">vertikala och horisontella byggnadsdelar som har sammanfogats och förankrats vid byggnadens stödkonstruktion och isolerats, för att skapa en inhägnad med kontinuerlig yta som, av sig själv eller tillsammans med byggnadskonstruktionen, erbjuder alla funktioner som en yttervägg vanligtvis har, men som inte har några av byggnadskonstruktionens bärande egenskaper</rdfs:comment>
        <rdfs:comment xml:lang="bg-bg">вертикални и хоризонтални конструктивни елементи, свързани помежду си, закрепени към основната конструкция на сградата и запълнени, за да образуват непрекъсната ограждаща пространството обвивка, която осигурява, самостоятелно или съвместно с конструкцията на сградата, всички изисквани функции към една външна стена, но без да изпълнява никакви функции свързани с носимоспособността на сградната конструкция</rdfs:comment>
        <rdfs:label xml:lang="en">Curtain Wall</rdfs:label>
        <rdfs:label xml:lang="nl">Gordijngevel</rdfs:label>
        <rdfs:label xml:lang="nl-nl">Gordijngevel</rdfs:label>
        <rdfs:label xml:lang="fr-fr">Mur rideau</rdfs:label>
        <rdfs:label xml:lang="de-de">Vorhangfassade</rdfs:label>
        <rdfs:label xml:lang="de-de">Vorhangfassadenbausatz</rdfs:label>
        <rdfs:label xml:lang="fi-fi">julkisivujärjestelmä</rdfs:label>
        <rdfs:label xml:lang="nb-no">påhengsvegg</rdfs:label>
        <rdfs:label xml:lang="sv-se">sats till utfackningsväggar</rdfs:label>
        <rdfs:label xml:lang="pl-pl">zestaw ściany osłonowej</rdfs:label>
        <rdfs:label xml:lang="bg-bg">монтажни модули за окачени фасади</rdfs:label>
        <rdfs:seeAlso rdf:resource="http://www.buildingsmart-tech.org/ifcOWL/IFC4_ADD2#IfcCurtainWall"/>
    </owl:Class>
    


    <!-- https://pi.pauwel.be/voc/buildingelement#DiscreteAccessory -->

    <owl:Class rdf:about="https://pi.pauwel.be/voc/buildingelement#DiscreteAccessory">
        <rdfs:subClassOf rdf:resource="https://pi.pauwel.be/voc/buildingelement#ElementComponent"/>
        <rdfs:comment xml:lang="en">A representation of different kinds of accessories included in or added to elements.</rdfs:comment>
        <rdfs:comment xml:lang="en">http://bsdd.buildingsmart.org/#concept/details/0W7W20qT8HuO00025QrE$V</rdfs:comment>
        <rdfs:label xml:lang="fr-fr">Accessoire composé</rdfs:label>
        <rdfs:label xml:lang="en">Discrete Accessory</rdfs:label>
        <rdfs:label xml:lang="de-de">Zusatzgerät / Einbauteil</rdfs:label>
        <rdfs:seeAlso rdf:resource="http://www.buildingsmart-tech.org/ifcOWL/IFC4_ADD2#IfcDiscreteAccessory"/>
    </owl:Class>
    


    <!-- https://pi.pauwel.be/voc/buildingelement#DiscreteAccessory-ANCHORPLATE -->

    <owl:Class rdf:about="https://pi.pauwel.be/voc/buildingelement#DiscreteAccessory-ANCHORPLATE">
        <rdfs:subClassOf rdf:resource="https://pi.pauwel.be/voc/buildingelement#DiscreteAccessory"/>
        <rdfs:comment xml:lang="en">http://bsdd.buildingsmart.org/#concept/details/1XD5ysVrvF$haI5OgtznWi</rdfs:comment>
        <rdfs:label xml:lang="en">Anchor Plate</rdfs:label>
        <rdfs:seeAlso rdf:resource="http://www.buildingsmart-tech.org/ifcOWL/IFC4_ADD2#IfcDiscreteAccessoryEnumType"/>
    </owl:Class>
    


    <!-- https://pi.pauwel.be/voc/buildingelement#DiscreteAccessory-BRACKET -->

    <owl:Class rdf:about="https://pi.pauwel.be/voc/buildingelement#DiscreteAccessory-BRACKET">
        <rdfs:subClassOf rdf:resource="https://pi.pauwel.be/voc/buildingelement#DiscreteAccessory"/>
        <rdfs:comment xml:lang="en">An artefact which is projecting from the side of a wall or other structure intended to support some other artefacts.        </rdfs:comment>
        <rdfs:comment xml:lang="nb-no">Brakkett for utstyr</rdfs:comment>
        <rdfs:comment xml:lang="nb-no">Innstøpningsbrakett</rdfs:comment>
        <rdfs:comment xml:lang="en">http://bsdd.buildingsmart.org/#concept/details/3EGCgYGC9F3PmaQ821Ax2u</rdfs:comment>
        <rdfs:comment xml:lang="en">http://bsdd.buildingsmart.org/#concept/details/3vHPwWoT0Hsm00051Mm008</rdfs:comment>
        <rdfs:comment xml:lang="en">http://bsdd.buildingsmart.org/#concept/details/3vHcVCoT0Hsm00051Mm008</rdfs:comment>
        <rdfs:label xml:lang="en">Bracket</rdfs:label>
        <rdfs:label xml:lang="nl-nl">Console</rdfs:label>
        <rdfs:label xml:lang="de-de">Winkellasche</rdfs:label>
        <rdfs:label xml:lang="en">bracket for innerwall</rdfs:label>
        <rdfs:label xml:lang="nb-no">brakett</rdfs:label>
        <rdfs:label xml:lang="nb-no">brakett innervegg</rdfs:label>
        <rdfs:label xml:lang="en">console</rdfs:label>
        <rdfs:label xml:lang="fr-fr">crochet</rdfs:label>
        <rdfs:label xml:lang="nb-no">innervegg</rdfs:label>
        <rdfs:label xml:lang="nb-no">innerveggbrakett</rdfs:label>
        <rdfs:label xml:lang="nb-no">innstøpningsbrakett</rdfs:label>
        <rdfs:seeAlso rdf:resource="http://www.buildingsmart-tech.org/ifcOWL/IFC4_ADD2#IfcDiscreteAccessoryEnumType"/>
    </owl:Class>
    


    <!-- https://pi.pauwel.be/voc/buildingelement#DiscreteAccessory-SHOE -->

    <owl:Class rdf:about="https://pi.pauwel.be/voc/buildingelement#DiscreteAccessory-SHOE">
        <rdfs:subClassOf rdf:resource="https://pi.pauwel.be/voc/buildingelement#DiscreteAccessory"/>
        <rdfs:comment xml:lang="en">http://bsdd.buildingsmart.org/#concept/details/1i44itooP5F9e53Jc$HR0o</rdfs:comment>
        <rdfs:label>Shoe</rdfs:label>
        <rdfs:label xml:lang="nb-no">søylesko</rdfs:label>
        <rdfs:seeAlso rdf:resource="http://www.buildingsmart-tech.org/ifcOWL/IFC4_ADD2#IfcDiscreteAccessoryEnumType"/>
    </owl:Class>
    


    <!-- https://pi.pauwel.be/voc/buildingelement#Door -->

    <owl:Class rdf:about="https://pi.pauwel.be/voc/buildingelement#Door">
        <rdfs:subClassOf rdf:resource="https://pi.pauwel.be/voc/buildingelement#BuildingElement"/>
        <rdfs:comment xml:lang="nb-no">Bygningsdel som dekker en åpning i utvendig eller innvendig vegg, og som kan åpnes eller stenges for passasje.</rdfs:comment>
        <rdfs:comment xml:lang="nb-no">En åpning i en barriære med et dørblad som kan lukke åpningen og en ramme som holder dørbladet.</rdfs:comment>
        <rdfs:comment xml:lang="en">a complete unit consisting of a door frame and a door leaf or leaves, supplied with the essential hardware and wheatherseal, as a product from a single source</rdfs:comment>
        <rdfs:comment xml:lang="en">construction for closing an opening intended primarily for access or egress or both. Typically consisting of a panel that swings on hinges or that slides or rotates</rdfs:comment>
        <rdfs:comment xml:lang="en">http://bsdd.buildingsmart.org/#concept/details/3vHRQ8oT0Hsm00051Mm008</rdfs:comment>
        <rdfs:label xml:lang="nl-nl">Deur</rdfs:label>
        <rdfs:label xml:lang="en">Door</rdfs:label>
        <rdfs:label xml:lang="da">Dør</rdfs:label>
        <rdfs:label xml:lang="de-de">Tür</rdfs:label>
        <rdfs:label xml:lang="de-de">Türeinheit</rdfs:label>
        <rdfs:label xml:lang="nb-no">dør</rdfs:label>
        <rdfs:label xml:lang="nb-no">dør med karm</rdfs:label>
        <rdfs:label xml:lang="fr-fr">porte</rdfs:label>
        <rdfs:seeAlso rdf:resource="http://www.buildingsmart-tech.org/ifcOWL/IFC4_ADD2#IfcDoor"/>
    </owl:Class>
    


    <!-- https://pi.pauwel.be/voc/buildingelement#Door-DOOR -->

    <owl:Class rdf:about="https://pi.pauwel.be/voc/buildingelement#Door-DOOR">
        <rdfs:subClassOf rdf:resource="https://pi.pauwel.be/voc/buildingelement#Door"/>
        <rdfs:comment xml:lang="en">A standard door usually within a wall opening, as a door panel in a curtain wall, or as a &quot;free standing&quot; door.</rdfs:comment>
        <rdfs:comment xml:lang="nb-no">Bygningsdel som dekker en åpning i utvendig eller innvendig vegg, og som kan åpnes eller stenges for passasje.</rdfs:comment>
        <rdfs:comment xml:lang="nb-no">En åpning i en barriære med et dørblad som kan lukke åpningen og en ramme som holder dørbladet.</rdfs:comment>
        <rdfs:comment xml:lang="en">a complete unit consisting of a door frame and a door leaf or leaves, supplied with the essential hardware and wheatherseal, as a product from a single source</rdfs:comment>
        <rdfs:comment xml:lang="en">construction for closing an opening intended primarily for access or egress or both. Typically consisting of a panel that swings on hinges or that slides or rotates</rdfs:comment>
        <rdfs:comment xml:lang="en">http://bsdd.buildingsmart.org/#concept/details/2reX7MzyDDPP8OCoYtmU7d</rdfs:comment>
        <rdfs:label xml:lang="nl-nl">Deur</rdfs:label>
        <rdfs:label xml:lang="en">Door</rdfs:label>
        <rdfs:label xml:lang="de-de">Tür</rdfs:label>
        <rdfs:label xml:lang="de-de">Türeinheit</rdfs:label>
        <rdfs:label xml:lang="fr-fr">bloc-porte</rdfs:label>
        <rdfs:label xml:lang="nl-nl">deur</rdfs:label>
        <rdfs:label xml:lang="nb-no">dør</rdfs:label>
        <rdfs:label xml:lang="nb-no">dør med karm</rdfs:label>
        <rdfs:label xml:lang="fr-fr">porte</rdfs:label>
        <rdfs:seeAlso rdf:resource="http://www.buildingsmart-tech.org/ifcOWL/IFC4_ADD2#IfcDoorEnumType"/>
    </owl:Class>
    


    <!-- https://pi.pauwel.be/voc/buildingelement#Door-GATE -->

    <owl:Class rdf:about="https://pi.pauwel.be/voc/buildingelement#Door-GATE">
        <rdfs:subClassOf rdf:resource="https://pi.pauwel.be/voc/buildingelement#Door"/>
        <rdfs:comment xml:lang="nb-no">Det engelske ordet &apos;gate&apos; og det franske ordet &apos;portail&apos; refererer til produkter utenfor bygninger, for eksempel i innhegninger, gjerder osv.
Det tyske ordet &apos;Tor&apos; refererer til alle produkter for å stenge åpninger, som tillater passering av kjøretøyer.</rdfs:comment>
        <rdfs:comment xml:lang="en">a movable barrier, usually on hinges, closing an opening in a fence, wall, or other enclosure</rdfs:comment>
        <rdfs:comment xml:lang="en">http://bsdd.buildingsmart.org/#concept/details/3C6qVkdNfEGOKvZBfksYwB</rdfs:comment>
        <rdfs:comment xml:lang="nb-no">innretning for å lukke en åpning som er beregnet for passering av kjøretøyer og personer</rdfs:comment>
        <rdfs:label xml:lang="en">Gate</rdfs:label>
        <rdfs:label xml:lang="nl-nl">Hek</rdfs:label>
        <rdfs:label xml:lang="nl-nl">Poort</rdfs:label>
        <rdfs:label xml:lang="de-de">Tor</rdfs:label>
        <rdfs:label xml:lang="fr-fr">fermeture</rdfs:label>
        <rdfs:label xml:lang="nb-no">port</rdfs:label>
        <rdfs:seeAlso rdf:resource="http://www.buildingsmart-tech.org/ifcOWL/IFC4_ADD2#IfcDoorEnumType"/>
    </owl:Class>
    


    <!-- https://pi.pauwel.be/voc/buildingelement#Door-TRAPDOOR -->

    <owl:Class rdf:about="https://pi.pauwel.be/voc/buildingelement#Door-TRAPDOOR">
        <rdfs:subClassOf rdf:resource="https://pi.pauwel.be/voc/buildingelement#Door"/>
        <rdfs:comment xml:lang="en">http://bsdd.buildingsmart.org/#concept/details/3_T7f4cxzB_ur2vAtd6pJe</rdfs:comment>
        <rdfs:label xml:lang="en">Roof Hatch</rdfs:label>
        <rdfs:label xml:lang="en">Trap Door</rdfs:label>
        <rdfs:label xml:lang="nb-no">takluke</rdfs:label>
        <rdfs:seeAlso rdf:resource="http://www.buildingsmart-tech.org/ifcOWL/IFC4_ADD2#IfcDoorEnumType"/>
    </owl:Class>
    


    <!-- https://pi.pauwel.be/voc/buildingelement#ElementComponent -->

    <owl:Class rdf:about="https://pi.pauwel.be/voc/buildingelement#ElementComponent">
        <rdfs:subClassOf rdf:resource="https://schema.org/Product"/>
        <rdfs:comment xml:lang="en">A representation for minor items included in, added to or connecting to or between elements, which usually are not of interest from the overall building structure viewpoint. However, these small parts may have vital and load carrying functions within the construction. These items do not provide any actual space boundaries. Typical examples include different kinds of fasteners and various accessories.</rdfs:comment>
        <rdfs:comment xml:lang="en">http://bsdd.buildingsmart.org/#concept/details/2pKpW0qSeHuO00025QrE$V</rdfs:comment>
        <rdfs:label xml:lang="fr-fr">Composant d&apos;élément</rdfs:label>
        <rdfs:label xml:lang="en">Element Component</rdfs:label>
        <rdfs:label xml:lang="de-de">Elementenbestandteil</rdfs:label>
        <rdfs:seeAlso rdf:resource="http://www.buildingsmart-tech.org/ifcOWL/IFC4_ADD2#IfcElementComponent"/>
    </owl:Class>
    


    <!-- https://pi.pauwel.be/voc/buildingelement#Fastener -->

    <owl:Class rdf:about="https://pi.pauwel.be/voc/buildingelement#Fastener">
        <rdfs:subClassOf rdf:resource="https://pi.pauwel.be/voc/buildingelement#ElementComponent"/>
        <rdfs:comment xml:lang="en">Jointing component that is used to operate a door, window, shutter, gate or drawer .</rdfs:comment>
        <rdfs:comment xml:lang="en">Representations of fixing parts which are used as fasteners to connect or join elements with other elements. </rdfs:comment>
        <rdfs:comment xml:lang="en">http://bsdd.buildingsmart.org/#concept/details/2$v8e0qUGHuO00025QrE$V</rdfs:comment>
        <rdfs:label xml:lang="de-de">Befestigungsmittel</rdfs:label>
        <rdfs:label xml:lang="fr-fr">Elément d&apos;assemblage</rdfs:label>
        <rdfs:label xml:lang="en">Fastener</rdfs:label>
        <rdfs:label xml:lang="nb-no">festeinnretning</rdfs:label>
        <rdfs:seeAlso rdf:resource="http://www.buildingsmart-tech.org/ifcOWL/IFC4_ADD2#IfcFastener"/>
    </owl:Class>
    


    <!-- https://pi.pauwel.be/voc/buildingelement#Fastener-GLUE -->

    <owl:Class rdf:about="https://pi.pauwel.be/voc/buildingelement#Fastener-GLUE">
        <rdfs:subClassOf rdf:resource="https://pi.pauwel.be/voc/buildingelement#Fastener"/>
        <rdfs:comment xml:lang="sv-se">bindemedel eller bindemedelslösning för hopfogning av fasta material</rdfs:comment>
        <rdfs:comment xml:lang="en">binder or binder solution for joining solid materials</rdfs:comment>
        <rdfs:comment xml:lang="en">http://bsdd.buildingsmart.org/#concept/details/097NQ9z4T7eOn7nJCQC0yI</rdfs:comment>
        <rdfs:label xml:lang="en">Glue</rdfs:label>
        <rdfs:label xml:lang="nb-no">lim</rdfs:label>
        <rdfs:label xml:lang="sv-se">lim</rdfs:label>
        <rdfs:seeAlso rdf:resource="http://www.buildingsmart-tech.org/ifcOWL/IFC4_ADD2#IfcFastenerEnumType"/>
    </owl:Class>
    


    <!-- https://pi.pauwel.be/voc/buildingelement#Fastener-MORTAR -->

    <owl:Class rdf:about="https://pi.pauwel.be/voc/buildingelement#Fastener-MORTAR">
        <rdfs:subClassOf rdf:resource="https://pi.pauwel.be/voc/buildingelement#Fastener"/>
        <rdfs:comment xml:lang="en">http://bsdd.buildingsmart.org/#concept/details/0dS2xSsC1BbvRjM1MIjNn5</rdfs:comment>
        <rdfs:label xml:lang="en">Mortar</rdfs:label>
        <rdfs:label xml:lang="nb-no">mørtel</rdfs:label>
        <rdfs:seeAlso rdf:resource="http://www.buildingsmart-tech.org/ifcOWL/IFC4_ADD2#IfcFastenerEnumType"/>
    </owl:Class>
    


    <!-- https://pi.pauwel.be/voc/buildingelement#Fastener-WELD -->

    <owl:Class rdf:about="https://pi.pauwel.be/voc/buildingelement#Fastener-WELD">
        <rdfs:subClassOf rdf:resource="https://pi.pauwel.be/voc/buildingelement#Fastener"/>
        <rdfs:comment xml:lang="en">a weld seam between parts of metallic material or other suitable materials</rdfs:comment>
        <rdfs:comment xml:lang="en-gb">a weld seam between parts of metallic material or other suitable materials</rdfs:comment>
        <rdfs:comment xml:lang="en">http://bsdd.buildingsmart.org/#concept/details/01DZw_Z2b4CwKEwBQ9ERPZ</rdfs:comment>
        <rdfs:label xml:lang="en">Weld</rdfs:label>
        <rdfs:label xml:lang="nb-no">sveis</rdfs:label>
        <rdfs:seeAlso rdf:resource="http://www.buildingsmart-tech.org/ifcOWL/IFC4_ADD2#IfcFastenerEnumType"/>
    </owl:Class>
    


    <!-- https://pi.pauwel.be/voc/buildingelement#Footing -->

    <owl:Class rdf:about="https://pi.pauwel.be/voc/buildingelement#Footing">
        <rdfs:subClassOf rdf:resource="https://pi.pauwel.be/voc/buildingelement#BuildingElement"/>
        <rdfs:comment xml:lang="en">A part of the foundation of a structure that spreads and transmits the load to the soil. Also characterized as shallow foundation, where the loads are transferred to the ground near the surface.</rdfs:comment>
        <rdfs:comment xml:lang="de-de">Flachgründung</rdfs:comment>
        <rdfs:comment xml:lang="en">http://bsdd.buildingsmart.org/#concept/details/2vyAW0qUWHuO00025QrE$V</rdfs:comment>
        <rdfs:label xml:lang="en">Footing</rdfs:label>
        <rdfs:label xml:lang="de-de">Fundament</rdfs:label>
        <rdfs:label xml:lang="nl-nl">Funderingsvoet</rdfs:label>
        <rdfs:label xml:lang="fr-fr">fondation</rdfs:label>
        <rdfs:seeAlso rdf:resource="http://www.buildingsmart-tech.org/ifcOWL/IFC4_ADD2#IfcFooting"/>
    </owl:Class>
    


    <!-- https://pi.pauwel.be/voc/buildingelement#Footing-CAISSON_FOUNDATION -->

    <owl:Class rdf:about="https://pi.pauwel.be/voc/buildingelement#Footing-CAISSON_FOUNDATION">
        <rdfs:subClassOf rdf:resource="https://pi.pauwel.be/voc/buildingelement#Footing"/>
        <rdfs:comment xml:lang="en">http://bsdd.buildingsmart.org/#concept/details/0MGkpmTGDFC80qy7qA0W2w</rdfs:comment>
        <rdfs:label xml:lang="en">Caisson Foundation</rdfs:label>
        <rdfs:label xml:lang="nb-no">senkekasse til fundament</rdfs:label>
        <rdfs:seeAlso rdf:resource="http://www.buildingsmart-tech.org/ifcOWL/IFC4_ADD2#IfcFootingEnumType"/>
    </owl:Class>
    


    <!-- https://pi.pauwel.be/voc/buildingelement#Footing-FOOTING_BEAM -->

    <owl:Class rdf:about="https://pi.pauwel.be/voc/buildingelement#Footing-FOOTING_BEAM">
        <rdfs:subClassOf rdf:resource="https://pi.pauwel.be/voc/buildingelement#Footing"/>
        <rdfs:comment xml:lang="en">http://bsdd.buildingsmart.org/#concept/details/3hRbiifMvFOgC3tEfSPD8X</rdfs:comment>
        <rdfs:label xml:lang="en">Footing Beam</rdfs:label>
        <rdfs:seeAlso rdf:resource="http://www.buildingsmart-tech.org/ifcOWL/IFC4_ADD2#IfcFootingEnumType"/>
    </owl:Class>
    


    <!-- https://pi.pauwel.be/voc/buildingelement#Footing-PAD_FOOTING -->

    <owl:Class rdf:about="https://pi.pauwel.be/voc/buildingelement#Footing-PAD_FOOTING">
        <rdfs:subClassOf rdf:resource="https://pi.pauwel.be/voc/buildingelement#Footing"/>
        <rdfs:comment xml:lang="en">http://bsdd.buildingsmart.org/#concept/details/1XJ0TK6AbBfxMCQLLkdnDr</rdfs:comment>
        <rdfs:label xml:lang="en">Pad Footing</rdfs:label>
        <rdfs:seeAlso rdf:resource="http://www.buildingsmart-tech.org/ifcOWL/IFC4_ADD2#IfcFootingEnumType"/>
    </owl:Class>
    


    <!-- https://pi.pauwel.be/voc/buildingelement#Footing-PILE_CAP -->

    <owl:Class rdf:about="https://pi.pauwel.be/voc/buildingelement#Footing-PILE_CAP">
        <rdfs:subClassOf rdf:resource="https://pi.pauwel.be/voc/buildingelement#Footing"/>
        <rdfs:comment xml:lang="en">http://bsdd.buildingsmart.org/#concept/details/3$LxhKMZjFuBdi75OQXj0L</rdfs:comment>
        <rdfs:label xml:lang="en">Pile Cap</rdfs:label>
        <rdfs:seeAlso rdf:resource="http://www.buildingsmart-tech.org/ifcOWL/IFC4_ADD2#IfcFootingEnumType"/>
    </owl:Class>
    


    <!-- https://pi.pauwel.be/voc/buildingelement#Footing-STRIP_FOOTING -->

    <owl:Class rdf:about="https://pi.pauwel.be/voc/buildingelement#Footing-STRIP_FOOTING">
        <rdfs:subClassOf rdf:resource="https://pi.pauwel.be/voc/buildingelement#Footing"/>
        <rdfs:comment xml:lang="en">http://bsdd.buildingsmart.org/#concept/details/0mDEbMPpzB9B_vQTUHZLHe</rdfs:comment>
        <rdfs:label xml:lang="en">Strip Footing</rdfs:label>
        <rdfs:label xml:lang="nb-no">platefundament</rdfs:label>
        <rdfs:seeAlso rdf:resource="http://www.buildingsmart-tech.org/ifcOWL/IFC4_ADD2#IfcFootingEnumType"/>
    </owl:Class>
    


    <!-- https://pi.pauwel.be/voc/buildingelement#MechanicalFastener -->

    <owl:Class rdf:about="https://pi.pauwel.be/voc/buildingelement#MechanicalFastener">
        <rdfs:subClassOf rdf:resource="https://pi.pauwel.be/voc/buildingelement#ElementComponent"/>
        <rdfs:comment xml:lang="en">A fastener connecting building elements mechanically. A single instance may represent one or many of actual mechanical fasteners, for example an array of bolts or a row of nails.</rdfs:comment>
        <rdfs:comment xml:lang="en">http://bsdd.buildingsmart.org/#concept/details/2$KV20qV0HuO00025QrE$V</rdfs:comment>
        <rdfs:label xml:lang="en">Mechanical Fastener</rdfs:label>
        <rdfs:label>MechanicalFastener</rdfs:label>
        <rdfs:label xml:lang="de-de">Mechanisches Befestigungsmittel</rdfs:label>
        <rdfs:label xml:lang="nb-no">mekanisk festemiddel</rdfs:label>
        <rdfs:seeAlso rdf:resource="http://www.buildingsmart-tech.org/ifcOWL/IFC4_ADD2#IfcMechanicalFastener"/>
    </owl:Class>
    


    <!-- https://pi.pauwel.be/voc/buildingelement#MechanicalFastener-ANCHORBOLT -->

    <owl:Class rdf:about="https://pi.pauwel.be/voc/buildingelement#MechanicalFastener-ANCHORBOLT">
        <rdfs:subClassOf rdf:resource="https://pi.pauwel.be/voc/buildingelement#MechanicalFastener"/>
        <rdfs:comment xml:lang="en">http://bsdd.buildingsmart.org/#concept/details/3NJqge3HD7du28Nje_S1Yv</rdfs:comment>
        <rdfs:label xml:lang="en">Anchor Bolt</rdfs:label>
        <rdfs:label xml:lang="nb-no">mekanisk ankerbolt</rdfs:label>
        <rdfs:seeAlso rdf:resource="http://www.buildingsmart-tech.org/ifcOWL/IFC4_ADD2#IfcMechanicalFastenerEnumType"/>
    </owl:Class>
    


    <!-- https://pi.pauwel.be/voc/buildingelement#MechanicalFastener-BOLT -->

    <owl:Class rdf:about="https://pi.pauwel.be/voc/buildingelement#MechanicalFastener-BOLT">
        <rdfs:subClassOf rdf:resource="https://pi.pauwel.be/voc/buildingelement#MechanicalFastener"/>
        <rdfs:comment xml:lang="en">a threaded cylindrical rod that engages with a similarly threaded hole in a nut or any other part to form a fastener. the mechanical fastener often also includes one or more washers and one or more nuts.</rdfs:comment>
        <rdfs:comment xml:lang="en">http://bsdd.buildingsmart.org/#concept/details/2yfVRHZ2X7heCLVLk0oVBK</rdfs:comment>
        <rdfs:label xml:lang="en">Bolt</rdfs:label>
        <rdfs:label xml:lang="nb-no">mekanisk festemiddel - bolt</rdfs:label>
        <rdfs:seeAlso rdf:resource="http://www.buildingsmart-tech.org/ifcOWL/IFC4_ADD2#IfcMechanicalFastenerEnumType"/>
    </owl:Class>
    


    <!-- https://pi.pauwel.be/voc/buildingelement#MechanicalFastener-DOWEL -->

    <owl:Class rdf:about="https://pi.pauwel.be/voc/buildingelement#MechanicalFastener-DOWEL">
        <rdfs:subClassOf rdf:resource="https://pi.pauwel.be/voc/buildingelement#MechanicalFastener"/>
        <rdfs:comment xml:lang="nb-no">Dybel</rdfs:comment>
        <rdfs:comment xml:lang="en">http://bsdd.buildingsmart.org/#concept/details/2jZSkKNyPBMwSeeMxlYWrc</rdfs:comment>
        <rdfs:comment xml:lang="en">http://bsdd.buildingsmart.org/#concept/details/3vHOxEoT0Hsm00051Mm008</rdfs:comment>
        <rdfs:comment xml:lang="en">rod protruding from the toe of the sheet pile, used for fixing sheet piles to the bed-rock</rdfs:comment>
        <rdfs:comment xml:lang="nb-no">stag som stikker ut fra foten av spuntnålen, og som brukes for å feste spunten til fjell</rdfs:comment>
        <rdfs:label>Dowel</rdfs:label>
        <rdfs:label xml:lang="de-de">Felsdübel</rdfs:label>
        <rdfs:label xml:lang="en">dowel</rdfs:label>
        <rdfs:label xml:lang="nb-no">dybel</rdfs:label>
        <rdfs:label xml:lang="fr-fr">goujon pour rocher</rdfs:label>
        <rdfs:label xml:lang="en">rock dowel</rdfs:label>
        <rdfs:seeAlso rdf:resource="http://www.buildingsmart-tech.org/ifcOWL/IFC4_ADD2#IfcMechanicalFastenerEnumType"/>
    </owl:Class>
    


    <!-- https://pi.pauwel.be/voc/buildingelement#MechanicalFastener-NAIL -->

    <owl:Class rdf:about="https://pi.pauwel.be/voc/buildingelement#MechanicalFastener-NAIL">
        <rdfs:subClassOf rdf:resource="https://pi.pauwel.be/voc/buildingelement#MechanicalFastener"/>
        <rdfs:comment xml:lang="en">http://bsdd.buildingsmart.org/#concept/details/1WICu7sp12cQ$$2QCHf$DB</rdfs:comment>
        <rdfs:label xml:lang="en">Nail</rdfs:label>
        <rdfs:label xml:lang="nb-no">spiker</rdfs:label>
        <rdfs:seeAlso rdf:resource="http://www.buildingsmart-tech.org/ifcOWL/IFC4_ADD2#IfcMechanicalFastenerEnumType"/>
    </owl:Class>
    


    <!-- https://pi.pauwel.be/voc/buildingelement#MechanicalFastener-NAILPLATE -->

    <owl:Class rdf:about="https://pi.pauwel.be/voc/buildingelement#MechanicalFastener-NAILPLATE">
        <rdfs:subClassOf rdf:resource="https://pi.pauwel.be/voc/buildingelement#MechanicalFastener"/>
        <rdfs:comment xml:lang="en">http://bsdd.buildingsmart.org/#concept/details/26FDcCBjH3BOLZTZb29fxk</rdfs:comment>
        <rdfs:label xml:lang="en">Nail Plate</rdfs:label>
        <rdfs:label xml:lang="nb-no">spikerplate</rdfs:label>
        <rdfs:seeAlso rdf:resource="http://www.buildingsmart-tech.org/ifcOWL/IFC4_ADD2#IfcMechanicalFastenerEnumType"/>
    </owl:Class>
    


    <!-- https://pi.pauwel.be/voc/buildingelement#MechanicalFastener-RIVET -->

    <owl:Class rdf:about="https://pi.pauwel.be/voc/buildingelement#MechanicalFastener-RIVET">
        <rdfs:subClassOf rdf:resource="https://pi.pauwel.be/voc/buildingelement#MechanicalFastener"/>
        <rdfs:comment xml:lang="en">http://bsdd.buildingsmart.org/#concept/details/1zynxAt3H1eAVfmukRcO4R</rdfs:comment>
        <rdfs:label xml:lang="en">Rivet</rdfs:label>
        <rdfs:label xml:lang="nb-no">nagle</rdfs:label>
        <rdfs:seeAlso rdf:resource="http://www.buildingsmart-tech.org/ifcOWL/IFC4_ADD2#IfcMechanicalFastenerEnumType"/>
    </owl:Class>
    


    <!-- https://pi.pauwel.be/voc/buildingelement#MechanicalFastener-SCREW -->

    <owl:Class rdf:about="https://pi.pauwel.be/voc/buildingelement#MechanicalFastener-SCREW">
        <rdfs:subClassOf rdf:resource="https://pi.pauwel.be/voc/buildingelement#MechanicalFastener"/>
        <rdfs:comment xml:lang="en">http://bsdd.buildingsmart.org/#concept/details/2NLmoal3LAGxceh8SPCvI7</rdfs:comment>
        <rdfs:label xml:lang="en">Screw</rdfs:label>
        <rdfs:label xml:lang="nb-no">skrue</rdfs:label>
        <rdfs:seeAlso rdf:resource="http://www.buildingsmart-tech.org/ifcOWL/IFC4_ADD2#IfcMechanicalFastenerEnumType"/>
    </owl:Class>
    


    <!-- https://pi.pauwel.be/voc/buildingelement#MechanicalFastener-SHEARCONNECTOR -->

    <owl:Class rdf:about="https://pi.pauwel.be/voc/buildingelement#MechanicalFastener-SHEARCONNECTOR">
        <rdfs:subClassOf rdf:resource="https://pi.pauwel.be/voc/buildingelement#MechanicalFastener"/>
        <rdfs:comment xml:lang="en">http://bsdd.buildingsmart.org/#concept/details/0sHCCoroj0pesEpqdsmtRT</rdfs:comment>
        <rdfs:label xml:lang="en">Shear Connector</rdfs:label>
        <rdfs:seeAlso rdf:resource="http://www.buildingsmart-tech.org/ifcOWL/IFC4_ADD2#IfcMechanicalFastenerEnumType"/>
    </owl:Class>
    


    <!-- https://pi.pauwel.be/voc/buildingelement#MechanicalFastener-STAPLE -->

    <owl:Class rdf:about="https://pi.pauwel.be/voc/buildingelement#MechanicalFastener-STAPLE">
        <rdfs:subClassOf rdf:resource="https://pi.pauwel.be/voc/buildingelement#MechanicalFastener"/>
        <rdfs:comment xml:lang="en">http://bsdd.buildingsmart.org/#concept/details/3ugeBu3lP8WANu_d7DFAtv</rdfs:comment>
        <rdfs:label xml:lang="en">Staple</rdfs:label>
        <rdfs:label xml:lang="nb-no">stift</rdfs:label>
        <rdfs:seeAlso rdf:resource="http://www.buildingsmart-tech.org/ifcOWL/IFC4_ADD2#IfcMechanicalFastenerEnumType"/>
    </owl:Class>
    


    <!-- https://pi.pauwel.be/voc/buildingelement#MechanicalFastener-STUDSHEARCONNECTOR -->

    <owl:Class rdf:about="https://pi.pauwel.be/voc/buildingelement#MechanicalFastener-STUDSHEARCONNECTOR">
        <rdfs:subClassOf rdf:resource="https://pi.pauwel.be/voc/buildingelement#MechanicalFastener"/>
        <rdfs:comment xml:lang="en">http://bsdd.buildingsmart.org/#concept/details/2VmXuOwNvFIxXMT91lYI9q</rdfs:comment>
        <rdfs:label xml:lang="en">Stud Shear Connector</rdfs:label>
        <rdfs:seeAlso rdf:resource="http://www.buildingsmart-tech.org/ifcOWL/IFC4_ADD2#IfcMechanicalFastenerEnumType"/>
    </owl:Class>
    


    <!-- https://pi.pauwel.be/voc/buildingelement#Member -->

    <owl:Class rdf:about="https://pi.pauwel.be/voc/buildingelement#Member">
        <rdfs:subClassOf rdf:resource="https://pi.pauwel.be/voc/buildingelement#BuildingElement"/>
        <rdfs:comment xml:lang="en">A structural member designed to carry loads between or beyond points of support. It is not required to be load bearing.  A linear architectural or structural element that cannot be expressed more specifically as either a beam or column.</rdfs:comment>
        <rdfs:comment xml:lang="en">http://bsdd.buildingsmart.org/#concept/details/11GXc0qV4HuO00025QrE$V</rdfs:comment>
        <rdfs:label xml:lang="en">Member</rdfs:label>
        <rdfs:label xml:lang="fr-fr">Membre</rdfs:label>
        <rdfs:label xml:lang="de-de">Stab / Stabträger</rdfs:label>
        <rdfs:label xml:lang="nb-no">konstruksjonsdel</rdfs:label>
        <rdfs:seeAlso rdf:resource="http://www.buildingsmart-tech.org/ifcOWL/IFC4_ADD2#IfcMember"/>
    </owl:Class>
    


    <!-- https://pi.pauwel.be/voc/buildingelement#Member-BRACE -->

    <owl:Class rdf:about="https://pi.pauwel.be/voc/buildingelement#Member-BRACE">
        <rdfs:subClassOf rdf:resource="https://pi.pauwel.be/voc/buildingelement#Member"/>
        <rdfs:comment xml:lang="en">http://bsdd.buildingsmart.org/#concept/details/0ccYVvWMX5jwoOSredVplR</rdfs:comment>
        <rdfs:label xml:lang="en">Brace</rdfs:label>
        <rdfs:label xml:lang="nb-no">avstiver</rdfs:label>
        <rdfs:seeAlso rdf:resource="http://www.buildingsmart-tech.org/ifcOWL/IFC4_ADD2#IfcMemberEnumType"/>
    </owl:Class>
    


    <!-- https://pi.pauwel.be/voc/buildingelement#Member-CHORD -->

    <owl:Class rdf:about="https://pi.pauwel.be/voc/buildingelement#Member-CHORD">
        <rdfs:subClassOf rdf:resource="https://pi.pauwel.be/voc/buildingelement#Member"/>
        <rdfs:comment xml:lang="en">http://bsdd.buildingsmart.org/#concept/details/1_qCPXQ3j1VBh_PCDSM2PC</rdfs:comment>
        <rdfs:label xml:lang="en">Chord</rdfs:label>
        <rdfs:label xml:lang="nb-no">gurt</rdfs:label>
        <rdfs:seeAlso rdf:resource="http://www.buildingsmart-tech.org/ifcOWL/IFC4_ADD2#IfcMemberEnumType"/>
    </owl:Class>
    


    <!-- https://pi.pauwel.be/voc/buildingelement#Member-COLLAR -->

    <owl:Class rdf:about="https://pi.pauwel.be/voc/buildingelement#Member-COLLAR">
        <rdfs:subClassOf rdf:resource="https://pi.pauwel.be/voc/buildingelement#Member"/>
        <rdfs:comment xml:lang="en">http://bsdd.buildingsmart.org/#concept/details/1r9F5o8Pv9mPKppdGc$YOw</rdfs:comment>
        <rdfs:label xml:lang="en">Collar</rdfs:label>
        <rdfs:label xml:lang="nb-no">krage</rdfs:label>
        <rdfs:seeAlso rdf:resource="http://www.buildingsmart-tech.org/ifcOWL/IFC4_ADD2#IfcMemberEnumType"/>
    </owl:Class>
    


    <!-- https://pi.pauwel.be/voc/buildingelement#Member-MEMBER -->

    <owl:Class rdf:about="https://pi.pauwel.be/voc/buildingelement#Member-MEMBER">
        <rdfs:subClassOf rdf:resource="https://pi.pauwel.be/voc/buildingelement#Member"/>
        <rdfs:comment xml:lang="en">A structural member designed to carry loads between or beyond points of support. It is not required to be load bearing.  A linear architectural or structural element that cannot be expressed more specifically as either a beam or column.</rdfs:comment>
        <rdfs:comment xml:lang="en">http://bsdd.buildingsmart.org/#concept/details/11GXc0qV4HuO00025QrE$V</rdfs:comment>
        <rdfs:label xml:lang="en">Member</rdfs:label>
        <rdfs:label xml:lang="fr-fr">Membre</rdfs:label>
        <rdfs:label xml:lang="de-de">Stab / Stabträger</rdfs:label>
        <rdfs:label xml:lang="nb-no">konstruksjonsdel</rdfs:label>
        <rdfs:seeAlso rdf:resource="http://www.buildingsmart-tech.org/ifcOWL/IFC4_ADD2#IfcMemberEnumType"/>
    </owl:Class>
    


    <!-- https://pi.pauwel.be/voc/buildingelement#Member-MULLION -->

    <owl:Class rdf:about="https://pi.pauwel.be/voc/buildingelement#Member-MULLION">
        <rdfs:subClassOf rdf:resource="https://pi.pauwel.be/voc/buildingelement#Member"/>
        <rdfs:comment xml:lang="en">http://bsdd.buildingsmart.org/#concept/details/2H6TZXz1vEFOlOdhLv3CD7</rdfs:comment>
        <rdfs:label xml:lang="en">Mullion</rdfs:label>
        <rdfs:label xml:lang="nb-no">midtstolpe</rdfs:label>
        <rdfs:seeAlso rdf:resource="http://www.buildingsmart-tech.org/ifcOWL/IFC4_ADD2#IfcMemberEnumType"/>
    </owl:Class>
    


    <!-- https://pi.pauwel.be/voc/buildingelement#Member-PLATE -->

    <owl:Class rdf:about="https://pi.pauwel.be/voc/buildingelement#Member-PLATE">
        <rdfs:subClassOf rdf:resource="https://pi.pauwel.be/voc/buildingelement#Member"/>
        <rdfs:comment xml:lang="en">A planar and often flat part with constant thickness. May carry loads between or beyond points of support, or provide stiffening. </rdfs:comment>
        <rdfs:comment xml:lang="en">http://bsdd.buildingsmart.org/#concept/details/3zdC5dewn4ROXxRERahlnc</rdfs:comment>
        <rdfs:label xml:lang="en">Plate</rdfs:label>
        <rdfs:label xml:lang="de-de">Platte / Paneel</rdfs:label>
        <rdfs:label xml:lang="fr-fr">plaque</rdfs:label>
        <rdfs:label xml:lang="nb-no">plate</rdfs:label>
        <rdfs:label xml:lang="nb-no">platevarmeveksler</rdfs:label>
        <rdfs:seeAlso rdf:resource="http://www.buildingsmart-tech.org/ifcOWL/IFC4_ADD2#IfcMemberEnumType"/>
    </owl:Class>
    


    <!-- https://pi.pauwel.be/voc/buildingelement#Member-POST -->

    <owl:Class rdf:about="https://pi.pauwel.be/voc/buildingelement#Member-POST">
        <rdfs:subClassOf rdf:resource="https://pi.pauwel.be/voc/buildingelement#Member"/>
        <rdfs:comment xml:lang="en">a linear member (usually used vertically) within a roof structure to support purlins</rdfs:comment>
        <rdfs:comment xml:lang="en-gb">a linear member (usually used vertically) within a roof structure to support purlins</rdfs:comment>
        <rdfs:comment xml:lang="en">http://bsdd.buildingsmart.org/#concept/details/3pLJTABEHCJeV4uMg1OJxY</rdfs:comment>
        <rdfs:label>Post</rdfs:label>
        <rdfs:label xml:lang="nb-no">stolpe</rdfs:label>
        <rdfs:seeAlso rdf:resource="http://www.buildingsmart-tech.org/ifcOWL/IFC4_ADD2#IfcMemberEnumType"/>
    </owl:Class>
    


    <!-- https://pi.pauwel.be/voc/buildingelement#Member-PURLIN -->

    <owl:Class rdf:about="https://pi.pauwel.be/voc/buildingelement#Member-PURLIN">
        <rdfs:subClassOf rdf:resource="https://pi.pauwel.be/voc/buildingelement#Member"/>
        <rdfs:comment xml:lang="en">http://bsdd.buildingsmart.org/#concept/details/2ClC__ZBT6lgGn9bEtyKAq</rdfs:comment>
        <rdfs:label>Purlin</rdfs:label>
        <rdfs:label xml:lang="nb-no">takås</rdfs:label>
        <rdfs:seeAlso rdf:resource="http://www.buildingsmart-tech.org/ifcOWL/IFC4_ADD2#IfcMemberEnumType"/>
    </owl:Class>
    


    <!-- https://pi.pauwel.be/voc/buildingelement#Member-RAFTER -->

    <owl:Class rdf:about="https://pi.pauwel.be/voc/buildingelement#Member-RAFTER">
        <rdfs:subClassOf rdf:resource="https://pi.pauwel.be/voc/buildingelement#Member"/>
        <rdfs:comment xml:lang="en">http://bsdd.buildingsmart.org/#concept/details/14MOjpDn1DYfI9uAgvn_Mm</rdfs:comment>
        <rdfs:comment xml:lang="nb-no">sperre</rdfs:comment>
        <rdfs:label xml:lang="en">Rafter</rdfs:label>
        <rdfs:seeAlso rdf:resource="http://www.buildingsmart-tech.org/ifcOWL/IFC4_ADD2#IfcMemberEnumType"/>
    </owl:Class>
    


    <!-- https://pi.pauwel.be/voc/buildingelement#Member-STRINGER -->

    <owl:Class rdf:about="https://pi.pauwel.be/voc/buildingelement#Member-STRINGER">
        <rdfs:subClassOf rdf:resource="https://pi.pauwel.be/voc/buildingelement#Member"/>
        <rdfs:comment xml:lang="en">http://bsdd.buildingsmart.org/#concept/details/31phWfaoDEDwTkU1_cQp7G</rdfs:comment>
        <rdfs:label xml:lang="en">Stringer</rdfs:label>
        <rdfs:label xml:lang="nb-no">vange</rdfs:label>
        <rdfs:seeAlso rdf:resource="http://www.buildingsmart-tech.org/ifcOWL/IFC4_ADD2#IfcMemberEnumType"/>
    </owl:Class>
    


    <!-- https://pi.pauwel.be/voc/buildingelement#Member-STRUT -->

    <owl:Class rdf:about="https://pi.pauwel.be/voc/buildingelement#Member-STRUT">
        <rdfs:subClassOf rdf:resource="https://pi.pauwel.be/voc/buildingelement#Member"/>
        <rdfs:comment xml:lang="en">http://bsdd.buildingsmart.org/#concept/details/0F1OouH1f9rPC$dWa4xYLb</rdfs:comment>
        <rdfs:label xml:lang="en">Strut</rdfs:label>
        <rdfs:label xml:lang="nb-no">trykkstav</rdfs:label>
        <rdfs:seeAlso rdf:resource="http://www.buildingsmart-tech.org/ifcOWL/IFC4_ADD2#IfcMemberEnumType"/>
    </owl:Class>
    


    <!-- https://pi.pauwel.be/voc/buildingelement#Member-STUD -->

    <owl:Class rdf:about="https://pi.pauwel.be/voc/buildingelement#Member-STUD">
        <rdfs:subClassOf rdf:resource="https://pi.pauwel.be/voc/buildingelement#Member"/>
        <rdfs:comment xml:lang="en">http://bsdd.buildingsmart.org/#concept/details/14DS4URKP2au1B2s5ghLFp</rdfs:comment>
        <rdfs:label xml:lang="en">Stud</rdfs:label>
        <rdfs:label xml:lang="nb-no">stender</rdfs:label>
        <rdfs:seeAlso rdf:resource="http://www.buildingsmart-tech.org/ifcOWL/IFC4_ADD2#IfcMemberEnumType"/>
    </owl:Class>
    


    <!-- https://pi.pauwel.be/voc/buildingelement#Pile -->

    <owl:Class rdf:about="https://pi.pauwel.be/voc/buildingelement#Pile">
        <rdfs:subClassOf rdf:resource="https://pi.pauwel.be/voc/buildingelement#BuildingElement"/>
        <rdfs:comment xml:lang="en">A vertical structural member of timber, concrete, or steel, driven into the earth as a foundation or support for a structure for the transfer of actions. </rdfs:comment>
        <rdfs:comment xml:lang="nb-no">En stråle av tømmer, betong eller stål, drevet ned i jorden som fundament eller støtte til en struktur.</rdfs:comment>
        <rdfs:comment xml:lang="en">http://bsdd.buildingsmart.org/#concept/details/3vHXEAoT0Hsm00051Mm008</rdfs:comment>
        <rdfs:comment xml:lang="nb-no">slankt bærende element i grunnen for overføring av laster. I denne europeiske standarden er slankhetsforholdet ikke begrenset</rdfs:comment>
        <rdfs:label xml:lang="de-de">Fundament / Tiefgründung</rdfs:label>
        <rdfs:label xml:lang="de-de">Pfahl</rdfs:label>
        <rdfs:label xml:lang="en">Pile</rdfs:label>
        <rdfs:label xml:lang="nb-no">pel</rdfs:label>
        <rdfs:label xml:lang="nb-no">pele</rdfs:label>
        <rdfs:label xml:lang="fr-fr">pieu</rdfs:label>
        <rdfs:label xml:lang="nb-no">pæl</rdfs:label>
        <rdfs:seeAlso rdf:resource="http://www.buildingsmart-tech.org/ifcOWL/IFC4_ADD2#IfcPile"/>
    </owl:Class>
    


    <!-- https://pi.pauwel.be/voc/buildingelement#Pile-BORED -->

    <owl:Class rdf:about="https://pi.pauwel.be/voc/buildingelement#Pile-BORED">
        <rdfs:subClassOf rdf:resource="https://pi.pauwel.be/voc/buildingelement#Pile"/>
        <rdfs:comment xml:lang="en">http://bsdd.buildingsmart.org/#concept/details/1INEbwMtrBy9rKhAuvXYmq</rdfs:comment>
        <rdfs:label xml:lang="en">Bored Pile</rdfs:label>
        <rdfs:label xml:lang="nb-no">boret pel</rdfs:label>
        <rdfs:seeAlso rdf:resource="http://www.buildingsmart-tech.org/ifcOWL/IFC4_ADD2#IfcPileEnumType"/>
    </owl:Class>
    


    <!-- https://pi.pauwel.be/voc/buildingelement#Pile-COHESION -->

    <owl:Class rdf:about="https://pi.pauwel.be/voc/buildingelement#Pile-COHESION">
        <rdfs:subClassOf rdf:resource="https://pi.pauwel.be/voc/buildingelement#Pile"/>
        <rdfs:comment xml:lang="en">http://bsdd.buildingsmart.org/#concept/details/3xzAjG3Uv5qeCDRxYCXd4d</rdfs:comment>
        <rdfs:label xml:lang="en">Cohesion Pile</rdfs:label>
        <rdfs:label xml:lang="nb-no">kohesjon pel</rdfs:label>
        <rdfs:seeAlso rdf:resource="http://www.buildingsmart-tech.org/ifcOWL/IFC4_ADD2#IfcPileEnumType"/>
    </owl:Class>
    


    <!-- https://pi.pauwel.be/voc/buildingelement#Pile-DRIVEN -->

    <owl:Class rdf:about="https://pi.pauwel.be/voc/buildingelement#Pile-DRIVEN">
        <rdfs:subClassOf rdf:resource="https://pi.pauwel.be/voc/buildingelement#Pile"/>
        <rdfs:comment xml:lang="en">http://bsdd.buildingsmart.org/#concept/details/2Qg5YD6TD299EHtweCaOOy</rdfs:comment>
        <rdfs:label xml:lang="en">Driven Pile</rdfs:label>
        <rdfs:label xml:lang="nb-no">rammet pel</rdfs:label>
        <rdfs:seeAlso rdf:resource="http://www.buildingsmart-tech.org/ifcOWL/IFC4_ADD2#IfcPileEnumType"/>
    </owl:Class>
    


    <!-- https://pi.pauwel.be/voc/buildingelement#Pile-FRICTION -->

    <owl:Class rdf:about="https://pi.pauwel.be/voc/buildingelement#Pile-FRICTION">
        <rdfs:subClassOf rdf:resource="https://pi.pauwel.be/voc/buildingelement#Pile"/>
        <rdfs:comment xml:lang="en">http://bsdd.buildingsmart.org/#concept/details/3LgOubO_D3EhcElUZP9dMe</rdfs:comment>
        <rdfs:label xml:lang="en">Friction Pile</rdfs:label>
        <rdfs:label xml:lang="nb-no">friksjonspele</rdfs:label>
        <rdfs:seeAlso rdf:resource="http://www.buildingsmart-tech.org/ifcOWL/IFC4_ADD2#IfcPileEnumType"/>
    </owl:Class>
    


    <!-- https://pi.pauwel.be/voc/buildingelement#Pile-JETGROUTING -->

    <owl:Class rdf:about="https://pi.pauwel.be/voc/buildingelement#Pile-JETGROUTING">
        <rdfs:subClassOf rdf:resource="https://pi.pauwel.be/voc/buildingelement#Pile"/>
        <rdfs:comment xml:lang="en">http://bsdd.buildingsmart.org/#concept/details/1tI0jqBjHEmADWyrGGYig6</rdfs:comment>
        <rdfs:label xml:lang="en">Jet Grouting Pile</rdfs:label>
        <rdfs:seeAlso rdf:resource="http://www.buildingsmart-tech.org/ifcOWL/IFC4_ADD2#IfcPileEnumType"/>
    </owl:Class>
    


    <!-- https://pi.pauwel.be/voc/buildingelement#Pile-SUPPORT -->

    <owl:Class rdf:about="https://pi.pauwel.be/voc/buildingelement#Pile-SUPPORT">
        <rdfs:subClassOf rdf:resource="https://pi.pauwel.be/voc/buildingelement#Pile"/>
        <rdfs:comment xml:lang="en">http://bsdd.buildingsmart.org/#concept/details/3qZud6iazFjOZ3wK3WoQch</rdfs:comment>
        <rdfs:label xml:lang="en">Support</rdfs:label>
        <rdfs:label xml:lang="nb-no">støtte</rdfs:label>
        <rdfs:seeAlso rdf:resource="http://www.buildingsmart-tech.org/ifcOWL/IFC4_ADD2#IfcPileEnumType"/>
    </owl:Class>
    


    <!-- https://pi.pauwel.be/voc/buildingelement#Plate -->

    <owl:Class rdf:about="https://pi.pauwel.be/voc/buildingelement#Plate">
        <rdfs:subClassOf rdf:resource="https://pi.pauwel.be/voc/buildingelement#BuildingElement"/>
        <rdfs:comment xml:lang="en">A planar and often flat part with constant thickness. May carry loads between or beyond points of support, or provide stiffening. </rdfs:comment>
        <rdfs:comment xml:lang="en">http://bsdd.buildingsmart.org/#concept/details/3z14Y0qVCHuO00025QrE$V</rdfs:comment>
        <rdfs:label xml:lang="en">Plate</rdfs:label>
        <rdfs:label xml:lang="de-de">Platte / Paneel</rdfs:label>
        <rdfs:label xml:lang="fr-fr">plaque</rdfs:label>
        <rdfs:label xml:lang="nb-no">plate</rdfs:label>
        <rdfs:seeAlso rdf:resource="http://www.buildingsmart-tech.org/ifcOWL/IFC4_ADD2#IfcPlate"/>
    </owl:Class>
    


    <!-- https://pi.pauwel.be/voc/buildingelement#Plate-CURTAIN_PANEL -->

    <owl:Class rdf:about="https://pi.pauwel.be/voc/buildingelement#Plate-CURTAIN_PANEL">
        <rdfs:subClassOf rdf:resource="https://pi.pauwel.be/voc/buildingelement#Plate"/>
        <rdfs:comment xml:lang="en">a planar element within a curtain wall, often consisting of a frame with fixed glazing</rdfs:comment>
        <rdfs:comment xml:lang="en-gb">a planar element within a curtain wall, often consisting of a frame with fixed glazing</rdfs:comment>
        <rdfs:comment xml:lang="en">http://bsdd.buildingsmart.org/#concept/details/2N7mbvPFL0QRlf$nLuQE0U</rdfs:comment>
        <rdfs:label xml:lang="en">Curtain Panel</rdfs:label>
        <rdfs:label xml:lang="nb-no">skjermpanel</rdfs:label>
        <rdfs:seeAlso rdf:resource="http://www.buildingsmart-tech.org/ifcOWL/IFC4_ADD2#IfcPlateEnumType"/>
    </owl:Class>
    


    <!-- https://pi.pauwel.be/voc/buildingelement#Plate-SHEET -->

    <owl:Class rdf:about="https://pi.pauwel.be/voc/buildingelement#Plate-SHEET">
        <rdfs:subClassOf rdf:resource="https://pi.pauwel.be/voc/buildingelement#Plate"/>
        <rdfs:comment xml:lang="en">http://bsdd.buildingsmart.org/#concept/details/2C4D8j05v51eRokWOWtlju</rdfs:comment>
        <rdfs:label xml:lang="en">Sheet</rdfs:label>
        <rdfs:seeAlso rdf:resource="http://www.buildingsmart-tech.org/ifcOWL/IFC4_ADD2#IfcPlateEnumType"/>
    </owl:Class>
    


    <!-- https://pi.pauwel.be/voc/buildingelement#Railing -->

    <owl:Class rdf:about="https://pi.pauwel.be/voc/buildingelement#Railing">
        <rdfs:subClassOf rdf:resource="https://pi.pauwel.be/voc/buildingelement#BuildingElement"/>
        <rdfs:comment xml:lang="en">A frame assembly adjacent to human circulation spaces and at some space boundaries where it is used in line of walls or to compliment walls. Designed to aid humans, either as an optional physical support, or to prevent injury by falling.</rdfs:comment>
        <rdfs:comment xml:lang="en">http://bsdd.buildingsmart.org/#concept/details/02irk0qVyHuO00025QrE$V</rdfs:comment>
        <rdfs:label xml:lang="fr-fr">Garde corps</rdfs:label>
        <rdfs:label xml:lang="de-de">Geländer</rdfs:label>
        <rdfs:label xml:lang="da">Gelænder</rdfs:label>
        <rdfs:label xml:lang="nl-nl">Hekwerk</rdfs:label>
        <rdfs:label xml:lang="nl">Leuning</rdfs:label>
        <rdfs:label xml:lang="en">Railing</rdfs:label>
        <rdfs:label xml:lang="nl-nl">Reling</rdfs:label>
        <rdfs:label xml:lang="fr-fr">garde-corps</rdfs:label>
        <rdfs:label xml:lang="nb-no">rekkverk</rdfs:label>
        <rdfs:seeAlso rdf:resource="http://www.buildingsmart-tech.org/ifcOWL/IFC4_ADD2#IfcRailing"/>
    </owl:Class>
    


    <!-- https://pi.pauwel.be/voc/buildingelement#Railing-BALUSTRADE -->

    <owl:Class rdf:about="https://pi.pauwel.be/voc/buildingelement#Railing-BALUSTRADE">
        <rdfs:subClassOf rdf:resource="https://pi.pauwel.be/voc/buildingelement#Railing"/>
        <rdfs:comment xml:lang="en">A balustrade is a separation construction alongside the edges of floors, roofs, stairs and ramps, protecting against falling into the deep.</rdfs:comment>
        <rdfs:comment xml:lang="en">http://bsdd.buildingsmart.org/#concept/details/0ZHKicPyL9l8uyCir_Dsef</rdfs:comment>
        <rdfs:comment xml:lang="en">http://bsdd.buildingsmart.org/#concept/details/30Ez0HE6XAHQh6wJkRK6T$</rdfs:comment>
        <rdfs:label xml:lang="en">Balustrade</rdfs:label>
        <rdfs:label xml:lang="de-de">Geländer</rdfs:label>
        <rdfs:label xml:lang="nl-nl">Hekwerk</rdfs:label>
        <rdfs:label xml:lang="nb-no">balustrader</rdfs:label>
        <rdfs:label xml:lang="nb-no">rekkverk</rdfs:label>
        <rdfs:seeAlso rdf:resource="http://www.buildingsmart-tech.org/ifcOWL/IFC4_ADD2#IfcRailingEnumType"/>
    </owl:Class>
    


    <!-- https://pi.pauwel.be/voc/buildingelement#Railing-GUARDRAIL -->

    <owl:Class rdf:about="https://pi.pauwel.be/voc/buildingelement#Railing-GUARDRAIL">
        <rdfs:subClassOf rdf:resource="https://pi.pauwel.be/voc/buildingelement#Railing"/>
        <rdfs:comment xml:lang="en">A frame assembly adjacent to human circulation spaces and at some space boundaries where it is used in line of walls or to compliment walls. Designed to aid humans, either as an optional physical support, or to prevent injury by falling.</rdfs:comment>
        <rdfs:comment xml:lang="en">http://bsdd.buildingsmart.org/#concept/details/2804vLstn5DfaH_vxv53w3</rdfs:comment>
        <rdfs:label xml:lang="fr-fr">Garde corps</rdfs:label>
        <rdfs:label xml:lang="de-de">Geländer</rdfs:label>
        <rdfs:label xml:lang="en">Guardrail</rdfs:label>
        <rdfs:label xml:lang="fr-fr">garde-corps</rdfs:label>
        <rdfs:label xml:lang="nb-no">rekkverk</rdfs:label>
        <rdfs:seeAlso rdf:resource="http://www.buildingsmart-tech.org/ifcOWL/IFC4_ADD2#IfcRailingEnumType"/>
    </owl:Class>
    


    <!-- https://pi.pauwel.be/voc/buildingelement#Railing-HANDRAIL -->

    <owl:Class rdf:about="https://pi.pauwel.be/voc/buildingelement#Railing-HANDRAIL">
        <rdfs:subClassOf rdf:resource="https://pi.pauwel.be/voc/buildingelement#Railing"/>
        <rdfs:comment xml:lang="nb-no">Håndlister, typisk i korridorer</rdfs:comment>
        <rdfs:comment xml:lang="en">http://bsdd.buildingsmart.org/#concept/details/3vHRZWoT0Hsm00051Mm008</rdfs:comment>
        <rdfs:label xml:lang="de-de">Handlauf</rdfs:label>
        <rdfs:label xml:lang="en">Handrail</rdfs:label>
        <rdfs:label xml:lang="nb-no">håndlist</rdfs:label>
        <rdfs:label xml:lang="fr-fr">main courante</rdfs:label>
        <rdfs:seeAlso rdf:resource="http://www.buildingsmart-tech.org/ifcOWL/IFC4_ADD2#IfcRailingEnumType"/>
    </owl:Class>
    


    <!-- https://pi.pauwel.be/voc/buildingelement#Ramp -->

    <owl:Class rdf:about="https://pi.pauwel.be/voc/buildingelement#Ramp">
        <rdfs:subClassOf rdf:resource="https://pi.pauwel.be/voc/buildingelement#BuildingElement"/>
        <rdfs:comment xml:lang="en">A vertical passageway which provides a human circulation link between one floor level and another floor level at a different elevation. Normally does not include steps.</rdfs:comment>
        <rdfs:comment xml:lang="nb-no">Rampe</rdfs:comment>
        <rdfs:comment xml:lang="en">http://bsdd.buildingsmart.org/#concept/details/0kpjo0qVyHuO00025QrE$V</rdfs:comment>
        <rdfs:label xml:lang="nl">Helling</rdfs:label>
        <rdfs:label xml:lang="en">Ramp</rdfs:label>
        <rdfs:label xml:lang="da">Rampe</rdfs:label>
        <rdfs:label xml:lang="de-de">Rampe</rdfs:label>
        <rdfs:label xml:lang="fr-fr">Rampe</rdfs:label>
        <rdfs:label xml:lang="nl-nl">helling</rdfs:label>
        <rdfs:label xml:lang="nl-nl">hellingbaan</rdfs:label>
        <rdfs:label xml:lang="nb-no">rampe</rdfs:label>
        <rdfs:label xml:lang="nb-no">skråplan</rdfs:label>
        <rdfs:seeAlso rdf:resource="http://www.buildingsmart-tech.org/ifcOWL/IFC4_ADD2#IfcRamp"/>
    </owl:Class>
    


    <!-- https://pi.pauwel.be/voc/buildingelement#Ramp-HALF_TURN_RAMP -->

    <owl:Class rdf:about="https://pi.pauwel.be/voc/buildingelement#Ramp-HALF_TURN_RAMP">
        <rdfs:subClassOf rdf:resource="https://pi.pauwel.be/voc/buildingelement#Ramp"/>
        <rdfs:comment xml:lang="en">http://bsdd.buildingsmart.org/#concept/details/1hJB5FgjL4_v2TrvOBjmzz</rdfs:comment>
        <rdfs:label xml:lang="en">Half Turn Ramp</rdfs:label>
        <rdfs:label xml:lang="nb-no">halv omdreining rampe</rdfs:label>
        <rdfs:seeAlso rdf:resource="http://www.buildingsmart-tech.org/ifcOWL/IFC4_ADD2#IfcRampEnumType"/>
    </owl:Class>
    


    <!-- https://pi.pauwel.be/voc/buildingelement#Ramp-QUARTER_TURN_RAMP -->

    <owl:Class rdf:about="https://pi.pauwel.be/voc/buildingelement#Ramp-QUARTER_TURN_RAMP">
        <rdfs:subClassOf rdf:resource="https://pi.pauwel.be/voc/buildingelement#Ramp"/>
        <rdfs:comment xml:lang="en">http://bsdd.buildingsmart.org/#concept/details/1FZ7G8CAP2UxmW6fnuOOfQ</rdfs:comment>
        <rdfs:label xml:lang="en">Quarter Turn Ramp</rdfs:label>
        <rdfs:label xml:lang="nb-no">rampe med en sving</rdfs:label>
        <rdfs:seeAlso rdf:resource="http://www.buildingsmart-tech.org/ifcOWL/IFC4_ADD2#IfcRampEnumType"/>
    </owl:Class>
    


    <!-- https://pi.pauwel.be/voc/buildingelement#Ramp-SPIRAL_RAMP -->

    <owl:Class rdf:about="https://pi.pauwel.be/voc/buildingelement#Ramp-SPIRAL_RAMP">
        <rdfs:subClassOf rdf:resource="https://pi.pauwel.be/voc/buildingelement#Ramp"/>
        <rdfs:comment xml:lang="en">http://bsdd.buildingsmart.org/#concept/details/2__YGgu4XCN9NmT3LhvE6V</rdfs:comment>
        <rdfs:label xml:lang="en">Spiral Ramp</rdfs:label>
        <rdfs:seeAlso rdf:resource="http://www.buildingsmart-tech.org/ifcOWL/IFC4_ADD2#IfcRampEnumType"/>
    </owl:Class>
    


    <!-- https://pi.pauwel.be/voc/buildingelement#Ramp-STRAIGHT_RUN_RAMP -->

    <owl:Class rdf:about="https://pi.pauwel.be/voc/buildingelement#Ramp-STRAIGHT_RUN_RAMP">
        <rdfs:subClassOf rdf:resource="https://pi.pauwel.be/voc/buildingelement#Ramp"/>
        <rdfs:comment xml:lang="en">http://bsdd.buildingsmart.org/#concept/details/1SYNqJ72H64g7EG2vm8VJu</rdfs:comment>
        <rdfs:label xml:lang="en">Straight Run Ramp</rdfs:label>
        <rdfs:seeAlso rdf:resource="http://www.buildingsmart-tech.org/ifcOWL/IFC4_ADD2#IfcRampEnumType"/>
    </owl:Class>
    


    <!-- https://pi.pauwel.be/voc/buildingelement#Ramp-TWO_QUARTER_TURN_RAMP -->

    <owl:Class rdf:about="https://pi.pauwel.be/voc/buildingelement#Ramp-TWO_QUARTER_TURN_RAMP">
        <rdfs:subClassOf rdf:resource="https://pi.pauwel.be/voc/buildingelement#Ramp"/>
        <rdfs:comment xml:lang="en">http://bsdd.buildingsmart.org/#concept/details/2wUjACPhnDyAgFiGarLaek</rdfs:comment>
        <rdfs:label xml:lang="en">Two Quarter Turn Ramp</rdfs:label>
        <rdfs:label xml:lang="nb-no">rampe med to svinger</rdfs:label>
        <rdfs:seeAlso rdf:resource="http://www.buildingsmart-tech.org/ifcOWL/IFC4_ADD2#IfcRampEnumType"/>
    </owl:Class>
    


    <!-- https://pi.pauwel.be/voc/buildingelement#Ramp-TWO_STRAIGHT_RUN_RAMP -->

    <owl:Class rdf:about="https://pi.pauwel.be/voc/buildingelement#Ramp-TWO_STRAIGHT_RUN_RAMP">
        <rdfs:subClassOf rdf:resource="https://pi.pauwel.be/voc/buildingelement#Ramp"/>
        <rdfs:comment xml:lang="en">http://bsdd.buildingsmart.org/#concept/details/2skPwOQSH1Ex7UR3SpDGbT</rdfs:comment>
        <rdfs:label xml:lang="en">Two Straight Run Ramp</rdfs:label>
        <rdfs:seeAlso rdf:resource="http://www.buildingsmart-tech.org/ifcOWL/IFC4_ADD2#IfcRampEnumType"/>
    </owl:Class>
    


    <!-- https://pi.pauwel.be/voc/buildingelement#RampFlight -->

    <owl:Class rdf:about="https://pi.pauwel.be/voc/buildingelement#RampFlight">
        <rdfs:subClassOf rdf:resource="https://pi.pauwel.be/voc/buildingelement#BuildingElement"/>
        <rdfs:comment xml:lang="en">A single inclined segment, or several inclined segments that are connected by a horizontal segment, referred to as a landing. </rdfs:comment>
        <rdfs:comment xml:lang="en">http://bsdd.buildingsmart.org/#concept/details/1kbSG0qVyHuO00025QrE$V</rdfs:comment>
        <rdfs:label xml:lang="en">Ramp Flight</rdfs:label>
        <rdfs:label xml:lang="de-de">Rampenlauf</rdfs:label>
        <rdfs:label xml:lang="fr-fr">Volée</rdfs:label>
        <rdfs:label xml:lang="nb-no">rampe</rdfs:label>
        <rdfs:seeAlso rdf:resource="http://www.buildingsmart-tech.org/ifcOWL/IFC4_ADD2#IfcRampFlight"/>
    </owl:Class>
    


    <!-- https://pi.pauwel.be/voc/buildingelement#RampFlight-SPIRAL -->

    <owl:Class rdf:about="https://pi.pauwel.be/voc/buildingelement#RampFlight-SPIRAL">
        <rdfs:subClassOf rdf:resource="https://pi.pauwel.be/voc/buildingelement#RampFlight"/>
        <rdfs:comment xml:lang="en">http://bsdd.buildingsmart.org/#concept/details/0CDsSbmyb4GA$0xajhCLYB</rdfs:comment>
        <rdfs:label xml:lang="en">Spiral</rdfs:label>
        <rdfs:label xml:lang="nb-no">spiral</rdfs:label>
        <rdfs:label xml:lang="nb-no">vindel</rdfs:label>
        <rdfs:seeAlso rdf:resource="http://www.buildingsmart-tech.org/ifcOWL/IFC4_ADD2#IfcRampFlightEnumType"/>
    </owl:Class>
    


    <!-- https://pi.pauwel.be/voc/buildingelement#RampFlight-STRAIGHT -->

    <owl:Class rdf:about="https://pi.pauwel.be/voc/buildingelement#RampFlight-STRAIGHT">
        <rdfs:subClassOf rdf:resource="https://pi.pauwel.be/voc/buildingelement#RampFlight"/>
        <rdfs:comment xml:lang="en">http://bsdd.buildingsmart.org/#concept/details/0fyv31IoL8mwvU9TcZR2FC</rdfs:comment>
        <rdfs:label xml:lang="en">Straight</rdfs:label>
        <rdfs:label xml:lang="nb-no">rett</rdfs:label>
        <rdfs:seeAlso rdf:resource="http://www.buildingsmart-tech.org/ifcOWL/IFC4_ADD2#IfcRampFlightEnumType"/>
    </owl:Class>
    


    <!-- https://pi.pauwel.be/voc/buildingelement#ReinforcingBar -->

    <owl:Class rdf:about="https://pi.pauwel.be/voc/buildingelement#ReinforcingBar">
        <rdfs:subClassOf rdf:resource="https://pi.pauwel.be/voc/buildingelement#ReinforcingElement"/>
        <rdfs:comment xml:lang="en">a reinforcing bar is usually made of steel with manufactured deformations in the surface, and used in concrete and masonry construction to provide additional strength. a single instance of this class may represent one or many of actual rebars, for example a row of rebars.</rdfs:comment>
        <rdfs:comment xml:lang="en">http://bsdd.buildingsmart.org/#concept/details/1zlbN6A$z4r8Er6nWNbSMZ</rdfs:comment>
        <rdfs:label xml:lang="de-de">Bewehrungsstab</rdfs:label>
        <rdfs:label xml:lang="en">Reinforcing Bar</rdfs:label>
        <rdfs:label xml:lang="nb-no">armeringsstang</rdfs:label>
        <rdfs:label xml:lang="fr-fr">barre d&apos;armature</rdfs:label>
        <rdfs:seeAlso rdf:resource="http://www.buildingsmart-tech.org/ifcOWL/IFC4_ADD2#IfcReinforcingBar"/>
    </owl:Class>
    


    <!-- https://pi.pauwel.be/voc/buildingelement#ReinforcingBar-ANCHORING -->

    <owl:Class rdf:about="https://pi.pauwel.be/voc/buildingelement#ReinforcingBar-ANCHORING">
        <rdfs:subClassOf rdf:resource="https://pi.pauwel.be/voc/buildingelement#ReinforcingBar"/>
        <rdfs:comment xml:lang="en">http://bsdd.buildingsmart.org/#concept/details/3X1mNZzk542ez6g92TTVdH</rdfs:comment>
        <rdfs:label xml:lang="en">Anchoring</rdfs:label>
        <rdfs:seeAlso rdf:resource="http://www.buildingsmart-tech.org/ifcOWL/IFC4_ADD2#IfcReinforcingBarEnumType"/>
    </owl:Class>
    


    <!-- https://pi.pauwel.be/voc/buildingelement#ReinforcingBar-EDGE -->

    <owl:Class rdf:about="https://pi.pauwel.be/voc/buildingelement#ReinforcingBar-EDGE">
        <rdfs:subClassOf rdf:resource="https://pi.pauwel.be/voc/buildingelement#ReinforcingBar"/>
        <rdfs:comment xml:lang="en">http://bsdd.buildingsmart.org/#concept/details/0tRGNh1sv19OvGghikeGYQ</rdfs:comment>
        <rdfs:label xml:lang="en">Edge</rdfs:label>
        <rdfs:seeAlso rdf:resource="http://www.buildingsmart-tech.org/ifcOWL/IFC4_ADD2#IfcReinforcingBarEnumType"/>
    </owl:Class>
    


    <!-- https://pi.pauwel.be/voc/buildingelement#ReinforcingBar-LIGATURE -->

    <owl:Class rdf:about="https://pi.pauwel.be/voc/buildingelement#ReinforcingBar-LIGATURE">
        <rdfs:subClassOf rdf:resource="https://pi.pauwel.be/voc/buildingelement#ReinforcingBar"/>
        <rdfs:comment xml:lang="en">http://bsdd.buildingsmart.org/#concept/details/09DzOB3qT10AwjdzYLo1LA</rdfs:comment>
        <rdfs:label xml:lang="en">Ligature</rdfs:label>
        <rdfs:seeAlso rdf:resource="http://www.buildingsmart-tech.org/ifcOWL/IFC4_ADD2#IfcReinforcingBarEnumType"/>
    </owl:Class>
    


    <!-- https://pi.pauwel.be/voc/buildingelement#ReinforcingBar-MAIN -->

    <owl:Class rdf:about="https://pi.pauwel.be/voc/buildingelement#ReinforcingBar-MAIN">
        <rdfs:subClassOf rdf:resource="https://pi.pauwel.be/voc/buildingelement#ReinforcingBar"/>
        <rdfs:comment xml:lang="en">http://bsdd.buildingsmart.org/#concept/details/0ZDnwDkMT9fhTxjjLnIpAX</rdfs:comment>
        <rdfs:label xml:lang="en">Main</rdfs:label>
        <rdfs:seeAlso rdf:resource="http://www.buildingsmart-tech.org/ifcOWL/IFC4_ADD2#IfcReinforcingBarEnumType"/>
    </owl:Class>
    


    <!-- https://pi.pauwel.be/voc/buildingelement#ReinforcingBar-PUNCHING -->

    <owl:Class rdf:about="https://pi.pauwel.be/voc/buildingelement#ReinforcingBar-PUNCHING">
        <rdfs:subClassOf rdf:resource="https://pi.pauwel.be/voc/buildingelement#ReinforcingBar"/>
        <rdfs:comment xml:lang="en">http://bsdd.buildingsmart.org/#concept/details/1RO$_IvNP7eQABna$VzMm_</rdfs:comment>
        <rdfs:label xml:lang="en">Punching</rdfs:label>
        <rdfs:seeAlso rdf:resource="http://www.buildingsmart-tech.org/ifcOWL/IFC4_ADD2#IfcReinforcingBarEnumType"/>
    </owl:Class>
    


    <!-- https://pi.pauwel.be/voc/buildingelement#ReinforcingBar-RING -->

    <owl:Class rdf:about="https://pi.pauwel.be/voc/buildingelement#ReinforcingBar-RING">
        <rdfs:subClassOf rdf:resource="https://pi.pauwel.be/voc/buildingelement#ReinforcingBar"/>
        <rdfs:comment xml:lang="en">http://bsdd.buildingsmart.org/#concept/details/2zA8DFnW5B8hiBjIlXcktx</rdfs:comment>
        <rdfs:label xml:lang="en">Ring</rdfs:label>
        <rdfs:seeAlso rdf:resource="http://www.buildingsmart-tech.org/ifcOWL/IFC4_ADD2#IfcReinforcingBarEnumType"/>
    </owl:Class>
    


    <!-- https://pi.pauwel.be/voc/buildingelement#ReinforcingBar-SHEAR -->

    <owl:Class rdf:about="https://pi.pauwel.be/voc/buildingelement#ReinforcingBar-SHEAR">
        <rdfs:subClassOf rdf:resource="https://pi.pauwel.be/voc/buildingelement#ReinforcingBar"/>
        <rdfs:comment xml:lang="en">http://bsdd.buildingsmart.org/#concept/details/220Wv8D4n11hjTIo_DzfBR</rdfs:comment>
        <rdfs:label xml:lang="en">Shear</rdfs:label>
        <rdfs:label xml:lang="nb-no">skive</rdfs:label>
        <rdfs:seeAlso rdf:resource="http://www.buildingsmart-tech.org/ifcOWL/IFC4_ADD2#IfcReinforcingBarEnumType"/>
    </owl:Class>
    


    <!-- https://pi.pauwel.be/voc/buildingelement#ReinforcingBar-STUD -->

    <owl:Class rdf:about="https://pi.pauwel.be/voc/buildingelement#ReinforcingBar-STUD">
        <rdfs:subClassOf rdf:resource="https://pi.pauwel.be/voc/buildingelement#ReinforcingBar"/>
        <rdfs:comment xml:lang="en">http://bsdd.buildingsmart.org/#concept/details/3cWXnrQEvAfRCh9LjK26$R</rdfs:comment>
        <rdfs:label xml:lang="en">Stud</rdfs:label>
        <rdfs:label xml:lang="nb-no">stender</rdfs:label>
        <rdfs:seeAlso rdf:resource="http://www.buildingsmart-tech.org/ifcOWL/IFC4_ADD2#IfcReinforcingBarEnumType"/>
    </owl:Class>
    


    <!-- https://pi.pauwel.be/voc/buildingelement#ReinforcingElement -->

    <owl:Class rdf:about="https://pi.pauwel.be/voc/buildingelement#ReinforcingElement">
        <rdfs:subClassOf rdf:resource="https://pi.pauwel.be/voc/buildingelement#ElementComponent"/>
        <rdfs:comment xml:lang="en">a reinforcing element represents bars, wires, strands, meshes, tendons, and other components embedded in concrete in such a manner that the reinforcement and the concrete act together in resisting forces.</rdfs:comment>
        <rdfs:comment xml:lang="en">http://bsdd.buildingsmart.org/#concept/details/1aiY$$Wf98m8a5cp3Hzgdu</rdfs:comment>
        <rdfs:label xml:lang="de-de">Bewehrung</rdfs:label>
        <rdfs:label xml:lang="en">Reinforcing Element</rdfs:label>
        <rdfs:label xml:lang="fr-fr">elément d&apos;armature</rdfs:label>
        <rdfs:seeAlso rdf:resource="http://www.buildingsmart-tech.org/ifcOWL/IFC4_ADD2#IfcReinforcingElement"/>
    </owl:Class>
    


    <!-- https://pi.pauwel.be/voc/buildingelement#ReinforcingMesh -->

    <owl:Class rdf:about="https://pi.pauwel.be/voc/buildingelement#ReinforcingMesh">
        <rdfs:subClassOf rdf:resource="https://pi.pauwel.be/voc/buildingelement#ReinforcingElement"/>
        <rdfs:comment xml:lang="en">a reinforcing mesh is a series of longitudinal and transverse wires or bars of various gauges, arranged at right angles to each other and welded at all points of intersection; usually used for concrete slab reinforcement. it is also known as welded wire fabric. in scope are plane meshes as well as bent meshes.</rdfs:comment>
        <rdfs:comment xml:lang="en">http://bsdd.buildingsmart.org/#concept/details/3R4n2h6wn67Q4clocrGT7J</rdfs:comment>
        <rdfs:label xml:lang="de-de">Bewehrungsmatte</rdfs:label>
        <rdfs:label xml:lang="en">Reinforcing Mesh</rdfs:label>
        <rdfs:label xml:lang="fr-fr">treillis</rdfs:label>
        <rdfs:seeAlso rdf:resource="http://www.buildingsmart-tech.org/ifcOWL/IFC4_ADD2#IfcReinforcingMesh"/>
    </owl:Class>
    


    <!-- https://pi.pauwel.be/voc/buildingelement#Roof -->

    <owl:Class rdf:about="https://pi.pauwel.be/voc/buildingelement#Roof">
        <rdfs:subClassOf rdf:resource="https://pi.pauwel.be/voc/buildingelement#BuildingElement"/>
        <rdfs:comment xml:lang="en">A covering of the top part of a building. Protects the building against the effects of weather.</rdfs:comment>
        <rdfs:comment xml:lang="en">http://bsdd.buildingsmart.org/#concept/details/2Iyg00qW4HuO00025QrE$V</rdfs:comment>
        <rdfs:label xml:lang="de-de">Dach</rdfs:label>
        <rdfs:label xml:lang="nl">Dak</rdfs:label>
        <rdfs:label xml:lang="en">Roof</rdfs:label>
        <rdfs:label xml:lang="da">Tag</rdfs:label>
        <rdfs:label xml:lang="fr-fr">toiture</rdfs:label>
        <rdfs:seeAlso rdf:resource="http://www.buildingsmart-tech.org/ifcOWL/IFC4_ADD2#IfcRoof"/>
    </owl:Class>
    


    <!-- https://pi.pauwel.be/voc/buildingelement#Roof-BARREL_ROOF -->

    <owl:Class rdf:about="https://pi.pauwel.be/voc/buildingelement#Roof-BARREL_ROOF">
        <rdfs:subClassOf rdf:resource="https://pi.pauwel.be/voc/buildingelement#Roof"/>
        <rdfs:comment xml:lang="en">http://bsdd.buildingsmart.org/#concept/details/172RLdein1b8WIbTtDLVbc</rdfs:comment>
        <rdfs:label xml:lang="en">Barrel Roof</rdfs:label>
        <rdfs:seeAlso rdf:resource="http://www.buildingsmart-tech.org/ifcOWL/IFC4_ADD2#IfcRoofEnumType"/>
    </owl:Class>
    


    <!-- https://pi.pauwel.be/voc/buildingelement#Roof-BUTTERFLY_ROOF -->

    <owl:Class rdf:about="https://pi.pauwel.be/voc/buildingelement#Roof-BUTTERFLY_ROOF">
        <rdfs:subClassOf rdf:resource="https://pi.pauwel.be/voc/buildingelement#Roof"/>
        <rdfs:comment xml:lang="en">http://bsdd.buildingsmart.org/#concept/details/2W6yLK2r968h2TWfGC2xWu</rdfs:comment>
        <rdfs:label xml:lang="en">Butterfly Roof</rdfs:label>
        <rdfs:seeAlso rdf:resource="http://www.buildingsmart-tech.org/ifcOWL/IFC4_ADD2#IfcRoofEnumType"/>
    </owl:Class>
    


    <!-- https://pi.pauwel.be/voc/buildingelement#Roof-DOME_ROOF -->

    <owl:Class rdf:about="https://pi.pauwel.be/voc/buildingelement#Roof-DOME_ROOF">
        <rdfs:subClassOf rdf:resource="https://pi.pauwel.be/voc/buildingelement#Roof"/>
        <rdfs:comment xml:lang="en">http://bsdd.buildingsmart.org/#concept/details/3UcE2aJPP4ewOoRn29unfZ</rdfs:comment>
        <rdfs:label xml:lang="en">Dome Roof</rdfs:label>
        <rdfs:label xml:lang="nb-no">kuppeltak</rdfs:label>
        <rdfs:seeAlso rdf:resource="http://www.buildingsmart-tech.org/ifcOWL/IFC4_ADD2#IfcRoofEnumType"/>
    </owl:Class>
    


    <!-- https://pi.pauwel.be/voc/buildingelement#Roof-FLAT_ROOF -->

    <owl:Class rdf:about="https://pi.pauwel.be/voc/buildingelement#Roof-FLAT_ROOF">
        <rdfs:subClassOf rdf:resource="https://pi.pauwel.be/voc/buildingelement#Roof"/>
        <rdfs:comment xml:lang="en">http://bsdd.buildingsmart.org/#concept/details/3IeKrtrMz2SQN7qpJt82e5</rdfs:comment>
        <rdfs:label xml:lang="en">Flat Roof</rdfs:label>
        <rdfs:label xml:lang="nb-no">flatt tak</rdfs:label>
        <rdfs:seeAlso rdf:resource="http://www.buildingsmart-tech.org/ifcOWL/IFC4_ADD2#IfcRoofEnumType"/>
    </owl:Class>
    


    <!-- https://pi.pauwel.be/voc/buildingelement#Roof-FREEFORM -->

    <owl:Class rdf:about="https://pi.pauwel.be/voc/buildingelement#Roof-FREEFORM">
        <rdfs:subClassOf rdf:resource="https://pi.pauwel.be/voc/buildingelement#Roof"/>
        <rdfs:comment xml:lang="en">http://bsdd.buildingsmart.org/#concept/details/2KVHvK7iXAEfKlD5hGIFEc</rdfs:comment>
        <rdfs:label xml:lang="en">Free Form Roof</rdfs:label>
        <rdfs:label xml:lang="nb-no">friform tak</rdfs:label>
        <rdfs:seeAlso rdf:resource="http://www.buildingsmart-tech.org/ifcOWL/IFC4_ADD2#IfcRoofEnumType"/>
    </owl:Class>
    


    <!-- https://pi.pauwel.be/voc/buildingelement#Roof-GABLE_ROOF -->

    <owl:Class rdf:about="https://pi.pauwel.be/voc/buildingelement#Roof-GABLE_ROOF">
        <rdfs:subClassOf rdf:resource="https://pi.pauwel.be/voc/buildingelement#Roof"/>
        <rdfs:comment xml:lang="en">http://bsdd.buildingsmart.org/#concept/details/0gHJNRNhz6LOTHVbnW$nEj</rdfs:comment>
        <rdfs:label xml:lang="en">Gable Roof</rdfs:label>
        <rdfs:label xml:lang="nb-no">gavl</rdfs:label>
        <rdfs:seeAlso rdf:resource="http://www.buildingsmart-tech.org/ifcOWL/IFC4_ADD2#IfcRoofEnumType"/>
    </owl:Class>
    


    <!-- https://pi.pauwel.be/voc/buildingelement#Roof-GAMBREL_ROOF -->

    <owl:Class rdf:about="https://pi.pauwel.be/voc/buildingelement#Roof-GAMBREL_ROOF">
        <rdfs:subClassOf rdf:resource="https://pi.pauwel.be/voc/buildingelement#Roof"/>
        <rdfs:comment xml:lang="en">http://bsdd.buildingsmart.org/#concept/details/2BnDhKP1HF3vXxnwqccewa</rdfs:comment>
        <rdfs:label xml:lang="en">Gambrel Roof</rdfs:label>
        <rdfs:label xml:lang="nb-no">gambrel tak</rdfs:label>
        <rdfs:seeAlso rdf:resource="http://www.buildingsmart-tech.org/ifcOWL/IFC4_ADD2#IfcRoofEnumType"/>
    </owl:Class>
    


    <!-- https://pi.pauwel.be/voc/buildingelement#Roof-HIPPED_GABLE_ROOF -->

    <owl:Class rdf:about="https://pi.pauwel.be/voc/buildingelement#Roof-HIPPED_GABLE_ROOF">
        <rdfs:subClassOf rdf:resource="https://pi.pauwel.be/voc/buildingelement#Roof"/>
        <rdfs:comment xml:lang="en">http://bsdd.buildingsmart.org/#concept/details/3Su_2ncLX1Oes0r3fNr4uE</rdfs:comment>
        <rdfs:label xml:lang="en">Hipped Gable Roof</rdfs:label>
        <rdfs:label xml:lang="nb-no">valm/saltak</rdfs:label>
        <rdfs:seeAlso rdf:resource="http://www.buildingsmart-tech.org/ifcOWL/IFC4_ADD2#IfcRoofEnumType"/>
    </owl:Class>
    


    <!-- https://pi.pauwel.be/voc/buildingelement#Roof-HIP_ROOF -->

    <owl:Class rdf:about="https://pi.pauwel.be/voc/buildingelement#Roof-HIP_ROOF">
        <rdfs:subClassOf rdf:resource="https://pi.pauwel.be/voc/buildingelement#Roof"/>
        <rdfs:comment xml:lang="en">http://bsdd.buildingsmart.org/#concept/details/0waejMcyT3zwP6nRClvfSx</rdfs:comment>
        <rdfs:label xml:lang="en">Hip Roof</rdfs:label>
        <rdfs:label xml:lang="nb-no">valmtak</rdfs:label>
        <rdfs:seeAlso rdf:resource="http://www.buildingsmart-tech.org/ifcOWL/IFC4_ADD2#IfcRoofEnumType"/>
    </owl:Class>
    


    <!-- https://pi.pauwel.be/voc/buildingelement#Roof-MANSARD_ROOF -->

    <owl:Class rdf:about="https://pi.pauwel.be/voc/buildingelement#Roof-MANSARD_ROOF">
        <rdfs:subClassOf rdf:resource="https://pi.pauwel.be/voc/buildingelement#Roof"/>
        <rdfs:comment xml:lang="en">http://bsdd.buildingsmart.org/#concept/details/1hB_MPg3j35vRsm_vutjD2</rdfs:comment>
        <rdfs:label xml:lang="en">Mansard Roof</rdfs:label>
        <rdfs:label xml:lang="nb-no">mansardtak</rdfs:label>
        <rdfs:seeAlso rdf:resource="http://www.buildingsmart-tech.org/ifcOWL/IFC4_ADD2#IfcRoofEnumType"/>
    </owl:Class>
    


    <!-- https://pi.pauwel.be/voc/buildingelement#Roof-PAVILION_ROOF -->

    <owl:Class rdf:about="https://pi.pauwel.be/voc/buildingelement#Roof-PAVILION_ROOF">
        <rdfs:subClassOf rdf:resource="https://pi.pauwel.be/voc/buildingelement#Roof"/>
        <rdfs:comment xml:lang="en">http://bsdd.buildingsmart.org/#concept/details/11Ltv09Eb7lRJW184fZ9gF</rdfs:comment>
        <rdfs:label xml:lang="en">Pavilion Roof</rdfs:label>
        <rdfs:label xml:lang="nb-no">paviljongtak</rdfs:label>
        <rdfs:seeAlso rdf:resource="http://www.buildingsmart-tech.org/ifcOWL/IFC4_ADD2#IfcRoofEnumType"/>
    </owl:Class>
    


    <!-- https://pi.pauwel.be/voc/buildingelement#Roof-RAINBOW_ROOF -->

    <owl:Class rdf:about="https://pi.pauwel.be/voc/buildingelement#Roof-RAINBOW_ROOF">
        <rdfs:subClassOf rdf:resource="https://pi.pauwel.be/voc/buildingelement#Roof"/>
        <rdfs:comment xml:lang="en">http://bsdd.buildingsmart.org/#concept/details/1MnaPoqUb0L8PGqS6yHzbq</rdfs:comment>
        <rdfs:label xml:lang="en">Rainbow Roof</rdfs:label>
        <rdfs:label xml:lang="nb-no">buetak</rdfs:label>
        <rdfs:seeAlso rdf:resource="http://www.buildingsmart-tech.org/ifcOWL/IFC4_ADD2#IfcRoofEnumType"/>
    </owl:Class>
    


    <!-- https://pi.pauwel.be/voc/buildingelement#Roof-SHED_ROOF -->

    <owl:Class rdf:about="https://pi.pauwel.be/voc/buildingelement#Roof-SHED_ROOF">
        <rdfs:subClassOf rdf:resource="https://pi.pauwel.be/voc/buildingelement#Roof"/>
        <rdfs:comment xml:lang="en">http://bsdd.buildingsmart.org/#concept/details/3GsCyHvinDMPWmecHluOEq</rdfs:comment>
        <rdfs:label xml:lang="en">Shed Roof</rdfs:label>
        <rdfs:label xml:lang="nb-no">pulttak</rdfs:label>
        <rdfs:seeAlso rdf:resource="http://www.buildingsmart-tech.org/ifcOWL/IFC4_ADD2#IfcRoofEnumType"/>
    </owl:Class>
    


    <!-- https://pi.pauwel.be/voc/buildingelement#ShadingDevice -->

    <owl:Class rdf:about="https://pi.pauwel.be/voc/buildingelement#ShadingDevice">
        <rdfs:subClassOf rdf:resource="https://pi.pauwel.be/voc/buildingelement#BuildingElement"/>
        <rdfs:comment xml:lang="en">Purpose built devices to protect from the sunlight, from natural light, or screening them from view. Shading devices can form part of the facade or can be mounted inside the building, they can be fixed or operable.
</rdfs:comment>
        <rdfs:comment xml:lang="en">http://bsdd.buildingsmart.org/#concept/details/11vQg0qWSHuO00025QrE$V</rdfs:comment>
        <rdfs:label xml:lang="da">Afskærmningsanordning</rdfs:label>
        <rdfs:label xml:lang="en">Shading Device</rdfs:label>
        <rdfs:label xml:lang="de-de">Sonnenschutz festeingebaut</rdfs:label>
        <rdfs:label xml:lang="nl">Zonnewering</rdfs:label>
        <rdfs:label xml:lang="fr-fr">protection solaire</rdfs:label>
        <rdfs:label xml:lang="nb-no">skjermingstype</rdfs:label>
        <rdfs:seeAlso rdf:resource="http://www.buildingsmart-tech.org/ifcOWL/IFC4_ADD2#IfcShadingDevice"/>
    </owl:Class>
    


    <!-- https://pi.pauwel.be/voc/buildingelement#ShadingDevice-AWNING -->

    <owl:Class rdf:about="https://pi.pauwel.be/voc/buildingelement#ShadingDevice-AWNING">
        <rdfs:subClassOf rdf:resource="https://pi.pauwel.be/voc/buildingelement#ShadingDevice"/>
        <rdfs:comment xml:lang="en">a rooflike shelter of canvas or other material extending over a doorway, from the top of a window, over a deck, etc., in order to provide protection, as from the sun</rdfs:comment>
        <rdfs:comment xml:lang="en">http://bsdd.buildingsmart.org/#concept/details/3NoPxSKmL7yQEzPT8cmssT</rdfs:comment>
        <rdfs:comment xml:lang="en">product made of fabric/material, located externally, above, in front of, or within an opening and extending in a horizontal and/or sloping and/or vertical plane</rdfs:comment>
        <rdfs:comment xml:lang="nb-no">produkt laget av stoff/materiale som plasseres utvendig over, foran eller i en åpning, og som stikker ut i et horisontalt og/eller skrånende og/eller vertikalt plan</rdfs:comment>
        <rdfs:label xml:lang="en">Awning</rdfs:label>
        <rdfs:label xml:lang="nl-nl">Zonwering</rdfs:label>
        <rdfs:label xml:lang="nb-no">markise</rdfs:label>
        <rdfs:label xml:lang="nb-no">solskjerming</rdfs:label>
    </owl:Class>
    


    <!-- https://pi.pauwel.be/voc/buildingelement#ShadingDevice-JALOUSIE -->

    <owl:Class rdf:about="https://pi.pauwel.be/voc/buildingelement#ShadingDevice-JALOUSIE">
        <rdfs:subClassOf rdf:resource="https://pi.pauwel.be/voc/buildingelement#ShadingDevice"/>
        <rdfs:comment xml:lang="nb-no">Solavskjerming, Persienner</rdfs:comment>
        <rdfs:comment xml:lang="en">http://bsdd.buildingsmart.org/#concept/details/1$w9Dw6W9DJvD2GfuZFMSR</rdfs:comment>
        <rdfs:comment xml:lang="en">http://bsdd.buildingsmart.org/#concept/details/3vHLsWoT0Hsm00051Mm008</rdfs:comment>
        <rdfs:comment xml:lang="en">product consisting of horizontal slats which can be tilted. it may be retracted by raising and stacking the slats.</rdfs:comment>
        <rdfs:label xml:lang="de-de">Jalousie</rdfs:label>
        <rdfs:label xml:lang="en">Jalousie</rdfs:label>
        <rdfs:label xml:lang="en">blinds</rdfs:label>
        <rdfs:label xml:lang="nb-no">lamell</rdfs:label>
        <rdfs:label xml:lang="nb-no">persienne</rdfs:label>
        <rdfs:label xml:lang="nb-no">persienner</rdfs:label>
        <rdfs:label xml:lang="nb-no">sjalusi</rdfs:label>
        <rdfs:label xml:lang="fr-fr">stores vénetiens</rdfs:label>
        <rdfs:label xml:lang="en">sun shading device</rdfs:label>
        <rdfs:label xml:lang="en">venetian blind</rdfs:label>
        <rdfs:seeAlso rdf:resource="http://www.buildingsmart-tech.org/ifcOWL/IFC4_ADD2#IfcShadingDeviceEnumType"/>
    </owl:Class>
    


    <!-- https://pi.pauwel.be/voc/buildingelement#ShadingDevice-SHUTTER -->

    <owl:Class rdf:about="https://pi.pauwel.be/voc/buildingelement#ShadingDevice-SHUTTER">
        <rdfs:subClassOf rdf:resource="https://pi.pauwel.be/voc/buildingelement#ShadingDevice"/>
        <rdfs:comment xml:lang="en">An artefact which is a part of an assembly that can be moved from a position where it permits contact, to a position where it becomes a part of the enclosure or partition shielding the fixed contacts.                </rdfs:comment>
        <rdfs:comment xml:lang="en">Movable component installed in an opening or duct to form a barrier for security purposes; used to control the passage of heat or light or to delay the spread of fire, smoke or gases.</rdfs:comment>
        <rdfs:comment xml:lang="nb-no">Solavskjerming, Solgardin</rdfs:comment>
        <rdfs:comment xml:lang="en">Sun-shading device</rdfs:comment>
        <rdfs:comment xml:lang="en">http://bsdd.buildingsmart.org/#concept/details/0w_lVI8P10c9rjT$RsNEVr</rdfs:comment>
        <rdfs:comment xml:lang="en">http://bsdd.buildingsmart.org/#concept/details/27f2fkTV50YwB1IZgMURLa</rdfs:comment>
        <rdfs:comment xml:lang="en">http://bsdd.buildingsmart.org/#concept/details/3vHUzKoT0Hsm00051Mm008</rdfs:comment>
        <rdfs:comment xml:lang="en">product installed either internally or externally to provide additional covering and/or protection to an opening</rdfs:comment>
        <rdfs:label xml:lang="de-de">Abschluß</rdfs:label>
        <rdfs:label xml:lang="en">Shutter</rdfs:label>
        <rdfs:label xml:lang="fr-fr">fermeture</rdfs:label>
        <rdfs:label xml:lang="nb-no">markise</rdfs:label>
        <rdfs:label xml:lang="nb-no">skodde</rdfs:label>
        <rdfs:label xml:lang="nb-no">solgardin</rdfs:label>
        <rdfs:seeAlso rdf:resource="http://www.buildingsmart-tech.org/ifcOWL/IFC4_ADD2#IfcShadingDeviceEnumType"/>
    </owl:Class>
    


    <!-- https://pi.pauwel.be/voc/buildingelement#Slab -->

    <owl:Class rdf:about="https://pi.pauwel.be/voc/buildingelement#Slab">
        <rdfs:subClassOf rdf:resource="https://pi.pauwel.be/voc/buildingelement#BuildingElement"/>
        <rdfs:comment xml:lang="en">A component of the construction that normally encloses a space vertically. May provide the lower support (floor) or upper construction (roof slab) in any space in a building.
Only the core or constructional part of this construction is considered to be a slab. The upper finish (flooring, roofing) and the lower finish (ceiling, suspended ceiling) are considered to be coverings. </rdfs:comment>
        <rdfs:comment xml:lang="en">http://bsdd.buildingsmart.org/#concept/details/3pXDk0qWSHuO00025QrE$V</rdfs:comment>
        <rdfs:label xml:lang="de-de">Decke / Dachfläche / Bodenplatte</rdfs:label>
        <rdfs:label xml:lang="da">Dæk</rdfs:label>
        <rdfs:label xml:lang="nl">Plaat</rdfs:label>
        <rdfs:label xml:lang="en">Slab</rdfs:label>
        <rdfs:label xml:lang="fr-fr">dalle</rdfs:label>
        <rdfs:label xml:lang="nb-no">dekke</rdfs:label>
        <rdfs:seeAlso rdf:resource="http://www.buildingsmart-tech.org/ifcOWL/IFC4_ADD2#IfcSlab"/>
    </owl:Class>
    


    <!-- https://pi.pauwel.be/voc/buildingelement#Slab-BASESLAB -->

    <owl:Class rdf:about="https://pi.pauwel.be/voc/buildingelement#Slab-BASESLAB">
        <rdfs:subClassOf rdf:resource="https://pi.pauwel.be/voc/buildingelement#Slab"/>
        <rdfs:comment xml:lang="en">http://bsdd.buildingsmart.org/#concept/details/1hBroEIeL9neS3mSSGZiyC</rdfs:comment>
        <rdfs:label>Base Slab</rdfs:label>
        <rdfs:label xml:lang="nb-no">støpt fundament</rdfs:label>
        <rdfs:seeAlso rdf:resource="http://www.buildingsmart-tech.org/ifcOWL/IFC4_ADD2#IfcSlabEnumType"/>
    </owl:Class>
    


    <!-- https://pi.pauwel.be/voc/buildingelement#Slab-FLOOR -->

    <owl:Class rdf:about="https://pi.pauwel.be/voc/buildingelement#Slab-FLOOR">
        <rdfs:subClassOf rdf:resource="https://pi.pauwel.be/voc/buildingelement#Slab"/>
        <rdfs:comment xml:lang="en">http://bsdd.buildingsmart.org/#concept/details/0jBALpJIv7vvlWkbd9HdCx</rdfs:comment>
        <rdfs:label xml:lang="en">Floor</rdfs:label>
        <rdfs:label xml:lang="nb-no">dekke</rdfs:label>
        <rdfs:label xml:lang="nb-no">gulv</rdfs:label>
        <rdfs:seeAlso rdf:resource="http://www.buildingsmart-tech.org/ifcOWL/IFC4_ADD2#IfcSlabEnumType"/>
    </owl:Class>
    


    <!-- https://pi.pauwel.be/voc/buildingelement#Slab-LANDING -->

    <owl:Class rdf:about="https://pi.pauwel.be/voc/buildingelement#Slab-LANDING">
        <rdfs:subClassOf rdf:resource="https://pi.pauwel.be/voc/buildingelement#Slab"/>
        <rdfs:comment xml:lang="en">http://bsdd.buildingsmart.org/#concept/details/3tQbZvvrfA8OUjU1kc2rUZ</rdfs:comment>
        <rdfs:label xml:lang="en">Landing</rdfs:label>
        <rdfs:label xml:lang="nb-no">repo</rdfs:label>
        <rdfs:seeAlso rdf:resource="http://www.buildingsmart-tech.org/ifcOWL/IFC4_ADD2#IfcSlabEnumType"/>
    </owl:Class>
    


    <!-- https://pi.pauwel.be/voc/buildingelement#Slab-ROOF -->

    <owl:Class rdf:about="https://pi.pauwel.be/voc/buildingelement#Slab-ROOF">
        <rdfs:subClassOf rdf:resource="https://pi.pauwel.be/voc/buildingelement#Slab"/>
        <rdfs:comment xml:lang="en">A covering of the top part of a building. Protects the building against the effects of weather.</rdfs:comment>
        <rdfs:comment xml:lang="en">http://bsdd.buildingsmart.org/#concept/details/3Hvwx39_rCaRS49F4qRGBb</rdfs:comment>
        <rdfs:label xml:lang="de-de">Dach</rdfs:label>
        <rdfs:label xml:lang="en">Roof</rdfs:label>
        <rdfs:label xml:lang="nb-no">flatt tak</rdfs:label>
        <rdfs:label xml:lang="fr-fr">toiture</rdfs:label>
        <rdfs:seeAlso rdf:resource="http://www.buildingsmart-tech.org/ifcOWL/IFC4_ADD2#IfcSlabEnumType"/>
    </owl:Class>
    


    <!-- https://pi.pauwel.be/voc/buildingelement#Stair -->

    <owl:Class rdf:about="https://pi.pauwel.be/voc/buildingelement#Stair">
        <rdfs:subClassOf rdf:resource="https://pi.pauwel.be/voc/buildingelement#BuildingElement"/>
        <rdfs:comment xml:lang="en">A vertical passageway allowing occupants to walk (step) from one floor level to another floor level at a different elevation. May include a landing as an intermediate floor slab.</rdfs:comment>
        <rdfs:comment xml:lang="en">http://bsdd.buildingsmart.org/#concept/details/3DhWM0qWmHuO00025QrE$V</rdfs:comment>
        <rdfs:label xml:lang="en">Stair</rdfs:label>
        <rdfs:label xml:lang="nl">Trap</rdfs:label>
        <rdfs:label xml:lang="nl-nl">Trap</rdfs:label>
        <rdfs:label xml:lang="da">Trappe</rdfs:label>
        <rdfs:label xml:lang="nl-nl">Trapslag</rdfs:label>
        <rdfs:label xml:lang="de-de">Treppe</rdfs:label>
        <rdfs:label xml:lang="fr-fr">escalier</rdfs:label>
        <rdfs:label xml:lang="nb-no">trapp</rdfs:label>
        <rdfs:seeAlso rdf:resource="http://www.buildingsmart-tech.org/ifcOWL/IFC4_ADD2#IfcStair"/>
    </owl:Class>
    


    <!-- https://pi.pauwel.be/voc/buildingelement#Stair-CURVED_RUN_STAIR -->

    <owl:Class rdf:about="https://pi.pauwel.be/voc/buildingelement#Stair-CURVED_RUN_STAIR">
        <rdfs:subClassOf rdf:resource="https://pi.pauwel.be/voc/buildingelement#Stair"/>
        <rdfs:comment xml:lang="en">a stair extending from one level to another without turns or winders. the stair is consisting of one curved flight.</rdfs:comment>
        <rdfs:comment xml:lang="en">http://bsdd.buildingsmart.org/#concept/details/1lkxIX8Gj23Bi50H2qpZB9</rdfs:comment>
        <rdfs:label xml:lang="en">Curved Run Stair</rdfs:label>
        <rdfs:seeAlso rdf:resource="http://www.buildingsmart-tech.org/ifcOWL/IFC4_ADD2#IfcStairEnumType"/>
    </owl:Class>
    


    <!-- https://pi.pauwel.be/voc/buildingelement#Stair-DOUBLE_RETURN_STAIR -->

    <owl:Class rdf:about="https://pi.pauwel.be/voc/buildingelement#Stair-DOUBLE_RETURN_STAIR">
        <rdfs:subClassOf rdf:resource="https://pi.pauwel.be/voc/buildingelement#Stair"/>
        <rdfs:comment xml:lang="en">a stair having one straight flight to a wide quarterspace landing, and two side flights from that landing into opposite directions. the stair is making a 90° turn. the direction of traffic is determined by the walking line.</rdfs:comment>
        <rdfs:comment xml:lang="en">http://bsdd.buildingsmart.org/#concept/details/3NNCQTceL7Uf8ZhJf40gs9</rdfs:comment>
        <rdfs:label xml:lang="en">Double Return Stair</rdfs:label>
        <rdfs:seeAlso rdf:resource="http://www.buildingsmart-tech.org/ifcOWL/IFC4_ADD2#IfcStairEnumType"/>
    </owl:Class>
    


    <!-- https://pi.pauwel.be/voc/buildingelement#Stair-HALF_TURN_STAIR -->

    <owl:Class rdf:about="https://pi.pauwel.be/voc/buildingelement#Stair-HALF_TURN_STAIR">
        <rdfs:subClassOf rdf:resource="https://pi.pauwel.be/voc/buildingelement#Stair"/>
        <rdfs:comment xml:lang="en">a stair making a 180° turn, consisting of two straight flights connected by a halfspace landing. the orientation of the turn is determined by the walking line.</rdfs:comment>
        <rdfs:comment xml:lang="en">http://bsdd.buildingsmart.org/#concept/details/3YmaH1onP90PM6kEWHUjFv</rdfs:comment>
        <rdfs:label xml:lang="en">Half Turn Stair</rdfs:label>
        <rdfs:seeAlso rdf:resource="http://www.buildingsmart-tech.org/ifcOWL/IFC4_ADD2#IfcStairEnumType"/>
    </owl:Class>
    


    <!-- https://pi.pauwel.be/voc/buildingelement#Stair-HALF_WINDING_STAIR -->

    <owl:Class rdf:about="https://pi.pauwel.be/voc/buildingelement#Stair-HALF_WINDING_STAIR">
        <rdfs:subClassOf rdf:resource="https://pi.pauwel.be/voc/buildingelement#Stair"/>
        <rdfs:comment xml:lang="en">http://bsdd.buildingsmart.org/#concept/details/0Vw081Hfz1AQne1V5CsfUA</rdfs:comment>
        <rdfs:label xml:lang="en">Half Winding Stair</rdfs:label>
        <rdfs:seeAlso rdf:resource="http://www.buildingsmart-tech.org/ifcOWL/IFC4_ADD2#IfcStairEnumType"/>
    </owl:Class>
    


    <!-- https://pi.pauwel.be/voc/buildingelement#Stair-QUARTER_TURN_STAIR -->

    <owl:Class rdf:about="https://pi.pauwel.be/voc/buildingelement#Stair-QUARTER_TURN_STAIR">
        <rdfs:subClassOf rdf:resource="https://pi.pauwel.be/voc/buildingelement#Stair"/>
        <rdfs:comment xml:lang="en">a stair making a 90° turn, consisting of two straight flights connected by a quarterspace landing. the direction of the turn is determined by the walking line.</rdfs:comment>
        <rdfs:comment xml:lang="en">http://bsdd.buildingsmart.org/#concept/details/1IEbbDJDHAFQb9SZweXH3x</rdfs:comment>
        <rdfs:label xml:lang="en">Quarter Turn Stair</rdfs:label>
        <rdfs:seeAlso rdf:resource="http://www.buildingsmart-tech.org/ifcOWL/IFC4_ADD2#IfcStairEnumType"/>
    </owl:Class>
    


    <!-- https://pi.pauwel.be/voc/buildingelement#Stair-QUARTER_WINDING_STAIR -->

    <owl:Class rdf:about="https://pi.pauwel.be/voc/buildingelement#Stair-QUARTER_WINDING_STAIR">
        <rdfs:subClassOf rdf:resource="https://pi.pauwel.be/voc/buildingelement#Stair"/>
        <rdfs:comment xml:lang="en">http://bsdd.buildingsmart.org/#concept/details/3PzSNWl5T1EgMXH$Tn6uuQ</rdfs:comment>
        <rdfs:label xml:lang="en">Quarter Winding Stair</rdfs:label>
        <rdfs:seeAlso rdf:resource="http://www.buildingsmart-tech.org/ifcOWL/IFC4_ADD2#IfcStairEnumType"/>
    </owl:Class>
    


    <!-- https://pi.pauwel.be/voc/buildingelement#Stair-SPIRAL_STAIR -->

    <owl:Class rdf:about="https://pi.pauwel.be/voc/buildingelement#Stair-SPIRAL_STAIR">
        <rdfs:subClassOf rdf:resource="https://pi.pauwel.be/voc/buildingelement#Stair"/>
        <rdfs:comment xml:lang="en">http://bsdd.buildingsmart.org/#concept/details/0UwQe$TXP47AhE5k0mZzCe</rdfs:comment>
        <rdfs:label xml:lang="en">Spiral Stair</rdfs:label>
        <rdfs:seeAlso rdf:resource="http://www.buildingsmart-tech.org/ifcOWL/IFC4_ADD2#IfcStairEnumType"/>
    </owl:Class>
    


    <!-- https://pi.pauwel.be/voc/buildingelement#Stair-STRAIGHT_RUN_STAIR -->

    <owl:Class rdf:about="https://pi.pauwel.be/voc/buildingelement#Stair-STRAIGHT_RUN_STAIR">
        <rdfs:subClassOf rdf:resource="https://pi.pauwel.be/voc/buildingelement#Stair"/>
        <rdfs:comment xml:lang="en">http://bsdd.buildingsmart.org/#concept/details/3p4WSJmK96Oe6HXE$jmWWy</rdfs:comment>
        <rdfs:label xml:lang="en">Straight Run Stair</rdfs:label>
        <rdfs:seeAlso rdf:resource="http://www.buildingsmart-tech.org/ifcOWL/IFC4_ADD2#IfcStairEnumType"/>
    </owl:Class>
    


    <!-- https://pi.pauwel.be/voc/buildingelement#Stair-THREE_QUARTER_TURN_STAIR -->

    <owl:Class rdf:about="https://pi.pauwel.be/voc/buildingelement#Stair-THREE_QUARTER_TURN_STAIR">
        <rdfs:subClassOf rdf:resource="https://pi.pauwel.be/voc/buildingelement#Stair"/>
        <rdfs:comment xml:lang="en">http://bsdd.buildingsmart.org/#concept/details/2jTG3NRNHCyhbsMbwK38v5</rdfs:comment>
        <rdfs:label xml:lang="en">Three Quarter Turn Stair</rdfs:label>
        <rdfs:seeAlso rdf:resource="http://www.buildingsmart-tech.org/ifcOWL/IFC4_ADD2#IfcStairEnumType"/>
    </owl:Class>
    


    <!-- https://pi.pauwel.be/voc/buildingelement#Stair-THREE_QUARTER_WINDING_STAIR -->

    <owl:Class rdf:about="https://pi.pauwel.be/voc/buildingelement#Stair-THREE_QUARTER_WINDING_STAIR">
        <rdfs:subClassOf rdf:resource="https://pi.pauwel.be/voc/buildingelement#Stair"/>
        <rdfs:comment xml:lang="en">http://bsdd.buildingsmart.org/#concept/details/0rPjGYk_LFnOayZFsJg3tr</rdfs:comment>
        <rdfs:label xml:lang="en">Three Quarter Winding Stair</rdfs:label>
        <rdfs:seeAlso rdf:resource="http://www.buildingsmart-tech.org/ifcOWL/IFC4_ADD2#IfcStairEnumType"/>
    </owl:Class>
    


    <!-- https://pi.pauwel.be/voc/buildingelement#Stair-TWO_CURVED_RUN_STAIR -->

    <owl:Class rdf:about="https://pi.pauwel.be/voc/buildingelement#Stair-TWO_CURVED_RUN_STAIR">
        <rdfs:subClassOf rdf:resource="https://pi.pauwel.be/voc/buildingelement#Stair"/>
        <rdfs:comment xml:lang="en">http://bsdd.buildingsmart.org/#concept/details/0cSo1dkGL8NunRzp$sQsTc</rdfs:comment>
        <rdfs:label xml:lang="en">Two Curved Run Stair</rdfs:label>
        <rdfs:seeAlso rdf:resource="http://www.buildingsmart-tech.org/ifcOWL/IFC4_ADD2#IfcStairEnumType"/>
    </owl:Class>
    


    <!-- https://pi.pauwel.be/voc/buildingelement#Stair-TWO_QUARTER_TURN_STAIR -->

    <owl:Class rdf:about="https://pi.pauwel.be/voc/buildingelement#Stair-TWO_QUARTER_TURN_STAIR">
        <rdfs:subClassOf rdf:resource="https://pi.pauwel.be/voc/buildingelement#Stair"/>
        <rdfs:comment xml:lang="en">a stair making a 180° turn, consisting of three straight flights connected by two quarterspace landings. the direction of the turns is determined by the walking line</rdfs:comment>
        <rdfs:comment xml:lang="en">http://bsdd.buildingsmart.org/#concept/details/0mW4DtraD3SA57fcejW4cS</rdfs:comment>
        <rdfs:label xml:lang="en">Two Quarter Turn Stair</rdfs:label>
        <rdfs:seeAlso rdf:resource="http://www.buildingsmart-tech.org/ifcOWL/IFC4_ADD2#IfcStairEnumType"/>
    </owl:Class>
    


    <!-- https://pi.pauwel.be/voc/buildingelement#Stair-TWO_QUARTER_WINDING_STAIR -->

    <owl:Class rdf:about="https://pi.pauwel.be/voc/buildingelement#Stair-TWO_QUARTER_WINDING_STAIR">
        <rdfs:subClassOf rdf:resource="https://pi.pauwel.be/voc/buildingelement#Stair"/>
        <rdfs:comment xml:lang="en">http://bsdd.buildingsmart.org/#concept/details/3SSlfuJ_nA49lzIOhda6Xr</rdfs:comment>
        <rdfs:label xml:lang="en">Two Quarter Winding Stair</rdfs:label>
        <rdfs:seeAlso rdf:resource="http://www.buildingsmart-tech.org/ifcOWL/IFC4_ADD2#IfcStairEnumType"/>
    </owl:Class>
    


    <!-- https://pi.pauwel.be/voc/buildingelement#Stair-TWO_STRAIGHT_RUN_STAIR -->

    <owl:Class rdf:about="https://pi.pauwel.be/voc/buildingelement#Stair-TWO_STRAIGHT_RUN_STAIR">
        <rdfs:subClassOf rdf:resource="https://pi.pauwel.be/voc/buildingelement#Stair"/>
        <rdfs:comment xml:lang="en">a straight stair consisting of two straight flights without turns but with one landing.</rdfs:comment>
        <rdfs:comment xml:lang="en">http://bsdd.buildingsmart.org/#concept/details/3VuqGJNz160B87TSrFhrM4</rdfs:comment>
        <rdfs:label xml:lang="en">Two Straight Run Stair</rdfs:label>
        <rdfs:seeAlso rdf:resource="http://www.buildingsmart-tech.org/ifcOWL/IFC4_ADD2#IfcStairEnumType"/>
    </owl:Class>
    


    <!-- https://pi.pauwel.be/voc/buildingelement#StairFlight -->

    <owl:Class rdf:about="https://pi.pauwel.be/voc/buildingelement#StairFlight">
        <rdfs:subClassOf rdf:resource="https://pi.pauwel.be/voc/buildingelement#BuildingElement"/>
        <rdfs:comment xml:lang="en">An assembly of building components in a single &quot;run&quot; of stair steps (not interrupted by a landing).</rdfs:comment>
        <rdfs:comment xml:lang="en">http://bsdd.buildingsmart.org/#concept/details/0pceq0qWqHuO00025QrE$V</rdfs:comment>
        <rdfs:label xml:lang="en">Stair Flight</rdfs:label>
        <rdfs:label xml:lang="fr-fr">Volée d&apos;escalier</rdfs:label>
        <rdfs:label xml:lang="nl-nl">trap</rdfs:label>
        <rdfs:label xml:lang="nb-no">trapp</rdfs:label>
        <rdfs:label xml:lang="nl-nl">trapslag</rdfs:label>
        <rdfs:label xml:lang="de-de">treppenlauf</rdfs:label>
        <rdfs:seeAlso rdf:resource="http://www.buildingsmart-tech.org/ifcOWL/IFC4_ADD2#IfcStairFlight"/>
    </owl:Class>
    


    <!-- https://pi.pauwel.be/voc/buildingelement#StairFlight-CURVED -->

    <owl:Class rdf:about="https://pi.pauwel.be/voc/buildingelement#StairFlight-CURVED">
        <rdfs:subClassOf rdf:resource="https://pi.pauwel.be/voc/buildingelement#StairFlight"/>
        <rdfs:comment xml:lang="en">http://bsdd.buildingsmart.org/#concept/details/2DeCDqEVHDjwFaGVpyNC89</rdfs:comment>
        <rdfs:label xml:lang="en">Curved</rdfs:label>
        <rdfs:label xml:lang="nb-no">trapp - kurvet</rdfs:label>
        <rdfs:seeAlso rdf:resource="http://www.buildingsmart-tech.org/ifcOWL/IFC4_ADD2#IfcStairFlightEnumType"/>
    </owl:Class>
    


    <!-- https://pi.pauwel.be/voc/buildingelement#StairFlight-FREEFORM -->

    <owl:Class rdf:about="https://pi.pauwel.be/voc/buildingelement#StairFlight-FREEFORM">
        <rdfs:subClassOf rdf:resource="https://pi.pauwel.be/voc/buildingelement#StairFlight"/>
        <rdfs:comment xml:lang="en">http://bsdd.buildingsmart.org/#concept/details/0uFuIDRO1EZPmcL8pEkVU$</rdfs:comment>
        <rdfs:label>Freeform</rdfs:label>
        <rdfs:label xml:lang="nb-no">friform</rdfs:label>
        <rdfs:label xml:lang="nb-no">friform tak</rdfs:label>
        <rdfs:seeAlso rdf:resource="http://www.buildingsmart-tech.org/ifcOWL/IFC4_ADD2#IfcStairFlightEnumType"/>
    </owl:Class>
    


    <!-- https://pi.pauwel.be/voc/buildingelement#StairFlight-SPIRAL -->

    <owl:Class rdf:about="https://pi.pauwel.be/voc/buildingelement#StairFlight-SPIRAL">
        <rdfs:subClassOf rdf:resource="https://pi.pauwel.be/voc/buildingelement#StairFlight"/>
        <rdfs:comment xml:lang="en">http://bsdd.buildingsmart.org/#concept/details/1zj3DVJij6IBVuIqOLbi46</rdfs:comment>
        <rdfs:label xml:lang="en">Spiral</rdfs:label>
        <rdfs:label xml:lang="en">scroll</rdfs:label>
        <rdfs:label xml:lang="nb-no">spiral</rdfs:label>
        <rdfs:label xml:lang="nb-no">vindel</rdfs:label>
        <rdfs:seeAlso rdf:resource="http://www.buildingsmart-tech.org/ifcOWL/IFC4_ADD2#IfcStairFlightEnumType"/>
    </owl:Class>
    


    <!-- https://pi.pauwel.be/voc/buildingelement#StairFlight-STRAIGHT -->

    <owl:Class rdf:about="https://pi.pauwel.be/voc/buildingelement#StairFlight-STRAIGHT">
        <rdfs:subClassOf rdf:resource="https://pi.pauwel.be/voc/buildingelement#StairFlight"/>
        <rdfs:comment xml:lang="en">http://bsdd.buildingsmart.org/#concept/details/247CeErMz16BZyRhwbAOdR</rdfs:comment>
        <rdfs:label xml:lang="en">Straight</rdfs:label>
        <rdfs:label xml:lang="nb-no">rett</rdfs:label>
        <rdfs:seeAlso rdf:resource="http://www.buildingsmart-tech.org/ifcOWL/IFC4_ADD2#IfcStairFlightEnumType"/>
    </owl:Class>
    


    <!-- https://pi.pauwel.be/voc/buildingelement#StairFlight-WINDER -->

    <owl:Class rdf:about="https://pi.pauwel.be/voc/buildingelement#StairFlight-WINDER">
        <rdfs:subClassOf rdf:resource="https://pi.pauwel.be/voc/buildingelement#StairFlight"/>
        <rdfs:comment xml:lang="en">http://bsdd.buildingsmart.org/#concept/details/3XVLP1SZf8YQfshhp0Vjph</rdfs:comment>
        <rdfs:label xml:lang="en">Winder</rdfs:label>
        <rdfs:label xml:lang="nb-no">svingtrapp</rdfs:label>
        <rdfs:seeAlso rdf:resource="http://www.buildingsmart-tech.org/ifcOWL/IFC4_ADD2#IfcStairFlightEnumType"/>
    </owl:Class>
    


    <!-- https://pi.pauwel.be/voc/buildingelement#Tendon -->

    <owl:Class rdf:about="https://pi.pauwel.be/voc/buildingelement#Tendon">
        <rdfs:subClassOf rdf:resource="https://pi.pauwel.be/voc/buildingelement#ReinforcingElement"/>
        <rdfs:comment xml:lang="en">a tendon is a steel element such as a wire, cable, bar, rod or strand used to impart prestress to concrete when the element is tensioned.</rdfs:comment>
        <rdfs:comment xml:lang="en">http://bsdd.buildingsmart.org/#concept/details/0GEDRkhJ9DdQ2MRE_CaSCF</rdfs:comment>
        <rdfs:label xml:lang="de-de">Spannglied</rdfs:label>
        <rdfs:label xml:lang="en">Tendon</rdfs:label>
        <rdfs:label xml:lang="fr-fr">cable</rdfs:label>
        <rdfs:seeAlso rdf:resource="http://www.buildingsmart-tech.org/ifcOWL/IFC4_ADD2#IfcTendon"/>
    </owl:Class>
    


    <!-- https://pi.pauwel.be/voc/buildingelement#Tendon-BAR -->

    <owl:Class rdf:about="https://pi.pauwel.be/voc/buildingelement#Tendon-BAR">
        <rdfs:subClassOf rdf:resource="https://pi.pauwel.be/voc/buildingelement#Tendon"/>
        <rdfs:comment xml:lang="en">http://bsdd.buildingsmart.org/#concept/details/3seMZXSSH4YfQCPjOcaoZG</rdfs:comment>
        <rdfs:label xml:lang="en">Bar</rdfs:label>
        <rdfs:seeAlso rdf:resource="http://www.buildingsmart-tech.org/ifcOWL/IFC4_ADD2#IfcTendonEnumType"/>
    </owl:Class>
    


    <!-- https://pi.pauwel.be/voc/buildingelement#Tendon-COATED -->

    <owl:Class rdf:about="https://pi.pauwel.be/voc/buildingelement#Tendon-COATED">
        <rdfs:subClassOf rdf:resource="https://pi.pauwel.be/voc/buildingelement#Tendon"/>
        <rdfs:comment xml:lang="en">http://bsdd.buildingsmart.org/#concept/details/1WLzEVaRD77A5KPd3$v9DB</rdfs:comment>
        <rdfs:label xml:lang="en">Coated</rdfs:label>
        <rdfs:seeAlso rdf:resource="http://www.buildingsmart-tech.org/ifcOWL/IFC4_ADD2#IfcTendonEnumType"/>
    </owl:Class>
    


    <!-- https://pi.pauwel.be/voc/buildingelement#Tendon-STRAND -->

    <owl:Class rdf:about="https://pi.pauwel.be/voc/buildingelement#Tendon-STRAND">
        <rdfs:subClassOf rdf:resource="https://pi.pauwel.be/voc/buildingelement#Tendon"/>
        <rdfs:comment xml:lang="en">http://bsdd.buildingsmart.org/#concept/details/1d4UrJXi92ivdu3FflJ62n</rdfs:comment>
        <rdfs:label xml:lang="en">Strand</rdfs:label>
        <rdfs:seeAlso rdf:resource="http://www.buildingsmart-tech.org/ifcOWL/IFC4_ADD2#IfcTendonEnumType"/>
    </owl:Class>
    


    <!-- https://pi.pauwel.be/voc/buildingelement#Tendon-WIRE -->

    <owl:Class rdf:about="https://pi.pauwel.be/voc/buildingelement#Tendon-WIRE">
        <rdfs:subClassOf rdf:resource="https://pi.pauwel.be/voc/buildingelement#Tendon"/>
        <rdfs:comment xml:lang="en">http://bsdd.buildingsmart.org/#concept/details/1NCnQvMs9AaRqwexu7DofF</rdfs:comment>
        <rdfs:label xml:lang="en">Wire</rdfs:label>
        <rdfs:seeAlso rdf:resource="http://www.buildingsmart-tech.org/ifcOWL/IFC4_ADD2#IfcTendonEnumType"/>
    </owl:Class>
    


    <!-- https://pi.pauwel.be/voc/buildingelement#TendonAnchor -->

    <owl:Class rdf:about="https://pi.pauwel.be/voc/buildingelement#TendonAnchor">
        <rdfs:subClassOf rdf:resource="https://pi.pauwel.be/voc/buildingelement#ReinforcingElement"/>
        <rdfs:comment xml:lang="en">a tendon anchor is the end connection for tendons in prestressed or posttensioned concrete.</rdfs:comment>
        <rdfs:comment xml:lang="en">http://bsdd.buildingsmart.org/#concept/details/0Z116ntsH6xBFYGYsNg38f</rdfs:comment>
        <rdfs:label xml:lang="de-de">Spanngliedanker</rdfs:label>
        <rdfs:label xml:lang="en">Tendon Anchor</rdfs:label>
        <rdfs:label xml:lang="fr-fr">ancrage</rdfs:label>
        <rdfs:seeAlso rdf:resource="http://www.buildingsmart-tech.org/ifcOWL/IFC4_ADD2#IfcTendonAnchor"/>
    </owl:Class>
    


    <!-- https://pi.pauwel.be/voc/buildingelement#TendonAnchor-COUPLER -->

    <owl:Class rdf:about="https://pi.pauwel.be/voc/buildingelement#TendonAnchor-COUPLER">
        <rdfs:subClassOf rdf:resource="https://pi.pauwel.be/voc/buildingelement#TendonAnchor"/>
        <rdfs:comment xml:lang="en">http://bsdd.buildingsmart.org/#concept/details/2yrjArQAnBL9EdTqIc7Uv7</rdfs:comment>
        <rdfs:label xml:lang="en">Coupler</rdfs:label>
        <rdfs:seeAlso rdf:resource="http://www.buildingsmart-tech.org/ifcOWL/IFC4_ADD2#IfcTendonAnchorEnumType"/>
    </owl:Class>
    


    <!-- https://pi.pauwel.be/voc/buildingelement#TendonAnchor-FIXED_END -->

    <owl:Class rdf:about="https://pi.pauwel.be/voc/buildingelement#TendonAnchor-FIXED_END">
        <rdfs:subClassOf rdf:resource="https://pi.pauwel.be/voc/buildingelement#TendonAnchor"/>
        <rdfs:comment xml:lang="en">http://bsdd.buildingsmart.org/#concept/details/133YYoKAv8mBxccTJtzWju</rdfs:comment>
        <rdfs:label xml:lang="en">Fixed End</rdfs:label>
        <rdfs:seeAlso rdf:resource="http://www.buildingsmart-tech.org/ifcOWL/IFC4_ADD2#IfcTendonAnchorEnumType"/>
    </owl:Class>
    


    <!-- https://pi.pauwel.be/voc/buildingelement#TendonAnchor-TENSIONING_END -->

    <owl:Class rdf:about="https://pi.pauwel.be/voc/buildingelement#TendonAnchor-TENSIONING_END">
        <rdfs:subClassOf rdf:resource="https://pi.pauwel.be/voc/buildingelement#TendonAnchor"/>
        <rdfs:comment xml:lang="en">http://bsdd.buildingsmart.org/#concept/details/2Bp8P7qwn1Hg1BaRHyCQP4</rdfs:comment>
        <rdfs:label xml:lang="en">Tensioning End</rdfs:label>
        <rdfs:seeAlso rdf:resource="http://www.buildingsmart-tech.org/ifcOWL/IFC4_ADD2#IfcTendonAnchorEnumType"/>
    </owl:Class>
    


    <!-- https://pi.pauwel.be/voc/buildingelement#TransportElement -->

    <owl:Class rdf:about="https://pi.pauwel.be/voc/buildingelement#TransportElement">
        <rdfs:subClassOf rdf:resource="https://schema.org/Product"/>
        <rdfs:comment xml:lang="en">A generalization of all transport related objects that move people, animals or goods within a building or building complex. Include elevator (lift), escalator, moving walkway, etc.</rdfs:comment>
        <rdfs:comment xml:lang="en">An element type defined by commonly shared information for occurrences of transport elements. The set of shared information may include:
common properties within shared property sets
common material information
common shape representations
It is used to define a transport element specification (i.e. the specific product information that is common to all occurrences of that beam type). </rdfs:comment>
        <rdfs:comment xml:lang="en">http://bsdd.buildingsmart.org/#concept/details/3ZSVc0qX4HuO00025QrE$V</rdfs:comment>
        <rdfs:label xml:lang="de-de">Beförderungsgerät</rdfs:label>
        <rdfs:label xml:lang="fr-fr">Equipement de transport</rdfs:label>
        <rdfs:label xml:lang="en">Transport Element</rdfs:label>
        <rdfs:label xml:lang="nb-no">transportelement</rdfs:label>
        <rdfs:seeAlso rdf:resource="http://www.buildingsmart-tech.org/ifcOWL/IFC4_ADD2#IfcTransportElement"/>
    </owl:Class>
    


    <!-- https://pi.pauwel.be/voc/buildingelement#TransportElement-CRANEWAY -->

    <owl:Class rdf:about="https://pi.pauwel.be/voc/buildingelement#TransportElement-CRANEWAY">
        <rdfs:subClassOf rdf:resource="https://pi.pauwel.be/voc/buildingelement#TransportElement"/>
        <rdfs:comment xml:lang="en">An artefact for raising, shifting and lowering heavy weights by means of a projecting swinging arm or with hoisting mechanism supported on an overhead track.        </rdfs:comment>
        <rdfs:comment xml:lang="en">a crane way system, normally including the crane rails, fasteners and the crane. it is primarily used to move heavy goods in a factory or other industry buildings</rdfs:comment>
        <rdfs:comment xml:lang="en-gb">a crane way system, normally including the crane rails, fasteners and the crane. it is primarily used to move heavy goods in a factory or other industry buildings</rdfs:comment>
        <rdfs:comment xml:lang="en">http://bsdd.buildingsmart.org/#concept/details/087V4aTMPA09OItHDUip4G</rdfs:comment>
        <rdfs:label xml:lang="en">Craneway</rdfs:label>
        <rdfs:label xml:lang="nb-no">kran</rdfs:label>
        <rdfs:label xml:lang="nb-no">kranbane</rdfs:label>
        <rdfs:seeAlso rdf:resource="http://www.buildingsmart-tech.org/ifcOWL/IFC4_ADD2#IfcTransportElementEnumType"/>
    </owl:Class>
    


    <!-- https://pi.pauwel.be/voc/buildingelement#TransportElement-ELEVATOR -->

    <owl:Class rdf:about="https://pi.pauwel.be/voc/buildingelement#TransportElement-ELEVATOR">
        <rdfs:subClassOf rdf:resource="https://pi.pauwel.be/voc/buildingelement#TransportElement"/>
        <rdfs:comment xml:lang="en">a permanent lifting equipment serving defined landing levels, comprising a car, whose dimensions and means of construction clearly permit the access of persons; running at least partially between rigid vertical guides or guides whose inclination to the ve</rdfs:comment>
        <rdfs:comment xml:lang="en">http://bsdd.buildingsmart.org/#concept/details/2qanav0WDASA8V5to62fCx</rdfs:comment>
        <rdfs:comment xml:lang="en">http://bsdd.buildingsmart.org/#concept/details/3vHX1_oT0Hsm00051Mm008</rdfs:comment>
        <rdfs:comment xml:lang="nb-no">permanent løfteutstyr som betjener definerte etasjenivåer, og som består av en stol hvis dimensjoner og konstruksjonsmåte klart gir adgang for personer, og som minst delvis beveger seg mellom stive, vertikale føringsskinner eller føringer hvor hellingen f</rdfs:comment>
        <rdfs:label xml:lang="de-de">Aufzug</rdfs:label>
        <rdfs:label>Elevator</rdfs:label>
        <rdfs:label xml:lang="en">Elevator</rdfs:label>
        <rdfs:label xml:lang="fr-fr">ascenseur</rdfs:label>
        <rdfs:label xml:lang="nb-no">heis</rdfs:label>
        <rdfs:label xml:lang="en">lift</rdfs:label>
        <rdfs:seeAlso rdf:resource="http://www.buildingsmart-tech.org/ifcOWL/IFC4_ADD2#IfcTransportElementEnumType"/>
    </owl:Class>
    


    <!-- https://pi.pauwel.be/voc/buildingelement#TransportElement-ESCALATOR -->

    <owl:Class rdf:about="https://pi.pauwel.be/voc/buildingelement#TransportElement-ESCALATOR">
        <rdfs:subClassOf rdf:resource="https://pi.pauwel.be/voc/buildingelement#TransportElement"/>
        <rdfs:comment xml:lang="en">http://bsdd.buildingsmart.org/#concept/details/377eo0WJOHu000025QrE$V</rdfs:comment>
        <rdfs:comment xml:lang="en">http://bsdd.buildingsmart.org/#concept/details/3vHZncoT0Hsm00051Mm008</rdfs:comment>
        <rdfs:comment xml:lang="en">power-driven, inclined, continuous moving stairway used for raising or lowering persons in which the user carrying surface (e.g. steps) remains horizontal</rdfs:comment>
        <rdfs:label>Escalator</rdfs:label>
        <rdfs:label xml:lang="de-de">Fahrtreppe</rdfs:label>
        <rdfs:label xml:lang="nl-nl">Roltrap</rdfs:label>
        <rdfs:label xml:lang="fr-fr">escalier roulant</rdfs:label>
        <rdfs:label xml:lang="nb-no">rulletrapp</rdfs:label>
        <rdfs:seeAlso rdf:resource="http://www.buildingsmart-tech.org/ifcOWL/IFC4_ADD2#IfcTransportElementEnumType"/>
    </owl:Class>
    


    <!-- https://pi.pauwel.be/voc/buildingelement#TransportElement-LIFTINGGEAR -->

    <owl:Class rdf:about="https://pi.pauwel.be/voc/buildingelement#TransportElement-LIFTINGGEAR">
        <rdfs:subClassOf rdf:resource="https://pi.pauwel.be/voc/buildingelement#TransportElement"/>
        <rdfs:comment xml:lang="en">a device used for lifting or lowering heavy goods. It may be manually operated or electrically or pneumatically driven</rdfs:comment>
        <rdfs:comment xml:lang="en-gb">a device used for lifting or lowering heavy goods. It may be manually operated or electrically or pneumatically driven</rdfs:comment>
        <rdfs:comment xml:lang="en">http://bsdd.buildingsmart.org/#concept/details/3qsVNaK3r6Uw2tccQdpTmo</rdfs:comment>
        <rdfs:label xml:lang="en">Lifting Gear</rdfs:label>
        <rdfs:label xml:lang="nb-no">løfteinretning</rdfs:label>
        <rdfs:seeAlso rdf:resource="http://www.buildingsmart-tech.org/ifcOWL/IFC4_ADD2#IfcTransportElementEnumType"/>
    </owl:Class>
    


    <!-- https://pi.pauwel.be/voc/buildingelement#TransportElement-MOVINGWALKWAY -->

    <owl:Class rdf:about="https://pi.pauwel.be/voc/buildingelement#TransportElement-MOVINGWALKWAY">
        <rdfs:subClassOf rdf:resource="https://pi.pauwel.be/voc/buildingelement#TransportElement"/>
        <rdfs:comment xml:lang="en">http://bsdd.buildingsmart.org/#concept/details/0Fn7lcsC5As81fnfma0hsy</rdfs:comment>
        <rdfs:label xml:lang="en">Moving Walkway</rdfs:label>
        <rdfs:label xml:lang="nb-no">rullebånd</rdfs:label>
        <rdfs:seeAlso rdf:resource="http://www.buildingsmart-tech.org/ifcOWL/IFC4_ADD2#IfcTransportElementEnumType"/>
    </owl:Class>
    


    <!-- https://pi.pauwel.be/voc/buildingelement#VibrationIsolator -->

    <owl:Class rdf:about="https://pi.pauwel.be/voc/buildingelement#VibrationIsolator">
        <rdfs:subClassOf rdf:resource="https://pi.pauwel.be/voc/buildingelement#ElementComponent"/>
        <rdfs:comment xml:lang="en">A device used to minimize the effects of vibration transmissibility in a building.</rdfs:comment>
        <rdfs:comment xml:lang="en">http://bsdd.buildingsmart.org/#concept/details/0Oy60xvFT7TO70hyDzhWWZ</rdfs:comment>
        <rdfs:label xml:lang="de-de">Schwingungsisolator</rdfs:label>
        <rdfs:label xml:lang="en">Vibration Isolator</rdfs:label>
        <rdfs:label xml:lang="fr-fr">isolateur de vibrations</rdfs:label>
        <rdfs:label xml:lang="fr-fr">isolation anti-vibratoire</rdfs:label>
        <rdfs:label xml:lang="nl-nl">trillingsisolator</rdfs:label>
        <rdfs:label xml:lang="nb-no">vibrasjonsisolator</rdfs:label>
        <rdfs:seeAlso rdf:resource="http://www.buildingsmart-tech.org/ifcOWL/IFC4_ADD2#IfcVibrationIsolator"/>
    </owl:Class>
    


    <!-- https://pi.pauwel.be/voc/buildingelement#VibrationIsolator-COMPRESSION -->

    <owl:Class rdf:about="https://pi.pauwel.be/voc/buildingelement#VibrationIsolator-COMPRESSION">
        <rdfs:subClassOf rdf:resource="https://pi.pauwel.be/voc/buildingelement#VibrationIsolator"/>
        <rdfs:comment xml:lang="en">compression type vibration isolator</rdfs:comment>
        <rdfs:comment xml:lang="en-gb">compression type vibration isolator</rdfs:comment>
        <rdfs:comment xml:lang="en">http://bsdd.buildingsmart.org/#concept/details/0EwSGR8PX1z9zHS_KHBRcA</rdfs:comment>
        <rdfs:label>Compression-based vibration isolator</rdfs:label>
        <rdfs:label xml:lang="nb-no">kompresjon</rdfs:label>
        <rdfs:seeAlso rdf:resource="http://www.buildingsmart-tech.org/ifcOWL/IFC4_ADD2#IfcVibrationIsolatorEnumType"/>
    </owl:Class>
    


    <!-- https://pi.pauwel.be/voc/buildingelement#VibrationIsolator-SPRING -->

    <owl:Class rdf:about="https://pi.pauwel.be/voc/buildingelement#VibrationIsolator-SPRING">
        <rdfs:subClassOf rdf:resource="https://pi.pauwel.be/voc/buildingelement#VibrationIsolator"/>
        <rdfs:comment xml:lang="en">http://bsdd.buildingsmart.org/#concept/details/3cKim0GJf3mxz7EqVVfQ8u</rdfs:comment>
        <rdfs:comment xml:lang="en">spring type vibration isolator</rdfs:comment>
        <rdfs:comment xml:lang="en-gb">spring type vibration isolator</rdfs:comment>
        <rdfs:label xml:lang="en">Spring</rdfs:label>
        <rdfs:label xml:lang="nb-no">fjær</rdfs:label>
        <rdfs:seeAlso rdf:resource="http://www.buildingsmart-tech.org/ifcOWL/IFC4_ADD2#IfcVibrationIsolatorEnumType"/>
    </owl:Class>
    


    <!-- https://pi.pauwel.be/voc/buildingelement#Wall -->

    <owl:Class rdf:about="https://pi.pauwel.be/voc/buildingelement#Wall">
        <rdfs:subClassOf rdf:resource="https://pi.pauwel.be/voc/buildingelement#BuildingElement"/>
        <rdfs:comment xml:lang="en">A vertical construction that bounds or subdivides spaces. Usually vertical, or nearly vertical, planar elements, often designed to bear structural loads. However not required to be load bearing.</rdfs:comment>
        <rdfs:comment xml:lang="en">http://bsdd.buildingsmart.org/#concept/details/2Xuqs0qXKHuO00025QrE$V</rdfs:comment>
        <rdfs:label xml:lang="nl">Muur</rdfs:label>
        <rdfs:label xml:lang="da">Væg</rdfs:label>
        <rdfs:label xml:lang="en">Wall</rdfs:label>
        <rdfs:label xml:lang="de-de">Wand</rdfs:label>
        <rdfs:label xml:lang="fr-fr">mur</rdfs:label>
        <rdfs:label xml:lang="nb-no">vegg</rdfs:label>
        <rdfs:label xml:lang="en">wall</rdfs:label>
        <rdfs:seeAlso rdf:resource="http://www.buildingsmart-tech.org/ifcOWL/IFC4_ADD2#IfcWall"/>
    </owl:Class>
    


    <!-- https://pi.pauwel.be/voc/buildingelement#Wall-ELEMENTEDWALL -->

    <owl:Class rdf:about="https://pi.pauwel.be/voc/buildingelement#Wall-ELEMENTEDWALL">
        <rdfs:subClassOf rdf:resource="https://pi.pauwel.be/voc/buildingelement#Wall"/>
        <rdfs:comment xml:lang="en">a stud wall framed with studs and faced with sheetings, sidings, wallboard, or plasterwork</rdfs:comment>
        <rdfs:comment xml:lang="en-gb">a stud wall framed with studs and faced with sheetings, sidings, wallboard, or plasterwork</rdfs:comment>
        <rdfs:comment xml:lang="en">http://bsdd.buildingsmart.org/#concept/details/0sVBQjaqvEcAVsdRJorFkQ</rdfs:comment>
        <rdfs:label xml:lang="en">Elemented Wall</rdfs:label>
        <rdfs:label xml:lang="nb-no">elementvegg</rdfs:label>
        <rdfs:label xml:lang="nb-no">systemvegg</rdfs:label>
        <rdfs:seeAlso rdf:resource="http://www.buildingsmart-tech.org/ifcOWL/IFC4_ADD2#IfcWallEnumType"/>
    </owl:Class>
    


    <!-- https://pi.pauwel.be/voc/buildingelement#Wall-MOVABLE -->

    <owl:Class rdf:about="https://pi.pauwel.be/voc/buildingelement#Wall-MOVABLE">
        <rdfs:subClassOf rdf:resource="https://pi.pauwel.be/voc/buildingelement#Wall"/>
        <rdfs:comment xml:lang="en">http://bsdd.buildingsmart.org/#concept/details/2nSQnTH_18RB$MO5daYxD0</rdfs:comment>
        <rdfs:label xml:lang="nb-no">Flyttbar</rdfs:label>
        <rdfs:label xml:lang="en">Movable Wall</rdfs:label>
        <rdfs:seeAlso rdf:resource="http://www.buildingsmart-tech.org/ifcOWL/IFC4_ADD2#IfcWallEnumType"/>
    </owl:Class>
    


    <!-- https://pi.pauwel.be/voc/buildingelement#Wall-PARAPET -->

    <owl:Class rdf:about="https://pi.pauwel.be/voc/buildingelement#Wall-PARAPET">
        <rdfs:subClassOf rdf:resource="https://pi.pauwel.be/voc/buildingelement#Wall"/>
        <rdfs:comment xml:lang="nb-no">Parapet/brystning
Opphøyet kant som stikker opp over tak</rdfs:comment>
        <rdfs:comment xml:lang="en">http://bsdd.buildingsmart.org/#concept/details/1uS$40WJmHu000025QrE$V</rdfs:comment>
        <rdfs:comment xml:lang="en">http://bsdd.buildingsmart.org/#concept/details/2BlEUUV2L2BBUdnPO3PtnQ</rdfs:comment>
        <rdfs:label xml:lang="nl-nl">Balustrade</rdfs:label>
        <rdfs:label xml:lang="nl-nl">Borstwering</rdfs:label>
        <rdfs:label xml:lang="en">Parapet Wall</rdfs:label>
        <rdfs:label xml:lang="en">balustrade</rdfs:label>
        <rdfs:label xml:lang="en">parapet</rdfs:label>
        <rdfs:label xml:lang="nb-no">parapet</rdfs:label>
        <rdfs:seeAlso rdf:resource="http://www.buildingsmart-tech.org/ifcOWL/IFC4_ADD2#IfcWallEnumType"/>
    </owl:Class>
    


    <!-- https://pi.pauwel.be/voc/buildingelement#Wall-PARTITIONING -->

    <owl:Class rdf:about="https://pi.pauwel.be/voc/buildingelement#Wall-PARTITIONING">
        <rdfs:subClassOf rdf:resource="https://pi.pauwel.be/voc/buildingelement#Wall"/>
        <rdfs:comment xml:lang="en">http://bsdd.buildingsmart.org/#concept/details/3DBpG2jff4GAXiQp8trskt</rdfs:comment>
        <rdfs:label xml:lang="en">Partitioning Wall</rdfs:label>
        <rdfs:label xml:lang="nb-no">skillevegg</rdfs:label>
        <rdfs:seeAlso rdf:resource="http://www.buildingsmart-tech.org/ifcOWL/IFC4_ADD2#IfcWallEnumType"/>
    </owl:Class>
    


    <!-- https://pi.pauwel.be/voc/buildingelement#Wall-PLUMBINGWALL -->

    <owl:Class rdf:about="https://pi.pauwel.be/voc/buildingelement#Wall-PLUMBINGWALL">
        <rdfs:subClassOf rdf:resource="https://pi.pauwel.be/voc/buildingelement#Wall"/>
        <rdfs:comment xml:lang="en">http://bsdd.buildingsmart.org/#concept/details/1YFt0DFB99uxbJnz4oFiew</rdfs:comment>
        <rdfs:label xml:lang="en">Plumbing Wall</rdfs:label>
        <rdfs:label xml:lang="nb-no">rør i vegg</rdfs:label>
        <rdfs:seeAlso rdf:resource="http://www.buildingsmart-tech.org/ifcOWL/IFC4_ADD2#IfcWallEnumType"/>
    </owl:Class>
    


    <!-- https://pi.pauwel.be/voc/buildingelement#Wall-POLYGONAL -->

    <owl:Class rdf:about="https://pi.pauwel.be/voc/buildingelement#Wall-POLYGONAL">
        <rdfs:subClassOf rdf:resource="https://pi.pauwel.be/voc/buildingelement#Wall"/>
        <rdfs:comment xml:lang="en">a polygonal wall, extruded vertically, where the wall thickness varies along the wall path</rdfs:comment>
        <rdfs:comment xml:lang="en-gb">a polygonal wall, extruded vertically, where the wall thickness varies along the wall path</rdfs:comment>
        <rdfs:comment xml:lang="en">http://bsdd.buildingsmart.org/#concept/details/0cJEMJHYj6Hh7Q1xNPsiIf</rdfs:comment>
        <rdfs:label xml:lang="en">Polygonal Wall</rdfs:label>
        <rdfs:label xml:lang="nb-no">mangekantet</rdfs:label>
        <rdfs:seeAlso rdf:resource="http://www.buildingsmart-tech.org/ifcOWL/IFC4_ADD2#IfcWallEnumType"/>
    </owl:Class>
    


    <!-- https://pi.pauwel.be/voc/buildingelement#Wall-SHEAR -->

    <owl:Class rdf:about="https://pi.pauwel.be/voc/buildingelement#Wall-SHEAR">
        <rdfs:subClassOf rdf:resource="https://pi.pauwel.be/voc/buildingelement#Wall"/>
        <rdfs:comment xml:lang="en">http://bsdd.buildingsmart.org/#concept/details/0MAk1miOTAJQpI0VGyMnjS</rdfs:comment>
        <rdfs:label xml:lang="en">Shear Wall</rdfs:label>
        <rdfs:label xml:lang="nb-no">skive</rdfs:label>
        <rdfs:seeAlso rdf:resource="http://www.buildingsmart-tech.org/ifcOWL/IFC4_ADD2#IfcWallEnumType"/>
    </owl:Class>
    


    <!-- https://pi.pauwel.be/voc/buildingelement#Wall-SOLIDWALL -->

    <owl:Class rdf:about="https://pi.pauwel.be/voc/buildingelement#Wall-SOLIDWALL">
        <rdfs:subClassOf rdf:resource="https://pi.pauwel.be/voc/buildingelement#Wall"/>
        <rdfs:comment xml:lang="en">http://bsdd.buildingsmart.org/#concept/details/2J1xt_ADz7heqvTyh5YGEM</rdfs:comment>
        <rdfs:label xml:lang="en">Solid Wall</rdfs:label>
        <rdfs:label xml:lang="nb-no">massiv vegg</rdfs:label>
        <rdfs:seeAlso rdf:resource="http://www.buildingsmart-tech.org/ifcOWL/IFC4_ADD2#IfcWallEnumType"/>
    </owl:Class>
    


    <!-- https://pi.pauwel.be/voc/buildingelement#Wall-STANDARD -->

    <owl:Class rdf:about="https://pi.pauwel.be/voc/buildingelement#Wall-STANDARD">
        <rdfs:subClassOf rdf:resource="https://pi.pauwel.be/voc/buildingelement#Wall"/>
        <rdfs:comment xml:lang="en">http://bsdd.buildingsmart.org/#concept/details/2HWHt8Yiz4m9UzhlqVFLeO</rdfs:comment>
        <rdfs:label xml:lang="en">Standard Wall</rdfs:label>
        <rdfs:seeAlso rdf:resource="http://www.buildingsmart-tech.org/ifcOWL/IFC4_ADD2#IfcWallEnumType"/>
    </owl:Class>
    


    <!-- https://pi.pauwel.be/voc/buildingelement#WallElementedCase -->

    <owl:Class rdf:about="https://pi.pauwel.be/voc/buildingelement#WallElementedCase">
        <rdfs:subClassOf rdf:resource="https://pi.pauwel.be/voc/buildingelement#Wall"/>
        <rdfs:comment xml:lang="en">A wall with certain constraints for the provision of its components.</rdfs:comment>
        <rdfs:comment xml:lang="en">http://bsdd.buildingsmart.org/#concept/details/2dG9W0qXKHuO00025QrE$V</rdfs:comment>
        <rdfs:label xml:lang="en">Elemented Wall Case</rdfs:label>
        <rdfs:label xml:lang="fr-fr">Mur composite</rdfs:label>
        <rdfs:label xml:lang="de-de">Wand elementiert</rdfs:label>
        <rdfs:seeAlso rdf:resource="http://www.buildingsmart-tech.org/ifcOWL/IFC4_ADD2#IfcWallElementedCase"/>
    </owl:Class>
    


    <!-- https://pi.pauwel.be/voc/buildingelement#Window -->

    <owl:Class rdf:about="https://pi.pauwel.be/voc/buildingelement#Window">
        <rdfs:subClassOf rdf:resource="https://pi.pauwel.be/voc/buildingelement#BuildingElement"/>
        <rdfs:comment xml:lang="pt-br">Abertura destinada a iluminar e ventilar os ambientes internos, além de facilitar a visão do exterior.</rdfs:comment>
        <rdfs:comment xml:lang="de-de">Bauteil zum Schließen einer Öffnung in einer Wand oder Satteldach, das Licht durchlassen und Belüftung ermöglichen kann</rdfs:comment>
        <rdfs:comment xml:lang="en">building component for closing an opening in a wall or pitched roof that will admit light and may provide ventilation</rdfs:comment>
        <rdfs:comment xml:lang="en-gb">building component for closing an opening in a wall or pitched roof that will admit light and may provide ventilation</rdfs:comment>
        <rdfs:comment xml:lang="sv-se">byggelement som används för att stänga en öppning i en vägg eller ett sadeltak som kan släppa in ljus och bidra med ventilation</rdfs:comment>
        <rdfs:comment xml:lang="it-it">componente costruttivo atto a chiudere un&apos;apertura in un muro o in un tetto a spiovente che ammetta la luce e possa fornire ventilazione</rdfs:comment>
        <rdfs:comment xml:lang="es-es">componente de construcción para cerrar una abertura en una pared o techo a dos aguas que deja pasar la luz y puede proporcionar ventilación</rdfs:comment>
        <rdfs:comment xml:lang="en">construction for closing a vertical or near-vertical opening in a wall or pitched roof which will admit light and may provide ventilation. Often a pane of glass framed and mounted to permit opening and closing</rdfs:comment>
        <rdfs:comment xml:lang="en-gb">construction for closing a vertical or near-vertical opening in a wall or pitched roof which will admit light and may provide ventilation. Often a pane of glass framed and mounted to permit opening and closing</rdfs:comment>
        <rdfs:comment xml:lang="nn-no">ein konstruksjon som står i ei opning som i ein vegg eller tak og som normalt er dekt av glas, med det føremålet å sleppa inn lys og luft. | konstruksjon for *lukking av ein vertikal eller nesten vertikal opning i ein vegg eller eit skråtak som skal sleppa igjennom lys kan gje ventilasjon. Ofte ei glasrute *innrammet og montert for å gjera muleg opning og lukking</rdfs:comment>
        <rdfs:comment xml:lang="pl-pl">element budynku służący do zamykania i otwierania, osadzony w ścianie lub w dachu dwuspadowym, przepuszczający światło i mogący zapewniać wentylację</rdfs:comment>
        <rdfs:comment xml:lang="nb-no">en konstruksjon som står i en åpning som i en vegg eller tak og som normalt er dekket av glass, med det formål å slippe inn lys og luft.</rdfs:comment>
        <rdfs:comment xml:lang="en">http://bsdd.buildingsmart.org/#concept/details/3vHUaooT0Hsm00051Mm008</rdfs:comment>
        <rdfs:comment xml:lang="nb-no">konstruksjon for lukking av en vertikal eller nesten vertikal åpning i en vegg eller et skråtak som skal slippe igjennom lys kan gi ventilasjon. Ofte en glassrute innrammet og montert for å muliggjøre åpning og lukking</rdfs:comment>
        <rdfs:comment xml:lang="dk-dk">konstruktion til lukning af en lodret eller næsten lodret åbning i en mur eller skråt tag, der lader lys trænge igennem og kan muliggøre ventilation. Ofte en rude i en karm og monteret, så den kan åbnes og lukkes</rdfs:comment>
        <rdfs:comment xml:lang="fi-fi">seinä- tai kattoaukon sulkeva, valoa läpipäästävä rakenneosa varustettuna mahdollisin ilmanvaihto-ominaisuuksin</rdfs:comment>
        <rdfs:comment xml:lang="fr-fr">une construction destinée à fermer une ouverture verticale ou quasi-verticale dans un mur ou un toit en pente qui laissera passer la lumière et pourra fournir une ventilation. souvent constituée d&apos;un panneau vitré monté sur un châssis permettant son ouverture et sa fermeture.</rdfs:comment>
        <rdfs:comment xml:lang="bg-bg">строителен компонент за затваряне на отвор в стена или скатен покрив, който служи за осветяване и евентуално за проветряване</rdfs:comment>
        <rdfs:label xml:lang="de-de">Fenster</rdfs:label>
        <rdfs:label xml:lang="nl">Raam</rdfs:label>
        <rdfs:label xml:lang="nl-nl">Raam</rdfs:label>
        <rdfs:label xml:lang="da">Vindue</rdfs:label>
        <rdfs:label xml:lang="en">Window</rdfs:label>
        <rdfs:label xml:lang="fr-fr">fenêtre</rdfs:label>
        <rdfs:label xml:lang="it-it">finestra</rdfs:label>
        <rdfs:label xml:lang="sv-se">fönster</rdfs:label>
        <rdfs:label xml:lang="fi-fi">ikkuna</rdfs:label>
        <rdfs:label xml:lang="pt-br">janela</rdfs:label>
        <rdfs:label xml:lang="pl-pl">okna</rdfs:label>
        <rdfs:label xml:lang="es-es">ventana</rdfs:label>
        <rdfs:label xml:lang="nn-no">vindauge</rdfs:label>
        <rdfs:label xml:lang="nb-no">vindu</rdfs:label>
        <rdfs:label xml:lang="dk-dk">vindue</rdfs:label>
        <rdfs:label xml:lang="en-gb">window</rdfs:label>
        <rdfs:label xml:lang="en">windowset</rdfs:label>
        <rdfs:label xml:lang="bg-bg">прозорец</rdfs:label>
        <rdfs:label xml:lang="ar-sa">نافذة</rdfs:label>
        <rdfs:label xml:lang="ja-jp">窓</rdfs:label>
        <rdfs:seeAlso rdf:resource="http://www.buildingsmart-tech.org/ifcOWL/IFC4_ADD2#IfcWindow"/>
    </owl:Class>
    


    <!-- https://pi.pauwel.be/voc/buildingelement#Window-LIGHTDOME -->

    <owl:Class rdf:about="https://pi.pauwel.be/voc/buildingelement#Window-LIGHTDOME">
        <rdfs:subClassOf rdf:resource="https://pi.pauwel.be/voc/buildingelement#Window"/>
        <rdfs:comment xml:lang="en">a special window that lies horizonally in a roof slab opening</rdfs:comment>
        <rdfs:comment xml:lang="en">http://bsdd.buildingsmart.org/#concept/details/3aXmro5wX3FeEqYU7Y7w5X</rdfs:comment>
        <rdfs:label xml:lang="en">Light dome</rdfs:label>
        <rdfs:label xml:lang="nb-no">lyskuppel</rdfs:label>
        <rdfs:seeAlso rdf:resource="http://www.buildingsmart-tech.org/ifcOWL/IFC4_ADD2#IfcWindowEnumType"/>
    </owl:Class>
    


    <!-- https://pi.pauwel.be/voc/buildingelement#Window-SKYLIGHT -->

    <owl:Class rdf:about="https://pi.pauwel.be/voc/buildingelement#Window-SKYLIGHT">
        <rdfs:subClassOf rdf:resource="https://pi.pauwel.be/voc/buildingelement#Window"/>
        <rdfs:comment xml:lang="nb-no">Overlys</rdfs:comment>
        <rdfs:comment xml:lang="en">construction for closing an opening in a flat roof or low pitched roof, intended primarily for lighting and consisting of a frame and glazing</rdfs:comment>
        <rdfs:comment xml:lang="en">http://bsdd.buildingsmart.org/#concept/details/1irgDncIrAVQwjja3JEbnb</rdfs:comment>
        <rdfs:label xml:lang="nl-nl">Daklicht</rdfs:label>
        <rdfs:label xml:lang="en">Skylight</rdfs:label>
        <rdfs:label xml:lang="nb-no">overlys</rdfs:label>
        <rdfs:seeAlso rdf:resource="http://www.buildingsmart-tech.org/ifcOWL/IFC4_ADD2#IfcWindowEnumType"/>
    </owl:Class>
    


    <!-- https://pi.pauwel.be/voc/buildingelement#Window-WINDOW -->

    <owl:Class rdf:about="https://pi.pauwel.be/voc/buildingelement#Window-WINDOW">
        <rdfs:subClassOf rdf:resource="https://pi.pauwel.be/voc/buildingelement#Window"/>
        <rdfs:comment xml:lang="en">A building element that is predominately used to provide natural light and fresh air. It includes vertical opening but also horizontal opening such as skylights or light domes. It includes constructions with swinging, pivoting, sliding, or revolving panels and fixed panels. A window consists of a lining and one or several panels.
NOTE  Definition according to ISO 6707-1
Construction for closing a vertical or near vertical opening in a wall or pitched roof that will admit light and may admit fresh air.</rdfs:comment>
        <rdfs:comment xml:lang="pt-br">Abertura destinada a iluminar e ventilar os ambientes internos, além de facilitar a visão do exterior.</rdfs:comment>
        <rdfs:comment xml:lang="de-de">Bauteil zum Schließen einer Öffnung in einer Wand oder Satteldach, das Licht durchlassen und Belüftung ermöglichen kann</rdfs:comment>
        <rdfs:comment xml:lang="nl-nl">Een raam is een constructie met een scheidingsfunctie en een lichttoetredingsfunctie.</rdfs:comment>
        <rdfs:comment xml:lang="en">building component for closing an opening in a wall or pitched roof that will admit light and may provide ventilation</rdfs:comment>
        <rdfs:comment xml:lang="en-gb">building component for closing an opening in a wall or pitched roof that will admit light and may provide ventilation</rdfs:comment>
        <rdfs:comment xml:lang="sv-se">byggelement som används för att stänga en öppning i en vägg eller ett sadeltak som kan släppa in ljus och bidra med ventilation</rdfs:comment>
        <rdfs:comment xml:lang="it-it">componente costruttivo atto a chiudere un&apos;apertura in un muro o in un tetto a spiovente che ammetta la luce e possa fornire ventilazione</rdfs:comment>
        <rdfs:comment xml:lang="es-es">componente de construcción para cerrar una abertura en una pared o techo a dos aguas que deja pasar la luz y puede proporcionar ventilación</rdfs:comment>
        <rdfs:comment xml:lang="en">construction for closing a vertical or near-vertical opening in a wall or pitched roof which will admit light and may provide ventilation. Often a pane of glass framed and mounted to permit opening and closing</rdfs:comment>
        <rdfs:comment xml:lang="en-gb">construction for closing a vertical or near-vertical opening in a wall or pitched roof which will admit light and may provide ventilation. Often a pane of glass framed and mounted to permit opening and closing</rdfs:comment>
        <rdfs:comment xml:lang="nn-no">ein konstruksjon som står i ei opning som i ein vegg eller tak og som normalt er dekt av glas, med det føremålet å sleppa inn lys og luft. | konstruksjon for *lukking av ein vertikal eller nesten vertikal opning i ein vegg eller eit skråtak som skal sleppa igjennom lys kan gje ventilasjon. Ofte ei glasrute *innrammet og montert for å gjera muleg opning og lukking</rdfs:comment>
        <rdfs:comment xml:lang="pl-pl">element budynku służący do zamykania i otwierania, osadzony w ścianie lub w dachu dwuspadowym, przepuszczający światło i mogący zapewniać wentylację</rdfs:comment>
        <rdfs:comment xml:lang="nb-no">en konstruksjon som står i en åpning som i en vegg eller tak og som normalt er dekket av glass, med det formål å slippe inn lys og luft.</rdfs:comment>
        <rdfs:comment xml:lang="en">http://bsdd.buildingsmart.org/#concept/details/3QkFVA4cD3YvP3Y3zVGFc3</rdfs:comment>
        <rdfs:comment xml:lang="nb-no">konstruksjon for lukking av en vertikal eller nesten vertikal åpning i en vegg eller et skråtak som skal slippe igjennom lys kan gi ventilasjon. Ofte en glassrute innrammet og montert for å muliggjøre åpning og lukking</rdfs:comment>
        <rdfs:comment xml:lang="dk-dk">konstruktion til lukning af en lodret eller næsten lodret åbning i en mur eller skråt tag, der lader lys trænge igennem og kan muliggøre ventilation. Ofte en rude i en karm og monteret, så den kan åbnes og lukkes</rdfs:comment>
        <rdfs:comment xml:lang="sv-se">objekt för tillträde till utrymme för enbart ljus</rdfs:comment>
        <rdfs:comment xml:lang="fi-fi">seinä- tai kattoaukon sulkeva, valoa läpipäästävä rakenneosa varustettuna mahdollisin ilmanvaihto-ominaisuuksin</rdfs:comment>
        <rdfs:comment xml:lang="en">space access object for light entry only</rdfs:comment>
        <rdfs:comment xml:lang="fr-fr">une construction destinée à fermer une ouverture verticale ou quasi-verticale dans un mur ou un toit en pente qui laissera passer la lumière et pourra fournir une ventilation. souvent constituée d&apos;un panneau vitré monté sur un châssis permettant son ouverture et sa fermeture.</rdfs:comment>
        <rdfs:comment xml:lang="bg-bg">строителен компонент за затваряне на отвор в стена или скатен покрив, който служи за осветяване и евентуално за проветряване</rdfs:comment>
        <rdfs:label xml:lang="de-de">Fenster</rdfs:label>
        <rdfs:label xml:lang="nl-nl">Raam</rdfs:label>
        <rdfs:label>Window</rdfs:label>
        <rdfs:label xml:lang="de-ch">fenster</rdfs:label>
        <rdfs:label xml:lang="fr-fr">fenêtre</rdfs:label>
        <rdfs:label xml:lang="it-it">finestra</rdfs:label>
        <rdfs:label xml:lang="sv-se">fönster</rdfs:label>
        <rdfs:label xml:lang="fi-fi">ikkuna</rdfs:label>
        <rdfs:label xml:lang="pt-br">janela</rdfs:label>
        <rdfs:label xml:lang="pl-pl">okna</rdfs:label>
        <rdfs:label xml:lang="es-es">ventana</rdfs:label>
        <rdfs:label xml:lang="nn-no">vindauge</rdfs:label>
        <rdfs:label xml:lang="nb-no">vindu</rdfs:label>
        <rdfs:label xml:lang="dk-dk">vindue</rdfs:label>
        <rdfs:label xml:lang="en-gb">window</rdfs:label>
        <rdfs:label xml:lang="bg-bg">прозорец</rdfs:label>
        <rdfs:label xml:lang="ar-sa">نافذة</rdfs:label>
        <rdfs:label xml:lang="ja-jp">窓</rdfs:label>
        <rdfs:seeAlso rdf:resource="http://www.buildingsmart-tech.org/ifcOWL/IFC4_ADD2#IfcWindowEnumType"/>
    </owl:Class>
    


    <!-- https://schema.org/Product -->

    <owl:Class rdf:about="https://schema.org/Product"/>
    


    <!-- https://w3id.org/bot#Building -->

    <owl:Class rdf:about="https://w3id.org/bot#Building">
        <rdfs:subClassOf rdf:resource="https://w3id.org/bot#Zone"/>
        <rdfs:subClassOf>
            <owl:Restriction>
                <owl:onProperty rdf:resource="http://www.semanticweb.org/arnak/ontologies/2022/7/DOR#hasFunctionalLayer"/>
                <owl:someValuesFrom rdf:resource="http://www.semanticweb.org/arnak/ontologies/2022/7/DOR#FunctionalLayer"/>
            </owl:Restriction>
        </rdfs:subClassOf>
        <owl:disjointWith rdf:resource="https://w3id.org/bot#Element"/>
        <owl:disjointWith rdf:resource="https://w3id.org/bot#Interface"/>
        <owl:disjointWith rdf:resource="https://w3id.org/bot#Site"/>
        <owl:disjointWith rdf:resource="https://w3id.org/bot#Space"/>
        <owl:disjointWith rdf:resource="https://w3id.org/bot#Storey"/>
        <rdfs:comment xml:lang="en">An independent unit of the built environment with a characteristic spatial structure, intended to serve at least one function or user activity [ISO 12006-2:2013]. A bot:Building is a part of the physical world or a virtual world that is inherently both located in this world and having a 3D spatial extent, is contained in a building site, and can contain one or more storeys that are vertically connected.</rdfs:comment>
        <rdfs:comment xml:lang="tr">Bir yapılı ortamına sahip, ve karakteri mekansal olan ve en az bir funksiyona veya kullanıcı etkinligini desteleyen bir bağımsız parcadir. </rdfs:comment>
        <rdfs:comment xml:lang="nl">Een onafhankelijke entiteit met een ruimtelijke structuur die onderdeel is van de gebouwde omgeving, en bedoeld is om minimaal één functie of gebruikersactiviteit te bedienen [ISO 12006-2:2013]. Een bot:Building is deel van de fysieke wereld of een virtuele wereld dat zowel gelokaliseerd kan worden in deze wereld als een ruimtelijke omvang heeft, is deel van een gebouwsite, en kan één of meerder verdiepingen bevatten die verticaal verbonden zijn.</rdfs:comment>
        <rdfs:comment xml:lang="de">Eine eigenständige Einheit der bebauten Umgebung mit einer charakteristischen räumlichen Struktur. Es besteht die Absicht das es eine Funktion oder Nutzung erlaubt [ISO 12006-2:2013]. Ein bot:Building ist Teil der realen und virtuellen Welt und hat eine räumliche Ausdehnung. Es ist enthalten in einem Grundstück und kann ein oder mehrere Stockwerke enthalten, die vertical miteinander verbunden sind.</rdfs:comment>
        <rdfs:comment xml:lang="sv">En oberoende enhet i den byggda miljön med en karaktäristisk rumslig struktur som stödjer minst en funktion eller användaraktivitet.  [ISO 12006-2:2013]. En bot:Building är en del av den fysiska världen eller en virtuell värld som har en spatial utsträckning i tre dimensioner, ligger på en plats, och kan ha en eller flera vertikalt förbundna våningar.</rdfs:comment>
        <rdfs:comment xml:lang="da">En uafhængig enhed i det bebyggede miljø med en karakteristisk rumlig struktur, beregnet til at betjene mindst en funktion eller brugeraktivitet [ISO 12006-2: 2013]. En bot:Building er en del af den fysiske verden eller en virtuel verden, der i sagens natur både er lokaliseret i denne verden og har en 3D rumlig afgrænsning, er indeholdt på et byggefelt og kan indeholde en eller flere etager, der er lodret forbundet.</rdfs:comment>
        <rdfs:comment xml:lang="sk">Nezávislá jednotka v (stavebnom) prostredí či verejnom priestore, s charakteristickou priestorovou štruktúrou a formou, ktorá má slúžiť aspoň pre jednu činnosť alebo funkciu uživateľa [ISO 12006-2:2013]. Bot:Building je súčasťou fyzického alebo virtuálneho sveta, ktorý je neodmyslitelnľ umiestnľný ako vo fyzickom svete, tak má 3D virtuálny priestorový rozsah, je umiestnený na stavenisku (&quot;Site&quot;) a môže obsahovať jedno alebo viac podlaží, ktoré sú vertikálne prepojené. </rdfs:comment>
        <rdfs:comment xml:lang="cs">Nezávislá jednotka v (stavebním) prostředí či veřejném prostoru, s charakteristickou prostorovou strukturou a formou, která má sloužit alespoň pro jednu činnost nebo funkci uživatele [ISO 12006-2: 2013]. 
Bot:Building je součástí fyzického nebo virtuálního světa, který je neodmyslitelně umístěn jak ve fyzickém světě, tak má 3D virtuální prostorový rozsah, je umístěn na staveništi (&quot;Site&quot;) a může obsahovat jedno nebo víc podlaží, která jsou vertikálně propojena. </rdfs:comment>
        <rdfs:comment xml:lang="fi">Rakennetun ympäristön itsenäinen osa, jolla on ominainen avaruudellinen rakenne, ja joka on tarkoitettu palvelemaan ainakin yhtä funktiota tai käyttäjäaktiviteettia [ISO 12006-2:2013]. bot:Building on fyysisen tai virtuaalisen maailman osa, joka luonnostaan sekä sijaitsee tässä maailmassa että omaa kolmiulotteiset tilalliset ulottuvuudet, sijaitsee tontilla, ja se voi sisältää yhden tai useamman kerroksen jotka ovat pystysuunnassa yhteydessä.</rdfs:comment>
        <rdfs:comment xml:lang="pt">Uma unidade independente do ambiente construído com uma estrutura espacial característica, destinada a servir pelo menos uma função do utilizador [ISO 12006-2:2013].
Um bot:Building é uma parte do mundo físico ou do mundo virtual que está inerentemente localizado neste mundo e que tem uma extensão espacial tridimensional, que está contido num sítio de construção e que contém um ou mais pisos que estão conectados verticalmente.</rdfs:comment>
        <rdfs:comment xml:lang="it">Un&apos;unità indipendente dell&apos;ambiente costruito con una struttura spaziale caratteristica, destinato a servire almeno una funzione o attività degli utenti [ISO 12006-2:2013]. Un bot:Building è parte del mondo fisico o virtuale che si trova intrinsecamente in questo mondo e ha una estensione spaziale tridimensionale, è contenuto in un sito e può contenere uno o più piani che sono connessi verticalmente.</rdfs:comment>
        <rdfs:comment xml:lang="fr">Une unité indépendante de l&apos;environnement bâti avec une structure spatiale caractéristique, conçue pour répondre à une fonction ou une activité de l&apos;utilisateur [ISO 12006-2:2013]</rdfs:comment>
        <rdfs:comment xml:lang="es">Unidad independiente del entorno construido con una estructura espacial característica, destinada a servir al menos una función o actividad del usuario [ISO 12006-2: 2013]. Un bot:Building es tanto una parte del mundo físico o virtual que se encuentra inherentemente situado en este mundo y que tiene una extensión espacial 3D, se encuentra en un emplazamiento de edificación, y puede contener uno o más pisos conectados verticalmente.</rdfs:comment>
        <rdfs:comment xml:lang="ca">Unitat independent de l’entorn construït amb una estructura espacial característica, destinada a servir almenys una funció o activitat de l’usuari [ISO 12006-2: 2013]. Un bot:Building és tant una part del món físic o virtual que es troba inherentment situat en aquest món i que té una extensió espacial 3D, es troba en un emplaçament d’edificació, i pot contenir un o més pisos connectats verticalment.</rdfs:comment>
        <rdfs:comment xml:lang="fa">یک واحد مستقل با ساختار مکانی مشخص از محیط ساخت وساز، که برای ارایه‌ی حداقل یک عملکرد یا فعالیت کاربری در نظرگرفته شده است [ISO 12006-2:2013]. یک bot:Building یک بخش از دنیای فیزیکی یا یک دنیای مجازی است که اساسا در این دنیا قرار دارد و دارای حدود مکانی سه بعدی است، دریک سایت ساختمان قرار گرفته ، و میتواند دربرگیرنده‌ی یک یا چند طبقه باشد که به صورت عمودی به هم متصل شده اند.</rdfs:comment>
        <rdfs:comment xml:lang="zh-cn">具有特定空间结构的建筑环境独立单元，旨在服务至少一种功能或用户活动[ISO 12006-2：2013]。 bot:Building是物理或虚拟世界的一部分，其既存在于其中，又具有3D空间范围。bot:Building包含在建筑工地中，并且可以包含一个或多个垂直连接的楼层。</rdfs:comment>
        <rdfs:isDefinedBy rdf:resource="https://w3id.org/bot#"/>
        <rdfs:label xml:lang="tr">Bina</rdfs:label>
        <rdfs:label xml:lang="cs">Budova</rdfs:label>
        <rdfs:label xml:lang="sk">Budova</rdfs:label>
        <rdfs:label xml:lang="en">Building</rdfs:label>
        <rdfs:label xml:lang="sv">Byggnad</rdfs:label>
        <rdfs:label xml:lang="da">Bygning</rdfs:label>
        <rdfs:label xml:lang="fr">Bâtiment</rdfs:label>
        <rdfs:label xml:lang="ca">Edifici</rdfs:label>
        <rdfs:label xml:lang="es">Edificio</rdfs:label>
        <rdfs:label xml:lang="it">Edificio</rdfs:label>
        <rdfs:label xml:lang="pt">Edifício</rdfs:label>
        <rdfs:label xml:lang="nl">Gebouw</rdfs:label>
        <rdfs:label xml:lang="de">Gebäude</rdfs:label>
        <rdfs:label xml:lang="fi">Rakennus</rdfs:label>
        <rdfs:label xml:lang="fa">ساختمان</rdfs:label>
        <rdfs:label xml:lang="zh-cn">建筑</rdfs:label>
        <ns:term_status>stable</ns:term_status>
    </owl:Class>
    


    <!-- https://w3id.org/bot#Element -->

    <owl:Class rdf:about="https://w3id.org/bot#Element">
        <owl:disjointWith rdf:resource="https://w3id.org/bot#Interface"/>
        <owl:disjointWith rdf:resource="https://w3id.org/bot#Site"/>
        <owl:disjointWith rdf:resource="https://w3id.org/bot#Space"/>
        <owl:disjointWith rdf:resource="https://w3id.org/bot#Storey"/>
        <owl:disjointWith rdf:resource="https://w3id.org/bot#Zone"/>
        <rdfs:comment xml:lang="tr">&quot;Karakteristik fonksiyonu, şekli veya konumu olan bir binanın bileşeni [ISO 12006-2: 2015, 3.4.7]</rdfs:comment>
        <rdfs:comment xml:lang="de">Bauteile bestehen aus mehreren Komponenten.</rdfs:comment>
        <rdfs:comment xml:lang="nl">Bestanddeel van een gebouwde entiteit met een karakteristieke technische functie, vorm of positie [ISO 12006-2:2015, 3.4.7]</rdfs:comment>
        <rdfs:comment xml:lang="da">Bestanddel af et bygværk med en karakteristisk funktion, form eller position [ISO 12006-2:2015, 3.4.7]</rdfs:comment>
        <rdfs:comment xml:lang="sv">Beståndsdel av ett byggnadsverk med en karaktäristisk teknisk funktion, form eller position [ISO 12006-2:2015, 3.4.7]</rdfs:comment>
        <rdfs:comment xml:lang="fr">Constituant d&apos;un bâtiment remplissant une fonction technique spécifique ou ayant une forme ou une position spécifiques [ISO 12006-2:2015, 3.4.7]</rdfs:comment>
        <rdfs:comment xml:lang="ca">Constituent d&apos;una entitat de construcció amb una funció tècnica característica, forma o posició [ISO 12006-2:2015, 3.4.7]</rdfs:comment>
        <rdfs:comment xml:lang="en">Constituent of a construction entity with a characteristic technical function, form or position [ISO 12006-2:2015, 3.4.7]</rdfs:comment>
        <rdfs:comment xml:lang="pt">Constituinte de uma entidade de construção com uma função técnica característica, forma ou posição [ISO 12006-2:2015, 3.4.7]</rdfs:comment>
        <rdfs:comment xml:lang="es">Constituyente de una entidad de construcción con una función técnica característica, forma o posición [ISO 12006-2:2015, 3.4.7]</rdfs:comment>
        <rdfs:comment xml:lang="it">Costituente di una entità costruttiva con una funzione tecnica caratteristica, forma o posizione [ISO 12006-2:2015, 3.4.7]</rdfs:comment>
        <rdfs:comment xml:lang="de">Das Bauteil ist im Bauwesen ein einzelnes Teil, ein Element oder eine Komponente, aus denen ein Bauwerk zusammengesetzt wird [ISO 12006-2:2015, 3.4.7]</rdfs:comment>
        <rdfs:comment xml:lang="fi">Rakennetun kokonaisuuden osa, jolla on ominainen tekninen funktio, muoto tai sijainti [ISO 12006-2:2015, 3.4.7]</rdfs:comment>
        <rdfs:comment xml:lang="cs">Součást stavební entity s charakteristickou technickou funkcí, formou, nebo umístěním [ISO 12006-2, 3.4.7]</rdfs:comment>
        <rdfs:comment xml:lang="sk">Súčasť stavebnej entity s charakteristickou funkciou, formou, alebo umestením [ISO 12006-2, 3.4.7]</rdfs:comment>
        <rdfs:comment xml:lang="fa">تشکیل دهنده‌ی یک واحد ساخت با عملکرد فنی، فرم و یا موقعیت   مشخص.</rdfs:comment>
        <rdfs:comment xml:lang="zh-cn">具有特定技术功能，形式或位置的建筑实体组成部分</rdfs:comment>
        <rdfs:isDefinedBy rdf:resource="https://w3id.org/bot#"/>
        <rdfs:label xml:lang="de">Bauteil (Bauwesen)</rdfs:label>
        <rdfs:label xml:lang="tr">Bina elemanı</rdfs:label>
        <rdfs:label xml:lang="en">Building element</rdfs:label>
        <rdfs:label xml:lang="sv">Byggdel</rdfs:label>
        <rdfs:label xml:lang="da">Bygningsdel</rdfs:label>
        <rdfs:label xml:lang="ca">Element de construcció</rdfs:label>
        <rdfs:label xml:lang="pt">Elemento arquitectónico</rdfs:label>
        <rdfs:label xml:lang="es">Elemento de construcción</rdfs:label>
        <rdfs:label xml:lang="it">Elemento di costruzione</rdfs:label>
        <rdfs:label xml:lang="fi">Elementti</rdfs:label>
        <rdfs:label xml:lang="nl">Gebouwelement</rdfs:label>
        <rdfs:label xml:lang="cs">Stavební prvek</rdfs:label>
        <rdfs:label xml:lang="sk">Stavebný prvok</rdfs:label>
        <rdfs:label xml:lang="fr">Élément d&apos;un bâtiment</rdfs:label>
        <rdfs:label xml:lang="fa">المان</rdfs:label>
        <rdfs:label xml:lang="zh-cn">构件</rdfs:label>
        <ns:term_status>stable</ns:term_status>
    </owl:Class>
    


    <!-- https://w3id.org/bot#Interface -->

    <owl:Class rdf:about="https://w3id.org/bot#Interface">
        <owl:disjointWith rdf:resource="https://w3id.org/bot#Site"/>
        <owl:disjointWith rdf:resource="https://w3id.org/bot#Space"/>
        <owl:disjointWith rdf:resource="https://w3id.org/bot#Storey"/>
        <owl:disjointWith rdf:resource="https://w3id.org/bot#Zone"/>
        <rdfs:comment xml:lang="en">A generic concept to qualify the relationship of two or more things in the world, where at least one is a building element or zone. Examples:
    - Qualification of heat transmission between zones through one or more building elements. This includes one-dimensional (surface) heat losses from one zone to another through a single building element, a two dimensional (line) loss from one zone to another through the connection in which the two elements meet or a three dimensional (point) loss from one zone to another through the connection where three elements (typically two walls and a slab) meet. 
    - Connection of an electric device to the electric system of a building. 
    - A door between one room and another.</rdfs:comment>
        <rdfs:comment xml:lang="tr">Arayüz, iki bina parçası, iki bölge veya bir bina parçası ile bir bölgenin buluştuğu alandır. İkisi arasındaki bağlantıyı nitelendirmek için kullanılabilir. Bir kullanım durumu, bir bölge ve birkaç bölgeyi kapsayan bir duvar arasındaki ısı transfer alanının niteliği olabilir.</rdfs:comment>
        <rdfs:comment xml:lang="pt">Conceito genérico para qualificar a relação entre duas ou mais coisas no mundo, onde pelo menos uma é um elemento de edifício ou uma zona. Exemplos:
- Qualificação de transmissão de calor entre zonas através de um ou mais elementos do edifício. Isto inclui perdas de calor unidimensionais (superfície) de uma zona para outra através de um único elemento do edifício, uma perda bidimensional (linha) de uma zona para outra através da conexão onde os dois elementos se encontram ou uma perda tridimensional (ponto) de uma zona para outra através da conexão onde três elementos se encontram (tipicamente duas paredes e uma laje).
- Conexão de um equipamento eléctrico ao sistema eléctrico de um edifício.
- Uma porta entre dois compartimentos.</rdfs:comment>
        <rdfs:comment xml:lang="ca">Concepte genèric per qualificar la relació de dues o més coses del món, on almenys una d&apos;elles és un element o zona constructiva. 
Exemples:
- Qualificació de la transmissió de calor entre zones a través d’un o més elements d’edificació. Això inclou pèrdues de calor (superficials) unidimensionals d&apos;una zona a una altra mitjançant un element de construcció, una pèrdua bidireccional (en línia) d&apos;una zona a una altra mitjançant la connexió en què es troben els dos elements, o una pèrdua tridimensional (en un punt) d’una zona a una altra mitjançant la connexió on es reuneixen tres elements (normalment dues parets i una llosa).
- Connexió d’un dispositiu elèctric al sistema elèctric d’un edifici.
- Una porta entre una habitació i una altra.</rdfs:comment>
        <rdfs:comment xml:lang="es">Concepto genérico para calificar la relación de dos o más cosas en el mundo, donde al menos una es un elemento o zona de construcción. 
Ejemplos:
- Calificación de la transmisión de calor entre zonas a través de uno o más elementos de construcción. Esto incluye pérdidas de calor unidimensionales (de superficie) de una zona a otra a través de un único elemento de construcción, una pérdida bidimensional (línea) de una zona a otra a través de la conexión en la que los dos elementos se encuentran, o una pérdida tridimensional de una zona a otra a través de la conexión donde se encuentran tres elementos (típicamente dos paredes y una losa).
- Conexión de un dispositivo eléctrico al sistema eléctrico de un edificio.
- Una puerta entre una habitación y otra.</rdfs:comment>
        <rdfs:comment xml:lang="it">Concetto generico per caratterizzare la relazione fra due o più cose nel mondo, dove almeno una di queste è un elemento di costruzione o una zona. Esempi:
 - La certificazione della trasmissione di calore tra zone attraverso uno o più elementi di costruzione. Questo include la dispersione termica unidimensionale (superficie) da una zona ad un&apos;altra attraverso un singolo elemento di costruzione, un dispersione bidimensionale (linea) da una zona ad un&apos;altra attraverso la connessione dove i due elementi si incontrano, una dispersione tridimensionale (punto) da una zona ad un&apos;altra attraverso la connessione dove tre elementi (tipicamente due pareti e una soletta) si incontrano.
 - Connessione di un dispositivo elettrico con un impianto elettrico di un edificio.
 - Una porta tra una stanza e un&apos;altra.</rdfs:comment>
        <rdfs:comment xml:lang="nl">Een generiek concept om een kwalificeerbare relatie te creëren tussen twee of meer dingen uit de wereld, waarbij er minstens één een gebouwelement of zone is. Voorbeelden:
     - kwalificeren van de warmte transmissie tussen gebouw zones doorheen één of meerdere gebouwelementen. Dit omvat ééndimensionele (oppervlakte) warmteverliezen van één zone naar een andere zone doorheen een gebouwelement, tweedimensionele (lijn) verliezen van één zone naar een andere zone doorheen de connectie tussen twee gebouwelementen of driedimensionele (punt) verliezen van één zone naar een andere zone doorheen de connectie tussen drie gebouwelementen (typisch twee muren en een vloer- of dakplaat).
     - Connectie tussen een elektrisch toestel en het elektrisch systeem van een gebouw.
     - Een deur tussen twee ruimtes</rdfs:comment>
        <rdfs:comment xml:lang="de">Ein allgemeines Konzept um eine qualifizierte Beziehung zwischen einem oder mehreren Dingen auf der Welt auszudrücken. Hierbei ist wenigstens eines der Dinge ein Bauteil oder eine Zone eines Gebäudes. Beispiele: - Qualifizierung des Wärmeübergangs durch ein oder mehrere Bauteile. Dies umfasst eindimensionale Wärmeübertragung (Fläche) durch ein Bauteil von einer Zone zur nächsten; zweidimensionaler Wärmeübergang (Linie) von einer Zone zur nächsten an der Kontaktstelle, an der sich diese treffen oder dreidimensional (Punkt) von einer zone zur nächsten an der drei Bauteile sich treffen  (typischerweise ist dies der Fall, wenn zwei Wände und die Decke sich treffen); - Verbindung eines elektrischen Geräts mit dem elektrischen Versorgungssystem eines Gebäudes; - Eine Tür zwischen zwei Räumen.</rdfs:comment>
        <rdfs:comment xml:lang="da">Et generisk koncept til at kvalificere forholdet mellem to eller flere ting i verden, hvoraf mindst den ene er en bygningsdel eller -zone. Eksempler:
    - Kvalificering af varmeoverførsel mellem zoner gennem en eller flere bygningsdele. Dette inkluderer endimensionelle (flade) varmetab fra en zone til en anden gennem en enkelt bygningsdel, todimensionelle (linie) tab fra en zone til en anden gennem den samling, hvor de to elementer mødes, eller tredimensionelle (punkt) tab fra en zone til en anden gennem samlingen, hvor tre elementer (typisk to vægge og et dæk) mødes.
    - Forbindelsen mellem et elektrisk device og det elektriske system i en bygning.
    - En dør mellem et rum og et andet.</rdfs:comment>
        <rdfs:comment xml:lang="sv">Ett generiskt koncept som beskriver relationen mellan två eller flera saker i världen, där åtminstone den ena är ett byggdel eller en zon. Exempelvis: 
- Beskrivning av värmeöverföring mellan zoner genom en eller flera byggdelar. Detta inkluderar endimensionella värmeförluster från en zon till en annan genom en enkel byggdels yta, tvådimensionella förluster från en zon till en annan genom linjen där zonernas respektive byggdelar möts, eller tredimentionella förluster från en zon till en annan genom en punkt där tre byggdelar (vanligtvis två väggar och en platta) möts.
- Kopplingen mellan en elektrisk apparatur och elsystemet i en byggnad.
- En dörr mellan ett rum och ett annat.</rdfs:comment>
        <rdfs:comment xml:lang="sk">Rozhranie je obecný koncept, ktorý definuje vzťah dvoch a viac vecí vo fyzickom svete, kde aspoň jeden z nich je stavebný prvok alebo zóna. 
Príklady:
- koncepcia prenosu tepla mezi zónami prostredníctvom jedného alebo viacero stavebných elementov.  To obshuje plošnú tepelnú výmenu z jednej do druhej zóny cez jeden stavebný element, ďalej to obsahuje tepelnou výmenu lineárnou väzbou, ďalej to obsahuje tepelnú výmenu bodom v/na elemente alebo elementoch (typicky dve steny a podlaha, či strop).
- spojenie elektrického zariadenia do elektrického systému v budove. 
- dvere medzi dvomi miestnosťami. 
</rdfs:comment>
        <rdfs:comment xml:lang="cs">Rozhraní je obecný koncept který definuje vztah dvou a víc věcí ve fyzickém světě, kde alespoň jeden z nich je stavební element nebo zóna. 
Příklady:
koncepce přenosu tepla mezi zónami prostřednictvím jednoho nebo vícero stavebních elementů. To obsahuje plošnou tepelnou výměnu z jedné do druhé zóna přes jeden stavební objekt, dále to obsahuje tepelnou výměnu lineární vazbou, dále to obsahuje tepelnou výměnu bodem v/na elementu nebo elementech (typicky dvě stěny a podlaha či strop). 
        - spojení elektrického zařízení do elektrického systému v budově.
        - dveře mezi dvěma pokoji
</rdfs:comment>
        <rdfs:comment xml:lang="fr">Une interface correspond à la surface où se rencontrent a) deux éléments d&apos;un bâtiment, b) deux zones ou  encore c) un élément d&apos;un bâtiment avec une zone. Un cas d&apos;utilisation type est constituée par la qualification de la zone de transmission de chaleur entre une zone et un mur couvrant plusieurs zones.</rdfs:comment>
        <rdfs:comment xml:lang="fi">Yleinen konsepti kahden tai useamman asian rajapinnan määrittämiseen, missä ainakin toinen asia on joko elementti tai vyöhyke. Esimerkkejä:
    - Kahden vyöhykkeen välillä yhden tai useamman elementin kautta tapahtuvan lämmönsiirtymisen määrittely. Tämä sisältää yksiulotteiset (pinta) lämpöhäviöt vyöhykeeltä toiselle yhden rakennuselementin kautta, kaksiulotteiset (jana) häviöt yhdeltä vyöhykkeeltä toiselle kahden elementin yhteenliitoskohdissa, tai kolmiulotteiset (piste) häviöt yhdeltä vyöhykkeeltä toiselle kolmen elementin (yleensä kaksi seinää ja taso) yhteenliitospisteessä.
    - Sähkölaitteen liitos rakennuksen sähköjärjestelmään.
    - Ovi kahden huoneen välillä.</rdfs:comment>
        <rdfs:comment xml:lang="fa">یک مفهوم کلی از شرایط رابطه بین دو یا چند چیزدر دنیا، در حالی که حداقل یکی از آنها المان یا منطقه است. مثال:
- شرایط انتقال گرما بین یک منطقه و منطقه دیگر از طریق یک یا چند المان ساختمان. این میتواند شامل انتقال/اتلاف گرمای یک بعدی (سطحی) از یک منطقه به منطقه‌ی دیگر از طریق یک المان ساختمان؛ یا، انتقال/اتلاف گرمای دو بعدی (خطی) از یک منطقه به منطقه‌ی دیگر از طریق اتصال بین دو المان ساختمان؛ و یا، انتقال/اتلاف گرمای سه بعدی (نقطه‌ای) از یک منطقه به منطقه‌ی دیگر از طریق برقراری اتصال بین سه المان ساختمان (معمولا دو دیوار و یک دال) باشد.
- ارتباط یک دستگاه الکتریکی با یک سیستم الکتریکی ساختمان.
- یک در بین یک اتاق و اتاق دیگر.
</rdfs:comment>
        <rdfs:comment xml:lang="zh-cn">这是一种通用概念，用于限定世界上两个或多个事物之间的关系，其中二者至少一个是建筑构件或区域。 比如说：
 -通过一个或多个建筑构件或建筑区域之间的热传递。 这包括通过单个建筑构件从一个区域到另一区域的一维（表面）热损失，通过两个构件的相接从一个区域到另一区域的二维（线）热损失或通过三个元素（通常是两堵墙和一个平板）的相接从一个区域到另一个区域的三维（点）损耗。
-将电气设备连接到建筑电气系统。
-房间之间的门
</rdfs:comment>
        <rdfs:isDefinedBy rdf:resource="https://w3id.org/bot#"/>
        <rdfs:label xml:lang="tr">Arayüzey</rdfs:label>
        <rdfs:label xml:lang="sv">Gränssnitt</rdfs:label>
        <rdfs:label xml:lang="da">Grænseflade</rdfs:label>
        <rdfs:label xml:lang="it">Interfaccia</rdfs:label>
        <rdfs:label xml:lang="en">Interface</rdfs:label>
        <rdfs:label xml:lang="fr">Interface</rdfs:label>
        <rdfs:label xml:lang="nl">Interface</rdfs:label>
        <rdfs:label xml:lang="pt">Interface</rdfs:label>
        <rdfs:label xml:lang="es">Interfaz</rdfs:label>
        <rdfs:label xml:lang="ca">Interfície</rdfs:label>
        <rdfs:label xml:lang="fi">Rajapinta</rdfs:label>
        <rdfs:label xml:lang="sk">Rozhranie
</rdfs:label>
        <rdfs:label xml:lang="cs">Rozhraní</rdfs:label>
        <rdfs:label xml:lang="de">Schnittstelle</rdfs:label>
        <rdfs:label xml:lang="fa">رابط</rdfs:label>
        <rdfs:label xml:lang="zh-cn">界面</rdfs:label>
        <ns:term_status>stable</ns:term_status>
    </owl:Class>
    


    <!-- https://w3id.org/bot#Site -->

    <owl:Class rdf:about="https://w3id.org/bot#Site">
        <rdfs:subClassOf rdf:resource="https://w3id.org/bot#Zone"/>
        <owl:disjointWith rdf:resource="https://w3id.org/bot#Space"/>
        <owl:disjointWith rdf:resource="https://w3id.org/bot#Storey"/>
        <rdfs:comment xml:lang="en">A part of the physical world or a virtual world that is inherently both located in this world and having a 3D spatial extent. It is intended to contain or contains one or more buildings.</rdfs:comment>
        <rdfs:comment xml:lang="tr">Bir veya daha fazla bina içeren alan.</rdfs:comment>
        <rdfs:comment xml:lang="nl">Een deel van de fysieke wereld of een virtuele wereld dat zowel gelokaliseerd kan worden in deze wereld als een ruimtelijke omvang heeft. Het is bedoeld om één of meerdere gebouwen te bevatten of bevat al één of meerdere gebouwen.</rdfs:comment>
        <rdfs:comment xml:lang="de">Ein Teil der realen oder virtuellen Welt die beide Teil dieser Welt sind und eine räumliche Ausdehnung hat. Es besteht die Absicht, dass es Gebäude enthält, oder es enthält ein oder mehr Gebäude.</rdfs:comment>
        <rdfs:comment xml:lang="da">En del af den fysiske verden eller en virtuel verden, der i sagens natur både er lokaliseret i denne verden og har en 3D rumlig afgrænsning. En byggegrund er beregnet til at indeholde, eller indeholder én eller flere bygninger.</rdfs:comment>
        <rdfs:comment xml:lang="sv">En del av den fysiska världen eller en virtuell värld som har en spatial utsträckning i tre dimensioner. Den är avsedd att innehålla, eller innehåller, en eller flera byggnader.</rdfs:comment>
        <rdfs:comment xml:lang="fi">Fyysisen tai virtuaalisen maailman osa, joka luonnostaan sekä sijaitsee tässä maailmassa että omaa kolmiulotteiset tilalliset ulottuvuudet. Sen on tarkoitus sisältää tai se sisältää yhden tai useamman rakennuksen.</rdfs:comment>
        <rdfs:comment xml:lang="sk">Stavenisko ako časť fyzického, alebo virtuálneho sveta, ktoré sú neodmysliteľne umiestnené ako vo fyzickom svete tak majúc 3D virtuálny priestorový rozsah. Zámerom staveniska je obsahovať aspoň jednu stavbu, napríklad budovu, či stavebnú konštrukciu.</rdfs:comment>
        <rdfs:comment xml:lang="cs">Staveniště jako část fyzického světa nebo virtuálního světa které jsou neodmyslitelně umístěna jak ve fyzickém světě tak majíce 3D virtuální prostorový rozsah. Záměrem staveniště je obsahovat alespoň jednu stavbu, např. budovu či stavební konstrukci.
</rdfs:comment>
        <rdfs:comment xml:lang="pt">Uma parte do mundo físico ou do mundo virtual que está inerentemente localizada neste mundo e que tem uma extensão espacial tridimensional. Contém ou destina-se a conter um ou mais edifícios.</rdfs:comment>
        <rdfs:comment xml:lang="fr">Un site comprend un ou plusieurs bâtiments</rdfs:comment>
        <rdfs:comment xml:lang="ca">Una part del món físic o un món virtual que es troba inherentment ubicada en aquest món i que té una extensió espacial en 3D. Està destinada a contenir un contingut o més edificis.</rdfs:comment>
        <rdfs:comment xml:lang="it">Una parte del mondo fisico o virtuale che si trova intrinsecamente in questo mondo e ha una estensione spaziale tridimensionale. Un sito contiene o è destinato a contenere uno o più edifici.</rdfs:comment>
        <rdfs:comment xml:lang="es">Una parte del mundo físico o un mundo virtual que está inherentemente ubicada en este mundo y que tiene una extensión espacial en 3D. Está destinado a contener o contiene uno o más edificios.</rdfs:comment>
        <rdfs:comment xml:lang="fa">بخشی از دنیای فیزیکی، و یا مجازی که اساساً در دنیا وجود دارد و دارای حدود مکانی سه بعدی است. یک عنصر سایت در برگیرنده‌ی یک یا چند ساختمان است.

</rdfs:comment>
        <rdfs:comment xml:lang="zh-cn">本质上是存在于物理世界或虚拟世界的一部分，并具有3D空间范围。它旨在包含一个或多个建筑物。</rdfs:comment>
        <rdfs:isDefinedBy rdf:resource="https://w3id.org/bot#"/>
        <rdfs:label xml:lang="tr">Arsa</rdfs:label>
        <rdfs:label xml:lang="da">Grund</rdfs:label>
        <rdfs:label xml:lang="de">Grundstück</rdfs:label>
        <rdfs:label xml:lang="ca">Lloc</rdfs:label>
        <rdfs:label xml:lang="sv">Plats</rdfs:label>
        <rdfs:label xml:lang="en">Site</rdfs:label>
        <rdfs:label xml:lang="fr">Site</rdfs:label>
        <rdfs:label xml:lang="es">Sitio</rdfs:label>
        <rdfs:label xml:lang="it">Sito</rdfs:label>
        <rdfs:label xml:lang="sk">Stavenisko, stavebný pozemok, stavebná plocha, zastavaná plocha.</rdfs:label>
        <rdfs:label xml:lang="cs">Staveniště, stavební pozemek, stavební plocha, zastavěná plocha.</rdfs:label>
        <rdfs:label xml:lang="pt">Sítio</rdfs:label>
        <rdfs:label xml:lang="nl">Terrein</rdfs:label>
        <rdfs:label xml:lang="fi">Tontti</rdfs:label>
        <rdfs:label xml:lang="fa">سایت</rdfs:label>
        <rdfs:label xml:lang="zh-cn">地点</rdfs:label>
        <ns:term_status>stable</ns:term_status>
    </owl:Class>
    


    <!-- https://w3id.org/bot#Space -->

    <owl:Class rdf:about="https://w3id.org/bot#Space">
        <rdfs:subClassOf rdf:resource="https://w3id.org/bot#Zone"/>
        <owl:disjointWith rdf:resource="https://w3id.org/bot#Storey"/>
        <rdfs:comment xml:lang="en">A part of the physical world or a virtual world whose 3D spatial extent is bounded actually or theoretically, and provides for certain functions within the zone it is contained in.</rdfs:comment>
        <rdfs:comment xml:lang="nl">Een deel van de fysieke wereld of een virtuele wereld waarvan de driedimensionale omvang feitelijk of virtueel begrensd is, en dat bepaalde activiteiten faciliteert in de zone die de ruimte bevat.</rdfs:comment>
        <rdfs:comment xml:lang="de">Ein Teil der realen oder virtuellen Welt, dessen räumliche Ausdehnung tatsächlich oder virtuell begrenzt ist. In der Zone in der es enthalten ist stellt es bestimmte Funktionen bereit.</rdfs:comment>
        <rdfs:comment xml:lang="da">En del af den fysiske verden eller en virtuel verden, hvis 3D-rumlige omfang er afgrænset faktisk eller teoretisk, og giver bestemte funktioner inden for den zone, den er indeholdt i.</rdfs:comment>
        <rdfs:comment xml:lang="sv">En del av den fysiska världen eller en virtuell värld vars spatiala utsträckning i tre dimensioner är faktiskt eller teoretiskt begränsad, och som tillhandahåller vissa funktioner för zonen den är inrymd i.</rdfs:comment>
        <rdfs:comment xml:lang="tr">Fiziksel dünyanın veya sanal dünyanın, 3D mekansal kapsamı gerçekte veya teorik olarak tanımlanmış olan ve içinde bulunduğu bölgede belirli fonksiyonları yerine getiren bir kısmıdır.</rdfs:comment>
        <rdfs:comment xml:lang="sk">Ohraničený troj-rozmerný rozsah definovaný fyzicky nebo pojmovo [ISO 12006-2 (DIS 2013), 3.4.3]</rdfs:comment>
        <rdfs:comment xml:lang="cs">Ohraničený troj-rozměrný rozsah definovaný fyzicky nebo pojmově [ISO 12006-2 (DIS 2013), 3.4.3]</rdfs:comment>
        <rdfs:comment xml:lang="fi">Osa fyysisestä -tai virtuaalista maailmasta, jonka 3D-tila on rajattu oikeasti tai teoreettisesti ja tarjoaa tiettyjä toimintoja vyöhykkeellä, johon se sisältyy.</rdfs:comment>
        <rdfs:comment xml:lang="pt">Uma parte do mundo físico ou de um mundo virtual cuja extensão espacial 3D esteja delimitada de forma efectiva ou teórica, que fornece certas funções dentro da zona em que está contido.</rdfs:comment>
        <rdfs:comment xml:lang="ca">Una part de el món físic o d&apos;un món virtual l&apos;extensió espacial tridimensional està limitada física o teòricament, i proveeix certes funcions dins de la zona on està continguda.</rdfs:comment>
        <rdfs:comment xml:lang="it">Una parte del mondo fisico o virtuale il cui spazio 3D è delimitato effettivamente o virtualmente, e fornisce determinate funzioni all&apos;interno della zona in cui è contenuta.</rdfs:comment>
        <rdfs:comment xml:lang="es">Una parte del mundo físico o de un mundo virtual cuya extensión espacial tridimensional está limitada física o teóricamente, y provee ciertas funciones dentro de la zona donde está contenida.</rdfs:comment>
        <rdfs:comment xml:lang="fr">Une partie du monde physique ou virtuel dont l&apos;extension 3D est limitée réellement ou théoriquement, et apporte des fonctions aux zones dans laquelle elle est contenue.</rdfs:comment>
        <rdfs:comment xml:lang="fa">بخشی از دنیای فیزیکی، و یا مجازی که وسعت مکانی سه بعدی آن از نظر حقیقی و یا تئوری محدود است، و عملکردهای مشخصی را در منطقه‌ای که در آن قرار گرفته ارائه می دهد.
</rdfs:comment>
        <rdfs:comment xml:lang="zh-cn">是物理世界或虚拟世界的一部分，其3D空间范围实际上或在理论上受到限制，可在其所包含的区域内提供某些功能。</rdfs:comment>
        <rdfs:isDefinedBy rdf:resource="https://w3id.org/bot#"/>
        <rdfs:label xml:lang="es">Espacio</rdfs:label>
        <rdfs:label xml:lang="ca">Espai</rdfs:label>
        <rdfs:label xml:lang="pt">Espaço</rdfs:label>
        <rdfs:label xml:lang="tr">Oda</rdfs:label>
        <rdfs:label xml:lang="fr">Pièce</rdfs:label>
        <rdfs:label xml:lang="sk">Priestor</rdfs:label>
        <rdfs:label xml:lang="cs">Prostor</rdfs:label>
        <rdfs:label xml:lang="de">Raum</rdfs:label>
        <rdfs:label xml:lang="nl">Ruimte</rdfs:label>
        <rdfs:label xml:lang="da">Rum</rdfs:label>
        <rdfs:label xml:lang="en">Space</rdfs:label>
        <rdfs:label xml:lang="it">Spazio</rdfs:label>
        <rdfs:label xml:lang="fi">Tila</rdfs:label>
        <rdfs:label xml:lang="sv">Utrymme</rdfs:label>
        <rdfs:label xml:lang="fa">فضا</rdfs:label>
        <rdfs:label xml:lang="zh-cn">空间</rdfs:label>
        <ns:term_status>stable</ns:term_status>
    </owl:Class>
    


    <!-- https://w3id.org/bot#Storey -->

    <owl:Class rdf:about="https://w3id.org/bot#Storey">
        <rdfs:subClassOf rdf:resource="https://w3id.org/bot#Zone"/>
        <rdfs:comment xml:lang="en">A part of the physical world or a virtual world that is inherently both located in this world and having a 3D spatial extent. A bot:Storey is contained in one or more buildings, and is intended to contain one or more spaces that are horizontally connected. Storeys of a building are connected by means of vertical connections such as elevators and stairs. A bot:Storey encompasses both zones above and below ground, for example, a building with 21 floors above ground, one ground floor and 3 basements is equal to the sentence: A building has 25 instances of bot:Storey.</rdfs:comment>
        <rdfs:comment xml:lang="tr">Bir binanın katı</rdfs:comment>
        <rdfs:comment xml:lang="fr">Correspond à un niveau du bâtiment</rdfs:comment>
        <rdfs:comment xml:lang="nl">Een deel van de fysieke wereld of een virtuele wereld dat zowel gelokaliseerd kan worden in deze wereld als een ruimtelijke omvang heeft. Een bot:Storey is deel van één of meerdere gebouwen, en is bedoeld om één of meerdere ruimtes te bevatten die horizontaal geconnecteerd zijn. De verdiepingen van een gebouw zijn verbonden door middel van verticale connecties zoals liften en trappen. Een bot:Storey omvat zowel zones boven als onder de grond, bijvoorbeeld een gebouw met 21 verdiepingen boven de grond, één gelijkvloers en 3 kelderverdiepingen is evenwaardig aan de zin: Een gebouw heeft 25 instanties van bot:Storey.</rdfs:comment>
        <rdfs:comment xml:lang="de">Ein Teil der realen oder virtuellen Welt die beide Teil dieser Welt sind und eine räumliche Ausdehnung hat. Ein bot:Storey ist in einem oder mehreren Gebäuden enthalten und es besteht die Absicht oder es ist der Fall, dass es ein oder mehrere Räume enthält, die horizontal miteinander verbunden sind. Geschosse eines Gebäudes sind vertikal miteinander verbunden, durch zum Beispiel Aufzüge oder Treppen. Ein bot:Storey umfassst zonen die über und unter der Erdoberfläche liegen. Zum Beispiel hat ein Gebäude mit 21 Geschossen über der Erde, ein Erdgeschoss und 3 Kellerstockwerken insgesamt 25 Instanzen von bot:Storey.</rdfs:comment>
        <rdfs:comment xml:lang="da">En del af den fysiske verden eller en virtuel verden, der i sagens natur både er lokaliseret i denne verden og har en 3D rumlig afgrænsning. En bot:Storey er indeholdt i en eller flere bygninger og er beregnet til at indeholde et eller flere rum, der er horisontalt forbundet. Etager i en bygning er forbundet ved hjælp af lodrette forbindelser såsom elevatorer og trapper. En bot:Storey omfatter både zoner over og under jorden, for eksempel en bygning med 21 etager over jorden, en stueetage og 3 kældre er lig med sætningen: En bygning har 25 tilfælde af bot:Storey.</rdfs:comment>
        <rdfs:comment xml:lang="sv">En del av den fysiska världen eller en virtuell värld som har en spatial utsträckning i tre dimensioner. En bot:Storey är inrymd i en eller flera byggnader, och är menad att innehålla ett eller flera utrymmen som är förbundna horisontellt. Sådana våningar i en byggnad är förbundna med hjälp av lodrätta förbindelser såsom hissar och trappor. Bot:Storey kan användas för att beskriva såväl våningar över som under mark; till exempel så har en byggnad med 21 våningar över marken, en entrénvåning, och tre källarvåningar totalt 25 bot:Storey-instanser.</rdfs:comment>
        <rdfs:comment xml:lang="fi">Fyysisen tai virtuaalisen maailman osa, joka luonnostaan sekä sijaitsee tässä maailmassa että omaa kolmiulotteiset tilalliset ulottuvuudet. bot:Storey sisältyy yhteen tai useampaan rakennukseen, ja sen tarkoitus on sisältää yksi tai useampi tila jotka ovat vaakasuunnassa yhteydessä. Rakennuksen kerrokset ovat yhteydessä toisiinsa pystysuuntaisilla yhteyksillä, kuten hisseillä ja rappusilla. bot:Storey kattaa vyöhykkeet sekä maan alla että päällä. Esimerkiksi rakennus, jossa on pohjakerros, 21 kerrosta sen yläpuolella, ja 3 kerrosta kellaria, on yhtäläinen seuraavan lauseen kanssa: rakennuksella on 25 bot:Storey instanssia.</rdfs:comment>
        <rdfs:comment xml:lang="pt">Uma parte do mundo físico ou do mundo virtual que está inerentemente localizada neste mundo e que tem uma extensão espacial tridimensional. 
Um bot:Storey está contido num ou mais edifícios e está destinado a conter um ou mais espaços que estejam conectados horizontalmente. Os pisos de um edifício estão ligados através de ligações verticais tais como escadas e elevadores.
Um bot:Storey abrange tanto as zonas acima como abaixo do solo; por exemplo, um edifício com 21 andares acima do solo, um piso térreo e três caves pode ser descrito como: um edifício que possui 25 instâncias de bot:Storey.</rdfs:comment>
        <rdfs:comment xml:lang="ca">Una part del món físic o virtual que està inherentment ubicat en aquest món i que té una extensió espacial en 3D. Un bot:Storey està contingut en un o més edificis, i està destinat a contenir un o més espais que estan connectats horitzontalment. Les plantes d&apos;un edifici estan connectades per mitjà de connexions verticals com ascensors i escales. Un bot:Storey abasta les dues zones sobre i sota de terra, per exemple, un edifici amb 21 pisos sobre terra, una planta baixa i 3 soterranis hauria de contenir 25 instàncies de bot:Storey.</rdfs:comment>
        <rdfs:comment xml:lang="it">Una parte del mondo fisico o virtuale che si trova intrinsecamente in questo mondo e ha una estensione spaziale tridimensionale. Un bot:Storey è contenuto in uno o più edifici ed è destinato a contenere uno o più spazi che sono connessi orizzontalmente. I piani di un edificio sono connessi attraverso connessioni verticali come ascensori e scale. Un bot:Storey comprende zone che si trovano sia sopra che sotto il livello del suolo; per esempio, un edificio con un piano terra, ulteriori 21 piani di altezza e 3 piani interrati corrisponde a un edificio con 25 istanze di bot:Storey.</rdfs:comment>
        <rdfs:comment xml:lang="es">Una parte del mundo físico o virtual que está inherentemente ubicado en este mundo y que tiene una extensión espacial en 3D. Un bot:Storey está contenido en uno o más edificios, y está destinado a contener uno o más espacios que están conectados horizontalmente. Las plantas de un edificio están conectadas por medio de conexiones verticales como ascensores y escaleras. Un bot:Storey abarca ambas zonas sobre y debajo del suelo, por ejemplo, un edificio con 21 pisos sobre el suelo, una planta baja y 3 sótanos debería contener 25 instancias de bot:Storey.</rdfs:comment>
        <rdfs:comment xml:lang="sk">Časť fyzického alebo virtuálneho sveta, ktorá je neodmyslitelne umiestnená ako vo fyzickom svete, tak má 3D virtuálny priestorový rozsah. Bot:Storey je obsiahnutý v jednej alebo viacero budovách a má obsahovať jeden alebo viacero priestorov, ktoré sú spojené horizontálne. Podlažia budovy sú spojené zvislými spojmi, ako je napríklad výťahová šachta, alebo schodisko. Bot:Storey zahŕňa ako zóny nad, tak pod úrovňou terénu, napríklad, prehlásenie: budova s 21 nadzemnými podlažiami, prízemím a 3 podzemnými podlažiami má rovnaký význam ako prehlásenie: budova má 25 inštancií bot:Storey.</rdfs:comment>
        <rdfs:comment xml:lang="cs">Část fyzického světa nebo virtuálního světa, která je neodmyslitelně umístěna jak ve fyzickém světě tak má 3D virtuální prostorový rozsah. Bot:Storey je obsažen v jedné nebo vícero budovách a má obsahovat jeden nebo vícero prostorů, které jsou spojeny horizontálně. Podlaží budovy jsou spojeny svislými spoji, jako je například výtahová šachta, nebo schodiště. Bot:Storey zahrnuje jak zóny nad tak pod úrovní terénu, například, prohlášení: budova s 21 nadzemními podlažími, jedním přízemím a 3 podzemními podlažími má stejný význam jako prohlášení: budova má 25 instancí bot:Storey.</rdfs:comment>
        <rdfs:comment xml:lang="fa">بخشی از دنیای فیزیکی، و یا مجازی که اساساً هم در دنیا وجود دارد و دارای حدود مکانی سه بعدی میباشند. یک bot:Storey در یک یا چند ساختمان قرار میگیرد، و دربرگیرنده‌ی یک یا چند فضا است که به صورت افقی به هم متصل شده اند.
طبقه های یک ساختمان از طریق اتصالات عمودی مانند آسانسور و پله به هم متصل میشوند. یک bot:Storey  هر دو منطقه بالا و زیر زمین را پوشش می‎دهد، برای مثال، یک ساختمان با 21 طبقه بالای زمین، یک طبقه همکف و3 طبفه یک ساختمان با 25 عنصر  bot:Storey  است.
</rdfs:comment>
        <rdfs:comment xml:lang="zh-cn">本质上是存在于物理世界或虚拟世界的一部分，并具有3D空间范围。bot：Storey包含在一个或多个建筑物中，其旨在包含一个或多个水平连接的空间。 建筑物的楼层通过垂直连接（例如电梯和楼梯）连接。 bot：Storey包含地上和地下两个区域，例如，一栋楼高21层，含有一楼及地下3个地下室的建筑物可以表达为：一栋建筑物有25个bot：Storey实例。</rdfs:comment>
        <rdfs:isDefinedBy rdf:resource="https://w3id.org/bot#"/>
        <rdfs:label xml:lang="da">Etage</rdfs:label>
        <rdfs:label xml:lang="de">Geschoss (Architektur)</rdfs:label>
        <rdfs:label xml:lang="tr">Kat</rdfs:label>
        <rdfs:label xml:lang="fi">Kerros</rdfs:label>
        <rdfs:label xml:lang="it">Piano di edificio</rdfs:label>
        <rdfs:label xml:lang="ca">Pis</rdfs:label>
        <rdfs:label xml:lang="es">Piso</rdfs:label>
        <rdfs:label xml:lang="pt">Piso</rdfs:label>
        <rdfs:label xml:lang="sk">Podlažie</rdfs:label>
        <rdfs:label xml:lang="cs">Podlaží</rdfs:label>
        <rdfs:label xml:lang="en">Storey</rdfs:label>
        <rdfs:label xml:lang="nl">Verdieping</rdfs:label>
        <rdfs:label xml:lang="sv">Våning</rdfs:label>
        <rdfs:label xml:lang="fr">Étage</rdfs:label>
        <rdfs:label xml:lang="fa">طبقه</rdfs:label>
        <rdfs:label xml:lang="zh-cn">楼层</rdfs:label>
        <ns:term_status>stable</ns:term_status>
    </owl:Class>
    


    <!-- https://w3id.org/bot#Zone -->

    <owl:Class rdf:about="https://w3id.org/bot#Zone">
        <rdfs:comment xml:lang="en">A part of the physical world or a virtual world that is inherently both located in this world and has a 3D spatial extent; Sub-classes of bot:Zone include bot:Site, bot:Building, bot:Storey, or bot:Space.  An instance of bot:Zone can contain other bot:Zone instances, making it possible to group or subdivide zones. An instance of bot:Zone can be adjacent to or intersecting other bot:Zone instances. Finally, a bot:Zone can instantiate three relations to bot:Element, which are either contained in (bot:containsElement), adjacent to it (bot:adjacentElement) or intersecting (bot:intersectingElement).</rdfs:comment>
        <rdfs:comment xml:lang="nl">Een deel van de fysieke wereld of een virtuele wereld dat zowel gelokaliseerd kan worden in deze wereld als een ruimtelijke omvang heeft; subklasses van bot:Zone zijn bot:Site, bot:Building, bot:Storey of bot:Space. Een instantie van bot:Zone kan een ander bot:Zone instantie bevatten, wat gebruikt kan worden om zones te groeperen of op te delen. Een instantie van bot:Zone kan aangrenzend zijn aan of snijdend met een andere bot:Zone instantie. Ten slotte kan een bot:Zone instantie drie relaties hebben met een bot:Element instantie dat het ofwel bevat (bot:containsElement), waar het aangrenzend aan is (bot:adjacentElement) of waarmee het snijdt (bot:intersectingElement).</rdfs:comment>
        <rdfs:comment xml:lang="de">Ein Teil der realen oder virtuellen Welt die beide Teil dieser Welt sind und eine räumliche Ausdehnung hat; Unterklassen von bot:Zone sind bot:Site, bot:Building, bot:Storey oder bot:Space. Eine Instanz von bot:Zone kann andere Instanzen von bot:Zone enthalten. So ist es möglich Instanzen von bot:Zone zu gruppieren, oder zu unterteilen. Eine Instanz einer bot:Zone kann an eine andere Instanz von bot:Zone angrenzen. Es bestehen drei Möglichkeiten Instanzen von bot:Zone und bot:Element in Beziehung zu setzen. Entweder ein Element ist in einer Zone enthalten (bot:containsElement), es grenzt an eine andere Zone an (bot:adjacentElement) oder es schneidet eine Zone (bot:intersectingElement).</rdfs:comment>
        <rdfs:comment xml:lang="da">En del af den fysiske verden eller en virtuel verden, der i sagens natur både er lokaliseret i denne verden og har en 3D rumlig afgrænsning; Underklasser af bot:Zone inkluderer bot:Site, bot:Building, bot:Storey eller bot:Space. En forekomst af bot:Zone kan indeholde andre bot:Zone-forekomster, hvilket gør det muligt at gruppere eller opdele zoner. En forekomst af bot:Zone kan støde op til andre bot:Zone-forekomster. Endelig kan en bot:Zone-forekomst instantiere to forbindelser til bot:Element, der enten er indeholdt i (bot:containsElement) eller tilstødende dertil (bot:adjacentElement).</rdfs:comment>
        <rdfs:comment xml:lang="sv">En del av den fysiska världen eller en virtuell värld som har en spatial utsträckning i tre dimensioner. Underklasser av bot:Zone inkluderar bot:Site, Bot:Building, bot:Storey, och bot:Space. En instans av bot:Zone kan innehålla andra bot:Zone-instanser, vilket gör det möjligt att gruppera eller dela upp zoner. En instans av bot:Zone kan kan ligga angränsande mot andra bot:Zone-instanser. Slutligen kan en instans av bot:Zone ha två relationer till instanser av bot:Element; den kan innehålla dem (bot:containsElement) eller ligga angränsande mot dem (bot:adjacentElement).



</rdfs:comment>
        <rdfs:comment xml:lang="tr">Fiziksel dünyanın veya sanal dünyanın, doğası gereği, hem bu dünyada bulunan ve hem de 3D bölgesel bir sınırlamaya sahip olan bir parça; Bot:Zone altsınıfları: bot:Site, bot:Building, bot:Storey yada bot:Space. Bir bot:Zone baska bot:Zone-olusumu icerebilir. Bir bot:Zone baska bot:Zone-olusumuyla bitisik olabilir. Son onlarak, bir bot:Zone, bir bot:Element ile iki baglantisi olabilir: ya içerir (bot: includeElement) veya bitisik olur (bot: adjacentElement).</rdfs:comment>
        <rdfs:comment xml:lang="fi">Fyysisen tai virtuaalisen maailman osa, joka luonnostaan sekä sijaitsee tässä maailmassa että omaa kolmiulotteiset tilalliset ulottuvuudet; bot:Zone:n alaluokkia ovat: bot:Site, bot:Building, bot:Storey ja bot:Space. bot:Zone-luokan instanssi voi sisältää muita bot:Zone-instansseja, mikä mahdollistaa vyöhykkeiden ryhmittelyn ja jaon osiin. bot:Zone voi olla muiden bot:Zone-instanssien vieressä tai leikata niitä. Lopuksi, bot:Zone voi instantioida kolmea relaatiota bot:Element:iin, jotka joko sisältyvät siihen (bot:containsElement), ovat sen veiressä (bot:adjacentElement) tai leikkaavat sitä (bot:intersectingElement).</rdfs:comment>
        <rdfs:comment xml:lang="pt">Uma parte do mundo físico ou de um mundo virtual que está inerentemente localizado neste mundo e que possui uma extensão espacial 3D. As Sub-classes de bot:Zone incluem bot:Site, bot:Building, bot:Storey ou bot:Space. Uma instância de bot:Zone pode conter outras instâncias de bot:Zone, tornando possível agrupar ou subdividir zonas. Uma instância de bot:Zone pode ser adjacente a ou intersectar outras instâncias de bot:Zone. Por fim, uma bot:Zone pode instanciar três relações com bot:Element, que ou estão contidas em (bot:containsElement), lhe são adjacentes (bot:adjacentElement) ou as intersecta (bot:intersectingElement).</rdfs:comment>
        <rdfs:comment xml:lang="ca">Una part de el món físic o d&apos;un món virtual que està inherentment ubicat en aquest món i que té una extensió espacial tridimensional; les subclasses de bot:Zone inclouen bot:Site, bot:Building, bot:Storey, o bot:Space. Una instància de bot:Zone pot contenir altres instàncies de bot:Zone, fent possible agrupar o subdividir zones. Una instància de bot:Zone pot ser adjacent a, o intersecar amb altres instàncies de bot:Zone. Finalment, un bot:Zone pot instanciar tres relacions amb bot:Element, que estan continguts en ella (bot:containsElement), són adjacents a ella (bot:adjacentElement), o amb els que interseca (bot:intersectingElement).</rdfs:comment>
        <rdfs:comment xml:lang="it">Una parte del mondo fisico o virtuale che è intrinsecamente ubicato in questo mondo e che ha un&apos;estensione spaziale tridimensionale; sottoclassi di bot:Zone includono bot:Site, bot:Building, bot:Storey, o bot:Space. Un&apos;istanza di bot:Zone può contenere altre istanze di bot:Zone, rendendo possibile il raggruppamento o la suddivisione di zone. Un&apos;istanza di bot:Zone può essere adiacente o intersecare altre istanze di bot:Zone. Infine, una bot:Zone può istanziare tre relazioni con bot:Element, il quale può essere contenuto (bot:containsElement), essere adiacente (bot:adjacentElement) o intersecare (bot:intersectingElement).</rdfs:comment>
        <rdfs:comment xml:lang="es">Una parte del mundo físico o de un mundo virtual que está inherentemente ubicada en este mundo y que tiene una extensión espacial tridimensional; las subclases de bot:Zone incluyen bot:Site, bot:Building, bot:Storey, o bot:Space. Una instancia de bot:Zone puede contener otras instancias de bot:Zone, lo que permite agrupar o subdividir zonas. Una instancia de bot:Zone puede ser adyacente a, o intersecar con otras instancias de bot:Zone. Finalmente, una bot:Zone puede instanciar tres relaciones con bot:Element, que están contenidas en ella (bot:containsElement), adyacentes a ella (bot:adjacentElement) o con los que interseca (bot:intersectingElement).</rdfs:comment>
        <rdfs:comment xml:lang="fr">Une partie du monde physique ou virtuel qui est inhéremment à la fois localisé dans ce monde et a une étendue spatiale 3D; les sous-classes de bot:Zone incluent bot:Site, bot:Building, bot:Storey, ou bot:Space. Une instance de bot:Zone peut contenir d&apos;autres instances de bot:Zone, ce qui permet de grouper ou sub-diviser les zones. Une instance de bot:Zone peut être adjacente ou intersectante à d&apos;autres bot:Zone. Enfin, une bot:Zone peut contenir (bot:containsElement), être adjacent (bot:adjacentElement) ou intersecter (bot:intersectingElement) un bot:Element.</rdfs:comment>
        <rdfs:comment xml:lang="sk">Časť fyzického alebo virtuálneho sveta, ktorý je dedične v tomto svete umiestnený a má charakter-rozmer priestoru, ktorý závisí na lokalizácii ako v tomto svete tak vo virtuálnomn svete. Podtriedy bot:Zone zahŕňajú bot:Site, bot:Building, bot:Storey, alebo bot:Space. Inštancia bot:Zone je schopná obsahovať iné bot:Zone inštancie, so schopnosťou zoskupovať alebo pod-rozdeľovať zóny. Inštancia bot:Zone môže byť dotýkajúca sa ďalšej bot:Zone inštancie. Finálne, bot:Zone môže definovať vzťahy k bot:Element, ktoré môžu byť typu zóna obsahuje prvok (bot:containsElement), alebo sa prvok môže zóny dotýkať (bot:adjacentElement).</rdfs:comment>
        <rdfs:comment xml:lang="cs">Část fyzického nebo virtuálního světa, který je dědičně v tomto světe umístěn a má charakter-rozměr prostoru který závisí na lokalizaci jak v reálnem světě, tak ve virtuálním světě. Podtřídy bot:Zone zahrňují bot:Site, bot:Building, bot:Storey, nebo bot:Space. Instance zóny bot:Zone jsou schopny obsahovat další bot:Zone instance se schopností je seskupovat nebo dělit na nižší zóny. Instance bot:Zone může být přiřazena-dotčena k další bot:Zone instanci. Nakonec bot:Zone může definovat dva vztahy elemetntu bot:Element, které jsou buďto obsaženy v zóně (bot:containsElement), nebo se jí dotýkají (bot:adjacentElement)</rdfs:comment>
        <rdfs:comment xml:lang="fa">بخشی از دنیای فیزیکی، و یا مجازی که اساساً در دنیا وجود دارد و دارای حدود مکانی سه بعدی است. زیرکلاس‌های bot:Zone عبارتند از bot:Site، bot:Building، bot:Storey، وbot:Space.
 یک عنصر bot:Zone میتواند دربرگیرنده‌ی عناصر دیگری از جنس bot:Zone  باشد و به این گونه امکان گروه بندی و جداسازی مناطق ختلف بوجود می‌آید. یک عنصر bot:Zone می‌تواند هم‌جوار عناصر دیگری از جنس bot:Zone باشد. در پایان، یک عنصر bot:Zone می‌تواند آغازگر دو نوع رابطه با عناصر bot:Element باشد که شامل دربرگیرندگی (bot:containsElement) وهم‌جواری  (bot:adjacentElement)  است.
</rdfs:comment>
        <rdfs:comment xml:lang="zh-cn">区域是物理世界或虚拟世界的一部分，既位于现实空间中又可在3D空间中拓展。bot:Zone的子集包括bot:Site, bot:Building, bot:Storey, or bot:Space。bot:Zone实例可包含其他bot:Zone实例，从而可以对区域进行分组或细分。 同时，bot：Zone的实例也可以与其他bot：Zone实例相邻。最后，bot：Zone可以实例化为bot：Element的两个关系，它们可以包含在（bot：containsElement）中，或者与其相邻（bot：adjacentElement）。</rdfs:comment>
        <rdfs:isDefinedBy rdf:resource="https://w3id.org/bot#"/>
        <rdfs:label xml:lang="tr">Bölge</rdfs:label>
        <rdfs:label xml:lang="fi">Vyöhyke</rdfs:label>
        <rdfs:label xml:lang="sv">Zon</rdfs:label>
        <rdfs:label xml:lang="ca">Zona</rdfs:label>
        <rdfs:label xml:lang="es">Zona</rdfs:label>
        <rdfs:label xml:lang="it">Zona</rdfs:label>
        <rdfs:label xml:lang="pt">Zona</rdfs:label>
        <rdfs:label xml:lang="da">Zone</rdfs:label>
        <rdfs:label xml:lang="de">Zone</rdfs:label>
        <rdfs:label xml:lang="en">Zone</rdfs:label>
        <rdfs:label xml:lang="fr">Zone</rdfs:label>
        <rdfs:label xml:lang="nl">Zone</rdfs:label>
        <rdfs:label xml:lang="cs">Zóna</rdfs:label>
        <rdfs:label xml:lang="sk">Zóna</rdfs:label>
        <rdfs:label xml:lang="fa">منطقه</rdfs:label>
        <rdfs:label xml:lang="zh-cn">区域</rdfs:label>
        <ns:term_status>stable</ns:term_status>
    </owl:Class>
    


    <!-- https://w3id.org/digitalconstruction/0.3/BuildingMaterials#CompositeMaterial -->

    <owl:Class rdf:about="https://w3id.org/digitalconstruction/0.3/BuildingMaterials#CompositeMaterial">
        <rdfs:subClassOf rdf:resource="https://w3id.org/digitalconstruction/0.3/BuildingMaterials#MaterialType"/>
        <owl:disjointWith rdf:resource="https://w3id.org/digitalconstruction/0.3/BuildingMaterials#InorganicNonMetallicMaterial"/>
        <owl:disjointWith rdf:resource="https://w3id.org/digitalconstruction/0.3/BuildingMaterials#MetallicMaterial"/>
        <owl:disjointWith rdf:resource="https://w3id.org/digitalconstruction/0.3/BuildingMaterials#OrganicaMaterial"/>
    </owl:Class>
    


    <!-- https://w3id.org/digitalconstruction/0.3/BuildingMaterials#Constituent -->

    <owl:Class rdf:about="https://w3id.org/digitalconstruction/0.3/BuildingMaterials#Constituent">
        <rdfs:subClassOf rdf:resource="https://w3id.org/digitalconstruction/0.3/BuildingMaterials#MaterialDefinition"/>
        <owl:disjointWith rdf:resource="https://w3id.org/digitalconstruction/0.3/BuildingMaterials#ConstituentSet"/>
        <owl:disjointWith rdf:resource="https://w3id.org/digitalconstruction/0.3/BuildingMaterials#Layer"/>
        <owl:disjointWith rdf:resource="https://w3id.org/digitalconstruction/0.3/BuildingMaterials#LayerSet"/>
        <owl:disjointWith rdf:resource="https://w3id.org/digitalconstruction/0.3/BuildingMaterials#Material"/>
        <owl:disjointWith rdf:resource="https://w3id.org/digitalconstruction/0.3/BuildingMaterials#Profile"/>
        <owl:disjointWith rdf:resource="https://w3id.org/digitalconstruction/0.3/BuildingMaterials#ProfileSet"/>
    </owl:Class>
    


    <!-- https://w3id.org/digitalconstruction/0.3/BuildingMaterials#ConstituentSet -->

    <owl:Class rdf:about="https://w3id.org/digitalconstruction/0.3/BuildingMaterials#ConstituentSet">
        <rdfs:subClassOf rdf:resource="https://w3id.org/digitalconstruction/0.3/BuildingMaterials#MaterialDefinition"/>
        <owl:disjointWith rdf:resource="https://w3id.org/digitalconstruction/0.3/BuildingMaterials#Layer"/>
        <owl:disjointWith rdf:resource="https://w3id.org/digitalconstruction/0.3/BuildingMaterials#LayerSet"/>
        <owl:disjointWith rdf:resource="https://w3id.org/digitalconstruction/0.3/BuildingMaterials#Material"/>
        <owl:disjointWith rdf:resource="https://w3id.org/digitalconstruction/0.3/BuildingMaterials#Profile"/>
        <owl:disjointWith rdf:resource="https://w3id.org/digitalconstruction/0.3/BuildingMaterials#ProfileSet"/>
    </owl:Class>
    


    <!-- https://w3id.org/digitalconstruction/0.3/BuildingMaterials#InorganicNonMetallicMaterial -->

    <owl:Class rdf:about="https://w3id.org/digitalconstruction/0.3/BuildingMaterials#InorganicNonMetallicMaterial">
        <rdfs:subClassOf rdf:resource="https://w3id.org/digitalconstruction/0.3/BuildingMaterials#MaterialType"/>
        <owl:disjointWith rdf:resource="https://w3id.org/digitalconstruction/0.3/BuildingMaterials#MetallicMaterial"/>
        <owl:disjointWith rdf:resource="https://w3id.org/digitalconstruction/0.3/BuildingMaterials#OrganicaMaterial"/>
    </owl:Class>
    


    <!-- https://w3id.org/digitalconstruction/0.3/BuildingMaterials#Layer -->

    <owl:Class rdf:about="https://w3id.org/digitalconstruction/0.3/BuildingMaterials#Layer">
        <rdfs:subClassOf rdf:resource="https://w3id.org/digitalconstruction/0.3/BuildingMaterials#MaterialDefinition"/>
        <owl:disjointWith rdf:resource="https://w3id.org/digitalconstruction/0.3/BuildingMaterials#LayerSet"/>
        <owl:disjointWith rdf:resource="https://w3id.org/digitalconstruction/0.3/BuildingMaterials#Material"/>
        <owl:disjointWith rdf:resource="https://w3id.org/digitalconstruction/0.3/BuildingMaterials#Profile"/>
        <owl:disjointWith rdf:resource="https://w3id.org/digitalconstruction/0.3/BuildingMaterials#ProfileSet"/>
    </owl:Class>
    


    <!-- https://w3id.org/digitalconstruction/0.3/BuildingMaterials#LayerSet -->

    <owl:Class rdf:about="https://w3id.org/digitalconstruction/0.3/BuildingMaterials#LayerSet">
        <rdfs:subClassOf rdf:resource="https://w3id.org/digitalconstruction/0.3/BuildingMaterials#MaterialDefinition"/>
        <owl:disjointWith rdf:resource="https://w3id.org/digitalconstruction/0.3/BuildingMaterials#Material"/>
        <owl:disjointWith rdf:resource="https://w3id.org/digitalconstruction/0.3/BuildingMaterials#Profile"/>
        <owl:disjointWith rdf:resource="https://w3id.org/digitalconstruction/0.3/BuildingMaterials#ProfileSet"/>
    </owl:Class>
    


    <!-- https://w3id.org/digitalconstruction/0.3/BuildingMaterials#Material -->

    <owl:Class rdf:about="https://w3id.org/digitalconstruction/0.3/BuildingMaterials#Material">
        <rdfs:subClassOf>
            <owl:Restriction>
                <owl:onProperty rdf:resource="http://www.semanticweb.org/arnak/ontologies/2022/7/DOR#hasSourceType"/>
                <owl:minQualifiedCardinality rdf:datatype="http://www.w3.org/2001/XMLSchema#nonNegativeInteger">1</owl:minQualifiedCardinality>
                <owl:onClass rdf:resource="http://www.semanticweb.org/arnak/ontologies/2022/7/DOR#MaterialSourceType"/>
            </owl:Restriction>
        </rdfs:subClassOf>
        <owl:disjointWith rdf:resource="https://w3id.org/digitalconstruction/0.3/BuildingMaterials#MaterialDefinition"/>
        <owl:disjointWith rdf:resource="https://w3id.org/digitalconstruction/0.3/BuildingMaterials#Profile"/>
        <owl:disjointWith rdf:resource="https://w3id.org/digitalconstruction/0.3/BuildingMaterials#ProfileSet"/>
        <rdfs:comment>a homogeneous or inhomogeneous substance that can be used to form elements (physical products or their components). [ISO 16739]</rdfs:comment>
        <rdfs:label>Material</rdfs:label>
    </owl:Class>
    


    <!-- https://w3id.org/digitalconstruction/0.3/BuildingMaterials#MaterialDefinition -->

    <owl:Class rdf:about="https://w3id.org/digitalconstruction/0.3/BuildingMaterials#MaterialDefinition"/>
    


    <!-- https://w3id.org/digitalconstruction/0.3/BuildingMaterials#MaterialType -->

    <owl:Class rdf:about="https://w3id.org/digitalconstruction/0.3/BuildingMaterials#MaterialType">
        <rdfs:comment>It represents the different types of a material.</rdfs:comment>
    </owl:Class>
    


    <!-- https://w3id.org/digitalconstruction/0.3/BuildingMaterials#MetallicMaterial -->

    <owl:Class rdf:about="https://w3id.org/digitalconstruction/0.3/BuildingMaterials#MetallicMaterial">
        <rdfs:subClassOf rdf:resource="https://w3id.org/digitalconstruction/0.3/BuildingMaterials#MaterialType"/>
        <owl:disjointWith rdf:resource="https://w3id.org/digitalconstruction/0.3/BuildingMaterials#OrganicaMaterial"/>
    </owl:Class>
    


    <!-- https://w3id.org/digitalconstruction/0.3/BuildingMaterials#OrganicaMaterial -->

    <owl:Class rdf:about="https://w3id.org/digitalconstruction/0.3/BuildingMaterials#OrganicaMaterial">
        <rdfs:subClassOf rdf:resource="https://w3id.org/digitalconstruction/0.3/BuildingMaterials#MaterialType"/>
    </owl:Class>
    


    <!-- https://w3id.org/digitalconstruction/0.3/BuildingMaterials#Profile -->

    <owl:Class rdf:about="https://w3id.org/digitalconstruction/0.3/BuildingMaterials#Profile">
        <rdfs:subClassOf rdf:resource="https://w3id.org/digitalconstruction/0.3/BuildingMaterials#MaterialDefinition"/>
        <owl:disjointWith rdf:resource="https://w3id.org/digitalconstruction/0.3/BuildingMaterials#ProfileSet"/>
    </owl:Class>
    


    <!-- https://w3id.org/digitalconstruction/0.3/BuildingMaterials#ProfileSet -->

    <owl:Class rdf:about="https://w3id.org/digitalconstruction/0.3/BuildingMaterials#ProfileSet">
        <rdfs:subClassOf rdf:resource="https://w3id.org/digitalconstruction/0.3/BuildingMaterials#MaterialDefinition"/>
    </owl:Class>
    


    <!-- https://w3id.org/dot#Causation -->

    <owl:Class rdf:about="https://w3id.org/dot#Causation">
        <rdfs:comment xml:lang="en">Represents the causation of a damage. 
Should be extended with domain-specific subclasses.</rdfs:comment>
        <rdfs:label xml:lang="en">Causation</rdfs:label>
    </owl:Class>
    


    <!-- https://w3id.org/dot#ClassifiedDamage -->

    <owl:Class rdf:about="https://w3id.org/dot#ClassifiedDamage">
        <rdfs:subClassOf rdf:resource="https://w3id.org/dot#Damage"/>
        <owl:disjointWith rdf:resource="https://w3id.org/dot#UnclassifiedDamage"/>
        <rdfs:comment xml:lang="en">A damage classification is used to denote the kind of damage. Subclasses of this class are defined in extensions 
			  such as CDO (Concrete Damage Ontology), NSO (the Natural Stone Ontology), etc.</rdfs:comment>
        <rdfs:label xml:lang="en">Classified Damage</rdfs:label>
    </owl:Class>
    


    <!-- https://w3id.org/dot#Damage -->

    <owl:Class rdf:about="https://w3id.org/dot#Damage">
        <rdfs:comment xml:lang="en">Damage is the harm to a structure resulting in impairment or loss of function, usefulness or value.
Instead of using dot:Damage, it is recommended to use one subclass of dot:Damage for respectively the damage topology (either dot:DamageArea or dot:DamageElement), the 
potential structural impact (either dot:StructuralDamage or dot:Defect) and the damage classification (either dot:UnclassifiedDamage or subclasses of dot:ClassifiedDamage).</rdfs:comment>
        <rdfs:label xml:lang="en">Damage</rdfs:label>
    </owl:Class>
    


    <!-- https://w3id.org/dot#DamageArea -->

    <owl:Class rdf:about="https://w3id.org/dot#DamageArea">
        <rdfs:subClassOf rdf:resource="https://w3id.org/dot#Damage"/>
        <owl:disjointWith rdf:resource="https://w3id.org/dot#DamageElement"/>
        <owl:disjointWith rdf:resource="https://w3id.org/dot#DamagePattern"/>
        <rdfs:comment xml:lang="en">Area in a component where damage is located. Holds collection of multiple DamageElements or DamagePatterns. Used to be attached with simplified geometry.</rdfs:comment>
        <rdfs:label xml:lang="en">Damage Area</rdfs:label>
    </owl:Class>
    


    <!-- https://w3id.org/dot#DamageElement -->

    <owl:Class rdf:about="https://w3id.org/dot#DamageElement">
        <rdfs:subClassOf rdf:resource="https://w3id.org/dot#Damage"/>
        <owl:disjointWith rdf:resource="https://w3id.org/dot#DamagePattern"/>
        <rdfs:comment xml:lang="en">Damage that is modeled on a very detailed level and belongs with other adjacent Damage Element instances to a broader damage area or damage pattern</rdfs:comment>
        <rdfs:label xml:lang="en">Damage Element</rdfs:label>
    </owl:Class>
    


    <!-- https://w3id.org/dot#DamagePattern -->

    <owl:Class rdf:about="https://w3id.org/dot#DamagePattern">
        <rdfs:comment xml:lang="en">Defines a group of associated or physically connected instances of Damage Element. Used as class for grouping inside an instance of Damage Area.</rdfs:comment>
        <rdfs:label xml:lang="en">Damage Pattern</rdfs:label>
    </owl:Class>
    


    <!-- https://w3id.org/dot#Defect -->

    <owl:Class rdf:about="https://w3id.org/dot#Defect">
        <rdfs:subClassOf rdf:resource="https://w3id.org/dot#Damage"/>
        <owl:disjointWith rdf:resource="https://w3id.org/dot#StructuralDamage"/>
        <rdfs:comment xml:lang="en">Should be used on nodes that are already classified as dot:DamageArea or dot:DamageElement.
Damage that does not impair the structural integrity of the structure, but can still have influence on the durability, usability and / or value.</rdfs:comment>
        <rdfs:label xml:lang="en">Defect</rdfs:label>
    </owl:Class>
    


    <!-- https://w3id.org/dot#Description -->

    <owl:Class rdf:about="https://w3id.org/dot#Description">
        <rdfs:subClassOf rdf:resource="https://w3id.org/dot#Documentation"/>
        <rdfs:comment xml:lang="en">Short textual documentation about a Damage or Structure Element. Generally created by the inspecting person.</rdfs:comment>
        <rdfs:label xml:lang="en">Description</rdfs:label>
    </owl:Class>
    


    <!-- https://w3id.org/dot#Documentation -->

    <owl:Class rdf:about="https://w3id.org/dot#Documentation">
        <rdfs:comment xml:lang="en">Material or data that provides information or evidence about the structure and its components or that serves as a record. Should only be used for damage-related documentation.</rdfs:comment>
        <rdfs:label xml:lang="en">Damage Documentation</rdfs:label>
    </owl:Class>
    


    <!-- https://w3id.org/dot#ExternalResource -->

    <owl:Class rdf:about="https://w3id.org/dot#ExternalResource">
        <rdfs:subClassOf rdf:resource="https://w3id.org/dot#Documentation"/>
        <rdfs:comment xml:lang="en">Document that is stored in a separate file, referenced by an external path.</rdfs:comment>
        <rdfs:label xml:lang="en">External Resource</rdfs:label>
    </owl:Class>
    


    <!-- https://w3id.org/dot#Inspection -->

    <owl:Class rdf:about="https://w3id.org/dot#Inspection">
        <rdfs:comment xml:lang="en">Careful examination or scrutiny in which an existing construction or a part of it is inspected and detected damages are recorded.
Should be repeated at regular time intervals.</rdfs:comment>
        <rdfs:label xml:lang="en">Inspection</rdfs:label>
    </owl:Class>
    


    <!-- https://w3id.org/dot#StructuralDamage -->

    <owl:Class rdf:about="https://w3id.org/dot#StructuralDamage">
        <rdfs:subClassOf rdf:resource="https://w3id.org/dot#Damage"/>
        <rdfs:comment xml:lang="en">Should be used on nodes that are already classified as dot:DamageArea or dot:DamageElement.
Damage that impairs the structural integrity of the structure.</rdfs:comment>
        <rdfs:label xml:lang="en">Structural Damage</rdfs:label>
    </owl:Class>
    


    <!-- https://w3id.org/dot#UnclassifiedDamage -->

    <owl:Class rdf:about="https://w3id.org/dot#UnclassifiedDamage">
        <rdfs:subClassOf rdf:resource="https://w3id.org/dot#Damage"/>
        <rdfs:comment xml:lang="en">A dot:Damage instance that is not further classified with domain-specific classes (subclasses of dot:ClassifiedDamage). 
This class can be used in cases where the damage classification is unknown.</rdfs:comment>
        <rdfs:label xml:lang="en">Unclassified Damage</rdfs:label>
    </owl:Class>
    <rdf:Description>
        <foaf:name>Pieter Pauwels</foaf:name>
    </rdf:Description>
    <rdf:Description>
        <foaf:name>Pieter Pauwels</foaf:name>
    </rdf:Description>
    <rdf:Description>
        <foaf:name>Pieter Pauwels</foaf:name>
    </rdf:Description>
    <rdf:Description>
        <foaf:name>Pieter Pauwels</foaf:name>
    </rdf:Description>
    <rdf:Description>
        <foaf:name>Al-Hakam Hamdan</foaf:name>
    </rdf:Description>
    


    <!-- 
    ///////////////////////////////////////////////////////////////////////////////////////
    //
    // Annotations
    //
    ///////////////////////////////////////////////////////////////////////////////////////
     -->

    <rdf:Description rdf:about="http://maxime-lefrancois.info/me#">
        <ns2:fn>Maxime Lefrançois</ns2:fn>
        <schema1:name>Maxime Lefrançois</schema1:name>
    </rdf:Description>
    <rdf:Description rdf:about="http://xmlns.com/foaf/0.1/account">
        <rdfs:comment>Indicates an account held by this agent.</rdfs:comment>
        <rdfs:isDefinedBy rdf:resource="http://xmlns.com/foaf/0.1/"/>
        <rdfs:label>account</rdfs:label>
        <ns:term_status>testing</ns:term_status>
    </rdf:Description>
    <rdf:Description rdf:about="http://xmlns.com/foaf/0.1/accountServiceHomepage">
        <rdfs:comment>Indicates a homepage of the service provide for this online account.</rdfs:comment>
        <rdfs:isDefinedBy rdf:resource="http://xmlns.com/foaf/0.1/"/>
        <rdfs:label>account service homepage</rdfs:label>
        <ns:term_status>testing</ns:term_status>
    </rdf:Description>
    <rdf:Description rdf:about="http://xmlns.com/foaf/0.1/based_near">
        <rdfs:comment>A location that something is based near, for some broadly human notion of near.</rdfs:comment>
        <rdfs:isDefinedBy rdf:resource="http://xmlns.com/foaf/0.1/"/>
        <rdfs:label>based near</rdfs:label>
        <ns:term_status>testing</ns:term_status>
    </rdf:Description>
    <rdf:Description rdf:about="http://xmlns.com/foaf/0.1/givenName">
        <rdfs:comment>The given name of some person.</rdfs:comment>
        <rdfs:isDefinedBy rdf:resource="http://xmlns.com/foaf/0.1/"/>
        <rdfs:label>Given name</rdfs:label>
        <ns:term_status>testing</ns:term_status>
    </rdf:Description>
    <rdf:Description rdf:about="http://xmlns.com/foaf/0.1/givenname">
        <rdfs:comment>The given name of some person.</rdfs:comment>
        <rdfs:isDefinedBy rdf:resource="http://xmlns.com/foaf/0.1/"/>
        <rdfs:label>Given name</rdfs:label>
        <ns:term_status>archaic</ns:term_status>
    </rdf:Description>
    <rdf:Description rdf:about="http://xmlns.com/foaf/0.1/holdsAccount">
        <rdfs:comment>Indicates an account held by this agent.</rdfs:comment>
        <rdfs:isDefinedBy rdf:resource="http://xmlns.com/foaf/0.1/"/>
        <rdfs:label>account</rdfs:label>
        <ns:term_status>archaic</ns:term_status>
    </rdf:Description>
    <rdf:Description rdf:about="http://xmlns.com/foaf/0.1/interest">
        <rdfs:comment>A page about a topic of interest to this person.</rdfs:comment>
        <rdfs:isDefinedBy rdf:resource="http://xmlns.com/foaf/0.1/"/>
        <rdfs:label>interest</rdfs:label>
        <ns:term_status>testing</ns:term_status>
    </rdf:Description>
    <rdf:Description rdf:about="http://xmlns.com/foaf/0.1/knows">
        <rdfs:comment>A person known by this person (indicating some level of reciprocated interaction between the parties).</rdfs:comment>
        <rdfs:isDefinedBy rdf:resource="http://xmlns.com/foaf/0.1/"/>
        <rdfs:label>knows</rdfs:label>
        <ns:term_status>stable</ns:term_status>
    </rdf:Description>
    <rdf:Description rdf:about="http://xmlns.com/foaf/0.1/member">
        <rdfs:comment>Indicates a member of a Group</rdfs:comment>
        <rdfs:isDefinedBy rdf:resource="http://xmlns.com/foaf/0.1/"/>
        <rdfs:label>member</rdfs:label>
        <ns:term_status>stable</ns:term_status>
    </rdf:Description>
    <rdf:Description rdf:about="http://xmlns.com/foaf/0.1/membershipClass">
        <rdfs:comment>Indicates the class of individuals that are a member of a Group</rdfs:comment>
        <rdfs:isDefinedBy rdf:resource="http://xmlns.com/foaf/0.1/"/>
        <rdfs:label>membershipClass</rdfs:label>
        <ns:term_status>unstable</ns:term_status>
    </rdf:Description>
    <rdf:Description rdf:about="http://xmlns.com/foaf/0.1/phone">
        <rdfs:comment>A phone,  specified using fully qualified tel: URI scheme (refs: http://www.w3.org/Addressing/schemes.html#tel).</rdfs:comment>
        <rdfs:isDefinedBy rdf:resource="http://xmlns.com/foaf/0.1/"/>
        <rdfs:label>phone</rdfs:label>
        <ns:term_status>testing</ns:term_status>
    </rdf:Description>
    <rdf:Description rdf:about="http://xmlns.com/foaf/0.1/publications">
        <rdfs:comment>A link to the publications of this person.</rdfs:comment>
        <rdfs:isDefinedBy rdf:resource="http://xmlns.com/foaf/0.1/"/>
        <rdfs:label>publications</rdfs:label>
        <ns:term_status>testing</ns:term_status>
    </rdf:Description>
    <rdf:Description rdf:about="http://xmlns.com/foaf/0.1/schoolHomepage">
        <rdfs:comment>A homepage of a school attended by the person.</rdfs:comment>
        <rdfs:isDefinedBy rdf:resource="http://xmlns.com/foaf/0.1/"/>
        <rdfs:label>schoolHomepage</rdfs:label>
        <ns:term_status>testing</ns:term_status>
    </rdf:Description>
    <rdf:Description rdf:about="http://xmlns.com/foaf/0.1/sha1">
        <rdfs:comment>A sha1sum hash, in hex.</rdfs:comment>
        <rdfs:isDefinedBy rdf:resource="http://xmlns.com/foaf/0.1/"/>
        <rdfs:label>sha1sum (hex)</rdfs:label>
        <ns:term_status>unstable</ns:term_status>
    </rdf:Description>
    <rdf:Description rdf:about="http://xmlns.com/foaf/0.1/thumbnail">
        <rdfs:comment>A derived thumbnail image.</rdfs:comment>
        <rdfs:isDefinedBy rdf:resource="http://xmlns.com/foaf/0.1/"/>
        <rdfs:label>thumbnail</rdfs:label>
        <ns:term_status>testing</ns:term_status>
    </rdf:Description>
    <rdf:Description rdf:about="http://xmlns.com/foaf/0.1/title">
        <rdfs:comment>Title (Mr, Mrs, Ms, Dr. etc)</rdfs:comment>
        <rdfs:isDefinedBy rdf:resource="http://xmlns.com/foaf/0.1/"/>
        <rdfs:label>title</rdfs:label>
        <ns:term_status>testing</ns:term_status>
    </rdf:Description>
    <rdf:Description rdf:about="http://xmlns.com/foaf/0.1/workInfoHomepage">
        <rdfs:comment>A work info homepage of some person; a page about their work for some organization.</rdfs:comment>
        <rdfs:isDefinedBy rdf:resource="http://xmlns.com/foaf/0.1/"/>
        <rdfs:label>work info homepage</rdfs:label>
        <ns:term_status>testing</ns:term_status>
    </rdf:Description>
    <rdf:Description rdf:about="http://xmlns.com/foaf/0.1/workplaceHomepage">
        <rdfs:comment>A workplace homepage of some person; the homepage of an organization they work for.</rdfs:comment>
        <rdfs:isDefinedBy rdf:resource="http://xmlns.com/foaf/0.1/"/>
        <rdfs:label>workplace homepage</rdfs:label>
        <ns:term_status>testing</ns:term_status>
    </rdf:Description>
    <rdf:Description rdf:about="https://orcid.org/0000-0001-8020-4609">
        <ns2:fn>Pieter Pauwels</ns2:fn>
        <schema1:name>Pieter Pauwels</schema1:name>
    </rdf:Description>
    <rdf:Description rdf:about="https://orcid.org/0000-0002-2033-859X">
        <ns2:fn>Georg Ferdinand Schneider</ns2:fn>
        <schema1:name>Georg Ferdinand Schneider</schema1:name>
    </rdf:Description>
    <rdf:Description rdf:about="https://orcid.org/0000-0002-6519-7057">
        <ns2:fn>Mads Holten Rasmussen</ns2:fn>
        <schema1:name>Mads Holten Rasmussen</schema1:name>
    </rdf:Description>
    <rdf:Description rdf:about="https://w3id.org/bot#aggregates">
        <rdfs:comment xml:lang="da">This property is DEPRECATED, use bot:hasSubElement instead // ORIGINAL definition: Forbinder et aggregat (en klynge af elementer, som kan behandles som en samlet enhed) med dets delelementer. For eksempel aggregerer et ventilationsaggregat, blandt andre elementer, en ventilator og et filter.
        
Eksempel på brug af bot:aggregates i en produkt-ontologi:
```
product:Fan             rdfs:subClassOf     bot:Element .
product:Filter          rdfs:subClassOf     bot:Element .
product:hasFan          rdfs:subPropertyOf  bot:aggregates ;
                        rdfs:range          product:Fan .
product:hasFilter       rdfs:subPropertyOf  product:aggregates ;
                        rdfs:range          product:Filter .
product:AirHandlingUnit rdfs:subClassOf     bot:Element ;
                        rdfs:subClassOf     [ owl:onProperty product:hasFan ; owl:someValuesFrom  product:Fan ] ;
                        rdfs:subClassOf     [ owl:onProperty product:hasFilter ; owl:someValuesFrom  product:Filter ] .
```</rdfs:comment>
        <rdfs:comment xml:lang="en">This property is DEPRECATED, use bot:hasSubElement instead // ORIGINAL definition: Links an aggregate (a cluster of elements that can be treated as a single unit) to its sub-elements. For example an Air Handling Unit aggregates, among other elements, a fan and a filter.
        
Example of how to use bot:aggregates in a product ontology:
```
product:Fan             rdfs:subClassOf     bot:Element .
product:Filter          rdfs:subClassOf     bot:Element .
product:hasFan          rdfs:subPropertyOf  bot:aggregates ;
                        rdfs:range          product:Fan .
product:hasFilter       rdfs:subPropertyOf  product:aggregates ;
                        rdfs:range          product:Filter .
product:AirHandlingUnit rdfs:subClassOf     bot:Element ;
                        rdfs:subClassOf     [ owl:onProperty product:hasFan ; owl:someValuesFrom  product:Fan ] ;
                        rdfs:subClassOf     [ owl:onProperty product:hasFilter ; owl:someValuesFrom  product:Filter ] .
```</rdfs:comment>
        <rdfs:label xml:lang="en">aggregates</rdfs:label>
        <rdfs:label xml:lang="da">aggregerer</rdfs:label>
        <rdfs:seeAlso rdf:resource="https://w3id.org/bot#hasSubElement"/>
        <owl:deprecated rdf:datatype="http://www.w3.org/2001/XMLSchema#boolean">true</owl:deprecated>
    </rdf:Description>
    <rdf:Description rdf:about="https://w3id.org/bot#has3DModel">
        <rdfs:comment xml:lang="it">Collega una istanza di bot:Zone o bot:Element ad un IRI che identifica il suo modello 3D. Questo modello 3D può essere descritto usando dei vocabolari RDF dedicati. Altrimenti, lo IRI del modello 3D potrebbe essere dereferenziabile, permettendo tramite esso di raggiungere la rappresentazione del modello 3D codificata secondo un formato esistente per modelli 3D.</rdfs:comment>
        <rdfs:comment xml:lang="da">Forbinder enhver instans af bot:Zone eller bot:Element med en IRI som identificerer dennes 3D-model. Denne 3D-model kan så beskrives ved brug af et dedikeret RDF-vokabular. Alternativt kan 3D-modellens IRI være dereferencerbar, sådan at der modtages en repræsentation af 3D-modellen i et eksisterende dataformat for 3D-modeller når IRIen slås op.</rdfs:comment>
        <rdfs:comment xml:lang="fi">Liittää vyöhykkeen (bot:Zone) tai elementin (bot:Element) sen 3D-mallin yksilöivään IRI:in. Tämä 3D-malli voi olla kuvattu jollakin siihen tarkoitetulla RDF-sanastolla. 3D-mallin IRI voi myös osoittaa johonkin olemassa olevalla dataformaatilla kuvattuun 3D-malliin, joka on ladattavissa IRI:n kautta.</rdfs:comment>
        <rdfs:comment xml:lang="en">Links any bot:Zone or bot:Element to a IRI that identifies its 3D Model. This 3D Model can then be described using some dedicated RDF vocabulary. Else, the 3D Model IRI could be dereferenceable, and when looking up the IRI one could retrieve a representation of the 3D Model with some existing data format for 3D models.</rdfs:comment>
        <rdfs:comment xml:lang="sv">Länkar en instans av bot:Zone eller bot:Element till en IRI som identifierar dennas 3D-modell. 3D-modellen kan beskrivas med något avsett RDF-vokabulär; alternativt så kan den peka ut mot en extern representation uttryckt i något existerande dataformat för 3D-modellering.</rdfs:comment>
        <rdfs:comment xml:lang="cs">Prepojuje akúkoľvek bot:Zone alebo bot:Element ku konkrétnemu IRI, ktoré identifikuje jej/jeho 3D model. Tento 3D model môže byť potom popísaný použitím konkrétnych RDF slovníkov. Alebo, konkrétne IRI konkrétneho 3D modelu môže byť dereferencovateľné a pokiaľ sa bude vyhľadávať podla IRI, vyhľadávajúci môže získať reprezentáciu 3D modelu pomocou/s existujúceho/cím datového/vým formátu/formátem pre reprezentáciu 3D modely.</rdfs:comment>
        <rdfs:comment xml:lang="sk">Propojuje jakoukoliv bot:Zone nebo bot:Element ke konkrétnímu IRI, které identifikuje její/jeho 3D model. Tento 3D model potom může být popsán využitím konkrétních RDF slovníků. Nebo, konkrétní IRI konkrétního 3D modelu může být dereferencovatelné, pokud se bude vyhledávat dle IRI, vyhledávající může získat reprezentaci 3D modelu pomocí/s existujícího/jícím datového/vým formátu/formátem pro reprezentaci 3D modelu.</rdfs:comment>
        <rdfs:comment xml:lang="pt">Relaciona qualquer bot:Zone ou bot:Element a um IRI que identifique o seu modelo 3D. Este modelo 3D pode ser descrito usando um vocabulário RDF dedicado. Caso contrário, o IRI do modelo 3D pode ser desreferenciável sendo possível receber, quando se pesquisa o IRI, uma representação do modelo 3D num qualquer formato de dados para modelos 3D.</rdfs:comment>
        <rdfs:comment xml:lang="fr">Relie tout bot:Zone ou bot:Element à un IRI qui identifie son modèle 3D. Ce modèle 3D peut ensuite être décrit à l&apos;aide d&apos;un vocabulaire RDF spécifique. Sinon, le modèle 3D de l&apos;IRI pourrait être déréférencé, et en recherchant l&apos;IRI, on pourrait obtenir une représentation du modèle 3D basée sur un format de données existant pour modèles 3D.</rdfs:comment>
        <rdfs:comment xml:lang="de">Verbindet eine Instanz von bot:Zone oder bot:Element zu einer IRI, die das zugehörige 3D Modell identifiziert. Das Modell kann in einem spezifischen RDF Vokabular kodiert sein. Andernfalls kann die IRI auch dereferenzierbar sein.</rdfs:comment>
        <rdfs:comment xml:lang="nl">Verbindt gelijk welke bot:Zone of bot:Element instantie met een IRI die een 3D model identificeert. Dit 3D model kan beschreven worden d.m.v. een gespecialiseerde RDF vocabularium. Anderzijds kan de IRI, indien opgevraagd, ook doorverwijzen naar een 3D model in een bestaand data formaat.</rdfs:comment>
        <rdfs:comment xml:lang="es">Vincula cualquier bot:Zone o bot:Element a un IRI que identifica su modelo 3D. Este modelo 3D se puede describir utilizando un vocabulario RDF dedicado. De lo contrario, el IRI del modelo 3D podría ser dereferenciable, y al buscar el IRI se podría recuperar una representación del modelo 3D con algún formato de datos existente para los modelos 3D.</rdfs:comment>
        <rdfs:comment xml:lang="ca">Vincula qualsevol bot:Zone o bot:Element a un IRI que identifica el seu model 3D. Aquest model 3D es pot descriure utilitzant un vocabulari RDF dedicat. En cas contrari, l&apos;IRI de el model 3D podria ser desreferenciable, i al buscar la IRI es podria recuperar una representació de el model 3D amb algun format de dades existent pels models 3D.</rdfs:comment>
        <rdfs:comment xml:lang="tr">bot:Zone&apos;nin herhangi bir örneğini bağlar ya da bot:Element&apos;i kendi 3D-modelini tanimlayan bir IRI ile bağlar. Bu 3D-model daha sonra özel bir RDF kelime kullanimi ile tanimlanabilir. Bu 3D model daha sonra özel bir RDF kelime kullanımı ile tanımlanabilir. Aksi takdirde, IRI&apos;nin kaydı silinebilir.</rdfs:comment>
        <rdfs:comment xml:lang="fa">رابطه یک عنصر  bot:Zoneیا bot:Element با یک IRI که مدل سه بعدی خود را مشخص می کند. این مدل سه بعدی را می توان با برخی کلمات اختصاصی RDF توصیف کرد. به عبارت دیگر، نشانی مدل سه بعدی می تواند ارائه ای از مدل سه بعدی را با برخی از قالب های داده موجود برای مدل های سه بعدی بازیابی کند.</rdfs:comment>
        <rdfs:comment xml:lang="zh-cn">将任何bot：Zone或bot：Element链接到标识其3D模型的IRI，然后可以使用一些专用的RDF词汇表来描述3D模型。 否则，3D模型IRI可能会被取消引用的，在此情况下，当查找IRI时，可以使用3D模型的某些现有数据格式检索3D模型。</rdfs:comment>
        <rdfs:isDefinedBy rdf:resource="https://w3id.org/bot#"/>
        <rdfs:label xml:lang="tr">3D modeli var</rdfs:label>
        <rdfs:label xml:lang="fr">a modèle 3D</rdfs:label>
        <rdfs:label xml:lang="it">ha modello 3D</rdfs:label>
        <rdfs:label xml:lang="da">har 3D-model</rdfs:label>
        <rdfs:label xml:lang="sv">har 3D-modell</rdfs:label>
        <rdfs:label xml:lang="en">has 3D model</rdfs:label>
        <rdfs:label xml:lang="de">hat 3D Modell</rdfs:label>
        <rdfs:label xml:lang="nl">heeft 3D model</rdfs:label>
        <rdfs:label xml:lang="cs">má 3D model</rdfs:label>
        <rdfs:label xml:lang="sk">má 3D model</rdfs:label>
        <rdfs:label xml:lang="fi">omaa 3D-mallin</rdfs:label>
        <rdfs:label xml:lang="pt">tem modelo 3D</rdfs:label>
        <rdfs:label xml:lang="es">tiene modelo 3D</rdfs:label>
        <rdfs:label xml:lang="ca">té model 3D</rdfs:label>
        <rdfs:label xml:lang="fa">مدل سه بعدی دارد</rdfs:label>
        <rdfs:label xml:lang="zh-cn">含有3D模型</rdfs:label>
        <ns:term_status>unstable</ns:term_status>
        <schema1:domainIncludes rdf:resource="https://w3id.org/bot#Element"/>
        <schema1:domainIncludes rdf:resource="https://w3id.org/bot#Zone"/>
    </rdf:Description>
    <rdf:Description rdf:about="https://w3id.org/bot#hasSimple3DModel">
        <rdfs:comment xml:lang="it">Collega una istanza di bot:Zone o bot:Element ad un modello 3D codificato come un literal.</rdfs:comment>
        <rdfs:comment xml:lang="da">Forbinder enhver instans af bot:Zone eller bot:Element med en 3D-model beskrevet som en literal.</rdfs:comment>
        <rdfs:comment xml:lang="fi">Liittää vyöhykkeen (bot:Zone) tai elementin (bot:Element) sen yksinkertaiseksi arvoksi enkoodattuun 3D-malliin.</rdfs:comment>
        <rdfs:comment xml:lang="en">Links any bot:Zone or bot:Element to a 3D Model encoded as a literal.</rdfs:comment>
        <rdfs:comment xml:lang="sv">Länkar en instans av bot:Zone eller bot:Element till en 3D-modell uttryckt som en RDF literal.</rdfs:comment>
        <rdfs:comment xml:lang="sk">Prepojuje akýkoľvek bot:Zone alebo bot:Element na 3D model definovaný ako literál.</rdfs:comment>
        <rdfs:comment xml:lang="cs">Propojuje jakýkoliv bot:Zone nebo bot:Element na 3D model definovaný jako literál.</rdfs:comment>
        <rdfs:comment xml:lang="fr">Relie tout bot:Zone ou bot:Element à un modèle 3D encodé comme</rdfs:comment>
        <rdfs:comment xml:lang="de">Verbindet jede bot:Zone oder bot:Element zu einem 3D Model, dass als Literal codiert ist.</rdfs:comment>
        <rdfs:comment xml:lang="nl">Verbindt gelijk welke bot:Zone of bot:Element instantie met een 3D model geëncodeerd in een literal.</rdfs:comment>
        <rdfs:comment xml:lang="es">Vincula cualquier bot:Zone o bot:Element a un modelo 3D codificado como literal.</rdfs:comment>
        <rdfs:comment xml:lang="pt">Vincula qualquer bot:Zone ou bot:Element a um Modelo 3D codificado como um literal.</rdfs:comment>
        <rdfs:comment xml:lang="ca">Vincula qualsevol bot:Zone o bot:Element a un model 3D codificat com literal.</rdfs:comment>
        <rdfs:comment xml:lang="tr">bot:Zone&apos;nin herhangi bir örneğini bağlar ya da bot:Element&apos;i bir literal olarak tanimlanan 3D-model ile bağlar.</rdfs:comment>
        <rdfs:comment xml:lang="fa">رابطه یک عنصر  bot:Zone یا  bot:Elementبا یک مدل سه بعدی که به صورت یک نوشته رمزگذاری شده است.</rdfs:comment>
        <rdfs:comment xml:lang="zh-cn">将任何bot：Zone或bot：Element链接到编码为文本的3D模型。</rdfs:comment>
        <rdfs:isDefinedBy rdf:resource="https://w3id.org/bot#"/>
        <rdfs:label xml:lang="tr">Basit bir 3D modeli var</rdfs:label>
        <rdfs:label xml:lang="fr">a modèle 3D simple</rdfs:label>
        <rdfs:label xml:lang="it">ha modello 3D semplice</rdfs:label>
        <rdfs:label xml:lang="sv">har enkel 3D-modell</rdfs:label>
        <rdfs:label xml:lang="da">har simpel 3D-model</rdfs:label>
        <rdfs:label xml:lang="en">has simple 3D model</rdfs:label>
        <rdfs:label xml:lang="de">hat einfaches 3D Modell</rdfs:label>
        <rdfs:label xml:lang="nl">heeft eenvoudig 3D model</rdfs:label>
        <rdfs:label xml:lang="cs">má jednoduchý 3D model</rdfs:label>
        <rdfs:label xml:lang="sk">má jednoduchý 3D model</rdfs:label>
        <rdfs:label xml:lang="fi">omaa yksinkertaisen 3D-mallin</rdfs:label>
        <rdfs:label xml:lang="pt">tem modelo 3D simples</rdfs:label>
        <rdfs:label xml:lang="es">tiene modelo 3D simple</rdfs:label>
        <rdfs:label xml:lang="ca">té un model 3D senzill</rdfs:label>
        <rdfs:label xml:lang="fa">مدل سه بعدی ساده دارد</rdfs:label>
        <rdfs:label xml:lang="zh-cn">含有简单的3D模型</rdfs:label>
        <ns:term_status>unstable</ns:term_status>
        <schema1:domainIncludes rdf:resource="https://w3id.org/bot#Element"/>
        <schema1:domainIncludes rdf:resource="https://w3id.org/bot#Zone"/>
    </rdf:Description>
    


    <!-- 
    ///////////////////////////////////////////////////////////////////////////////////////
    //
    // General axioms
    //
    ///////////////////////////////////////////////////////////////////////////////////////
     -->

    <rdf:Description>
        <rdf:type rdf:resource="http://www.w3.org/2002/07/owl#AllDisjointClasses"/>
        <owl:members rdf:parseType="Collection">
            <rdf:Description rdf:about="http://xmlns.com/foaf/0.1/EngineeringOffice"/>
            <rdf:Description rdf:about="http://xmlns.com/foaf/0.1/PlantOperator"/>
            <rdf:Description rdf:about="http://xmlns.com/foaf/0.1/PublicAdministration"/>
        </owl:members>
    </rdf:Description>
    <rdf:Description>
        <rdf:type rdf:resource="http://www.w3.org/2002/07/owl#AllDisjointClasses"/>
        <owl:members rdf:parseType="Collection">
            <rdf:Description rdf:about="https://w3id.org/digitalconstruction/0.3/BuildingMaterials#CompositeMaterial"/>
            <rdf:Description rdf:about="https://w3id.org/digitalconstruction/0.3/BuildingMaterials#InorganicNonMetallicMaterial"/>
            <rdf:Description rdf:about="https://w3id.org/digitalconstruction/0.3/BuildingMaterials#MetallicMaterial"/>
            <rdf:Description rdf:about="https://w3id.org/digitalconstruction/0.3/BuildingMaterials#OrganicaMaterial"/>
        </owl:members>
    </rdf:Description>
    <rdf:Description>
        <rdf:type rdf:resource="http://www.w3.org/2002/07/owl#AllDisjointClasses"/>
        <owl:members rdf:parseType="Collection">
            <rdf:Description rdf:about="https://w3id.org/digitalconstruction/0.3/BuildingMaterials#Constituent"/>
            <rdf:Description rdf:about="https://w3id.org/digitalconstruction/0.3/BuildingMaterials#ConstituentSet"/>
            <rdf:Description rdf:about="https://w3id.org/digitalconstruction/0.3/BuildingMaterials#Layer"/>
            <rdf:Description rdf:about="https://w3id.org/digitalconstruction/0.3/BuildingMaterials#LayerSet"/>
            <rdf:Description rdf:about="https://w3id.org/digitalconstruction/0.3/BuildingMaterials#Profile"/>
            <rdf:Description rdf:about="https://w3id.org/digitalconstruction/0.3/BuildingMaterials#ProfileSet"/>
        </owl:members>
    </rdf:Description>
    <rdf:Description>
        <rdf:type rdf:resource="http://www.w3.org/2002/07/owl#AllDisjointProperties"/>
        <owl:members rdf:parseType="Collection">
            <rdf:Description rdf:about="https://w3id.org/digitalconstruction/0.3/BuildingMaterials#hasDefinedValue"/>
            <rdf:Description rdf:about="https://w3id.org/digitalconstruction/0.3/BuildingMaterials#hasEstimatedValue"/>
            <rdf:Description rdf:about="https://w3id.org/digitalconstruction/0.3/BuildingMaterials#hasMeasuredValue"/>
        </owl:members>
    </rdf:Description>
</rdf:RDF>



<!-- Generated by the OWL API (version 4.5.25.2023-02-15T19:15:49Z) https://github.com/owlcs/owlapi -->

